@prefix cc:       <http://creativecommons.org/ns#> .
@prefix cert:     <http://www.w3.org/ns/auth/cert#> .
@prefix dbp:      <http://dbpedia.org/property/> .
@prefix dc:       <http://purl.org/dc/elements/1.1/> .
@prefix dcterms:  <http://purl.org/dc/elements/1.1/> .
@prefix doap:     <http://usefulinc.com/ns/doap#> .
@prefix exif:     <http://www.w3.org/2003/12/exif/ns#> .
@prefix fn:       <http://www.w3.org/2005/xpath-functions#> .
@prefix foaf:     <http://xmlns.com/foaf/0.1/> .
@prefix geo:      <http://www.w3.org/2003/01/geo/wgs84_pos#> .
@prefix geonames: <http://www.geonames.org/ontology#> .
@prefix gr:       <http://purl.org/goodrelations/v1#> .
@prefix gs1:      <https://gs1.org/voc/> .
@prefix log:      <http://www.w3.org/2000/10/swap/log#> .
@prefix owl:      <http://www.w3.org/2002/07/owl#> .
@prefix rdf:      <http://www.w3.org/1999/02/22-rdf-syntax-ns#> .
@prefix rdfs:     <http://www.w3.org/2000/01/rdf-schema#> .
@prefix rei:      <http://www.w3.org/2004/06/rei#> .
@prefix rsa:      <http://www.w3.org/ns/auth/rsa#> .
@prefix rss:      <http://purl.org/rss/1.0/> .
@prefix schema:   <http://schema.org/> .
@prefix sfn:      <http://www.w3.org/ns/sparql#> .
@prefix sioc:     <http://rdfs.org/sioc/ns#> .
@prefix skos:     <http://www.w3.org/2004/02/skos/core#> .
@prefix sw:       <http://www.w3.org/2003/06/sw-vocab-status/ns#> .
@prefix swrc:     <http://swrc.ontoware.org/ontology#> .
@prefix types:    <http://rdfs.org/sioc/types#> .
@prefix vann:     <http://purl.org/vocab/vann/> .
@prefix vcard:    <http://www.w3.org/2006/vcard/ns#> .
@prefix voaf:     <http://purl.org/vocommons/voaf#> .
@prefix wot:      <http://xmlns.com/wot/0.1/> .
@prefix xhtml:    <http://www.w3.org/1999/xhtml#> .
@prefix xsd:      <http://www.w3.org/2001/XMLSchema#> .

gs1:
	rdf:type                       owl:Ontology , voaf:Vocabulary ;
	<dc11:title>                   "GS1 Vocabulary" ;
	dc:contributors                "Eric Kauz, Mark Harrison, Phil Archer" ;
	dc:creator                     <https://www.gs1.org/> ;
	dc:description:                "The GS1 RDF vocabulary, described using W3C RDF Schema and the Web Ontology Language. The vocabulary builds on and refers to schema.org where appropriate."@en ;
	dc:identifier:                 "GS1 Vocabulary" ;
	dc:issued:                     "2017-11-20"^^xsd:date ;
	dc:lastModified                "2024-03-20"^^xsd:date ;
	vann:preferredNamespacePrefix  "gs1" ;
	vann:preferredNamespaceUri     gs1: ;
	voaf:extends                   schema: ;
	voaf:hasEquivalencesWith       schema: ;
	voaf:specializes               schema: ;
	schema:license                 "data:text/html;charset=UTF-8,<p>GS1&reg;, under its IP Policy, seeks to avoid uncertainty regarding intellectual property claims by requiring the participants in the Work Groups that developed this vocabulary to agree to grant to GS1 members a royalty-free licence or a RAND licence to Necessary Claims, as that term is defined in the GS1 IP Policy. Furthermore, attention is drawn to the possibility that an implementation of one or more features of this vocabulary may be the subject of a patent or other intellectual property     right that does not involve a Necessary Claim. Any such patent or other intellectual property right is not subject to the licencing obligations of GS1. Moreover, the agreement to grant licences provided under the GS1 IP Policy does not include IP rights and any claims of third parties who were not participants in the Work Groups. Accordingly, GS1 recommends that any organisation developing an implementation designed to be in conformance with this vocabulary should determine whether there are any     patents that may encompass a specific implementation that the organisation is developing in compliance with the vocabulary and whether a licence under a patent or other intellectual property right is needed. Such a determination of a need for licencing should be made in view of the details of the specific system designed by the organisation in consultation with their own patent counsel. THIS DOCUMENT IS PROVIDED &quot;AS IS&quot; WITH NO WARRANTIES WHATSOEVER, INCLUDING ANY WARRANTY OF MERCHANTABILITY, NONINFRINGMENT, FITNESS FOR PARTICULAR PURPOSE, OR ANY WARRANTY OTHER WISE ARISING OUT OF THIS SPECIFICATION. GS1 disclaims all liability for any damages arising from use or misuse of this vocabulary, whether special, indirect, consequential, or compensatory damages, and including liability for infringement of any intellectual property     rights, relating to use of information in or reliance upon this document. GS1 retains the right to make changes to this vocabulary at any time, without notice. GS1 makes no warranty for the use of this vocabulary and assumes no responsibility for any errors which may appear in the vocabulary, nor does it make a commitment to update the     information contained herein. GS1 and the GS1 logo are registered trademarks of GS1 AISBL.</p><p>Copyright 2015-2019 GS1 AISBL</p><p>Licensed under the Apache License, Version 2.0 (the &quot;License&quot;); you may not use this file except in compliance with the License. You may obtain a copy of the License at <a href=&quot;http://www.apache.org/licenses/LICENSE-2.0&quot; target=&quot;blank&quot;>http://www.apache.org/licenses/LICENSE-2.0</a>.<p><p>Unless required by applicable law or agreed to in writing, software distributed under the License is distributed on an &quot;AS IS&quot; BASIS, WITHOUT WARRANTIES OR CONDITIONS OF ANY KIND, either express or implied. See the License for the specific language governing permissions and limitations under the License.</p>" ;
	owl:versionInfo                "1.10" .


dc:date
	rdf:type  owl:AnnotationProperty .

dc:description
	rdf:type  owl:AnnotationProperty .

dc:title
	rdf:type  owl:AnnotationProperty .

sw:term_status
	rdf:type  owl:AnnotationProperty .


_:b0
	rdf:type     owl:Class ;
	owl:unionOf  ( gs1:Organization gs1:Place ) .

_:b1
	rdf:type     owl:Class ;
	owl:unionOf  ( gs1:Offer gs1:PriceSpecification ) .

gs1:AdditionalProductClassificationDetails
	rdf:type          rdfs:Class , owl:Class ;
	rdfs:comment      "A product classification for the product other than the Global Product Classification(GPC brick value)."@en ;
	rdfs:isDefinedBy  gs1: ;
	rdfs:label        "Additional Product Classification Details"@en ;
	rdfs:subClassOf   owl:Thing ;
	sw:term_status    "stable" .

gs1:AdditiveDetails
	rdf:type  owl:Class , rdfs:Class ;
	rdfs:comment      "A set of details about one of the additives within the product."@en ;
	rdfs:isDefinedBy  gs1: ;
	rdfs:label        "Additive Details"@en ;
	rdfs:subClassOf   owl:Thing ;
	sw:term_status    "stable" .

gs1:AllergenDetails
	rdf:type  rdfs:Class , owl:Class ;
	rdfs:comment      "Details of an allergen for a product."@en ;
	rdfs:isDefinedBy  gs1: ;
	rdfs:label        "Allergen Details"@en ;
	rdfs:subClassOf   owl:Thing ;
	sw:term_status    "stable" .

gs1:AuthenticityDetails
	rdf:type          owl:Class , rdfs:Class ;
	rdfs:comment      "A set of details about covert or overt security features that may contribute to checking the authenticity of a product or product instance."@en ;
	rdfs:isDefinedBy  gs1: ;
	rdfs:label        "Authenticity Details"@en ;
	rdfs:subClassOf   owl:Thing ;
	sw:term_status    "stable" .

gs1:AwardPrizeDetails
	rdf:type          owl:Class , rdfs:Class ;
	rdfs:comment      "Describes a prize or award won by a product or organization."@en ;
	rdfs:isDefinedBy  gs1: ;
	rdfs:label        "Award Prize"@en ;
	rdfs:subClassOf   owl:Thing ;
	sw:term_status    "stable" .

gs1:Beverage
	rdf:type    owl:Class , rdfs:Class ;
	rdfs:comment      "Any potable liquid."@en ;
	rdfs:isDefinedBy  gs1: ;
	rdfs:label        "Beverage"@en ;
	rdfs:subClassOf   gs1:FoodBeverageTobaccoProduct ;
	sw:term_status    "stable" .

gs1:Brand
	rdf:type       rdfs:Class , owl:Class ;
	rdfs:comment      "Information on brands and sub-brands for a product."@en ;
	rdfs:isDefinedBy  gs1: ;
	rdfs:label        "Brand"@en ;
	rdfs:subClassOf   owl:Thing ;
	sw:term_status    "stable" ;
	skos:exactMatch   schema:Brand .

gs1:CertificationDetails
	rdf:type          rdfs:Class , owl:Class ;
	rdfs:comment      "Certification issued by a certifying body to a certification subject (Organization, Place, Product)."@en ;
	rdfs:isDefinedBy  gs1: ;
	rdfs:label        "Certification"@en ;
	rdfs:subClassOf   owl:Thing ;
	sw:term_status    "stable" .

gs1:Clothing
	rdf:type    rdfs:Class , owl:Class ;
	rdfs:comment      " A product that is worn on the body."@en ;
	rdfs:isDefinedBy  gs1: ;
	rdfs:label        "Clothing"@en ;
	rdfs:subClassOf   gs1:WearableProduct ;
	sw:term_status    "stable" .

gs1:ColourCodeDetails
	rdf:type          owl:Class , rdfs:Class ;
	rdfs:comment      "A set of colour code details (colour code, party controlling the code list) for the product."@en ;
	rdfs:isDefinedBy  gs1: ;
	rdfs:label        "Colour Code Details"@en ;
	rdfs:subClassOf   owl:Thing ;
	sw:term_status    "stable" .

gs1:ContactPoint
	rdf:type  rdfs:Class , owl:Class ;
	rdfs:comment      "Information on an individual or department acting as point of contact for an organiation."@en ;
	rdfs:isDefinedBy  gs1: ;
	rdfs:label        "Contact"@en ;
	rdfs:subClassOf   owl:Thing ;
	sw:term_status    "stable" ;
	skos:exactMatch   schema:ContactPoint .

gs1:Country
	rdf:type     rdfs:Class , owl:Class ;
	rdfs:comment      "Country is a complex data type that indicates a country and a country subdivision."@en ;
	rdfs:isDefinedBy  gs1: ;
	rdfs:label        "Country"@en ;
	rdfs:subClassOf   owl:Thing ;
	sw:term_status    "stable" ;
	skos:exactMatch   schema:Country .

gs1:DietTypeCodeDetails
	rdf:type          owl:Class , rdfs:Class ;
	rdfs:comment      "A set of diet type code details (diet type code and diet type sub code) for the product."@en ;
	rdfs:isDefinedBy  gs1: ;
	rdfs:label        "Diet Type Code Details"@en ;
	rdfs:subClassOf   owl:Thing ;
	sw:term_status    "stable" .

gs1:Discount
	rdf:type    owl:Class , rdfs:Class ;
	rdfs:comment      "Provides information on a discount applicable to an offer for example 2 percent."@en ;
	rdfs:isDefinedBy  gs1: ;
	rdfs:label        "Discount"@en ;
	sw:term_status    "unstable" .

gs1:FoodAndBeveragePreparationInformation
	rdf:type          owl:Class , rdfs:Class ;
	rdfs:comment      "Food and Beverage Preparation Information is a complex data type that indicates a preparation state code and preparation instructions."@en ;
	rdfs:isDefinedBy  gs1: ;
	rdfs:label        "Food and Beverage Preparation Information"@en ;
	rdfs:subClassOf   owl:Thing ;
	sw:term_status    "stable" .

gs1:FoodBeverageTobaccoIngredientDetails
	rdf:type          rdfs:Class , owl:Class ;
	rdfs:comment      "Food Beverage Tobacco Ingredient is a complex data type that includes an ingredient statement and details."@en ;
	rdfs:isDefinedBy  gs1: ;
	rdfs:label        "Food Beverage Tobacco Ingredient"@en ;
	rdfs:subClassOf   owl:Thing ;
	sw:term_status    "stable" .

gs1:FoodBeverageTobaccoProduct
	rdf:type          owl:Class , rdfs:Class ;
	rdfs:comment      "A food, beverage or tobacco product."@en ;
	rdfs:isDefinedBy  gs1: ;
	rdfs:label        "Food Beverage Tobacco Product"@en ;
	rdfs:subClassOf   gs1:Product ;
	sw:term_status    "stable" .

gs1:Footwear
	rdf:type    rdfs:Class , owl:Class ;
	rdfs:comment      " Outerwear that is worn on the feet such as shoes or boots."@en ;
	rdfs:isDefinedBy  gs1: ;
	rdfs:label        "Footwear"@en ;
	rdfs:subClassOf   gs1:WearableProduct ;
	sw:term_status    "stable" .

gs1:FruitsVegetables
	rdf:type  owl:Class , rdfs:Class ;
	rdfs:comment      "Contains properties related specifically to fruit and vegetable products."@en ;
	rdfs:isDefinedBy  gs1: ;
	rdfs:label        "Fruits and Vegetables"@en ;
	rdfs:subClassOf   gs1:FoodBeverageTobaccoProduct ;
	sw:term_status    "stable" .

gs1:GeoCoordinates
	rdf:type  owl:Class , rdfs:Class ;
	rdfs:comment      "The geographic coordinates of a place or event."@en ;
	rdfs:isDefinedBy  gs1: ;
	rdfs:label        "GeoCoordinates"@en ;
	rdfs:subClassOf   owl:Thing ;
	sw:term_status    "stable" ;
	skos:exactMatch   schema:GeoCoordinates .

gs1:GeoShape
	rdf:type    owl:Class , rdfs:Class ;
	rdfs:comment      "The geographic shape of a place. A GeoShape can be described using several properties whose values are based on latitude/longitude pairs. Either whitespace or commas can be used to separate latitude and longitude; whitespace should be used when writing a list of several such points."@en ;
	rdfs:isDefinedBy  gs1: ;
	rdfs:label        "GeoShape"@en ;
	rdfs:subClassOf   owl:Thing ;
	sw:term_status    "stable" ;
	skos:exactMatch   schema:GeoShape .

gs1:LocationID_Details
	rdf:type          rdfs:Class , owl:Class ;
	rdfs:comment      "Government bodies, trade organisations, and other parties issue identifiers that are associated to locations. Linking these identifiers to GLN and one another supports consolidating records, mapping related, collaborative identifiers, enhances search ability and enables more efficient transitions between identifiers.  This class provides a mechanism for connecting and sharing location identifiers."@en ;
	rdfs:isDefinedBy  gs1: ;
	rdfs:label        "Location ID Details"@en ;
	rdfs:subClassOf   owl:Thing ;
	sw:term_status    "stable" .

gs1:LocationStatusHistory
	rdf:type          rdfs:Class , owl:Class ;
	rdfs:comment      "Over the lifetime of a location, it may go through periods of being active and inactive. gs1:LocationStatusHistory allows changes in status to be communicated in advance and tracked over time."@en ;
	rdfs:isDefinedBy  gs1: ;
	rdfs:label        "Location Status History"@en ;
	rdfs:subClassOf   owl:Thing ;
	sw:term_status    "stable" .

gs1:MeatPoultry
	rdf:type  rdfs:Class , owl:Class ;
	rdfs:comment      "Meat and poultry products."@en ;
	rdfs:isDefinedBy  gs1: ;
	rdfs:label        "Meat Poultry"@en ;
	rdfs:subClassOf   gs1:FoodBeverageTobaccoProduct ;
	sw:term_status    "stable" .

gs1:MilkButterCreamYogurtCheeseEggsSubstitutes
	rdf:type          rdfs:Class , owl:Class ;
	rdfs:comment      "Milk butter cream yogurts cheese eggs and any substitutes for these products."@en ;
	rdfs:isDefinedBy  gs1: ;
	rdfs:label        "Milk Butter Cream Yogurt Cheese Eggs Substitutes"@en ;
	rdfs:subClassOf   gs1:FoodBeverageTobaccoProduct ;
	sw:term_status    "stable" .

gs1:NutritionMeasurementType
	rdf:type          owl:Class , rdfs:Class ;
	rdfs:comment      "A class providing nutritional value and intake percent."@en ;
	rdfs:isDefinedBy  gs1: ;
	rdfs:label        "Nutrition Measurement Type"@en ;
	rdfs:subClassOf   gs1:QuantitativeValue ;
	sw:term_status    "stable" .

gs1:Offer
	rdf:type       rdfs:Class , owl:Class ;
	rdfs:comment      "An offer to transfer some rights to an item or to provide a service,for example, an offer to sell tickets to an event, to rent the DVD of a movie, to stream a TV show over the internet, to repair a motorcycle, or to loan a book."@en ;
	rdfs:isDefinedBy  gs1: ;
	rdfs:label        "Offer"@en ;
	rdfs:subClassOf   owl:Thing ;
	sw:term_status    "stable" ;
	skos:exactMatch   schema:Offer .

gs1:OrganicClaimDetails
	rdf:type          rdfs:Class , owl:Class ;
	rdfs:comment      "A set of organic claim details for the product."@en ;
	rdfs:isDefinedBy  gs1: ;
	rdfs:label        "Organic Claim Details"@en ;
	rdfs:subClassOf   owl:Thing ;
	sw:term_status    "stable" .

gs1:Organization
	rdf:type  rdfs:Class , owl:Class ;
	rdfs:comment      "An Organization is any legal or physical entity involved at any point in any supply chain and upon which there is a need to retrieve predefined information. An Organization is uniquely identified by a Global Location Number (GLN)."@en ;
	rdfs:isDefinedBy  gs1: ;
	rdfs:label        "Organization"@en ;
	rdfs:subClassOf   owl:Thing ;
	sw:term_status    "stable" ;
	skos:exactMatch   schema:Organization .

gs1:OrganizationID_Details
	rdf:type          rdfs:Class , owl:Class ;
	rdfs:comment      "Government bodies, trade organisations, and other parties issue identifiers that are associated to legal entities and/or functions. Linking these identifiers to GLN and one another supports consolidating records, mapping related, collaborative identifiers, enhances search ability and enables more efficient transitions between identifiers.  This class provides a mechanism for connecting and sharing party identifiers."@en ;
	rdfs:isDefinedBy  gs1: ;
	rdfs:label        "Organisation ID Details"@en ;
	rdfs:subClassOf   owl:Thing ;
	sw:term_status    "stable" .

gs1:OrganizationStatusHistory
	rdf:type          rdfs:Class , owl:Class ;
	rdfs:comment      "Over the lifetime of an organisation, it may go through periods of being active and inactive. gs1:OrganizationStatusHistory allows changes in status to be communicated in advance and tracked over time."@en ;
	rdfs:isDefinedBy  gs1: ;
	rdfs:label        "Organisation Status History"@en ;
	rdfs:subClassOf   owl:Thing ;
	sw:term_status    "stable" .

gs1:PackagingDetails
	rdf:type  rdfs:Class , owl:Class ;
	rdfs:comment      "Details on packaging for a product for example packaging type (bottle), materials, features, recycling, etc.."@en ;
	rdfs:isDefinedBy  gs1: ;
	rdfs:label        "Packaging"@en ;
	rdfs:subClassOf   owl:Thing ;
	sw:term_status    "stable" .

gs1:PackagingMaterialDetails
	rdf:type          rdfs:Class , owl:Class ;
	rdfs:comment      "Information on any material used for packaging."@en ;
	rdfs:isDefinedBy  gs1: ;
	rdfs:label        "Packaging Material Details"@en ;
	rdfs:subClassOf   owl:Thing ;
	sw:term_status    "stable" .

gs1:Place
	rdf:type       owl:Class , rdfs:Class ;
	rdfs:comment      "Entities that have a somewhat fixed, physical location."@en ;
	rdfs:isDefinedBy  gs1: ;
	rdfs:label        "Place"@en ;
	rdfs:subClassOf   owl:Thing ;
	sw:term_status    "stable" ;
	skos:broadMatch   schema:Place .

gs1:PostalAddress
	rdf:type  owl:Class , rdfs:Class ;
	rdfs:comment      "The location at which a particular organization or person may be found or reached."@en ;
	rdfs:isDefinedBy  gs1: ;
	rdfs:label        "Address"@en ;
	rdfs:subClassOf   owl:Thing ;
	sw:term_status    "stable" ;
	skos:exactMatch   schema:PostalAddress .

gs1:PriceSpecification
	rdf:type          owl:Class , rdfs:Class ;
	rdfs:comment      "A structured value representing a monetary amount, consisting of a value and currency code."@en ;
	rdfs:isDefinedBy  gs1: ;
	rdfs:label        "Price Specification"@en ;
	rdfs:subClassOf   owl:Thing ;
	sw:term_status    "stable" ;
	skos:exactMatch   schema:PriceSpecification .

gs1:Product
	rdf:type     rdfs:Class , owl:Class ;
	rdfs:comment      "Any item (product or service) upon which there is a need to retrieve pre-defined information and that may be priced, or ordered, or invoiced at any point in any supply chain."@en ;
	rdfs:isDefinedBy  gs1: ;
	rdfs:label        "Product"@en ;
	rdfs:subClassOf   owl:Thing ;
	sw:term_status    "stable" ;
	skos:exactMatch   schema:Product .

gs1:ProductYieldDetails
	rdf:type          rdfs:Class , owl:Class ;
	rdfs:comment      "A grouping of properties related to the yield of a food or beverage product according to a specified type of preparation."@en ;
	rdfs:isDefinedBy  gs1: ;
	rdfs:label        "Product Yield Details"@en ;
	rdfs:subClassOf   owl:Thing ;
	sw:term_status    "stable" .

gs1:QuantitativeValue
	rdf:type          owl:Class , rdfs:Class ;
	rdfs:comment      "A point value or interval for product characteristics and other purposes. A unit of measurement is also specified."@en ;
	rdfs:isDefinedBy  gs1: ;
	rdfs:label        "Measurement Type"@en ;
	rdfs:subClassOf   owl:Thing ;
	sw:term_status    "stable" ;
	skos:exactMatch   schema:QuantitativeValue , gr:QuantitativeValue .

gs1:ReferencedFileDetails
	rdf:type          rdfs:Class , owl:Class ;
	rdfs:comment      "Provides URL and other information on a referenced electronic file."@en ;
	rdfs:isDefinedBy  gs1: ;
	rdfs:label        "Referenced File"@en ;
	rdfs:subClassOf   schema:MediaObject , owl:Thing ;
	sw:term_status    "stable" .

gs1:ReturnablePackageDepositDetails
	rdf:type          rdfs:Class , owl:Class ;
	rdfs:comment      "Details of the deposit for returnable packaging for a product."@en ;
	rdfs:isDefinedBy  gs1: ;
	rdfs:label        "Returnable Package Deposit Details"@en ;
	rdfs:subClassOf   owl:Thing ;
	sw:term_status    "stable" .

gs1:Seafood
	rdf:type     rdfs:Class , owl:Class ;
	rdfs:comment      "Seafood Products including fish and shellfish."@en ;
	rdfs:isDefinedBy  gs1: ;
	rdfs:label        "Seafood"@en ;
	rdfs:subClassOf   gs1:FoodBeverageTobaccoProduct ;
	sw:term_status    "stable" .

gs1:SizeCodeDetails
	rdf:type  owl:Class , rdfs:Class ;
	rdfs:comment      "A grouping of properties related to the representing the size of a product, by specifying a value from a specified code list."@en ;
	rdfs:isDefinedBy  gs1: ;
	rdfs:label        "Size Code Details"@en ;
	rdfs:subClassOf   owl:Thing ;
	sw:term_status    "stable" .

gs1:SizeDetails
	rdf:type  rdfs:Class , owl:Class ;
	rdfs:comment      "A grouping of properties related to the size of a wearable product"@en ;
	rdfs:isDefinedBy  gs1: ;
	rdfs:label        "Size Details"@en ;
	rdfs:subClassOf   owl:Thing ;
	sw:term_status    "stable" .

gs1:TargetMarketDetails
	rdf:type          rdfs:Class , owl:Class ;
	rdfs:comment      "A set of target market details (product release date and associated countries) for the product."@en ;
	rdfs:isDefinedBy  gs1: ;
	rdfs:label        "Target Market Details"@en ;
	rdfs:subClassOf   owl:Thing ;
	sw:term_status    "stable" .

gs1:TextileMaterialDetails
	rdf:type          rdfs:Class , owl:Class ;
	rdfs:comment      "Details on the composition of any materials used to make a product using textiles."@en ;
	rdfs:isDefinedBy  gs1: ;
	rdfs:label        "Textile Material"@en ;
	rdfs:subClassOf   owl:Thing ;
	sw:term_status    "stable" .

gs1:TypeCode
	rdf:type    rdfs:Class , owl:Class ;
	rdfs:comment      "A code list."@en ;
	rdfs:isDefinedBy  gs1: ;
	rdfs:label        "Type Code"@en ;
	rdfs:subClassOf   owl:Thing ;
	sw:term_status    "stable" .

gs1:WarrantyPromise
	rdf:type  owl:Class , rdfs:Class ;
	rdfs:comment      "An assurance that the product is reliable and that repairs or replacement will be done free of charge within a given time limit and under certain conditions in the event of a defect."@en ;
	rdfs:isDefinedBy  gs1: ;
	rdfs:label        "Warranty"@en ;
	rdfs:subClassOf   owl:Thing ;
	sw:term_status    "stable" ;
	skos:exactMatch   schema:WarrantyPromise .

gs1:WearableProduct
	rdf:type  owl:Class , rdfs:Class ;
	rdfs:comment      "Products that are worn on the body."@en ;
	rdfs:isDefinedBy  gs1: ;
	rdfs:label        "Wearable Product"@en ;
	rdfs:subClassOf   gs1:Product ;
	sw:term_status    "stable" .


gs1:acceptedPaymentMethod
	rdf:type          owl:ObjectProperty , rdf:Property ;
	rdfs:comment      "Code indicating a means of payment, for example, BANK_CHEQUE, CASH, etc."@en ;
	rdfs:domain       gs1:Offer ;
	rdfs:isDefinedBy  gs1: ;
	rdfs:label        "Accepted Payment Method"@en ;
	rdfs:range        gs1:PaymentMethod ;
	sw:term_status    "stable" ;
	skos:exactMatch   schema:acceptedPaymentMethod .

gs1:activityIdeas
	rdf:type  owl:ObjectProperty , rdf:Property ;
	rdfs:comment        "A link to ideas for using a product or engaging in other forms of entertainment, particularly with children."@en ;
	rdfs:domain         owl:Thing ;
	rdfs:label          "Activity Ideas"@en ;
	rdfs:range          xsd:anyURI ;
	rdfs:subPropertyOf  gs1:linkType ;
	sw:term_status      "stable" .

gs1:additionalLocationID
	rdf:type          owl:ObjectProperty , rdf:Property ;
	rdfs:comment      "Location identifiers assigned and managed by government bodies, trade organisations, and other entities."@en ;
	rdfs:domain       gs1:Place ;
	rdfs:isDefinedBy  gs1: ;
	rdfs:label        "Has Additional Location ID"@en ;
	rdfs:range        gs1:LocationID_Details ;
	sw:term_status    "stable" .

gs1:additionalOrganizationID
	rdf:type          owl:ObjectProperty , rdf:Property ;
	rdfs:comment      "Party/organisation identifiers assigned and managed by government bodies, trade organisations, and other entities."@en ;
	rdfs:domain       gs1:Organization ;
	rdfs:isDefinedBy  gs1: ;
	rdfs:label        "Has Additional Organization ID"@en ;
	rdfs:range        gs1:OrganizationID_Details ;
	sw:term_status    "stable" .

gs1:additionalOrganizationIdentificationTypeValue
	rdf:type          rdf:Property , owl:DatatypeProperty ;
	rdfs:comment      "The value associated with the Additional Organization Identification Type Value."@en ;
	rdfs:domain       gs1:Organization ;
	rdfs:isDefinedBy  gs1: ;
	rdfs:label        "Additional Organization Identification Type Value"@en ;
	rdfs:range        xsd:string ;
	sw:term_status    "stable" .

gs1:additionalProductClassification
	rdf:type          rdf:Property , owl:ObjectProperty ;
	rdfs:comment      "Relates to a set of additional product classification details"@en ;
	rdfs:domain       gs1:Product ;
	rdfs:isDefinedBy  gs1: ;
	rdfs:label        "Has Additional Product Classification"@en ;
	rdfs:range        gs1:AdditionalProductClassificationDetails ;
	sw:term_status    "stable" .

gs1:additionalProductClassificationCode
	rdf:type          owl:DatatypeProperty , owl:FunctionalProperty , rdf:Property ;
	rdfs:comment      "Code specifying the applied additional product classification scheme."@en ;
	rdfs:domain       gs1:AdditionalProductClassificationDetails ;
	rdfs:isDefinedBy  gs1: ;
	rdfs:label        "Additional Product Classification Code"@en ;
	rdfs:range        xsd:string ;
	sw:term_status    "stable" .

gs1:additionalProductClassificationCodeDescription
	rdf:type          owl:FunctionalProperty , owl:DatatypeProperty , rdf:Property ;
	rdfs:comment      "A description related to  the additional product classification code value."@en ;
	rdfs:domain       gs1:AdditionalProductClassificationDetails ;
	rdfs:isDefinedBy  gs1: ;
	rdfs:label        "Additional Product Classification Code Description"@en ;
	rdfs:range        rdf:langString ;
	sw:term_status    "stable" .

gs1:additionalProductClassificationValue
	rdf:type          rdf:Property , owl:DatatypeProperty , owl:FunctionalProperty ;
	rdfs:comment      "Code specifying an additional product classification other than the GS1 Global Product Classification. The applied classification scheme is specified as additional information together with the classification value."@en ;
	rdfs:domain       gs1:AdditionalProductClassificationDetails ;
	rdfs:isDefinedBy  gs1: ;
	rdfs:label        "Additional Product Classification Value"@en ;
	rdfs:range        xsd:string ;
	sw:term_status    "stable" .

gs1:additionalProductDescription
	rdf:type          owl:DatatypeProperty , owl:FunctionalProperty , rdf:Property ;
	rdfs:comment      "Additional variants necessary to communicate to the industry to help define the product. Multiple variants can be established for each GTIN for e.g. Style, Colour, and Fragrance ."@en ;
	rdfs:domain       gs1:Product ;
	rdfs:isDefinedBy  gs1: ;
	rdfs:label        "Additional Product Description"@en ;
	rdfs:range        rdf:langString ;
	sw:term_status    "stable" .

gs1:additive
	rdf:type    owl:ObjectProperty , rdf:Property ;
	rdfs:comment      "Relates to details about any additives that a product may contain."@en ;
	rdfs:domain       gs1:Product ;
	rdfs:isDefinedBy  gs1: ;
	rdfs:label        "Has Additive"@en ;
	rdfs:range        gs1:AdditiveDetails ;
	sw:term_status    "stable" .

gs1:additiveLevelOfContainment
	rdf:type          rdf:Property , owl:ObjectProperty , owl:FunctionalProperty ;
	rdfs:comment      "Code indicating the level of presence of the additive."@en ;
	rdfs:domain       gs1:AdditiveDetails ;
	rdfs:isDefinedBy  gs1: ;
	rdfs:label        "Additive Level Of Containment"@en ;
	rdfs:range        gs1:LevelOfContainmentCode ;
	sw:term_status    "stable" .

gs1:additiveName
	rdf:type  owl:FunctionalProperty , owl:DatatypeProperty , rdf:Property ;
	rdfs:comment      "The name of any additive or genetic modification contained or not contained in the product ."@en ;
	rdfs:domain       gs1:AdditiveDetails ;
	rdfs:isDefinedBy  gs1: ;
	rdfs:label        "Additive Name"@en ;
	rdfs:range        rdf:langString ;
	sw:term_status    "stable" .

gs1:address
	rdf:type     owl:ObjectProperty , rdf:Property ;
	rdfs:comment      "The postal address for an organization or place."@en ;
	rdfs:domain       _:b0 ;
	rdfs:isDefinedBy  gs1: ;
	rdfs:label        "Has Postal Address"@en ;
	rdfs:range        gs1:PostalAddress ;
	sw:term_status    "stable" ;
	skos:exactMatch   schema:address .

gs1:addressCountry
	rdf:type  rdf:Property , owl:ObjectProperty ;
	rdfs:comment      "Code specifying the country (and country subdivision) for the address using ISO 3166-1."@en ;
	rdfs:domain       gs1:PostalAddress ;
	rdfs:isDefinedBy  gs1: ;
	rdfs:label        "Address Country"@en ;
	rdfs:range        gs1:Country ;
	sw:term_status    "stable" ;
	skos:exactMatch   schema:addressCountry .

gs1:addressLocality
	rdf:type  owl:DatatypeProperty , rdf:Property ;
	rdfs:comment      "Text specifying the name of the locality, for example a city."@en ;
	rdfs:domain       gs1:PostalAddress ;
	rdfs:isDefinedBy  gs1: ;
	rdfs:label        "Address Locality"@en ;
	rdfs:range        rdf:langString ;
	sw:term_status    "stable" ;
	skos:exactMatch   schema:addressLocality , vcard:locality .

gs1:addressRegion
	rdf:type  rdf:Property , owl:DatatypeProperty ;
	rdfs:comment      "Text specifying a province or state in abbreviated format for example NJ."@en ;
	rdfs:domain       gs1:PostalAddress ;
	rdfs:isDefinedBy  gs1: ;
	rdfs:label        "Province State Code"@en ;
	rdfs:range        rdf:langString ;
	sw:term_status    "stable" ;
	skos:exactMatch   schema:addressRegion , vcard:region .

gs1:addressSuburb
	rdf:type  rdf:Property , owl:DatatypeProperty ;
	rdfs:comment      "A suburb within a town or city."@en ;
	rdfs:domain       gs1:PostalAddress ;
	rdfs:isDefinedBy  gs1: ;
	rdfs:label        "Address Suburb"@en ;
	rdfs:range        rdf:langString ;
	sw:term_status    "stable" .

gs1:afterHoursContact
	rdf:type            rdf:Property , owl:ObjectProperty ;
	rdfs:comment        "Links to after-hours contact information. For general contact details, gs1:contactPoint SHALL be used."@en ;
	rdfs:domain         _:b0 ;
	rdfs:isDefinedBy    gs1: ;
	rdfs:label          "Has After Hours Contact"@en ;
	rdfs:range          gs1:ContactPoint ;
	rdfs:subPropertyOf  schema:contactPoint , gs1:contactPoint ;
	sw:term_status      "stable" ;
	skos:broadMatch     schema:contactPoint .

gs1:alcoholicBeverageSubregion
	rdf:type          owl:DatatypeProperty , rdf:Property ;
	rdfs:comment      "A legally defined geographical region where the grapes for a wine were grown also known as an appellation. It is recommended to populate this property with an ISO 3166-2 code to indicate country and subdivision."@en ;
	rdfs:domain       gs1:Beverage ;
	rdfs:isDefinedBy  gs1: ;
	rdfs:label        "Alcoholic Beverage Sub-region"@en ;
	rdfs:range        rdf:langString ;
	sw:term_status    "stable" .

gs1:allergenInfo
	rdf:type  owl:ObjectProperty , rdf:Property ;
	rdfs:comment        "A link to a description of the allergen information."@en ;
	rdfs:domain         owl:Thing ;
	rdfs:label          "Allergen information"@en ;
	rdfs:range          xsd:anyURI ;
	rdfs:subPropertyOf  gs1:linkType ;
	sw:term_status      "stable" .

gs1:allergenLevelOfContainmentCode
	rdf:type          rdf:Property , owl:ObjectProperty ;
	rdfs:comment      "Code specifying the level of presence of the allergen."@en ;
	rdfs:domain       gs1:AllergenDetails ;
	rdfs:isDefinedBy  gs1: ;
	rdfs:label        "Allergen Level Of Containment"@en ;
	rdfs:range        gs1:LevelOfContainmentCode ;
	sw:term_status    "stable" .

gs1:allergenSpecificationAgency
	rdf:type          owl:DatatypeProperty , rdf:Property ;
	rdfs:comment      "The agency or other organization that defines or manages the criteria for allergen containment."@en ;
	rdfs:domain       gs1:FoodBeverageTobaccoProduct ;
	rdfs:isDefinedBy  gs1: ;
	rdfs:label        "Allergen Specification Agency"@en ;
	rdfs:range        rdf:langString ;
	sw:term_status    "stable" .

gs1:allergenSpecificationName
	rdf:type          rdf:Property , owl:DatatypeProperty ;
	rdfs:comment      "Free text field containing the name and version of the regulation or standard that defines the criteria of allergen containment."@en ;
	rdfs:domain       gs1:FoodBeverageTobaccoProduct ;
	rdfs:isDefinedBy  gs1: ;
	rdfs:label        "Allergen Specification Name"@en ;
	rdfs:range        rdf:langString ;
	sw:term_status    "stable" .

gs1:allergenStatement
	rdf:type          rdf:Property , owl:DatatypeProperty ;
	rdfs:comment      "Textual description of the presence or absence of allergens as governed by local rules and regulations, specified as one string."@en ;
	rdfs:domain       gs1:FoodBeverageTobaccoProduct ;
	rdfs:isDefinedBy  gs1: ;
	rdfs:label        "Allergen Statement"@en ;
	rdfs:range        rdf:langString ;
	sw:term_status    "stable" .

gs1:allergenType
	rdf:type  owl:ObjectProperty , rdf:Property ;
	rdfs:comment      "Code specifying the type of allergen."@en ;
	rdfs:domain       gs1:AllergenDetails ;
	rdfs:isDefinedBy  gs1: ;
	rdfs:label        "Allergen Type Code"@en ;
	rdfs:range        gs1:AllergenTypeCode ;
	sw:term_status    "stable" .

gs1:anatomicalForm
	rdf:type  owl:ObjectProperty , rdf:Property ;
	rdfs:comment      "Describes the meat product in terms of whether it is the whole animal or part of the animal which has been cut such as the muscle, bone, organ, or fat."@en ;
	rdfs:domain       gs1:MeatPoultry ;
	rdfs:isDefinedBy  gs1: ;
	rdfs:label        "Anatomical Form"@en ;
	rdfs:range        gs1:AnatomicalFormCode ;
	sw:term_status    "stable" .

gs1:appDownload
	rdf:type   owl:ObjectProperty , rdf:Property ;
	rdfs:comment        "A link to a related mobile app"@en ;
	rdfs:domain         owl:Thing ;
	rdfs:label          "App download"@en ;
	rdfs:range          xsd:anyURI ;
	rdfs:subPropertyOf  gs1:linkType ;
	sw:term_status      "stable" .

gs1:applicableTo
	rdf:type  rdf:Property , owl:DatatypeProperty ;
	rdfs:comment      "A property linking a gs1:linkType to the primary GS1 key(s) for which it can be used. Similar to rdfs:Domain but the value space is a GS1 Application Identifier, not a class."@en ;
	rdfs:domain       gs1:linkType ;
	rdfs:isDefinedBy  gs1: ;
	rdfs:label        "Applicable to"@en ;
	rdfs:range        gs1:AI ;
	sw:term_status    "stable" .

gs1:audioFile
	rdf:type   owl:ObjectProperty , rdf:Property ;
	rdfs:comment      "Link to a file containing an audio clip which is relevant to the product. Examples are commercials, or instructional/ how to use audio files."@en ;
	rdfs:domain       gs1:Product ;
	rdfs:isDefinedBy  gs1: ;
	rdfs:label        "Has Audio File"@en ;
	rdfs:range        gs1:ReferencedFileDetails ;
	sw:term_status    "stable" .

gs1:authenticity
	rdf:type  owl:ObjectProperty , rdf:Property ;
	rdfs:comment      "Links to details of covert/overt security markings that may be used to check authenticity of a product instance."@en ;
	rdfs:domain       gs1:Product ;
	rdfs:isDefinedBy  gs1: ;
	rdfs:label        "Has Authenticity Details"@en ;
	rdfs:range        gs1:AuthenticityDetails ;
	sw:term_status    "stable" .

gs1:authenticitySecurityFeatureInstructions
	rdf:type          owl:DatatypeProperty , rdf:Property ;
	rdfs:comment      "Provides human-readable instructions about how to locate a physical security marking and read a value from it."@en ;
	rdfs:domain       gs1:AuthenticityDetails ;
	rdfs:isDefinedBy  gs1: ;
	rdfs:label        "Authenticity Security Feature Instructions"@en ;
	rdfs:range        rdf:langString ;
	sw:term_status    "stable" .

gs1:authenticitySecurityFeatureInstructionsURL
	rdf:type          owl:ObjectProperty , rdf:Property ;
	rdfs:comment      "Links to online instructions about how to locate a physical security marking and read a value from it."@en ;
	rdfs:domain       gs1:AuthenticityDetails ;
	rdfs:isDefinedBy  gs1: ;
	rdfs:label        "Authenticity Security Feature Instructions Link"@en ;
	rdfs:range        xsd:anyURI ;
	sw:term_status    "stable" .

gs1:authenticitySecurityFeatureRegularExpression
	rdf:type          owl:DatatypeProperty , rdf:Property ;
	rdfs:comment      "Links to a regular expression to be used to perform syntax validation (plausibility checking) of a string value read from a physical security marking."@en ;
	rdfs:domain       gs1:AuthenticityDetails ;
	rdfs:isDefinedBy  gs1: ;
	rdfs:label        "Authenticity Security Feature Regular Expression"@en ;
	rdfs:range        xsd:string ;
	sw:term_status    "stable" .

gs1:authenticitySecurityFeatureType
	rdf:type          owl:ObjectProperty , rdf:Property ;
	rdfs:comment      "Links to a URI code value indicating a particular type of physical security marking."@en ;
	rdfs:domain       gs1:AuthenticityDetails ;
	rdfs:isDefinedBy  gs1: ;
	rdfs:label        "Authenticity Security Feature Type"@en ;
	rdfs:range        gs1:SecurityMarking ;
	sw:term_status    "stable" .

gs1:authenticitySecurityFeatureValue
	rdf:type          owl:DatatypeProperty , rdf:Property ;
	rdfs:comment      "Links to a string value read from a physical security marking."@en ;
	rdfs:domain       gs1:AuthenticityDetails ;
	rdfs:isDefinedBy  gs1: ;
	rdfs:label        "Authenticity Security Feature Value"@en ;
	rdfs:range        xsd:string ;
	sw:term_status    "stable" .

gs1:availabilityEnds
	rdf:type  owl:DatatypeProperty , rdf:Property ;
	rdfs:comment      "The date from which the product is no longer available from the information provider, including seasonal or temporary product and services ."@en ;
	rdfs:domain       gs1:Offer ;
	rdfs:isDefinedBy  gs1: ;
	rdfs:label        "Availability Ends"@en ;
	rdfs:range        xsd:dateTime ;
	sw:term_status    "stable" ;
	skos:exactMatch   schema:availabilityEnds .

gs1:availabilityStarts
	rdf:type          rdf:Property , owl:DatatypeProperty ;
	rdfs:comment      "The date from which the product is available from the information provider, including seasonal or temporary product and services."@en ;
	rdfs:domain       gs1:Offer ;
	rdfs:isDefinedBy  gs1: ;
	rdfs:label        "Availability Starts"@en ;
	rdfs:range        xsd:dateTime ;
	sw:term_status    "stable" ;
	skos:exactMatch   schema:availabilityStarts .

gs1:availableAtOrFrom
	rdf:type          rdf:Property , owl:ObjectProperty ;
	rdfs:comment      "The location the offered product or service is available from."@en ;
	rdfs:domain       gs1:Offer ;
	rdfs:isDefinedBy  gs1: ;
	rdfs:label        "Available At/From"@en ;
	rdfs:range        gs1:Place ;
	sw:term_status    "stable" ;
	skos:exactMatch   schema:availableAtOrFrom .

gs1:availableLanguage
	rdf:type            rdf:Property , owl:DatatypeProperty ;
	rdfs:comment        "ISO 639-1 code specifying the language of a specified contact point."@en ;
	rdfs:domain         gs1:ContactPoint ;
	rdfs:isDefinedBy    gs1: ;
	rdfs:label          "Available Language"@en ;
	rdfs:range          xsd:string ;
	rdfs:subPropertyOf  schema:availableLanguage ;
	sw:term_status      "stable" ;
	skos:related        schema:ContactPoint .

gs1:awardPrize
	rdf:type  rdf:Property , owl:ObjectProperty ;
	rdfs:comment      "An award or prize given to the product."@en ;
	rdfs:domain       gs1:Product ;
	rdfs:isDefinedBy  gs1: ;
	rdfs:label        "Has Award Prize"@en ;
	rdfs:range        gs1:AwardPrizeDetails ;
	sw:term_status    "stable" .

gs1:awardPrizeCode
	rdf:type  owl:DatatypeProperty , rdf:Property ;
	rdfs:comment      "Indicates the achievement of the product in relation to a prize or award, e.g. winner, runner-up, shortlisted."@en ;
	rdfs:domain       gs1:AwardPrizeDetails ;
	rdfs:isDefinedBy  gs1: ;
	rdfs:label        "Award Prize Code"@en ;
	rdfs:range        xsd:string ;
	sw:term_status    "stable" .

gs1:awardPrizeCountryCode
	rdf:type          owl:ObjectProperty , rdf:Property ;
	rdfs:comment      "An ISO standard code identifying the country in which a prize or award is given. It is recommended to populate this property with an ISO 3166-1 country code."@en ;
	rdfs:domain       gs1:AwardPrizeDetails ;
	rdfs:isDefinedBy  gs1: ;
	rdfs:label        "Award Prize Country Code"@en ;
	rdfs:range        gs1:Country ;
	sw:term_status    "stable" .

gs1:awardPrizeDescription
	rdf:type          rdf:Property , owl:DatatypeProperty ;
	rdfs:comment      "Text that describes the awards won."@en ;
	rdfs:domain       gs1:AwardPrizeDetails ;
	rdfs:isDefinedBy  gs1: ;
	rdfs:label        "Award Prize Description"@en ;
	rdfs:range        rdf:langString ;
	sw:term_status    "stable" .

gs1:awardPrizeJury
	rdf:type  owl:DatatypeProperty , rdf:Property ;
	rdfs:comment      "Free text listing members of the jury that awarded the prize."@en ;
	rdfs:domain       gs1:AwardPrizeDetails ;
	rdfs:isDefinedBy  gs1: ;
	rdfs:label        "Award Prize Jury"@en ;
	rdfs:range        rdf:langString ;
	sw:term_status    "stable" .

gs1:awardPrizeName
	rdf:type  owl:DatatypeProperty , rdf:Property ;
	rdfs:comment      "The name of a prize or award which the product has received."@en ;
	rdfs:domain       gs1:AwardPrizeDetails ;
	rdfs:isDefinedBy  gs1: ;
	rdfs:label        "Award Prize Name"@en ;
	rdfs:range        rdf:langString ;
	sw:term_status    "stable" .

gs1:awardPrizeYear
	rdf:type  rdf:Property , owl:DatatypeProperty ;
	rdfs:comment      "The year in which a prize or award was given."@en ;
	rdfs:domain       gs1:AwardPrizeDetails ;
	rdfs:isDefinedBy  gs1: ;
	rdfs:label        "Award Prize Year"@en ;
	rdfs:range        xsd:gYear ;
	sw:term_status    "stable" .

gs1:baseLocation
	rdf:type  owl:ObjectProperty , rdf:Property ;
	rdfs:comment      "A fixed physical location where a mobile location most commonly resides. If gs1:glnType is present, gs1:baseLocationGLN SHALL only be used when gs1:glnType is gs1:GLN_TypeCode-MOBILE_PHYSICAL_LOCATION"@en ;
	rdfs:domain       gs1:Place ;
	rdfs:isDefinedBy  gs1: ;
	rdfs:label        "Base Location"@en ;
	rdfs:range        gs1:Place ;
	sw:term_status    "stable" .

gs1:bestBeforeDate
	rdf:type  rdf:Property , owl:ObjectProperty ;
	rdfs:comment      "Best before date on the label or package signifies the end of the period under which the product will retain specific quality attributes or claims even though the product may continue to retain positive quality attributes after this date. Best before date is primarily used for consumer information and may be a regulatory requirement."@en ;
	rdfs:domain       schema:Product , gs1:Product ;
	rdfs:isDefinedBy  gs1: ;
	rdfs:label        "Best Before Date"@en ;
	rdfs:range        xsd:date ;
	sw:term_status    "stable" ;
	skos:altLabel     "Best Before Date"@en ;
	skos:notation     "15"^^gs1:AI ;
	skos:prefLabel    "15" .

gs1:beverageVintage
	rdf:type  rdf:Property , owl:DatatypeProperty ;
	rdfs:comment      "The year in which the majority of ingredients are harvested and/or the alcoholic beverage is produced. Determination as to whether the vintage year is the harvest date or production date is according to requirements in the Target Market."@en ;
	rdfs:domain       gs1:Beverage ;
	rdfs:isDefinedBy  gs1: ;
	rdfs:label        "Beverage Vintage"@en ;
	rdfs:range        xsd:string ;
	sw:term_status    "stable" .

gs1:biotinPerNutrientBasis
	rdf:type          owl:ObjectProperty , rdf:Property ;
	rdfs:comment      "Biotin Acid per specified nutrient basis quantity."@en ;
	rdfs:domain       gs1:FoodBeverageTobaccoProduct ;
	rdfs:isDefinedBy  gs1: ;
	rdfs:label        "Biotin Per Nutrient Basis Quantity"@en ;
	rdfs:range        gs1:NutritionMeasurementType ;
	sw:term_status    "stable" .

gs1:bonelessClaim
	rdf:type  owl:ObjectProperty , rdf:Property ;
	rdfs:comment      "The descriptive term that is used by the product manufacturer to identify whether the product makes a specific claim to contain no bones."@en ;
	rdfs:domain       gs1:MeatPoultry ;
	rdfs:isDefinedBy  gs1: ;
	rdfs:label        "Boneless Claim"@en ;
	rdfs:range        gs1:NonbinaryLogicCode ;
	sw:term_status    "stable" .

gs1:brand
	rdf:type         owl:ObjectProperty , rdf:Property ;
	rdfs:comment        "The brand of the product that appears on the consumer package."@en ;
	rdfs:domain         gs1:Product ;
	rdfs:isDefinedBy    gs1: ;
	rdfs:label          "Has Brand"@en ;
	rdfs:range          gs1:Brand ;
	rdfs:subPropertyOf  schema:brand ;
	sw:term_status      "stable" .

gs1:brandHomepageClinical
	rdf:type            owl:ObjectProperty , rdf:Property ;
	rdfs:comment        "A link to a brand presence aimed at clinical professionals."@en ;
	rdfs:domain         owl:Thing ;
	rdfs:label          "Information for professionals about this brand"@en ;
	rdfs:range          xsd:anyURI ;
	rdfs:subPropertyOf  gs1:linkType ;
	sw:term_status      "stable" .

gs1:brandHomepagePatient
	rdf:type            owl:ObjectProperty , rdf:Property ;
	rdfs:comment        "A link to a brand presence aimed at patients."@en ;
	rdfs:domain         owl:Thing ;
	rdfs:label          "Information for patients about this brand"@en ;
	rdfs:range          xsd:anyURI ;
	rdfs:subPropertyOf  gs1:linkType ;
	sw:term_status      "stable" .

gs1:brandName
	rdf:type     rdf:Property , owl:DatatypeProperty ;
	rdfs:comment        "The brand name of the product that appears on the consumer package."@en ;
	rdfs:domain         gs1:Brand ;
	rdfs:isDefinedBy    gs1: ;
	rdfs:label          "Brand Name"@en ;
	rdfs:range          rdf:langString ;
	rdfs:subPropertyOf  schema:name ;
	sw:term_status      "stable" ;
	skos:related        schema:Brand .

gs1:brandOwner
	rdf:type    owl:ObjectProperty , rdf:Property ;
	rdfs:comment        "The brand owner of the product. The organization that is responsible for allocating the GTIN to the product."@en ;
	rdfs:domain         gs1:Product ;
	rdfs:isDefinedBy    gs1: ;
	rdfs:label          "Has Brand Owner"@en ;
	rdfs:range          gs1:Organization ;
	rdfs:subPropertyOf  schema:brand ;
	sw:term_status      "stable" .

gs1:calciumPerNutrientBasis
	rdf:type          owl:ObjectProperty , rdf:Property ;
	rdfs:comment      "Calcium per specified nutrient basis quantity."@en ;
	rdfs:domain       gs1:FoodBeverageTobaccoProduct ;
	rdfs:isDefinedBy  gs1: ;
	rdfs:label        "Calcium Per Nutrient Basis Quantity"@en ;
	rdfs:range        gs1:NutritionMeasurementType ;
	sw:term_status    "stable" .

gs1:carbohydratesPerNutrientBasis
	rdf:type          rdf:Property , owl:ObjectProperty ;
	rdfs:comment      "Carbohydrates per specified nutrient basis quantity."@en ;
	rdfs:domain       gs1:FoodBeverageTobaccoProduct ;
	rdfs:isDefinedBy  gs1: ;
	rdfs:label        "Carbohydrates Per Nutrient Basis Quantity"@en ;
	rdfs:range        gs1:NutritionMeasurementType ;
	sw:term_status    "stable" .

gs1:careersInfo
	rdf:type   owl:ObjectProperty , rdf:Property ;
	rdfs:comment        "A link to information about jobs, careers, or other employment opportunities associated to an organisation or location."@en ;
	rdfs:domain         owl:Thing ;
	rdfs:label          "Careers information"@en ;
	rdfs:range          xsd:anyURI ;
	rdfs:subPropertyOf  gs1:linkType ;
	sw:term_status      "stable" .

gs1:catchZone
	rdf:type   owl:DatatypeProperty , rdf:Property ;
	rdfs:comment      "Free text field describing the sea zone from which the product was caught in."@en ;
	rdfs:domain       gs1:Seafood ;
	rdfs:isDefinedBy  gs1: ;
	rdfs:label        "Catch Zone"@en ;
	rdfs:range        rdf:langString ;
	sw:term_status    "stable" .

gs1:certification
	rdf:type  owl:ObjectProperty , rdf:Property ;
	rdfs:comment      "Certification information about a product, organisation or location."@en ;
	rdfs:domain       [ rdf:type     owl:Class ;
	owl:unionOf  ( gs1:Product gs1:Organization gs1:Place )
	] ;
	rdfs:isDefinedBy  gs1: ;
	rdfs:label        "Has Certification"@en ;
	rdfs:range        gs1:CertificationDetails ;
	sw:term_status    "stable" .

gs1:certificationAgency
	rdf:type          owl:DatatypeProperty , rdf:Property ;
	rdfs:comment      "Name of the organisation issuing the certification standard or other requirement being met ."@en ;
	rdfs:domain       gs1:CertificationDetails ;
	rdfs:isDefinedBy  gs1: ;
	rdfs:label        "Certification Agency"@en ;
	rdfs:range        rdf:langString ;
	sw:term_status    "stable" .

gs1:certificationAgencyURL
	rdf:type          owl:ObjectProperty , rdf:Property ;
	rdfs:comment      "URL of the organisation issuing the certification standard or other requirement being met. e.g. https://www.msc.org , https://www.fsc.org"@en ;
	rdfs:domain       gs1:CertificationDetails ;
	rdfs:isDefinedBy  gs1: ;
	rdfs:label        "Certification Agency URL"@en ;
	rdfs:range        gs1:Organization ;
	sw:term_status    "stable" .

gs1:certificationAuditDate
	rdf:type          rdf:Property , owl:DatatypeProperty ;
	rdfs:comment      "Date of completion of the auditing needed for certification"@en ;
	rdfs:domain       gs1:CertificationDetails ;
	rdfs:isDefinedBy  gs1: ;
	rdfs:label        "Certification Audit Date"@en ;
	rdfs:range        xsd:date ;
	sw:term_status    "stable" .

gs1:certificationEndDate
	rdf:type          rdf:Property , owl:DatatypeProperty ;
	rdfs:comment      "Last date of validity for the certification. (After this date the certification lapses and would need to be renewed/replaced)"@en ;
	rdfs:domain       gs1:CertificationDetails ;
	rdfs:isDefinedBy  gs1: ;
	rdfs:label        "Certification End Date"@en ;
	rdfs:range        xsd:date ;
	sw:term_status    "stable" .

gs1:certificationIdentification
	rdf:type          rdf:Property , owl:DatatypeProperty ;
	rdfs:comment      "A reference (i.e, to a certificate instance) issued to confirm that a product, party or location has passed certification. e.g. 'XSC-C-12345'"@en ;
	rdfs:domain       gs1:CertificationDetails ;
	rdfs:isDefinedBy  gs1: ;
	rdfs:label        "Certification Identification"@en ;
	rdfs:range        xsd:string ;
	sw:term_status    "stable" .

gs1:certificationInfo
	rdf:type            owl:ObjectProperty , rdf:Property ;
	rdfs:comment        "A link to certification information."@en ;
	rdfs:domain         owl:Thing ;
	rdfs:label          "Certification Information"@en ;
	rdfs:range          xsd:anyURI ;
	rdfs:subPropertyOf  gs1:linkType ;
	sw:term_status      "stable" .

gs1:certificationStandard
	rdf:type          rdf:Property , owl:DatatypeProperty ;
	rdfs:comment      "Name of the certification standard. Free text. Example: 'Egg classification' ."@en ;
	rdfs:domain       gs1:CertificationDetails ;
	rdfs:isDefinedBy  gs1: ;
	rdfs:label        "Certification Standard"@en ;
	rdfs:range        rdf:langString ;
	sw:term_status    "stable" .

gs1:certificationStartDate
	rdf:type          rdf:Property , owl:DatatypeProperty ;
	rdfs:comment      "First date of validity for the certification"@en ;
	rdfs:domain       gs1:CertificationDetails ;
	rdfs:isDefinedBy  gs1: ;
	rdfs:label        "Certification Start Date"@en ;
	rdfs:range        xsd:date ;
	sw:term_status    "stable" .

gs1:certificationStatement
	rdf:type          rdf:Property , owl:DatatypeProperty ;
	rdfs:comment      "Certification scope statement of the individual certification instance. The same certificationStandard can be issued with different values of certificationStatement in different instances."@en ;
	rdfs:domain       gs1:CertificationDetails ;
	rdfs:isDefinedBy  gs1: ;
	rdfs:label        "Certification Statement"@en ;
	rdfs:range        rdf:langString ;
	sw:term_status    "stable" .

gs1:certificationStatus
	rdf:type          rdf:Property , owl:ObjectProperty ;
	rdfs:comment      "Indicates the current status of the certification, e.g. active or inactive."@en ;
	rdfs:domain       gs1:CertificationDetails ;
	rdfs:isDefinedBy  gs1: ;
	rdfs:label        "Certification Status"@en ;
	rdfs:range        gs1:CertificationStatus ;
	sw:term_status    "stable" .

gs1:certificationSubject
	rdf:type          rdf:Property , owl:ObjectProperty ;
	rdfs:comment      "References the object (e.g. product, asset, container), party or location being certified. If multiple values are specified, the certification details apply to the logical conjunction (AND) of groups of different types, while a logical disjunction (OR) applies within each group of the same type. For example, two sibling organisations O1 and O2 can process products P1 and P2 at locations L1 and L2: meaning that either organisation can process either product at either location (OR); but the certificate holds for the combinations of organisation (either O1 OR O2) AND product (either P1 OR P2) AND location (either L1 OR L2)"@en ;
	rdfs:domain       gs1:CertificationDetails ;
	rdfs:isDefinedBy  gs1: ;
	rdfs:label        "Certification Subject"@en ;
	rdfs:range        owl:Thing ;
	sw:term_status    "stable" .

gs1:certificationType
	rdf:type          rdf:Property , owl:ObjectProperty ;
	rdfs:comment      "Indicates the type of certification"@en ;
	rdfs:domain       gs1:CertificationDetails ;
	rdfs:isDefinedBy  gs1: ;
	rdfs:label        "Certification Type"@en ;
	rdfs:range        owl:Thing ;
	sw:term_status    "stable" .

gs1:certificationURI
	rdf:type  rdf:Property , owl:DatatypeProperty ;
	rdfs:comment      "If gs1:certificationURI is present, it should point to data about this individual certificate within a repository maintained by the certification agency."@en ;
	rdfs:domain       gs1:CertificationDetails ;
	rdfs:isDefinedBy  gs1: ;
	rdfs:label        "Certification URI"@en ;
	rdfs:range        xsd:anyURI ;
	sw:term_status    "stable" .

gs1:certificationValue
	rdf:type          rdf:Property , owl:DatatypeProperty ;
	rdfs:comment      "The certification's standard value. Example: '4'."@en ;
	rdfs:domain       gs1:CertificationDetails ;
	rdfs:isDefinedBy  gs1: ;
	rdfs:label        "Certification Value"@en ;
	rdfs:range        rdf:langString ;
	sw:term_status    "stable" .

gs1:cheeseFirmness
	rdf:type  owl:ObjectProperty , rdf:Property ;
	rdfs:comment      "The firmness of the cheese product for example EXTRA_HARD."@en ;
	rdfs:domain       gs1:MilkButterCreamYogurtCheeseEggsSubstitutes ;
	rdfs:isDefinedBy  gs1: ;
	rdfs:label        "Cheese Firmness"@en ;
	rdfs:range        gs1:CheeseFirmnessCode ;
	sw:term_status    "stable" .

gs1:cheeseMaturationPeriodDescription
	rdf:type          owl:DatatypeProperty , rdf:Property ;
	rdfs:comment      "A descriptive way to specify a date range as some cheeses are matured over a period of time, but not an exact period. For example 3 to 4 weeks, over 1 year etc. The term maturation is also known in other markets as Aged."@en ;
	rdfs:domain       gs1:MilkButterCreamYogurtCheeseEggsSubstitutes ;
	rdfs:isDefinedBy  gs1: ;
	rdfs:label        "Cheese Maturation Period Description"@en ;
	rdfs:range        rdf:langString ;
	sw:term_status    "stable" .

gs1:chloridePerNutrientBasis
	rdf:type          rdf:Property , owl:ObjectProperty ;
	rdfs:comment      "Chloride per specified nutrient basis quantity."@en ;
	rdfs:domain       gs1:FoodBeverageTobaccoProduct ;
	rdfs:isDefinedBy  gs1: ;
	rdfs:label        "Chloride Per Nutrient Basis Quantity"@en ;
	rdfs:range        gs1:NutritionMeasurementType ;
	sw:term_status    "stable" .

gs1:cholesterolPerNutrientBasis
	rdf:type          rdf:Property , owl:ObjectProperty ;
	rdfs:comment      "Cholesterol per specified nutrient basis quantity."@en ;
	rdfs:domain       gs1:FoodBeverageTobaccoProduct ;
	rdfs:isDefinedBy  gs1: ;
	rdfs:label        "Cholesterol Per Nutrient Basis Quantity"@en ;
	rdfs:range        gs1:NutritionMeasurementType ;
	sw:term_status    "stable" .

gs1:chromiumPerNutrientBasis
	rdf:type          owl:ObjectProperty , rdf:Property ;
	rdfs:comment      "Chromium per specified nutrient basis quantity."@en ;
	rdfs:domain       gs1:FoodBeverageTobaccoProduct ;
	rdfs:isDefinedBy  gs1: ;
	rdfs:label        "Chromium Per Nutrient Basis Quantity"@en ;
	rdfs:range        gs1:NutritionMeasurementType ;
	sw:term_status    "stable" .

gs1:circle
	rdf:type      rdf:Property , owl:DatatypeProperty ;
	rdfs:comment      "A circle is the circular region of a specified radius centred at a specified latitude and longitude. A circle is expressed as a pair followed by a radius in meters."@en ;
	rdfs:domain       gs1:GeoShape ;
	rdfs:isDefinedBy  gs1: ;
	rdfs:label        "Circle"@en ;
	rdfs:range        xsd:string ;
	sw:term_status    "stable" ;
	skos:exactMatch   schema:circle .

gs1:clothingCut
	rdf:type  owl:DatatypeProperty , rdf:Property ;
	rdfs:comment      "Supplemental information to indicate the clothing cut or silhouette make of the garment. For example, silhouette details for a pair of jeans such as boot cut, or loose fit, comfort fit."@en ;
	rdfs:domain       gs1:Clothing ;
	rdfs:isDefinedBy  gs1: ;
	rdfs:label        "Clothing Cut"@en ;
	rdfs:range        rdf:langString ;
	sw:term_status    "stable" .

gs1:collarType
	rdf:type  rdf:Property , owl:DatatypeProperty ;
	rdfs:comment      "A free text description of the type of collar on the garment."@en ;
	rdfs:domain       gs1:Clothing ;
	rdfs:isDefinedBy  gs1: ;
	rdfs:label        "Collar Type"@en ;
	rdfs:range        rdf:langString ;
	sw:term_status    "stable" .

gs1:colourCode
	rdf:type  rdf:Property , owl:ObjectProperty ;
	rdfs:comment      "Relates to a set of details about the colour code for a product"@en ;
	rdfs:domain       gs1:Product ;
	rdfs:isDefinedBy  gs1: ;
	rdfs:label        "Has Colour Code"@en ;
	rdfs:range        gs1:ColourCodeDetails ;
	sw:term_status    "stable" .

gs1:colourCodeList
	rdf:type  owl:FunctionalProperty , owl:ObjectProperty , rdf:Property ;
	rdfs:comment      "The parties controlling the colour code lists. Dependent on colour code value."@en ;
	rdfs:domain       gs1:ColourCodeDetails ;
	rdfs:isDefinedBy  gs1: ;
	rdfs:label        "Colour Code List"@en ;
	rdfs:range        gs1:ColourCodeListCode ;
	sw:term_status    "stable" .

gs1:colourCodeValue
	rdf:type  owl:FunctionalProperty , owl:DatatypeProperty , rdf:Property ;
	rdfs:comment      "A code indicating the colour of an object according to a specific code list. The applied code list is specified as additional information together with the colour code."@en ;
	rdfs:domain       gs1:ColourCodeDetails ;
	rdfs:isDefinedBy  gs1: ;
	rdfs:label        "Colour Code"@en ;
	rdfs:range        xsd:string ;
	sw:term_status    "stable" .

gs1:colourDescription
	rdf:type          owl:DatatypeProperty , rdf:Property , owl:FunctionalProperty ;
	rdfs:comment      "A description of the colour of an object."@en ;
	rdfs:domain       gs1:Product ;
	rdfs:isDefinedBy  gs1: ;
	rdfs:label        "Colour Description"@en ;
	rdfs:range        rdf:langString ;
	sw:term_status    "stable" ;
	skos:closeMatch   schema:color ;
	skos:related      schema:Product .

gs1:consumerFirstAvailabilityDateTime
	rdf:type          rdf:Property , owl:DatatypeProperty , owl:FunctionalProperty ;
	rdfs:comment      "The first date/time that the buyer is allowed to sell the product to consumers. Usually related to a specific geography. ISO 8601 date format CCYY-MM-DDTHH:MM:SS."@en ;
	rdfs:domain       gs1:TargetMarketDetails ;
	rdfs:isDefinedBy  gs1: ;
	rdfs:label        "Consumer First Availability Date Time"@en ;
	rdfs:range        xsd:dateTime ;
	sw:term_status    "stable" .

gs1:consumerHandlingStorage
	rdf:type          owl:ObjectProperty , rdf:Property ;
	rdfs:comment      "Link to a website, file, or image containing the manufacturer's recommendations for how the consumer or end user should store and handle the product."@en ;
	rdfs:domain       gs1:Product ;
	rdfs:isDefinedBy  gs1: ;
	rdfs:label        "Has Consumer Handling Storage"@en ;
	rdfs:range        gs1:ReferencedFileDetails ;
	sw:term_status    "stable" .

gs1:consumerHandlingStorageInfo
	rdf:type            owl:ObjectProperty , rdf:Property ;
	rdfs:comment        "A link to information about safe handling and storage for consumer use."@en ;
	rdfs:domain         owl:Thing ;
	rdfs:label          "Consumer handling and storage information"@en ;
	rdfs:range          xsd:anyURI ;
	rdfs:subPropertyOf  gs1:linkType ;
	sw:term_status      "stable" .

gs1:consumerLifestage
	rdf:type          rdf:Property , owl:ObjectProperty ;
	rdfs:comment      "Indicates, with reference to the product branding, labelling or packaging, the descriptive term that is used by the product manufacturer to identify the period or stage in the consumer's life during which the product is considered to be suitable."@en ;
	rdfs:domain       gs1:WearableProduct ;
	rdfs:isDefinedBy  gs1: ;
	rdfs:label        "Consumer Lifestage"@en ;
	rdfs:range        gs1:ConsumerLifestageCode ;
	sw:term_status    "stable" .

gs1:consumerPackageDisclaimer
	rdf:type          rdf:Property , owl:FunctionalProperty , owl:DatatypeProperty ;
	rdfs:comment      "Additional information that should be used in advertising and in displaying."@en ;
	rdfs:domain       gs1:Product ;
	rdfs:isDefinedBy  gs1: ;
	rdfs:label        "Consumer Package Disclaimer"@en ;
	rdfs:range        rdf:langString ;
	sw:term_status    "stable" .

gs1:consumerProductVariant
	rdf:type          owl:ObjectProperty , rdf:Property ;
	rdfs:comment      "The consumer product variant may be used to distinguish one variant of a retail consumer trade item from another if the change does not require the allocation of a different Global Trade Item Number (per the GTIN Management Standard), but communication between trading partners is required to support consumers. The brand owner is responsible for assigning the consumer product variant."@en ;
	rdfs:domain       gs1:Product , schema:Product ;
	rdfs:isDefinedBy  gs1: ;
	rdfs:label        "Consumer Product Variant"@en ;
	rdfs:range        xsd:string ;
	sw:term_status    "stable" ;
	skos:altLabel     "Consumer Product Variant"@en ;
	skos:notation     "22"^^gs1:AI ;
	skos:prefLabel    "22" .

gs1:consumerSafetyInformation
	rdf:type          owl:DatatypeProperty , owl:FunctionalProperty , rdf:Property ;
	rdfs:comment      "Information on consumer safety regarding the product."@en ;
	rdfs:domain       gs1:Product ;
	rdfs:isDefinedBy  gs1: ;
	rdfs:label        "Consumer Safety Information"@en ;
	rdfs:range        rdf:langString ;
	sw:term_status    "stable" .

gs1:consumerSalesCondition
	rdf:type          rdf:Property , owl:ObjectProperty ;
	rdfs:comment      "A code indicating restrictions imposed on the product regarding how it can be sold to the consumer for example Prescription Required."@en ;
	rdfs:domain       gs1:Product ;
	rdfs:isDefinedBy  gs1: ;
	rdfs:label        "Consumer Sales Condition Code"@en ;
	rdfs:range        gs1:ConsumerSalesConditionsCode ;
	sw:term_status    "stable" .

gs1:consumerStorageInstructions
	rdf:type          owl:DatatypeProperty , rdf:Property , owl:FunctionalProperty ;
	rdfs:comment      "Expresses in text the consumer storage instructions of a product which are normally held on the label or accompanying the product. This information may or may not be labelled on the pack."@en ;
	rdfs:domain       gs1:Product ;
	rdfs:isDefinedBy  gs1: ;
	rdfs:label        "Consumer Storage Instructions"@en ;
	rdfs:range        rdf:langString ;
	sw:term_status    "stable" .

gs1:consumerUsageInstructions
	rdf:type          owl:DatatypeProperty , owl:FunctionalProperty , rdf:Property ;
	rdfs:comment      "Free text containing the usage instructions of a product, which are normally held on the label or accompanying the product. This information may or may not be labelled on the pack."@en ;
	rdfs:domain       gs1:Product ;
	rdfs:isDefinedBy  gs1: ;
	rdfs:label        "Consumer Usage Instructions"@en ;
	rdfs:range        rdf:langString ;
	sw:term_status    "stable" .

gs1:contactPoint
	rdf:type  owl:ObjectProperty , rdf:Property ;
	rdfs:comment        "Contact information. To specify a contact specifically designated for after-hours support, see gs1:afterHoursContact"@en ;
	rdfs:domain         _:b0 ;
	rdfs:isDefinedBy    gs1: ;
	rdfs:label          "Has Business Contact"@en ;
	rdfs:range          gs1:ContactPoint ;
	rdfs:subPropertyOf  schema:contactPoint ;
	sw:term_status      "stable" .

gs1:contactTitle
	rdf:type  rdf:Property , owl:DatatypeProperty ;
	rdfs:comment      "The job title of the person that can be contacted for example Manager."@en ;
	rdfs:domain       gs1:ContactPoint ;
	rdfs:isDefinedBy  gs1: ;
	rdfs:label        "Contact Title"@en ;
	rdfs:range        rdf:langString ;
	sw:term_status    "stable" ;
	skos:closeMatch   schema:jobTitle ;
	skos:related      schema:Person .

gs1:contactType
	rdf:type  owl:DatatypeProperty , rdf:Property ;
	rdfs:comment      "The function or role of a contact for example Customer Support."@en ;
	rdfs:domain       gs1:ContactPoint ;
	rdfs:isDefinedBy  gs1: ;
	rdfs:label        "Contact Type"@en ;
	rdfs:range        rdf:langString ;
	sw:term_status    "stable" ;
	skos:exactMatch   schema:contactType .

gs1:containedInPlace
	rdf:type  owl:ObjectProperty , rdf:Property ;
	rdfs:comment      "Designates the larger physical location a sub-location is located within. To specify sub-locations of a physical location, see gs1:containsPlace."@en ;
	rdfs:domain       gs1:Place ;
	rdfs:isDefinedBy  gs1: ;
	rdfs:label        "Contained in Place"@en ;
	rdfs:range        gs1:Place ;
	sw:term_status    "stable" .

gs1:containsPlace
	rdf:type  owl:ObjectProperty , rdf:Property ;
	rdfs:comment      "Designates a sub-location (e.g., floor, room, shelf) within the physical location being identified. There may be multiple sub-locations associated to a single, physical location. To specify the larger physical location the sub-location is located within, see gs1:containedInPlace"@en ;
	rdfs:domain       gs1:Place ;
	rdfs:isDefinedBy  gs1: ;
	rdfs:label        "Contains Place"@en ;
	rdfs:range        gs1:Place ;
	sw:term_status    "stable" .

gs1:convenienceLevelPercent
	rdf:type          owl:DatatypeProperty , rdf:Property ;
	rdfs:comment      "An indication of the ease of preparation for semi-prepared products. The convenience level indicates the level of preparation in percentage required to prepare and helps the consumer to assess how long it will take to prepare the meal."@en ;
	rdfs:domain       gs1:FoodAndBeveragePreparationInformation ;
	rdfs:isDefinedBy  gs1: ;
	rdfs:label        "Convenience Level Percent"@en ;
	rdfs:range        xsd:float ;
	sw:term_status    "stable" .

gs1:coordinateReferenceSystem
	rdf:type          rdf:Property , owl:DatatypeProperty ;
	rdfs:comment      "Open standard spatial reference systems or coordinate reference systems that provide coordinate-based local, regional or global system used to locate geographical entities.  Values should be URIs already defined by the IOPG Geomatics Committee (https://epsg.org/), such as https://epsg.io/4326 (WGS84); https://epsg.io/4267 (NAD27); https://epsg.io/4230 (ED50); https://epsg.io/4618 (SAD69); https://epsg.io/4269 (NAD83).  For elevation values, gs1:elevation SHALL be used."@en ;
	rdfs:domain       gs1:GeoCoordinates ;
	rdfs:isDefinedBy  gs1: ;
	rdfs:label        "Coordinate Reference System"@en ;
	rdfs:range        xsd:anyURI ;
	sw:term_status    "stable" .

gs1:copperPerNutrientBasis
	rdf:type          rdf:Property , owl:ObjectProperty ;
	rdfs:comment      "Copper per specified nutrient basis quantity."@en ;
	rdfs:domain       gs1:FoodBeverageTobaccoProduct ;
	rdfs:isDefinedBy  gs1: ;
	rdfs:label        "Copper Per Nutrient Basis Quantity"@en ;
	rdfs:range        gs1:NutritionMeasurementType ;
	sw:term_status    "stable" .

gs1:countryCode
	rdf:type  rdf:Property , owl:DatatypeProperty ;
	rdfs:comment      "A short text string code (see values defined in ISO 3166) specifying the country in which a processing or other activity is performed, for example processing, bottling, manufacturing."@en , "Code specifying the country for the address using ISO 3166-1."@en ;
	rdfs:domain       gs1:Country ;
	rdfs:isDefinedBy  gs1: ;
	rdfs:label        "Country Code"@en ;
	rdfs:range        xsd:string ;
	sw:term_status    "stable" ;
	skos:closeMatch   schema:addressCountry ;
	skos:related      schema:PostalAddress .

gs1:countryOfAssembly
	rdf:type          rdf:Property , owl:ObjectProperty ;
	rdfs:comment      "The place where product is assembled."@en ;
	rdfs:domain       gs1:Product ;
	rdfs:isDefinedBy  gs1: ;
	rdfs:label        "Has Country Of Assembly"@en ;
	rdfs:range        gs1:Country ;
	sw:term_status    "stable" .

gs1:countryOfLastProcessing
	rdf:type          owl:ObjectProperty , rdf:Property ;
	rdfs:comment      "The place where the product or ingredient was last processed and tested before importation."@en ;
	rdfs:domain       gs1:Product ;
	rdfs:isDefinedBy  gs1: ;
	rdfs:label        "Has Country Of Last Processing"@en ;
	rdfs:range        gs1:Country ;
	sw:term_status    "stable" .

gs1:countryOfOrigin
	rdf:type  owl:ObjectProperty , rdf:Property ;
	rdfs:comment      "Code indicating the country of origin of the product."@en ;
	rdfs:domain       gs1:Product ;
	rdfs:isDefinedBy  gs1: ;
	rdfs:label        "Has Country Of Origin"@en ;
	rdfs:range        gs1:Country ;
	sw:term_status    "stable" .

gs1:countryOfOriginStatement
	rdf:type          owl:DatatypeProperty , rdf:Property , owl:FunctionalProperty ;
	rdfs:comment      "A description of the geographic area the item may have originated from or has been processed."@en ;
	rdfs:domain       gs1:Product ;
	rdfs:isDefinedBy  gs1: ;
	rdfs:label        "Country Of Origin Statement"@en ;
	rdfs:range        rdf:langString ;
	sw:term_status    "stable" .

gs1:countrySubdivisionCode
	rdf:type          owl:DatatypeProperty , rdf:Property ;
	rdfs:comment      "A short text string code (see values defined in ISO 3166_2) specifying the country subdivision in which an activity is performed, for example processing, bottling, manufacturing."@en ;
	rdfs:domain       gs1:Country ;
	rdfs:isDefinedBy  gs1: ;
	rdfs:label        "Country Subdivision Code"@en ;
	rdfs:range        xsd:string ;
	sw:term_status    "stable" .

gs1:countyCode
	rdf:type  owl:DatatypeProperty , rdf:Property ;
	rdfs:comment      "A code that identifies a county. A county is a territorial division in some countries, forming the chief unit of local administration. In the US, a county is a political and administrative division of a state."@en ;
	rdfs:domain       gs1:PostalAddress ;
	rdfs:isDefinedBy  gs1: ;
	rdfs:label        "County Code"@en ;
	rdfs:range        xsd:string ;
	sw:term_status    "stable" .

gs1:crossStreet
	rdf:type  rdf:Property , owl:DatatypeProperty ;
	rdfs:comment      "A street intersecting a main street (usually at right angles) and continuing on both sides of it."@en ;
	rdfs:domain       gs1:PostalAddress ;
	rdfs:isDefinedBy  gs1: ;
	rdfs:label        "Cross Street"@en ;
	rdfs:range        rdf:langString ;
	sw:term_status    "stable" .

gs1:customerSupportCentre
	rdf:type          owl:ObjectProperty , rdf:Property ;
	rdfs:comment      "The organization which provides product support to the trading partner organization to which merchandise is sold."@en ;
	rdfs:domain       gs1:Product ;
	rdfs:isDefinedBy  gs1: ;
	rdfs:label        "Has Customer Support Centre"@en ;
	rdfs:range        gs1:Organization ;
	sw:term_status    "stable" .

gs1:dailyValueIntakePercent
	rdf:type          owl:DatatypeProperty , rdf:Property ;
	rdfs:comment      "The percentage of the recommended daily intake of a nutrient as recommended by authorities of the target market. Is expressed relative to the serving size and base daily value intake."@en ;
	rdfs:domain       gs1:NutritionMeasurementType ;
	rdfs:isDefinedBy  gs1: ;
	rdfs:label        "Daily Value Intake Percent"@en ;
	rdfs:range        xsd:float .

gs1:defaultLink
	rdf:type   owl:ObjectProperty , rdf:Property ;
	rdfs:comment        "The default link for a given identified item to which a resolver will redirect unless there is information in the request that is a better match."@en ;
	rdfs:domain         owl:Thing ;
	rdfs:label          "Default link"@en ;
	rdfs:range          xsd:anyURI ;
	rdfs:subPropertyOf  gs1:linkType ;
	sw:term_status      "stable" .

gs1:defaultLinkMulti
	rdf:type  owl:ObjectProperty , rdf:Property ;
	rdfs:comment        "A set of 'default links' that may be differentiated by information in the HTTP request headers sent to a resolver to enable a better match than the single default link."@en ;
	rdfs:domain         owl:Thing ;
	rdfs:label          "Default linkMulti"@en ;
	rdfs:range          xsd:anyURI ;
	rdfs:subPropertyOf  gs1:linkType ;
	sw:term_status      "stable" .

gs1:department
	rdf:type  rdf:Property , owl:DatatypeProperty ;
	rdfs:comment      "The name of a division of an organization dealing with a specific activity"@en ;
	rdfs:domain       gs1:Organization ;
	rdfs:isDefinedBy  gs1: ;
	rdfs:label        "Department"@en ;
	rdfs:range        rdf:langString ;
	sw:term_status    "stable" ;
	skos:closeMatch   schema:department .

gs1:dependentProprietaryProduct
	rdf:type          rdf:Property , owl:ObjectProperty ;
	rdfs:comment      "Dependent products are products which are required to make the current product functional."@en ;
	rdfs:domain       gs1:Product ;
	rdfs:isDefinedBy  gs1: ;
	rdfs:label        "Has Dependent Proprietary Product"@en ;
	rdfs:range        gs1:Product ;
	rdfs:seeAlso      schema:isConsumableFor , schema:isAccessoryOrSparePartFor ;
	sw:term_status    "stable" ;
	skos:broadMatch   schema:isSimilarTo .

gs1:descriptiveSize
	rdf:type  rdf:Property , owl:FunctionalProperty , owl:DatatypeProperty ;
	rdfs:comment      "An alphanumeric size factor the brand owner wishes to communicate to the consumer. IE Jumbo, Capri, Full Length, Maxi."@en ;
	rdfs:domain       gs1:Product ;
	rdfs:isDefinedBy  gs1: ;
	rdfs:label        "Descriptive Size"@en ;
	rdfs:range        rdf:langString ;
	sw:term_status    "stable" .

gs1:dietCode
	rdf:type    rdf:Property , owl:DatatypeProperty ;
	rdfs:comment      "Links to multiple pairs of gs1:DietTypeCode and diet type sub code (free-form text string)."@en ;
	rdfs:domain       gs1:FoodBeverageTobaccoProduct ;
	rdfs:isDefinedBy  gs1: ;
	rdfs:label        "Diet Code"@en ;
	rdfs:range        gs1:DietTypeCodeDetails ;
	sw:term_status    "stable" .

gs1:dietType
	rdf:type    owl:ObjectProperty , rdf:Property ;
	rdfs:comment      "Code indicating the diet the product is suitable for example Kosher."@en ;
	rdfs:domain       gs1:DietTypeCodeDetails ;
	rdfs:isDefinedBy  gs1: ;
	rdfs:label        "Diet Type Code"@en ;
	rdfs:range        gs1:DietTypeCode ;
	sw:term_status    "stable" .

gs1:dietTypeDescription
	rdf:type          owl:DatatypeProperty , rdf:Property ;
	rdfs:comment      "Free text for indication of diet not stated in the list of diets."@en ;
	rdfs:domain       gs1:FoodBeverageTobaccoProduct ;
	rdfs:isDefinedBy  gs1: ;
	rdfs:label        "Diet Type Description"@en ;
	rdfs:range        rdf:langString ;
	sw:term_status    "stable" .

gs1:dietTypeSubcode
	rdf:type  owl:DatatypeProperty , rdf:Property ;
	rdfs:comment      "Indicates a set of agreements or a certificate name that guarantees the product is permitted in a particular diet. A diet type subcode is a subclassification of a specific diet type. For example, Pareve is a diet type subcode of Kosher."@en ;
	rdfs:domain       gs1:DietTypeCodeDetails ;
	rdfs:isDefinedBy  gs1: ;
	rdfs:label        "Diet Type Sub-code"@en ;
	rdfs:range        rdf:langString ;
	sw:term_status    "stable" .

gs1:digitalAddress
	rdf:type  owl:DatatypeProperty , rdf:Property ;
	rdfs:comment      "The location reference associated to a digital place. If gs1:glnType is present, SHALL only be associated if the value of gs1:glnType is gs1:GLN_TypeCode-DIGITAL_LOCATION."@en ;
	rdfs:domain       gs1:Place ;
	rdfs:isDefinedBy  gs1: ;
	rdfs:label        "Has Digital Address"@en ;
	rdfs:range        xsd:string ;
	sw:term_status    "stable" .

gs1:digitalLocationName
	rdf:type          owl:DatatypeProperty , rdf:Property ;
	rdfs:comment      "The name of a digital place. To specify the name of a physical location, see gs1:physicalLocationName."@en ;
	rdfs:domain       gs1:Place ;
	rdfs:isDefinedBy  gs1: ;
	rdfs:label        "Digital Location Name"@en ;
	rdfs:range        rdf:langString ;
	sw:term_status    "stable" .

gs1:discountRepeatsPerMultipleMinimum
	rdf:type          owl:DatatypeProperty , rdf:Property ;
	rdfs:comment      "If specified and set to true, the discount is available for each time the minimum qualifying criteria are met.  This can be used to express '$10 off each $50 spend', which is distinct from a 20% discount because it is quantized in units of spending."@en ;
	rdfs:domain       gs1:Discount ;
	rdfs:isDefinedBy  gs1: ;
	rdfs:label        "Discount Repeats Per Multiple Minimum"@en ;
	rdfs:range        xsd:boolean ;
	sw:term_status    "unstable" .

gs1:discountType
	rdf:type  rdf:Property , owl:DatatypeProperty ;
	rdfs:comment      "A code that specifies the type of payment discount applicable to an offer, for example BOGO."@en ;
	rdfs:domain       gs1:Discount ;
	rdfs:isDefinedBy  gs1: ;
	rdfs:label        "Discount Type"@en ;
	rdfs:range        gs1:DiscountTypeCode ;
	sw:term_status    "unstable" .

gs1:drainedWeight
	rdf:type  rdf:Property , owl:FunctionalProperty , owl:ObjectProperty ;
	rdfs:comment        "The weight of the product when drained of its liquid. For example 225 GRM, Jar of pickles in vinegar."@en ;
	rdfs:domain         gs1:FoodBeverageTobaccoProduct ;
	rdfs:isDefinedBy    gs1: ;
	rdfs:label          "Drained Weight"@en ;
	rdfs:range          gs1:QuantitativeValue ;
	rdfs:subPropertyOf  schema:weight ;
	sw:term_status      "stable" .

gs1:dueDate
	rdf:type     rdf:Property , owl:ObjectProperty ;
	rdfs:comment      "The date by which an invoice should be paid. This data element represents an attribute of a payment slip reference number, AI (8020), and a Global Location Number (GLN) of the invoicing party."@en ;
	rdfs:domain       gs1:Product , schema:Product ;
	rdfs:isDefinedBy  gs1: ;
	rdfs:label        "Due Date"@en ;
	rdfs:range        xsd:date ;
	sw:term_status    "stable" ;
	skos:altLabel     "Due Date"@en ;
	skos:notation     "12"^^gs1:AI ;
	skos:prefLabel    "12" .

gs1:durationOfWarranty
	rdf:type          owl:ObjectProperty , rdf:Property ;
	rdfs:comment      "The time period that the warranty is valid within."@en ;
	rdfs:domain       gs1:WarrantyPromise ;
	rdfs:isDefinedBy  gs1: ;
	rdfs:label        "Duration Of Warranty"@en ;
	rdfs:range        gs1:QuantitativeValue ;
	sw:term_status    "stable" ;
	skos:exactMatch   schema:durationOfWarranty .

gs1:dutyFeeTaxAmount
	rdf:type  rdf:Property , owl:DatatypeProperty ;
	rdfs:comment      "The current tax or duty or fee amount applicable to the product, expressed as a floating-point numeric value that is qualified by the corresponding currency. See also gs1:priceCurrency."@en ;
	rdfs:domain       gs1:PriceSpecification ;
	rdfs:isDefinedBy  gs1: ;
	rdfs:label        "Duty Fee Tax Amount"@en ;
	rdfs:range        xsd:float ;
	rdfs:seeAlso      gs1:priceCurrency ;
	sw:term_status    "stable" .

gs1:dutyFeeTaxDescription
	rdf:type          owl:DatatypeProperty , rdf:Property ;
	rdfs:comment      "A description of tax type for example Taxes sure les supports audio."@en ;
	rdfs:domain       gs1:PriceSpecification ;
	rdfs:isDefinedBy  gs1: ;
	rdfs:label        "Duty Fee Tax Description"@en ;
	rdfs:range        rdf:langString ;
	sw:term_status    "stable" .

gs1:dutyFeeTaxRate
	rdf:type  owl:DatatypeProperty , rdf:Property ;
	rdfs:comment      "The current tax or duty rate percentage applicable to the product."@en ;
	rdfs:domain       gs1:PriceSpecification ;
	rdfs:isDefinedBy  gs1: ;
	rdfs:label        "Duty Fee Tax Rate"@en ;
	rdfs:range        xsd:float ;
	sw:term_status    "stable" .

gs1:elevation
	rdf:type   rdf:Property , owl:DatatypeProperty ;
	rdfs:comment      "The elevation of a location (WGS 84). Values may be of the form 'NUMBER UNITOFMEASUREMENT' (e.g., '1,000 m', '3,200 ft') while numbers alone SHALL be a value in meters."@en ;
	rdfs:domain       gs1:GeoCoordinates ;
	rdfs:isDefinedBy  gs1: ;
	rdfs:label        "Elevation"@en ;
	rdfs:range        xsd:string ;
	sw:term_status    "stable" ;
	skos:exactMatch   schema:elevation .

gs1:eligibleQuantity
	rdf:type  rdf:Property , owl:ObjectProperty ;
	rdfs:comment        "The quantity including unit of measure for which the offer for good or service is valid.  If this is not specified, an eligible quantity of 1 should be assumed."@en ;
	rdfs:domain         _:b1 ;
	rdfs:isDefinedBy    gs1: ;
	rdfs:label          "Eligible Quantity"@en ;
	rdfs:range          gs1:QuantitativeValue ;
	rdfs:subPropertyOf  schema:eligibleQuantity ;
	sw:term_status      "stable" ;
	skos:exactMatch     schema:eligibleQuantity .

gs1:eligibleQuantityMaximum
	rdf:type            rdf:Property , owl:ObjectProperty ;
	rdfs:comment        "The maximum quantity including unit of measure for which the offer for good or service is valid."@en ;
	rdfs:domain         _:b1 ;
	rdfs:isDefinedBy    gs1: ;
	rdfs:label          "Eligible Quantity Maximum"@en ;
	rdfs:range          gs1:QuantitativeValue ;
	rdfs:subPropertyOf  schema:eligibleQuantity ;
	sw:term_status      "stable" ;
	skos:broadMatch     schema:eligibleQuantity .

gs1:eligibleQuantityMinimum
	rdf:type            rdf:Property , owl:ObjectProperty ;
	rdfs:comment        "The minimum quantity including unit of measure for which the offer for good or service is valid."@en ;
	rdfs:domain         _:b1 ;
	rdfs:isDefinedBy    gs1: ;
	rdfs:label          "Eligible Quantity Minimum"@en ;
	rdfs:range          gs1:QuantitativeValue ;
	rdfs:subPropertyOf  schema:eligibleQuantity ;
	sw:term_status      "stable" ;
	skos:broadMatch     schema:eligibleQuantity .

gs1:eligibleTradeChannel
	rdf:type          rdf:Property , owl:DatatypeProperty ;
	rdfs:comment      "A code determining the location where a user can redeem the offer, for example ONLINE_ONLY. "@en ;
	rdfs:domain       gs1:Discount ;
	rdfs:isDefinedBy  gs1: ;
	rdfs:label        "Eligible Trade Channel"@en ;
	rdfs:range        gs1:TradeChannelCode ;
	sw:term_status    "unstable" .

gs1:email
	rdf:type       rdf:Property , owl:DatatypeProperty ;
	rdfs:comment      "Creating/sending/receiving of unstructured free text messages or documents using computer network, a mini-computer or an attached modem and regular telephone line or other electronic transmission media."@en ;
	rdfs:domain       gs1:ContactPoint ;
	rdfs:isDefinedBy  gs1: ;
	rdfs:label        "E-mail"@en ;
	rdfs:range        xsd:string ;
	sw:term_status    "stable" ;
	skos:exactMatch   schema:email , vcard:hasEmail .

gs1:energyFromFatPerNutrientBasis
	rdf:type          rdf:Property , owl:ObjectProperty ;
	rdfs:comment      "Energy from Fat per specified nutrient basis quantity."@en ;
	rdfs:domain       gs1:FoodBeverageTobaccoProduct ;
	rdfs:isDefinedBy  gs1: ;
	rdfs:label        "Energy from Fat Per Nutrient Basis Quantity"@en ;
	rdfs:range        gs1:NutritionMeasurementType ;
	sw:term_status    "stable" .

gs1:energyPerNutrientBasis
	rdf:type          owl:ObjectProperty , rdf:Property ;
	rdfs:comment      "Energy Per specified nutrient basis quantity."@en ;
	rdfs:domain       gs1:FoodBeverageTobaccoProduct ;
	rdfs:isDefinedBy  gs1: ;
	rdfs:label        "Energy Per Nutrient Basis Quantity"@en ;
	rdfs:range        gs1:NutritionMeasurementType ;
	sw:term_status    "stable" .

gs1:epcis
	rdf:type         owl:ObjectProperty , rdf:Property ;
	rdfs:comment        "A link to an EPCIS repository of visibility event data."@en ;
	rdfs:domain         owl:Thing ;
	rdfs:label          "EPC Information Services (EPCIS) repository"@en ;
	rdfs:range          xsd:anyURI ;
	rdfs:subPropertyOf  gs1:linkType ;
	sw:term_status      "stable" .

gs1:epil
	rdf:type          owl:ObjectProperty , rdf:Property ;
	rdfs:comment        "A link to an electronic patient information leaflet."@en ;
	rdfs:domain         owl:Thing ;
	rdfs:label          "Electronic Patient Information Leaflet"@en ;
	rdfs:range          xsd:anyURI ;
	rdfs:subPropertyOf  gs1:linkType ;
	sw:term_status      "stable" .

gs1:equivalentProduct
	rdf:type            owl:ObjectProperty , rdf:Property ;
	rdfs:comment        "A product which can be substituted for the product based on supplier-defined functional equivalence to the product."@en ;
	rdfs:domain         gs1:Product ;
	rdfs:isDefinedBy    gs1: ;
	rdfs:label          "Has Equivalent Product"@en ;
	rdfs:range          gs1:Product ;
	rdfs:subPropertyOf  schema:isSimilarTo ;
	sw:term_status      "stable" .

gs1:eventsInfo
	rdf:type    owl:ObjectProperty , rdf:Property ;
	rdfs:comment        "A link to event details.  For a page specifically for scheduling a reservation or booking an appointment, see gs1:scheduleTime."@en ;
	rdfs:domain         owl:Thing ;
	rdfs:label          "Events information"@en ;
	rdfs:range          xsd:anyURI ;
	rdfs:subPropertyOf  gs1:linkType ;
	sw:term_status      "stable" .

gs1:exactDiscountAmount
	rdf:type          owl:DatatypeProperty , rdf:Property ;
	rdfs:comment      "Links to a gs1:PriceSpecification that indicates in terms of an amount and specified currency, the exact discount on the sales price associated with a particular gs1:Discount. This property can be used to express '$10 off'."@en ;
	rdfs:domain       gs1:Discount ;
	rdfs:isDefinedBy  gs1: ;
	rdfs:label        "Exact Discount Amount"@en ;
	rdfs:range        gs1:PriceSpecification ;
	sw:term_status    "unstable" .

gs1:exactDiscountPercentage
	rdf:type          rdf:Property , owl:DatatypeProperty ;
	rdfs:comment      "A floating-point value indicating an exact percentage discount on the sales price associated with a particular gs1:Discount.  This property can be used to express '15% discount'."@en ;
	rdfs:domain       gs1:Discount ;
	rdfs:isDefinedBy  gs1: ;
	rdfs:label        "Exact Discount Percentage"@en ;
	rdfs:range        xsd:float ;
	sw:term_status    "unstable" .

gs1:exclusionDescription
	rdf:type          rdf:Property , owl:ObjectProperty ;
	rdfs:comment      " A text description of any products, brands, or categories that cannot be used with the offer"@en ;
	rdfs:domain       gs1:Discount ;
	rdfs:isDefinedBy  gs1: ;
	rdfs:label        "Exclusion Description"@en ;
	rdfs:range        rdf:langString ;
	sw:term_status    "unstable" .

gs1:expirationDate
	rdf:type  rdf:Property , owl:ObjectProperty ;
	rdfs:comment      "The expiration date is the date that determines the limit of consumption or use of a product/coupon. Its meaning is determined based on the trade item context (e.g., for food, the date will indicate the possibility of a direct health risk resulting from use of the product after the date, for pharmaceutical products, it will indicate the possibility of an indirect health risk resulting from the ineffectiveness of the product after the date). It is often referred to as 'use by date' or 'maximum durability date'."@en ;
	rdfs:domain       gs1:Product , schema:Product ;
	rdfs:isDefinedBy  gs1: ;
	rdfs:label        "Expiration Date"@en ;
	rdfs:range        xsd:date ;
	sw:term_status    "stable" ;
	skos:altLabel     "Expiration Date"@en ;
	skos:notation     "17"^^gs1:AI ;
	skos:prefLabel    "17" .

gs1:expirationDateTime
	rdf:type          owl:ObjectProperty , rdf:Property ;
	rdfs:comment      "The manufacturer determines the expiration date and time, which is relevant only for short duration and for items that will not be sent on long distances and not outside of the time zone. A typical application of AI (7003) is in hospitals or public pharmacies for special, customised, products which may have a 'life duration' shorter than one single day. The life duration varies according the pharmaceutical substances used in the treatment. The precise expiration date and time is defined at the end of the manufacturing process, and can be barcoded on the product label as an attribute to the item's GTIN. Where there is no business requirement to express the expiration date to the nearest hour (or less), AI (17) Expiration date should be used."@en ;
	rdfs:domain       schema:Product , gs1:Product ;
	rdfs:isDefinedBy  gs1: ;
	rdfs:label        "Expiration Date and Time"@en ;
	rdfs:range        xsd:date ;
	sw:term_status    "stable" ;
	skos:altLabel     "Expiration Date and Time"@en ;
	skos:notation     "7003"^^gs1:AI ;
	skos:prefLabel    "7003" .

gs1:faqs
	rdf:type          owl:ObjectProperty , rdf:Property ;
	rdfs:comment        "A link to a set of frequently asked questions."@en ;
	rdfs:domain         owl:Thing ;
	rdfs:label          "Frequently Asked Questions"@en ;
	rdfs:range          xsd:anyURI ;
	rdfs:subPropertyOf  gs1:linkType ;
	sw:term_status      "stable" .

gs1:fatInMilkContent
	rdf:type  rdf:Property , owl:DatatypeProperty ;
	rdfs:comment      "The percentage of fat contained in milk content of the product."@en ;
	rdfs:domain       gs1:MilkButterCreamYogurtCheeseEggsSubstitutes ;
	rdfs:isDefinedBy  gs1: ;
	rdfs:label        "Fat In Milk Content"@en ;
	rdfs:range        xsd:float ;
	sw:term_status    "stable" .

gs1:fatPerNutrientBasis
	rdf:type          owl:ObjectProperty , rdf:Property ;
	rdfs:comment      "Fat per specified nutrient basis quantity."@en ;
	rdfs:domain       gs1:FoodBeverageTobaccoProduct ;
	rdfs:isDefinedBy  gs1: ;
	rdfs:label        "Fat Per Nutrient Basis Quantity"@en ;
	rdfs:range        gs1:NutritionMeasurementType ;
	sw:term_status    "stable" .

gs1:fatpercentageInDryMatter
	rdf:type          owl:DatatypeProperty , rdf:Property ;
	rdfs:comment      "The amount of fat contained in the base product expressed in percentage."@en ;
	rdfs:domain       gs1:MilkButterCreamYogurtCheeseEggsSubstitutes ;
	rdfs:isDefinedBy  gs1: ;
	rdfs:label        "Fat In Dry Matter"@en ;
	rdfs:range        xsd:float ;
	sw:term_status    "stable" .

gs1:faxNumber
	rdf:type   owl:DatatypeProperty , rdf:Property ;
	rdfs:comment      "A fax number used for transmitting and reproducing fixed graphic material over telephone lines or other electronic transmission media."@en ;
	rdfs:domain       gs1:ContactPoint ;
	rdfs:isDefinedBy  gs1: ;
	rdfs:label        "Telefax"@en ;
	rdfs:range        xsd:string ;
	sw:term_status    "stable" ;
	skos:exactMatch   schema:faxNumber .

gs1:fibrePerNutrientBasis
	rdf:type          owl:ObjectProperty , rdf:Property ;
	rdfs:comment      "Fibre per specified nutrient basis quantity."@en ;
	rdfs:domain       gs1:FoodBeverageTobaccoProduct ;
	rdfs:isDefinedBy  gs1: ;
	rdfs:label        "Fibre Per Nutrient Basis Quantity"@en ;
	rdfs:range        gs1:NutritionMeasurementType ;
	sw:term_status    "stable" .

gs1:fileLanguageCode
	rdf:type  rdf:Property , owl:DatatypeProperty ;
	rdfs:comment        "The specified language to which the digital asset is targeted. It is recommended to use the ISO 639-1 language code."@en ;
	rdfs:domain         gs1:ReferencedFileDetails ;
	rdfs:isDefinedBy    gs1: ;
	rdfs:label          "File Language Code"@en ;
	rdfs:range          xsd:string ;
	rdfs:subPropertyOf  schema:inLanguage ;
	sw:term_status      "stable" ;
	skos:related        schema:CreativeWork .

gs1:filePixelHeight
	rdf:type  owl:DatatypeProperty , rdf:Property ;
	rdfs:comment        "The number of pixels along the vertical axis of the image."@en ;
	rdfs:domain         gs1:ReferencedFileDetails ;
	rdfs:isDefinedBy    gs1: ;
	rdfs:label          "File Pixel Height"@en ;
	rdfs:range          xsd:integer ;
	rdfs:subPropertyOf  schema:height ;
	sw:term_status      "stable" ;
	skos:related        schema:MediaObject .

gs1:filePixelWidth
	rdf:type  owl:DatatypeProperty , rdf:Property ;
	rdfs:comment        "The number of pixels along the horizontal axis of the image."@en ;
	rdfs:domain         gs1:ReferencedFileDetails ;
	rdfs:isDefinedBy    gs1: ;
	rdfs:label          "File Pixel Width"@en ;
	rdfs:range          xsd:integer ;
	rdfs:subPropertyOf  schema:width ;
	sw:term_status      "stable" ;
	skos:related        schema:MediaObject .

gs1:firstFreezeDate
	rdf:type  owl:ObjectProperty , rdf:Property ;
	rdfs:comment      "The first freeze date is applicable to products that are frozen directly after slaughtering, harvesting, catching or after initial processing of the product. Examples include fresh meat, meat products or fishery products. The first freeze date is determined by the organisation conducting the freezing."@en ;
	rdfs:domain       schema:Product , gs1:Product ;
	rdfs:isDefinedBy  gs1: ;
	rdfs:label        "First Freeze Date"@en ;
	rdfs:range        xsd:date ;
	sw:term_status    "stable" ;
	skos:altLabel     "First Freeze Date"@en ;
	skos:notation     "7006"^^gs1:AI ;
	skos:prefLabel    "7006" .

gs1:fishType
	rdf:type    owl:DatatypeProperty , rdf:Property ;
	rdfs:comment      "The type of fish for example Sea bass."@en ;
	rdfs:domain       gs1:Seafood ;
	rdfs:isDefinedBy  gs1: ;
	rdfs:label        "Fish Type"@en ;
	rdfs:range        rdf:langString ;
	sw:term_status    "stable" .

gs1:fluoridePerNutrientBasis
	rdf:type          owl:ObjectProperty , rdf:Property ;
	rdfs:comment      "Fluoride per specified nutrient basis quantity."@en ;
	rdfs:domain       gs1:FoodBeverageTobaccoProduct ;
	rdfs:isDefinedBy  gs1: ;
	rdfs:label        "Fluoride Per Nutrient Basis Quantity"@en ;
	rdfs:range        gs1:NutritionMeasurementType ;
	sw:term_status    "stable" .

gs1:folicAcidPerNutrientBasis
	rdf:type          owl:ObjectProperty , rdf:Property ;
	rdfs:comment      "Folic Acid per specified nutrient basis quantity."@en ;
	rdfs:domain       gs1:FoodBeverageTobaccoProduct ;
	rdfs:isDefinedBy  gs1: ;
	rdfs:label        "Folic Acid Per Nutrient Basis Quantity"@en ;
	rdfs:range        gs1:NutritionMeasurementType ;
	sw:term_status    "stable" .

gs1:foodBeverageRefrigerationClaim
	rdf:type          rdf:Property , owl:ObjectProperty ;
	rdfs:comment      "Identifies whether or not the product requires refrigeration."@en ;
	rdfs:domain       gs1:FoodBeverageTobaccoProduct ;
	rdfs:isDefinedBy  gs1: ;
	rdfs:label        "Food Beverage Refrigeration Claim"@en ;
	rdfs:range        gs1:FoodBeverageRefrigerationClaimCode ;
	sw:term_status    "stable" .

gs1:foodBeverageTargetUse
	rdf:type          rdf:Property , owl:ObjectProperty ;
	rdfs:comment      "The type of meal the food or beverage product is targeted to for example Breakfast."@en ;
	rdfs:domain       gs1:FoodBeverageTobaccoProduct ;
	rdfs:isDefinedBy  gs1: ;
	rdfs:label        "Food Beverage Target Use"@en ;
	rdfs:range        gs1:FoodBeverageTargetUseCode ;
	sw:term_status    "stable" .

gs1:footwearFasteningType
	rdf:type          rdf:Property , owl:ObjectProperty ;
	rdfs:comment      "Something that mechanically joins or affixes two or more parts together in a footwear product for example a shoe lace."@en ;
	rdfs:domain       gs1:Footwear ;
	rdfs:isDefinedBy  gs1: ;
	rdfs:label        "Fastening Type"@en ;
	rdfs:range        gs1:FootwearFasteningTypeCode ;
	sw:term_status    "stable" .

gs1:footwearUpperType
	rdf:type          owl:ObjectProperty , rdf:Property ;
	rdfs:comment      "The descriptive term that is used by the product manufacturer to identify whether the footwear upper is open or closed. Otherwise known as Open or Closed Upper."@en ;
	rdfs:domain       gs1:Footwear ;
	rdfs:isDefinedBy  gs1: ;
	rdfs:label        "Footwear Upper Type"@en ;
	rdfs:range        gs1:UpperTypeCode ;
	sw:term_status    "stable" .

gs1:freshOrSeawaterFarmed
	rdf:type          rdf:Property , owl:ObjectProperty ;
	rdfs:comment      "A code determining whether the fish originated from the sea or was farmed."@en ;
	rdfs:domain       gs1:Seafood ;
	rdfs:isDefinedBy  gs1: ;
	rdfs:label        "Fresh or Seawater Farmed"@en ;
	rdfs:range        gs1:FreshOrSeawaterFarmedCode ;
	sw:term_status    "stable" .

gs1:functionalName
	rdf:type  rdf:Property , owl:FunctionalProperty , owl:DatatypeProperty ;
	rdfs:comment      "Describes use of the product or service by the consumer. Should help clarify the product classification associated with the GTIN."@en ;
	rdfs:domain       gs1:Product ;
	rdfs:isDefinedBy  gs1: ;
	rdfs:label        "Functional Name"@en ;
	rdfs:range        rdf:langString ;
	sw:term_status    "stable" .

gs1:geneticallyModifiedDeclaration
	rdf:type          owl:ObjectProperty , rdf:Property ;
	rdfs:comment      "A statement of the presence or absence of genetically modified protein or DNA."@en ;
	rdfs:domain       gs1:FoodBeverageTobaccoProduct ;
	rdfs:isDefinedBy  gs1: ;
	rdfs:label        "Genetically Modified Declaration Code"@en ;
	rdfs:range        gs1:LevelOfContainmentCode ;
	sw:term_status    "stable" .

gs1:geo
	rdf:type         owl:ObjectProperty , rdf:Property ;
	rdfs:comment      "Links to information about geocoordinates or geoshapes for a place."@en ;
	rdfs:domain       gs1:Place ;
	rdfs:isDefinedBy  gs1: ;
	rdfs:label        "Has Geocoordinates"@en ;
	rdfs:range        [ rdf:type     owl:Class ;
	owl:unionOf  ( gs1:GeoCoordinates gs1:GeoShape )
	] ;
	sw:term_status    "stable" ;
	skos:exactMatch   schema:geo .

gs1:glnType
	rdf:type     owl:ObjectProperty , rdf:Property ;
	rdfs:comment      "Indicates what type of thing is being identified by a GLN."@en ;
	rdfs:domain       _:b0 ;
	rdfs:isDefinedBy  gs1: ;
	rdfs:label        "Has GLN Type"@en ;
	rdfs:range        gs1:GLN_TypeCode ;
	sw:term_status    "stable" .

gs1:globalLocationNumber
	rdf:type          owl:DatatypeProperty , rdf:Property ;
	rdfs:comment      "A Global Location Number (GLN) is the GS1 Identification Key used to identify physical locations or parties. The key comprises a GS1 Company Prefix, Location Reference and Check Digit. For more information see https://www.gs1.org/gln."@en ;
	rdfs:domain       _:b0 ;
	rdfs:isDefinedBy  gs1: ;
	rdfs:label        "Global Location Number (GLN)"@en ;
	rdfs:range        xsd:string ;
	sw:term_status    "stable" ;
	skos:exactMatch   schema:globalLocationNumber .

gs1:gpcCategoryCode
	rdf:type  rdf:Property , owl:FunctionalProperty , owl:DatatypeProperty ;
	rdfs:comment      "8-digit code (GPC Brick Value) specifying a product category according to the GS1 Global Product Classification (GPC) standard. For more information see https://www.gs1.org/gpc"@en ;
	rdfs:domain       gs1:Product ;
	rdfs:isDefinedBy  gs1: ;
	rdfs:label        "GPC Category Code"@en ;
	rdfs:range        xsd:string ;
	sw:term_status    "stable" .

gs1:gpcCategoryDescription
	rdf:type          rdf:Property , owl:FunctionalProperty , owl:DatatypeProperty ;
	rdfs:comment      "A description of the code specifying a product category according to the GS1 Global Product Classification (GPC) standard."@en ;
	rdfs:domain       gs1:Product ;
	rdfs:isDefinedBy  gs1: ;
	rdfs:label        "GPC Category Description"@en ;
	rdfs:range        rdf:langString ;
	sw:term_status    "stable" .

gs1:grossArea
	rdf:type   owl:ObjectProperty , rdf:Property , owl:FunctionalProperty ;
	rdfs:comment      "The overall area of the item including packaging. This can be given using a number of different AI ranges that depend on the units in which the area is measured."@en ;
	rdfs:domain       gs1:Product ;
	rdfs:isDefinedBy  gs1: ;
	rdfs:label        "Gross area"@en ;
	rdfs:range        gs1:QuantitativeValue ;
	sw:term_status    "stable" ;
	skos:altLabel     "Gross area"@en ;
	skos:prefLabel    "334n, 353n, 354n, 355n" .

gs1:grossVolume
	rdf:type  owl:FunctionalProperty , rdf:Property , owl:ObjectProperty ;
	rdfs:comment      "The overall volume of the item including packaging. This can be given using a number of different AI ranges that depend on the units in which the volume is measured."@en ;
	rdfs:domain       gs1:Product ;
	rdfs:isDefinedBy  gs1: ;
	rdfs:label        "Gross volume"@en ;
	rdfs:range        gs1:QuantitativeValue ;
	sw:term_status    "stable" ;
	skos:altLabel     "Gross volume"@en ;
	skos:prefLabel    "335n, 336n, 362n, 363n, 367n, 368n, 369n" .

gs1:grossWeight
	rdf:type   rdf:Property , owl:ObjectProperty , owl:FunctionalProperty ;
	rdfs:comment        "Used to identify the gross weight of the product. The gross weight includes all packaging materials of the product. At pallet level the productGrossWeight includes the weight of the pallet itself. For example, 200 GRM, value - total pounds, total grams, etc."@en ;
	rdfs:domain         gs1:Product ;
	rdfs:isDefinedBy    gs1: ;
	rdfs:label          "Gross Weight"@en ;
	rdfs:range          gs1:QuantitativeValue ;
	rdfs:subPropertyOf  schema:weight ;
	sw:term_status      "stable" .

gs1:growingMethod
	rdf:type  owl:ObjectProperty , rdf:Property ;
	rdfs:comment      "The process through which fresh produce is grown and cultivated."@en ;
	rdfs:domain       gs1:Product ;
	rdfs:isDefinedBy  gs1: ;
	rdfs:label        "Growing Method"@en ;
	rdfs:range        gs1:GrowingMethodCode ;
	sw:term_status    "stable" .

gs1:gtin
	rdf:type        rdf:Property , owl:FunctionalProperty , owl:DatatypeProperty ;
	rdfs:comment      "A Global Trade Item Number (GTIN) is the 14 digit GS1 Identification Key used to identify products. The key comprises a GS1 Company Prefix followed by an Item Reference Number and a Check Digit. See https://www.gs1.org/gtin  for more details."@en ;
	rdfs:domain       schema:Product , gs1:Product ;
	rdfs:isDefinedBy  gs1: ;
	rdfs:label        "GTIN"@en ;
	rdfs:range        xsd:string ;
	sw:term_status    "stable" ;
	skos:altLabel     "GTIN" ;
	skos:closeMatch   schema:gtin12 , schema:gtin8 , schema:gtin13 ;
	skos:exactMatch   schema:gtin14 ;
	skos:notation     "01"^^gs1:AI ;
	skos:prefLabel    "01" .

gs1:handledBy
	rdf:type     owl:ObjectProperty , rdf:Property ;
	rdfs:comment        "Used when one resolver redirects all request URIs that match a given pattern without further processing, such as from GS1 to a brand-operated service. See section 7.7.1 of the Digital Link standard, version 1.1. "@en ;
	rdfs:domain         owl:Thing ;
	rdfs:label          "Handled by"@en ;
	rdfs:range          xsd:anyURI ;
	rdfs:subPropertyOf  gs1:linkType ;
	sw:term_status      "stable" .

gs1:harvestDate
	rdf:type  rdf:Property , owl:ObjectProperty ;
	rdfs:comment      "The harvest date. For example, the harvest date can be the date when an animal was slaughtered or killed, a fish has been harvested, or a crop was harvested. This date  is determined by the organisation conducting the harvesting. Different organisations may use more specific terminology when referring to their specific needs and use terms such as: Date of catch or slaughter date. "@en ;
	rdfs:domain       schema:Product , gs1:Product ;
	rdfs:isDefinedBy  gs1: ;
	rdfs:label        "Harvest Date."@en ;
	rdfs:range        xsd:date ;
	sw:term_status    "stable" ;
	skos:altLabel     "Harvest Date."@en ;
	skos:notation     "7007"^^gs1:AI ;
	skos:prefLabel    "7007" .

gs1:harvestDateEnd
	rdf:type  owl:ObjectProperty , rdf:Property ;
	rdfs:comment      "The harvest end date. For example, the harvest end date can be the date when an animal was slaughtered or killed, a fish has been harvested, or a crop was harvested. This end date is determined by the organisation conducting the harvesting. Different organisations may use more specific terminology when referring to their specific needs and use terms such as: Date of catch or slaughter date. When referring to animals the date range refers to the whole animal and all meat or fish cuts derived from this animal."@en ;
	rdfs:domain       schema:Product , gs1:Product ;
	rdfs:isDefinedBy  gs1: ;
	rdfs:label        "Harvest Date End"@en ;
	rdfs:range        xsd:date ;
	sw:term_status    "stable" ;
	skos:altLabel     "Harvest Date End"@en ;
	skos:notation     "7007"^^gs1:AI ;
	skos:prefLabel    "7007" .

gs1:harvestDateStart
	rdf:type  owl:ObjectProperty , rdf:Property ;
	rdfs:comment      "The harvest start date. For example, the harvest start date can be the date when an animal was slaughtered or killed, a fish has been harvested, or a crop was harvested. This start date is determined by the organisation conducting the harvesting. Different organisations may use more specific terminology when referring to their specific needs and use terms such as: Date of catch or slaughter date. When referring to animals the date range refers to the whole animal and all meat or fish cuts derived from this animal."@en ;
	rdfs:domain       gs1:Product , schema:Product ;
	rdfs:isDefinedBy  gs1: ;
	rdfs:label        "Harvest Date Start"@en ;
	rdfs:range        xsd:date ;
	sw:term_status    "stable" ;
	skos:altLabel     "Harvest Date Start"@en ;
	skos:notation     "7007"^^gs1:AI ;
	skos:prefLabel    "7007" .

gs1:hasAllergen
	rdf:type  owl:ObjectProperty , rdf:Property ;
	rdfs:comment      "Relates to details about allergens"@en ;
	rdfs:domain       gs1:FoodBeverageTobaccoProduct ;
	rdfs:isDefinedBy  gs1: ;
	rdfs:label        "Has Allergen"@en ;
	rdfs:range        gs1:AllergenDetails ;
	sw:term_status    "stable" .

gs1:hasBatchLotNumber
	rdf:type          rdf:Property , owl:ObjectProperty ;
	rdfs:comment      "The batch or lot number associates an item with information the manufacturer considers relevant for traceability of the trade item to which the element string is applied. The data may refer to the trade item itself or to items contained. The number may be, for example, a production lot number, a shift number, a machine number, a time, or an internal production code. In cases where the same product is manufactured in different locations the brand owner and the manufacturer are responsible for ensuring the non-duplication of batch/lot numbers for a GTIN. For the re-use of batch/lot numbers with a GTIN, sector-specific constraints need to be considered."@en ;
	rdfs:domain       gs1:Product , schema:Product ;
	rdfs:isDefinedBy  gs1: ;
	rdfs:label        "Batch/Lot Identifier"@en ;
	rdfs:range        xsd:string ;
	sw:term_status    "stable" ;
	skos:altLabel     "Batch/Lot Identifier"@en ;
	skos:notation     "10"^^gs1:AI ;
	skos:prefLabel    "10" .

gs1:hasPrimaryLocation
	rdf:type          rdf:Property , owl:ObjectProperty ;
	rdfs:comment      "Links to the place(s) that this organisation designates as their primary location(s)."@en ;
	rdfs:domain       gs1:Organization ;
	rdfs:isDefinedBy  gs1: ;
	rdfs:label        "Has primary location"@en ;
	rdfs:range        gs1:Place ;
	sw:term_status    "stable" .

gs1:hasRetailers
	rdf:type  owl:ObjectProperty , rdf:Property ;
	rdfs:comment        "A link to a list of retailers."@en ;
	rdfs:domain         owl:Thing ;
	rdfs:label          "Has Retailers"@en ;
	rdfs:range          xsd:anyURI ;
	rdfs:subPropertyOf  gs1:linkType ;
	sw:term_status      "stable" .

gs1:hasReturnablePackageDeposit
	rdf:type          rdf:Property , owl:ObjectProperty ;
	rdfs:comment      "links to details of amounts refunded for returnable package in a specified region."@en ;
	rdfs:domain       gs1:PackagingDetails ;
	rdfs:isDefinedBy  gs1: ;
	rdfs:label        "Has Returnable Package Deposit Details"@en ;
	rdfs:range        gs1:ReturnablePackageDepositDetails ;
	sw:term_status    "stable" .

gs1:hasSerialNumber
	rdf:type  owl:ObjectProperty , rdf:Property ;
	rdfs:comment      "A serial number is assigned to an entity for its lifetime. When combined with a GTIN, a serial number uniquely identifies an individual item. The serial number field is alphanumeric and may include all characters contained in figure 7.11-1. The brand owner and the manufacturer are responsible for ensuring the non-duplication of serial numbers for a GTIN. For the re-use of serial numbers with a GTIN, sector-specific constraints need to be considered."@en ;
	rdfs:domain       schema:Product , gs1:Product ;
	rdfs:isDefinedBy  gs1: ;
	rdfs:label        "Serial Number"@en ;
	rdfs:range        xsd:string ;
	sw:term_status    "stable" ;
	skos:altLabel     "Serial Number"@en ;
	skos:notation     "21"^^gs1:AI ;
	skos:prefLabel    "21" .

gs1:hasThirdPartyControlledSerialNumber
	rdf:type          rdf:Property , owl:ObjectProperty ;
	rdfs:comment      "This identifier is assigned to an entity for its lifetime. When combined with a GTIN, a TPX uniquely identifies an individual item and forms a unit pack Unique Identifier (upUI) for tobacco traceability per EU 2018/574. The serial number field is alphanumeric and may include all characters contained in figure 7.11-1. The Third Party determines the TPX, but the TPX shall begin with the ID Issuer Unique Identification Code (UIC), followed by GS1 UIC Extension 1, and GS1 UIC Extension 2."@en ;
	rdfs:domain       schema:Product , gs1:Product ;
	rdfs:isDefinedBy  gs1: ;
	rdfs:label        "Third-Party Controlled Serial Number"@en ;
	rdfs:range        xsd:string ;
	sw:term_status    "stable" ;
	skos:altLabel     "Third-Party Controlled Serial Number"@en ;
	skos:notation     "235"^^gs1:AI ;
	skos:prefLabel    "235" .

gs1:healthClaimDescription
	rdf:type          rdf:Property , owl:FunctionalProperty , owl:DatatypeProperty ;
	rdfs:comment      "A description of health claims according to regulations of the target market."@en ;
	rdfs:domain       gs1:Product ;
	rdfs:isDefinedBy  gs1: ;
	rdfs:label        "Health Claim"@en ;
	rdfs:range        rdf:langString ;
	sw:term_status    "stable" .

gs1:homepage
	rdf:type      owl:ObjectProperty , rdf:Property ;
	rdfs:comment        "A link to general information about an organisation or brand. Typically the homepage of an organisation's website. It may include links to further information such as certifications, careers, payments, reservations, etc."@en ;
	rdfs:domain         owl:Thing ;
	rdfs:label          "Organisation Information Page"@en ;
	rdfs:range          xsd:anyURI ;
	rdfs:subPropertyOf  gs1:linkType ;
	sw:term_status      "stable" .

gs1:image
	rdf:type       owl:ObjectProperty , rdf:Property ;
	rdfs:comment      "Link to a file containing a visual representation of the product."@en ;
	rdfs:domain       gs1:Product ;
	rdfs:isDefinedBy  gs1: ;
	rdfs:label        "Has Product Image"@en ;
	rdfs:range        gs1:ReferencedFileDetails ;
	sw:term_status    "stable" ;
	skos:closeMatch   foaf:depiction , schema:image .

gs1:inPackageDepth
	rdf:type  owl:ObjectProperty , rdf:Property ;
	rdfs:comment      "The depth of the product in its packaging, as measured according to the GS1 Package Measurement Rules. See https://www.gs1.org/package-measurement-rules-implementation-guide for more details."@en ;
	rdfs:domain       gs1:Product ;
	rdfs:isDefinedBy  gs1: ;
	rdfs:label        "In Package Depth"@en ;
	rdfs:range        gs1:QuantitativeValue ;
	sw:term_status    "stable" ;
	skos:related      schema:depth .

gs1:inPackageDiameter
	rdf:type          rdf:Property , owl:ObjectProperty ;
	rdfs:comment      "The measurement of the diameter of the product in its package at its largest point. For example, 165 MMT."@en ;
	rdfs:domain       gs1:Product ;
	rdfs:isDefinedBy  gs1: ;
	rdfs:label        "In Package Diameter"@en ;
	rdfs:range        gs1:QuantitativeValue ;
	sw:term_status    "stable" .

gs1:inPackageHeight
	rdf:type  owl:ObjectProperty , rdf:Property ;
	rdfs:comment      "The height of the product in the package, as measured according to the GS1 Package Measurement Rules. See https://www.gs1.org/package-measurement-rules-implementation-guide for more details."@en ;
	rdfs:domain       gs1:Product ;
	rdfs:isDefinedBy  gs1: ;
	rdfs:label        "In Package Height"@en ;
	rdfs:range        gs1:QuantitativeValue ;
	sw:term_status    "stable" ;
	skos:related      schema:height .

gs1:inPackageWidth
	rdf:type  owl:ObjectProperty , rdf:Property ;
	rdfs:comment      "The width of the product in the package, as measured according to the GS1 Package Measurement Rules. See https://www.gs1.org/package-measurement-rules-implementation-guide for more details."@en ;
	rdfs:domain       gs1:Product ;
	rdfs:isDefinedBy  gs1: ;
	rdfs:label        "In Package Width"@en ;
	rdfs:range        gs1:QuantitativeValue ;
	sw:term_status    "stable" ;
	skos:related      schema:width .

gs1:includedAccessories
	rdf:type          owl:DatatypeProperty , rdf:Property , owl:FunctionalProperty ;
	rdfs:comment      "Any included object or device not part of the core product itself but which adds to its functionality or use."@en ;
	rdfs:domain       gs1:Product ;
	rdfs:isDefinedBy  gs1: ;
	rdfs:label        "Included Accessories"@en ;
	rdfs:range        rdf:langString ;
	rdfs:seeAlso      schema:isAccessoryOrSparePartFor ;
	sw:term_status    "stable" ;
	skos:related      schema:isAccessoryOrSparePartFor .

gs1:ingredient
	rdf:type  owl:ObjectProperty , rdf:Property ;
	rdfs:comment      "Links to information about ingredients of a specific Food/Beverage/Tobacco product."@en ;
	rdfs:domain       gs1:FoodBeverageTobaccoProduct ;
	rdfs:isDefinedBy  gs1: ;
	rdfs:label        "Has Food And Beverage Ingredient Information"@en ;
	rdfs:range        gs1:FoodBeverageTobaccoIngredientDetails ;
	sw:term_status    "stable" .

gs1:ingredientContentPercentage
	rdf:type          rdf:Property , owl:DatatypeProperty ;
	rdfs:comment      "Quantity of the ingredient contained in the product as a percentage of the total product ingredients. This is used in conjunction with ingredientName."@en ;
	rdfs:domain       gs1:FoodBeverageTobaccoIngredientDetails ;
	rdfs:isDefinedBy  gs1: ;
	rdfs:label        "Ingredient Content Percentage"@en ;
	rdfs:range        xsd:float ;
	sw:term_status    "stable" .

gs1:ingredientName
	rdf:type  rdf:Property , owl:DatatypeProperty ;
	rdfs:comment      "Free text field describing an ingredient or ingredient group. Ingredients include any additives (colourings, preservatives, e-numbers, etc.) that are encompassed."@en ;
	rdfs:domain       gs1:FoodBeverageTobaccoIngredientDetails ;
	rdfs:isDefinedBy  gs1: ;
	rdfs:label        "Ingredient Name"@en ;
	rdfs:range        rdf:langString ;
	sw:term_status    "stable" .

gs1:ingredientOfConcern
	rdf:type          owl:DatatypeProperty , rdf:Property ;
	rdfs:comment      "Indicates a claim to an ingredient, considered to be a concern for regulatory or other reasons, and which is 'contained' within the product but may not need to specify the amount whether approximate, or an accurate measurement be given."@en ;
	rdfs:domain       gs1:FoodBeverageTobaccoProduct ;
	rdfs:isDefinedBy  gs1: ;
	rdfs:label        "Ingredient of Concern"@en ;
	rdfs:range        rdf:langString ;
	sw:term_status    "stable" .

gs1:ingredientSequence
	rdf:type          rdf:Property , owl:DatatypeProperty ;
	rdfs:comment      "Integer (1, 2, 3...) indicating the ingredient order by content percentage of the product. (major ingredient = 1, second ingredient = 2) etc."@en ;
	rdfs:domain       gs1:FoodBeverageTobaccoIngredientDetails ;
	rdfs:isDefinedBy  gs1: ;
	rdfs:label        "Ingredient Sequence"@en ;
	rdfs:range        xsd:integer ;
	sw:term_status    "stable" .

gs1:ingredientStatement
	rdf:type          rdf:Property , owl:DatatypeProperty ;
	rdfs:comment      "Information on the constituent ingredient make up of the product specified as one string."@en ;
	rdfs:domain       gs1:FoodBeverageTobaccoProduct ;
	rdfs:isDefinedBy  gs1: ;
	rdfs:label        "Ingredient Statement"@en ;
	rdfs:range        rdf:langString ;
	sw:term_status    "stable" .

gs1:ingredientsInfo
	rdf:type  owl:ObjectProperty , rdf:Property ;
	rdfs:comment        "A link to facts about ingredients."@en ;
	rdfs:domain         owl:Thing ;
	rdfs:label          "Ingredients information"@en ;
	rdfs:range          xsd:anyURI ;
	rdfs:subPropertyOf  gs1:linkType ;
	sw:term_status      "stable" .

gs1:initialCertificationDate
	rdf:type          rdf:Property , owl:DatatypeProperty ;
	rdfs:comment      "The date when the certification was originally issued. May differ from the certificationStartDate of the current recertification cycle."@en ;
	rdfs:domain       gs1:CertificationDetails ;
	rdfs:isDefinedBy  gs1: ;
	rdfs:label        "Initial Certification Date"@en ;
	rdfs:range        xsd:date ;
	sw:term_status    "stable" .

gs1:instructions
	rdf:type  owl:ObjectProperty , rdf:Property ;
	rdfs:comment        "A link to instructions, such as assembly instructions, usage tips etc."@en ;
	rdfs:domain         owl:Thing ;
	rdfs:label          "Instructions"@en ;
	rdfs:range          xsd:anyURI ;
	rdfs:subPropertyOf  gs1:linkType ;
	sw:term_status      "stable" .

gs1:instructionsForUse
	rdf:type          rdf:Property , owl:ObjectProperty ;
	rdfs:comment      "Link to a file containing the Instructions For Use."@en ;
	rdfs:domain       gs1:Product ;
	rdfs:isDefinedBy  gs1: ;
	rdfs:label        "Has Instructions For Use"@en ;
	rdfs:range        gs1:ReferencedFileDetails ;
	sw:term_status    "stable" .

gs1:iodinePerNutrientBasis
	rdf:type          owl:ObjectProperty , rdf:Property ;
	rdfs:comment      "Iodine per specified nutrient basis quantity."@en ;
	rdfs:domain       gs1:FoodBeverageTobaccoProduct ;
	rdfs:isDefinedBy  gs1: ;
	rdfs:label        "Iodine Per Nutrient Basis Quantity"@en ;
	rdfs:range        gs1:NutritionMeasurementType ;
	sw:term_status    "stable" .

gs1:ironPerNutrientBasis
	rdf:type          rdf:Property , owl:ObjectProperty ;
	rdfs:comment      "Iron per specified nutrient basis quantity."@en ;
	rdfs:domain       gs1:FoodBeverageTobaccoProduct ;
	rdfs:isDefinedBy  gs1: ;
	rdfs:label        "Iron Per Nutrient Basis Quantity"@en ;
	rdfs:range        gs1:NutritionMeasurementType ;
	sw:term_status    "stable" .

gs1:irradiatedCode
	rdf:type  rdf:Property , owl:ObjectProperty ;
	rdfs:comment      "Indicates if radiation has been applied to the product."@en ;
	rdfs:domain       gs1:FoodBeverageTobaccoProduct ;
	rdfs:isDefinedBy  gs1: ;
	rdfs:label        "Irradiated Code"@en ;
	rdfs:range        gs1:NonbinaryLogicCode ;
	sw:term_status    "stable" .

gs1:isCarbonated
	rdf:type  rdf:Property , owl:ObjectProperty ;
	rdfs:comment      "Used to identify whether or not a beverage product is naturally effervescent or has been made effervescent by the addition of carbon dioxide gas."@en ;
	rdfs:domain       gs1:Beverage ;
	rdfs:isDefinedBy  gs1: ;
	rdfs:label        "Is Carbonated"@en ;
	rdfs:range        gs1:NonbinaryLogicCode ;
	sw:term_status    "stable" .

gs1:isDecaffeinated
	rdf:type  rdf:Property , owl:ObjectProperty ;
	rdfs:comment      "The descriptive term that is used by the product manufacturer to identify whether or not the product contains caffeine."@en ;
	rdfs:domain       gs1:Beverage ;
	rdfs:isDefinedBy  gs1: ;
	rdfs:label        "Is Decaffeinated"@en ;
	rdfs:range        gs1:NonbinaryLogicCode ;
	sw:term_status    "stable" .

gs1:isFromConcentrate
	rdf:type          rdf:Property , owl:ObjectProperty ;
	rdfs:comment      "Used to identify whether or not the product claims to be made from a concentrated formulation."@en ;
	rdfs:domain       gs1:Beverage ;
	rdfs:isDefinedBy  gs1: ;
	rdfs:label        "Is From Concentrate"@en ;
	rdfs:range        gs1:NonbinaryLogicCode ;
	sw:term_status    "stable" .

gs1:isHomogenised
	rdf:type  rdf:Property , owl:ObjectProperty ;
	rdfs:comment      "A The indication whether or not the milk used was actively homogenised. The homogenisation of milk is a technical process in the dairy. The milk fat is milled to such an extent that further creaming is prevented."@en ;
	rdfs:domain       gs1:MilkButterCreamYogurtCheeseEggsSubstitutes ;
	rdfs:isDefinedBy  gs1: ;
	rdfs:label        "Is Homogenised"@en ;
	rdfs:range        gs1:NonbinaryLogicCode ;
	sw:term_status    "stable" .

gs1:isInstant
	rdf:type   rdf:Property , owl:ObjectProperty ;
	rdfs:comment      "Determines whether the product is instant."@en ;
	rdfs:domain       gs1:FoodBeverageTobaccoProduct ;
	rdfs:isDefinedBy  gs1: ;
	rdfs:label        "Is Instant"@en ;
	rdfs:range        gs1:NonbinaryLogicCode ;
	sw:term_status    "stable" .

gs1:isMaternity
	rdf:type  owl:ObjectProperty , rdf:Property ;
	rdfs:comment      "Indicates, with reference to the product branding, labelling or packaging, the descriptive term that is used by the product manufacturer to identify if the product is intended as maternity wear."@en ;
	rdfs:domain       gs1:Clothing ;
	rdfs:isDefinedBy  gs1: ;
	rdfs:label        "Is Maternity"@en ;
	rdfs:range        gs1:NonbinaryLogicCode ;
	sw:term_status    "stable" .

gs1:isOnlyAvailableThroughRetailer
	rdf:type          owl:DatatypeProperty , rdf:Property ;
	rdfs:comment      "If specified and set to true, the discount is only available through the retailer making the offer."@en ;
	rdfs:domain       gs1:Discount ;
	rdfs:isDefinedBy  gs1: ;
	rdfs:label        "Only Available Through Retailer"@en ;
	rdfs:range        xsd:boolean ;
	sw:term_status    "stable" .

gs1:isOnlyWithMailingListSignup
	rdf:type          rdf:Property , owl:DatatypeProperty ;
	rdfs:comment      "If specified and set to true, the discount is only available for customers who have signed up to the retailer's mailing list."@en ;
	rdfs:domain       gs1:Discount ;
	rdfs:isDefinedBy  gs1: ;
	rdfs:label        "Only For Retailer Mailing List Members"@en ;
	rdfs:range        xsd:boolean ;
	sw:term_status    "unstable" .

gs1:isOnlyWithPaymentCard
	rdf:type          owl:DatatypeProperty , rdf:Property ;
	rdfs:comment      "If specified, the discount is only available when purchasing using one of the specified payment card types."@en ;
	rdfs:domain       gs1:Discount ;
	rdfs:isDefinedBy  gs1: ;
	rdfs:label        "Only With Payment Card"@en ;
	rdfs:range        gs1:PaymentMethod ;
	sw:term_status    "unstable" .

gs1:isOnlyWithRetailerLoyaltyCard
	rdf:type          owl:DatatypeProperty , rdf:Property ;
	rdfs:comment      "If specified and set to true, the discount is only available for holders of the retailer's own loyalty card."@en ;
	rdfs:domain       gs1:Discount ;
	rdfs:isDefinedBy  gs1: ;
	rdfs:label        "Only For Retailer Loyalty Cardholders"@en ;
	rdfs:range        xsd:boolean ;
	sw:term_status    "unstable" .

gs1:isOnlyWithRetailerPaymentCard
	rdf:type          rdf:Property , owl:DatatypeProperty ;
	rdfs:comment      "If specified and set to true, the discount is only available for holders of the retailer's own store payment card."@en ;
	rdfs:domain       gs1:Discount ;
	rdfs:isDefinedBy  gs1: ;
	rdfs:label        "Only For Retailer Payment Cardholders"@en ;
	rdfs:range        xsd:boolean ;
	sw:term_status    "unstable" .

gs1:isPatterned
	rdf:type  rdf:Property , owl:ObjectProperty ;
	rdfs:comment      "The descriptive term that is used by the product manufacturer to identify whether or not the product has a patterned design."@en ;
	rdfs:domain       gs1:WearableProduct ;
	rdfs:isDefinedBy  gs1: ;
	rdfs:label        "Is Patterned"@en ;
	rdfs:range        gs1:NonbinaryLogicCode ;
	sw:term_status    "stable" .

gs1:isPittedStoned
	rdf:type  rdf:Property , owl:ObjectProperty ;
	rdfs:comment      "The descriptive term that is used by the product manufacturer to identify whether or not a fruit or vegetable product has been de-stoned or pitted prior to being offered for sale."@en ;
	rdfs:domain       gs1:FruitsVegetables ;
	rdfs:isDefinedBy  gs1: ;
	rdfs:label        "Is Pitted Stoned"@en ;
	rdfs:range        gs1:NonbinaryLogicCode ;
	sw:term_status    "stable" .

gs1:isProductRecalled
	rdf:type          owl:DatatypeProperty , rdf:Property , owl:FunctionalProperty ;
	rdfs:comment      "An indicator for the product to determine if the Manufacturer or Supplier has recalled the product."@en ;
	rdfs:domain       gs1:Product ;
	rdfs:isDefinedBy  gs1: ;
	rdfs:label        "Is Product Recalled"@en ;
	rdfs:range        xsd:boolean ;
	sw:term_status    "stable" .

gs1:isPromoterExclusiveOffer
	rdf:type          rdf:Property , owl:DatatypeProperty ;
	rdfs:comment      "Determines whether the offer is only provided by the promoter"@en ;
	rdfs:domain       gs1:Discount ;
	rdfs:isDefinedBy  gs1: ;
	rdfs:label        "Is Promoter Exclusive Offer"@en ;
	rdfs:range        xsd:boolean ;
	sw:term_status    "unstable" .

gs1:isRindEdible
	rdf:type  owl:ObjectProperty , rdf:Property ;
	rdfs:comment      "An indicator whether or not the cheese rind is edible. Some cheeses are coated in plastic or their surface is treated with other traditional substances to increase their shelf life. This can result in the rind no longer being edible."@en ;
	rdfs:domain       gs1:MilkButterCreamYogurtCheeseEggsSubstitutes ;
	rdfs:isDefinedBy  gs1: ;
	rdfs:label        "Is Rind Edible"@en ;
	rdfs:range        gs1:NonbinaryLogicCode ;
	sw:term_status    "stable" .

gs1:isSeedless
	rdf:type  rdf:Property , owl:ObjectProperty ;
	rdfs:comment      "Determines whether the product is seedless as grown."@en ;
	rdfs:domain       gs1:FruitsVegetables ;
	rdfs:isDefinedBy  gs1: ;
	rdfs:label        "Is Seedless"@en ;
	rdfs:range        gs1:NonbinaryLogicCode ;
	sw:term_status    "stable" .

gs1:isShelledPeeled
	rdf:type  owl:ObjectProperty , rdf:Property ;
	rdfs:comment      "The descriptive term that is used by the product manufacturer to identify whether or not the product or its contents have been shelled/peeled prior to being offered for sale."@en ;
	rdfs:domain       gs1:FruitsVegetables ;
	rdfs:isDefinedBy  gs1: ;
	rdfs:label        "Is Shelled or Peeled"@en ;
	rdfs:range        gs1:NonbinaryLogicCode ;
	sw:term_status    "stable" .

gs1:isSliced
	rdf:type    rdf:Property , owl:ObjectProperty ;
	rdfs:comment      "Determines whether the product comes pre-sliced."@en ;
	rdfs:domain       gs1:FoodBeverageTobaccoProduct ;
	rdfs:isDefinedBy  gs1: ;
	rdfs:label        "Is Sliced"@en ;
	rdfs:range        gs1:NonbinaryLogicCode ;
	sw:term_status    "stable" .

gs1:isThermal
	rdf:type   owl:ObjectProperty , rdf:Property ;
	rdfs:comment      "The descriptive term that is used to identify whether the product is thermal."@en ;
	rdfs:domain       gs1:WearableProduct ;
	rdfs:isDefinedBy  gs1: ;
	rdfs:label        "Is Thermal"@en ;
	rdfs:range        gs1:NonbinaryLogicCode ;
	sw:term_status    "stable" .

gs1:isVintage
	rdf:type   rdf:Property , owl:ObjectProperty ;
	rdfs:comment      "Identifies whether the product makes claim to being vintage."@en ;
	rdfs:domain       gs1:Beverage ;
	rdfs:isDefinedBy  gs1: ;
	rdfs:label        "Is Vintage"@en ;
	rdfs:range        gs1:NonbinaryLogicCode ;
	sw:term_status    "stable" .

gs1:isWashedReadyToEat
	rdf:type          owl:ObjectProperty , rdf:Property ;
	rdfs:comment      "Determines whether product has been prewashed and is ready to eat."@en ;
	rdfs:domain       gs1:FruitsVegetables ;
	rdfs:isDefinedBy  gs1: ;
	rdfs:label        "Is Washed Ready To Eat"@en ;
	rdfs:range        gs1:NonbinaryLogicCode ;
	sw:term_status    "stable" .

gs1:isWaterproof
	rdf:type  rdf:Property , owl:ObjectProperty ;
	rdfs:comment      "The descriptive term that is used to identify whether or not the product claims to provide waterproofing to the applied surface."@en ;
	rdfs:domain       gs1:WearableProduct ;
	rdfs:isDefinedBy  gs1: ;
	rdfs:label        "Is Waterproof"@en ;
	rdfs:range        gs1:NonbinaryLogicCode ;
	sw:term_status    "stable" .

gs1:isWearableItemDisposable
	rdf:type          owl:ObjectProperty , rdf:Property ;
	rdfs:comment      "Identifies whether or not the product is intended to be disposed of after single use or a limited period of use."@en ;
	rdfs:domain       gs1:WearableProduct ;
	rdfs:isDefinedBy  gs1: ;
	rdfs:label        "Is Wearable Item Disposable"@en ;
	rdfs:range        gs1:NonbinaryLogicCode ;
	sw:term_status    "stable" .

gs1:itemOffered
	rdf:type  rdf:Property , owl:ObjectProperty ;
	rdfs:comment      "The product included in the offer."@en ;
	rdfs:domain       gs1:Offer ;
	rdfs:isDefinedBy  gs1: ;
	rdfs:label        "Item Offered"@en ;
	rdfs:range        gs1:Product ;
	sw:term_status    "stable" ;
	skos:exactMatch   schema:itemOffered .

gs1:juiceContentPercent
	rdf:type          owl:DatatypeProperty , rdf:Property ;
	rdfs:comment      "The fruit juice content of the product expressed as a percentage."@en ;
	rdfs:domain       gs1:FoodBeverageTobaccoProduct ;
	rdfs:isDefinedBy  gs1: ;
	rdfs:label        "Juice Content Percent"@en ;
	rdfs:range        xsd:float ;
	sw:term_status    "stable" .

gs1:jws
	rdf:type           owl:ObjectProperty , rdf:Property ;
	rdfs:comment        "A link to a JSON Web Signature"@en ;
	rdfs:domain         gs1:Product , schema:Product ;
	rdfs:label          "JSON Web Signature"@en ;
	rdfs:range          xsd:anyURI ;
	rdfs:subPropertyOf  gs1:linkType ;
	sw:term_status      "stable" .

gs1:latitude
	rdf:type     owl:DatatypeProperty , rdf:Property ;
	rdfs:comment       "Angular distance North or South from the earth's equator measured through 90 degrees."@en ;
	rdfs:domain        gs1:GeoCoordinates ;
	rdfs:isDefinedBy   gs1: ;
	rdfs:label         "Latitude"@en ;
	rdfs:range         xsd:string ;
	sw:term_status     "stable" ;
	skos:exactMatch    schema:latitude ;
	skos:relatedMatch  geo:lat .

gs1:leasedFrom
	rdf:type  rdf:Property , owl:ObjectProperty ;
	rdfs:comment      "Links to the organisation (lessor) from which this place is leased."@en ;
	rdfs:domain       gs1:Place ;
	rdfs:isDefinedBy  gs1: ;
	rdfs:label        "Leased from"@en ;
	rdfs:range        gs1:Organization ;
	sw:term_status    "stable" .

gs1:leasedTo
	rdf:type    rdf:Property , owl:ObjectProperty ;
	rdfs:comment      "Links to the organisation(s) (lessee(s)) to which this place is leased. Property SHOULD be applied to a specific sub-location, rather than a main location, wherever possible."@en ;
	rdfs:domain       gs1:Place ;
	rdfs:isDefinedBy  gs1: ;
	rdfs:label        "Leased to"@en ;
	rdfs:range        gs1:Organization ;
	sw:term_status    "stable" .

gs1:leaveReview
	rdf:type   owl:ObjectProperty , rdf:Property ;
	rdfs:comment        "A link through which a review can be added."@en ;
	rdfs:domain         owl:Thing ;
	rdfs:label          "Leave a review"@en ;
	rdfs:range          xsd:anyURI ;
	rdfs:subPropertyOf  gs1:linkType ;
	sw:term_status      "stable" .

gs1:lesseeOf
	rdf:type    rdf:Property , owl:ObjectProperty ;
	rdfs:comment      "Links to the place(s) for which this organisation is the lessee (i.e., this organisation leases those places from another organisation, the lessor)."@en ;
	rdfs:domain       gs1:Organization ;
	rdfs:isDefinedBy  gs1: ;
	rdfs:label        "Lessee of location"@en ;
	rdfs:range        gs1:Place ;
	sw:term_status    "stable" .

gs1:lessorFor
	rdf:type   rdf:Property , owl:ObjectProperty ;
	rdfs:comment      "Links to the place(s) for which this organisation is the lessor (i.e., this organisation leases those places to others)."@en ;
	rdfs:domain       gs1:Organization ;
	rdfs:isDefinedBy  gs1: ;
	rdfs:label        "Lessor for"@en ;
	rdfs:range        gs1:Place ;
	sw:term_status    "stable" .

gs1:line
	rdf:type        rdf:Property , owl:DatatypeProperty ;
	rdfs:comment      "A line is a point-to-point path consisting of two or more point objects separated by a space. A single line segment (i.e., straight line) is expressed as two points.  A multi-line path (i.e., open polygon) is expressed as a series of three or more points. For a closed shape, gs1:polygon SHALL be used."@en ;
	rdfs:domain       gs1:GeoShape ;
	rdfs:isDefinedBy  gs1: ;
	rdfs:label        "Line"@en ;
	rdfs:range        xsd:string ;
	sw:term_status    "stable" ;
	skos:exactMatch   schema:line .

gs1:linkType
	rdf:type     owl:ObjectProperty , rdf:Property ;
	rdfs:comment       "Provides a URL for related information or services. This is not expected to be used directly but provides a super property for all other link types in the GS1 ecosystem."@en ;
	rdfs:domain        owl:Thing ;
	rdfs:isDefinedBy   gs1: ;
	rdfs:label         "Link Type"@en ;
	rdfs:range         xsd:anyURI ;
	sw:term_status     "stable" ;
	skos:altLabel      "Link Type"@en ;
	skos:broader       schema:url ;
	skos:relatedMatch  schema:mainEntityOfPage , schema:sameAs .

gs1:location
	rdf:type    rdf:Property , owl:ObjectProperty ;
	rdfs:comment      "The place(s) associated with an organization."@en ;
	rdfs:domain       gs1:Organization ;
	rdfs:isDefinedBy  gs1: ;
	rdfs:label        "Has Location"@en ;
	rdfs:range        gs1:Place ;
	sw:term_status    "stable" ;
	skos:exactMatch   schema:location .

gs1:locationGLN
	rdf:type  owl:DatatypeProperty , rdf:Property ;
	rdfs:comment      "13-digit GLN that is being used to identify a physical or digital location. If gs1:glnType is present, gs1:locationGLN SHALL only be used when gs1:GLN_TypeCode includes FIXED_PHYSICAL_LOCATION, MOBILE_PHYSICAL_LOCATION, or DIGITAL_LOCATION"@en ;
	rdfs:domain       gs1:Place ;
	rdfs:isDefinedBy  gs1: ;
	rdfs:label        "Location GLN"@en ;
	rdfs:range        xsd:string ;
	sw:term_status    "stable" .

gs1:locationHistory
	rdf:type  owl:ObjectProperty , rdf:Property ;
	rdfs:comment      "Provides details on if and when a location is active or inactive."@en ;
	rdfs:domain       gs1:Place ;
	rdfs:isDefinedBy  gs1: ;
	rdfs:label        "Has Location History"@en ;
	rdfs:range        gs1:LocationStatusHistory ;
	sw:term_status    "stable" .

gs1:locationID
	rdf:type  owl:DatatypeProperty , rdf:Property ;
	rdfs:comment      "Identifier value associated to a location. This value SHALL follow rules set forth by the administrating organisation designated in gs1:LocationID_Type."@en ;
	rdfs:domain       gs1:LocationID_Details ;
	rdfs:isDefinedBy  gs1: ;
	rdfs:label        "Location ID"@en ;
	rdfs:range        xsd:string ;
	sw:term_status    "stable" .

gs1:locationID_Qualifier
	rdf:type          owl:DatatypeProperty , rdf:Property ;
	rdfs:comment      "Secondary qualifier to supplement gs1:LocationID_Type meaning. May be used with proprietary ID code values to define identifier administrator."@en ;
	rdfs:domain       gs1:LocationID_Details ;
	rdfs:isDefinedBy  gs1: ;
	rdfs:label        "Location ID Qualifier"@en ;
	rdfs:range        xsd:string ;
	sw:term_status    "stable" .

gs1:locationID_Type
	rdf:type  owl:ObjectProperty , rdf:Property ;
	rdfs:comment      "Organisation that administers the gs1:locationID or the name of the ID itself.  Value from gs1:LocationID_Type code list."@en ;
	rdfs:domain       gs1:LocationID_Details ;
	rdfs:isDefinedBy  gs1: ;
	rdfs:label        "Location ID"@en ;
	rdfs:range        gs1:LocationID_Type ;
	sw:term_status    "stable" .

gs1:locationID_URI
	rdf:type  owl:ObjectProperty , rdf:Property ;
	rdfs:comment      "A URI that links to information about the gs1:locationID."@en ;
	rdfs:domain       gs1:LocationID_Details ;
	rdfs:isDefinedBy  gs1: ;
	rdfs:label        "Location ID URI"@en ;
	rdfs:range        xsd:anyURI ;
	sw:term_status    "stable" .

gs1:locationInfo
	rdf:type  owl:ObjectProperty , rdf:Property ;
	rdfs:comment        "A link to a map, directions, or other location-related information.  For B2B location  information, see gs1:logisticsInfo.  For details specific to hours of operation, see gs1:openingHoursInfo"@en ;
	rdfs:domain         owl:Thing ;
	rdfs:label          "Location information"@en ;
	rdfs:range          xsd:anyURI ;
	rdfs:subPropertyOf  gs1:linkType ;
	sw:term_status      "stable" .

gs1:locationRole
	rdf:type  rdf:Property , owl:ObjectProperty ;
	rdfs:comment      "A location classification based on the purpose, type of site and/or what occurs there. Repeatable value from gs1:LocationRoleType code list."@en ;
	rdfs:domain       gs1:Place ;
	rdfs:isDefinedBy  gs1: ;
	rdfs:label        "Location Role"@en ;
	rdfs:range        gs1:LocationRoleType ;
	sw:term_status    "stable" .

gs1:locationStatus
	rdf:type  owl:ObjectProperty , rdf:Property ;
	rdfs:comment      "Designation of active/inactive status of a location."@en ;
	rdfs:domain       gs1:LocationStatusHistory ;
	rdfs:isDefinedBy  gs1: ;
	rdfs:label        "Location Status"@en ;
	rdfs:range        gs1:StatusType ;
	sw:term_status    "stable" .

gs1:logisticsInfo
	rdf:type  owl:ObjectProperty , rdf:Property ;
	rdfs:comment        "A link to B2B logistics information related to a physical location."@en ;
	rdfs:domain         owl:Thing ;
	rdfs:label          "Logistics information"@en ;
	rdfs:range          xsd:anyURI ;
	rdfs:subPropertyOf  gs1:linkType ;
	sw:term_status      "stable" .

gs1:longitude
	rdf:type    owl:DatatypeProperty , rdf:Property ;
	rdfs:comment       "The arc or portion of the earth's equator intersected between the meridian of a given place and the prime meridian and expressed in degrees"@en ;
	rdfs:domain        gs1:GeoCoordinates ;
	rdfs:isDefinedBy   gs1: ;
	rdfs:label         "Longitude"@en ;
	rdfs:range         xsd:string ;
	sw:term_status     "stable" ;
	skos:exactMatch    schema:longitude ;
	skos:relatedMatch  geo:long .

gs1:loyaltyProgram
	rdf:type  owl:ObjectProperty , rdf:Property ;
	rdfs:comment        "A link to information about a loyalty program, including a member's current status and/or a registration option for new members"@en ;
	rdfs:domain         owl:Thing ;
	rdfs:label          "Loyalty program"@en ;
	rdfs:range          xsd:anyURI ;
	rdfs:subPropertyOf  gs1:linkType ;
	sw:term_status      "stable" .

gs1:magnesiumPerNutrientBasis
	rdf:type          owl:ObjectProperty , rdf:Property ;
	rdfs:comment      "Magnesium per specified nutrient basis quantity."@en ;
	rdfs:domain       gs1:FoodBeverageTobaccoProduct ;
	rdfs:isDefinedBy  gs1: ;
	rdfs:label        "Magnesium Per Nutrient Basis Quantity"@en ;
	rdfs:range        gs1:NutritionMeasurementType ;
	sw:term_status    "stable" .

gs1:makesOffer
	rdf:type  rdf:Property , owl:ObjectProperty ;
	rdfs:comment      "An offer made by an organization."@en ;
	rdfs:domain       gs1:Organization ;
	rdfs:isDefinedBy  gs1: ;
	rdfs:label        "Makes Offer"@en ;
	rdfs:range        gs1:Offer ;
	sw:term_status    "stable" ;
	skos:exactMatch   schema:makesOffer .

gs1:managedBy
	rdf:type   rdf:Property , owl:ObjectProperty ;
	rdfs:comment      "Links to the organisation that manages this place or organisation, as designated by the owner or another organisation."@en ;
	rdfs:domain       _:b0 ;
	rdfs:isDefinedBy  gs1: ;
	rdfs:label        "Managed by"@en ;
	rdfs:range        gs1:Organization ;
	sw:term_status    "stable" .

gs1:managedFor
	rdf:type  rdf:Property , owl:ObjectProperty ;
	rdfs:comment      "Links to the organisation(s) for whom this place is managed. Property SHOULD be applied to a specific sub-location, rather than a main location, wherever possible."@en ;
	rdfs:domain       gs1:Place ;
	rdfs:isDefinedBy  gs1: ;
	rdfs:label        "Managed for"@en ;
	rdfs:range        gs1:Organization ;
	sw:term_status    "stable" .

gs1:manages
	rdf:type     rdf:Property , owl:ObjectProperty ;
	rdfs:comment      "Links to the place(s) or organisation(s) that this organisation manages, on behalf of the owner or another organisation."@en ;
	rdfs:domain       gs1:Organization ;
	rdfs:isDefinedBy  gs1: ;
	rdfs:label        "Manages"@en ;
	rdfs:range        _:b0 ;
	sw:term_status    "stable" .

gs1:manganesePerNutrientBasis
	rdf:type          owl:ObjectProperty , rdf:Property ;
	rdfs:comment      "Manganese per specified nutrient basis quantity."@en ;
	rdfs:domain       gs1:FoodBeverageTobaccoProduct ;
	rdfs:isDefinedBy  gs1: ;
	rdfs:label        "Manganese Per Nutrient Basis Quantity"@en ;
	rdfs:range        gs1:NutritionMeasurementType ;
	sw:term_status    "stable" .

gs1:manufacturer
	rdf:type  owl:ObjectProperty , rdf:Property ;
	rdfs:comment      "The organization that produces the item."@en ;
	rdfs:domain       gs1:Product ;
	rdfs:isDefinedBy  gs1: ;
	rdfs:label        "Has Manufacturer"@en ;
	rdfs:range        gs1:Organization ;
	sw:term_status    "stable" ;
	skos:exactMatch   schema:manufacturer .

gs1:manufacturerPreparationCode
	rdf:type          rdf:Property , owl:ObjectProperty ;
	rdfs:comment      "Code indicating the preparation methods that a manufacturer has used in the manufacturing of a product for example DEEP_FRY."@en ;
	rdfs:domain       gs1:FoodAndBeveragePreparationInformation ;
	rdfs:isDefinedBy  gs1: ;
	rdfs:label        "Manufacturer Preparation Code"@en ;
	rdfs:range        gs1:PreparationTypeCode ;
	sw:term_status    "stable" .

gs1:manufacturersWarranty
	rdf:type          owl:ObjectProperty , rdf:Property ;
	rdfs:comment      "The warranty associated with the product."@en ;
	rdfs:domain       gs1:Product ;
	rdfs:isDefinedBy  gs1: ;
	rdfs:label        "Has Manufacturer's Warranty"@en ;
	rdfs:range        gs1:WarrantyPromise ;
	rdfs:seeAlso      schema:warranty ;
	sw:term_status    "stable" ;
	skos:broadMatch   schema:warranty .

gs1:manufacturingPlant
	rdf:type          owl:ObjectProperty , rdf:Property ;
	rdfs:comment      "A physical location consisting of one or more buildings with facilities for manufacturing."@en ;
	rdfs:domain       gs1:Product ;
	rdfs:isDefinedBy  gs1: ;
	rdfs:label        "Has Manufacturing Plant"@en ;
	rdfs:range        gs1:Organization ;
	sw:term_status    "stable" .

gs1:massPerUnitArea
	rdf:type  owl:FunctionalProperty , owl:ObjectProperty , rdf:Property ;
	rdfs:comment      "The mass per unit area of the item. This can be given using a number of different AI ranges that depend on the units in which the mass and area are measured."@en ;
	rdfs:domain       gs1:Product ;
	rdfs:isDefinedBy  gs1: ;
	rdfs:label        "Mass per unit area"@en ;
	rdfs:range        gs1:QuantitativeValue ;
	sw:term_status    "stable" ;
	skos:altLabel     "Mass per unit area"@en ;
	skos:prefLabel    "337n" .

gs1:masterData
	rdf:type    owl:ObjectProperty , rdf:Property ;
	rdfs:comment        "A link to a source of structured master data for the entity. This is typically for B2B applications."@en ;
	rdfs:domain         owl:Thing ;
	rdfs:label          "Master data"@en ;
	rdfs:range          xsd:anyURI ;
	rdfs:subPropertyOf  gs1:linkType ;
	sw:term_status      "stable" .

gs1:maturationMethod
	rdf:type  rdf:Property , owl:ObjectProperty ;
	rdfs:comment      "The method of maturity for the item for example tree ripened or jet fresh."@en ;
	rdfs:domain       gs1:FruitsVegetables ;
	rdfs:isDefinedBy  gs1: ;
	rdfs:label        "Maturation Method Code"@en ;
	rdfs:range        gs1:MaturationMethodCode ;
	sw:term_status    "stable" .

gs1:maxPrice
	rdf:type    owl:DatatypeProperty , rdf:Property ;
	rdfs:comment      "Provides a maximum price value as a floating-point numeric value that is qualified by the corresponding currency. See also gs1:priceCurrency"@en ;
	rdfs:domain       gs1:PriceSpecification ;
	rdfs:isDefinedBy  gs1: ;
	rdfs:label        "Maximum Price"@en ;
	rdfs:range        xsd:float ;
	rdfs:seeAlso      gs1:priceCurrency ;
	sw:term_status    "stable" ;
	skos:exactMatch   schema:maxPrice .

gs1:maximumDiscountAmount
	rdf:type          rdf:Property , owl:DatatypeProperty ;
	rdfs:comment      "Links to a gs1:PriceSpecification that indicates in terms of an amount and specified currency, the maximum discount on the sales price associated with a particular gs1:Discount. This property can be used to express 'up to $10 off'."@en ;
	rdfs:domain       gs1:Discount ;
	rdfs:isDefinedBy  gs1: ;
	rdfs:label        "Maximum Discount Amount"@en ;
	rdfs:range        gs1:PriceSpecification ;
	sw:term_status    "unstable" .

gs1:maximumDiscountPercentage
	rdf:type          rdf:Property , owl:DatatypeProperty ;
	rdfs:comment      "A floating-point value indicating a maximum percentage discount on the sales price associated with a particular gs1:Discount.  This property can be used to express 'up to 15% discount'."@en ;
	rdfs:domain       gs1:Discount ;
	rdfs:isDefinedBy  gs1: ;
	rdfs:label        "Maximum Discount Percentage"@en ;
	rdfs:range        xsd:float ;
	sw:term_status    "unstable" .

gs1:maximumOptimumConsumptionTemperature
	rdf:type          rdf:Property , owl:ObjectProperty ;
	rdfs:comment      "The upper limit drinking temperature of the optimum range of the drinking temperature. The optimum range of the drinking temperature is a recommendation and is based on the experience of the individual producer. Allows for the representation of the same value in different units of measure but not multiple values."@en ;
	rdfs:domain       gs1:FoodAndBeveragePreparationInformation ;
	rdfs:isDefinedBy  gs1: ;
	rdfs:label        "Maximum Optimum Consumption Temperature"@en ;
	rdfs:range        gs1:QuantitativeValue ;
	sw:term_status    "stable" .

gs1:maximumQualifyingItems
	rdf:type          owl:DatatypeProperty , rdf:Property ;
	rdfs:comment      "Specifies the maximum number of items that qualify for a particular gs1:Discount. This property can be used to express 'maximum N items per customer'."@en ;
	rdfs:domain       gs1:Discount ;
	rdfs:isDefinedBy  gs1: ;
	rdfs:label        "Maximum Qualifying Items"@en ;
	rdfs:range        xsd:integer ;
	sw:term_status    "unstable" .

gs1:maximumQualifyingSpend
	rdf:type          rdf:Property , owl:DatatypeProperty ;
	rdfs:comment      "Links to a gs1:PriceSpecification that indicates in terms of an amount and specified currency, the maximum spend that qualifies for a particular gs1:Discount. This property can be used to express 'for purchases of up to $100'."@en ;
	rdfs:domain       gs1:Discount ;
	rdfs:isDefinedBy  gs1: ;
	rdfs:label        "Maximum Qualifying Spend"@en ;
	rdfs:range        gs1:PriceSpecification ;
	sw:term_status    "unstable" .

gs1:meatPoultryType
	rdf:type  owl:DatatypeProperty , rdf:Property ;
	rdfs:comment      "The fish, meat, or poultry type for this food and beverage item."@en ;
	rdfs:domain       gs1:MeatPoultry ;
	rdfs:isDefinedBy  gs1: ;
	rdfs:label        "Meat Poultry Type Code"@en ;
	rdfs:range        rdf:langString ;
	sw:term_status    "stable" .

gs1:menuInfo
	rdf:type      owl:ObjectProperty , rdf:Property ;
	rdfs:comment        "A link to menu details. This may include food menus, services, or other offerings provided by an organisation or at a location.  For details specific to allergens only, see gs1:allergenInfo .  For details specific to nutrition information only, see gs1:nutritionalInfo .  For details specific to ingredients only, see gs1:ingredientsInfo ."@en ;
	rdfs:domain         owl:Thing ;
	rdfs:label          "Menu information"@en ;
	rdfs:range          xsd:anyURI ;
	rdfs:subPropertyOf  gs1:linkType ;
	sw:term_status      "stable" .

gs1:minPrice
	rdf:type    owl:DatatypeProperty , rdf:Property ;
	rdfs:comment      "Provides a minimum price value as a floating-point numeric value that is qualified by the corresponding currency. See also gs1:priceCurrency"@en ;
	rdfs:domain       gs1:PriceSpecification ;
	rdfs:isDefinedBy  gs1: ;
	rdfs:label        "Minimum Price"@en ;
	rdfs:range        xsd:float ;
	rdfs:seeAlso      gs1:priceCurrency ;
	sw:term_status    "stable" ;
	skos:exactMatch   schema:minPrice .

gs1:minimumDiscountAmount
	rdf:type          rdf:Property , owl:DatatypeProperty ;
	rdfs:comment      "Links to a gs1:PriceSpecification that indicates in terms of an amount and specified currency, the minimum discount on the sales price associated with a particular gs1:Discount. This property can be used to express 'at least $10 off'."@en ;
	rdfs:domain       gs1:Discount ;
	rdfs:isDefinedBy  gs1: ;
	rdfs:label        "Minimum Discount Amount"@en ;
	rdfs:range        gs1:PriceSpecification ;
	sw:term_status    "unstable" .

gs1:minimumDiscountPercentage
	rdf:type          owl:DatatypeProperty , rdf:Property ;
	rdfs:comment      "A floating-point value indicating a minimum percentage discount on the sales price associated with a particular gs1:Discount.  This property can be used to express 'at least 15% discount'."@en ;
	rdfs:domain       gs1:Discount ;
	rdfs:isDefinedBy  gs1: ;
	rdfs:label        "Minimum Discount Percentage"@en ;
	rdfs:range        xsd:float ;
	sw:term_status    "unstable" .

gs1:minimumFishContent
	rdf:type          owl:ObjectProperty , rdf:Property ;
	rdfs:comment      "The minimum amount of fish contained in a food and beverage product expressed as a measurement."@en ;
	rdfs:domain       gs1:Seafood ;
	rdfs:isDefinedBy  gs1: ;
	rdfs:label        "Minimum Fish Content"@en ;
	rdfs:range        gs1:QuantitativeValue ;
	sw:term_status    "stable" .

gs1:minimumMeatPoultryContent
	rdf:type          owl:ObjectProperty , rdf:Property ;
	rdfs:comment      "The minimum amount of fish, meat or poultry contained in a food and beverage product expressed as a measurement."@en ;
	rdfs:domain       gs1:MeatPoultry ;
	rdfs:isDefinedBy  gs1: ;
	rdfs:label        "Minimum Meat Poultry Content"@en ;
	rdfs:range        gs1:QuantitativeValue ;
	sw:term_status    "stable" .

gs1:minimumOptimumConsumptionTemperature
	rdf:type          owl:ObjectProperty , rdf:Property ;
	rdfs:comment      "The lower limit drinking temperature of the optimum range of the drinking temperature. The optimum range of the drinking temperature is a recommendation and is based on the experience of the individual producer. Allows for the representation of the same value in different units of measure but not multiple values."@en ;
	rdfs:domain       gs1:FoodAndBeveragePreparationInformation ;
	rdfs:isDefinedBy  gs1: ;
	rdfs:label        "Minimum Optimum Consumption Temperature"@en ;
	rdfs:range        gs1:QuantitativeValue ;
	sw:term_status    "stable" .

gs1:minimumQualifyingItems
	rdf:type          rdf:Property , owl:DatatypeProperty ;
	rdfs:comment      "Specifies the minimum number of items that must be purchased to qualify for a particular gs1:Discount. This property can be used to express 'if you buy at least N items'."@en ;
	rdfs:domain       gs1:Discount ;
	rdfs:isDefinedBy  gs1: ;
	rdfs:label        "Minimum Qualifying Items"@en ;
	rdfs:range        xsd:integer ;
	sw:term_status    "unstable" .

gs1:minimumQualifyingSpend
	rdf:type          rdf:Property , owl:DatatypeProperty ;
	rdfs:comment      "Links to a gs1:PriceSpecification that indicates in terms of an amount and specified currency, the minimum spend required to qualify for a particular gs1:Discount. This property can be used to express 'if you spend at least $100'."@en ;
	rdfs:domain       gs1:Discount ;
	rdfs:isDefinedBy  gs1: ;
	rdfs:label        "Minimum Qualifying Spend"@en ;
	rdfs:range        gs1:PriceSpecification ;
	sw:term_status    "unstable" .

gs1:molybdenumPerNutrientBasis
	rdf:type          rdf:Property , owl:ObjectProperty ;
	rdfs:comment      "Molybdenum per specified nutrient basis quantity."@en ;
	rdfs:domain       gs1:FoodBeverageTobaccoProduct ;
	rdfs:isDefinedBy  gs1: ;
	rdfs:label        "Molybdenum Per Nutrient Basis Quantity"@en ;
	rdfs:range        gs1:NutritionMeasurementType ;
	sw:term_status    "stable" .

gs1:monounsaturatedFatPerNutrientBasis
	rdf:type          rdf:Property , owl:ObjectProperty ;
	rdfs:comment      "Monounsaturated fat per specified nutrient basis quantity."@en ;
	rdfs:domain       gs1:FoodBeverageTobaccoProduct ;
	rdfs:isDefinedBy  gs1: ;
	rdfs:label        "Monounsaturated Fat Per Nutrient Basis Quantity"@en ;
	rdfs:range        gs1:NutritionMeasurementType ;
	sw:term_status    "stable" .

gs1:netArea
	rdf:type     owl:FunctionalProperty , rdf:Property , owl:ObjectProperty ;
	rdfs:comment      "The net area of the item. This can be given using a number of different AI ranges that depend on the units in which the area is measured."@en ;
	rdfs:domain       gs1:Product ;
	rdfs:isDefinedBy  gs1: ;
	rdfs:label        "Net area"@en ;
	rdfs:range        gs1:QuantitativeValue ;
	sw:term_status    "stable" ;
	skos:altLabel     "Net area"@en ;
	skos:prefLabel    "314n, 350n, 351n" .

gs1:netContent
	rdf:type  owl:FunctionalProperty , rdf:Property , owl:ObjectProperty ;
	rdfs:comment      "The quantity of the product contained by a package, usually as claimed on the label. Indicates the net content of the total product. For fixed value products use the value claimed on the package, to avoid variable fill rate issue that arises with some product which are sold by volume or weight, and whose actual content may vary slightly from batch to batch."@en ;
	rdfs:domain       gs1:Product ;
	rdfs:isDefinedBy  gs1: ;
	rdfs:label        "Net content"@en ;
	rdfs:range        gs1:QuantitativeValue ;
	sw:term_status    "stable" ;
	skos:altLabel     "Net content"@en ;
	skos:prefLabel    "360n, 361n, 364n, 365n, 366n" .

gs1:netWeight
	rdf:type     owl:FunctionalProperty , owl:ObjectProperty , rdf:Property ;
	rdfs:comment        "Used to identify the net weight of the product. Net Weight excludes all packaging material, including the packaging material of all lower-level GTINs. Example:11.5 kgm."@en ;
	rdfs:domain         gs1:Product ;
	rdfs:isDefinedBy    gs1: ;
	rdfs:label          "Net weight"@en ;
	rdfs:range          gs1:QuantitativeValue ;
	rdfs:subPropertyOf  schema:weight ;
	sw:term_status      "stable" ;
	skos:altLabel       "Net weight"@en ;
	skos:prefLabel      "310n, 320n, 356n, 357n" .

gs1:niacinPerNutrientBasis
	rdf:type          owl:ObjectProperty , rdf:Property ;
	rdfs:comment      "Niacin per specified nutrient basis quantity."@en ;
	rdfs:domain       gs1:FoodBeverageTobaccoProduct ;
	rdfs:isDefinedBy  gs1: ;
	rdfs:label        "Niacin Per Nutrient Basis Quantity"@en ;
	rdfs:range        gs1:NutritionMeasurementType ;
	sw:term_status    "stable" .

gs1:numberOfServingsPerPackage
	rdf:type          rdf:Property , owl:DatatypeProperty ;
	rdfs:comment      "The total number of servings contained in the package."@en ;
	rdfs:domain       gs1:FoodBeverageTobaccoProduct ;
	rdfs:isDefinedBy  gs1: ;
	rdfs:label        "Number of Servings Per Package"@en ;
	rdfs:range        xsd:float ;
	sw:term_status    "stable" .

gs1:numberOfServingsPerPackageMeasurementPrecision
	rdf:type          rdf:Property , owl:ObjectProperty ;
	rdfs:comment      "Code indicating whether the number of servings per package is exact or approximate."@en ;
	rdfs:domain       gs1:FoodBeverageTobaccoProduct ;
	rdfs:isDefinedBy  gs1: ;
	rdfs:label        "Number of Servings Per Package Measurement Precision"@en ;
	rdfs:range        gs1:MeasurementPrecisionCode ;
	sw:term_status    "stable" .

gs1:numberOfServingsRangeDescription
	rdf:type          rdf:Property , owl:DatatypeProperty ;
	rdfs:comment      "A free text field specifying a range for the number of servings contained in the package."@en ;
	rdfs:domain       gs1:FoodBeverageTobaccoProduct ;
	rdfs:isDefinedBy  gs1: ;
	rdfs:label        "Number of Servings Range Description"@en ;
	rdfs:range        rdf:langString ;
	sw:term_status    "stable" .

gs1:nutrientBasisQuantity
	rdf:type          owl:ObjectProperty , rdf:Property ;
	rdfs:comment      "Quantity on which the nutrient information has been based; for example, per 100 grams. When specified, nutrientBasisQuantity establishes the basis for all contained nutrient records."@en ;
	rdfs:domain       gs1:FoodBeverageTobaccoProduct ;
	rdfs:isDefinedBy  gs1: ;
	rdfs:label        "Nutrient Basis Quantity"@en ;
	rdfs:range        gs1:QuantitativeValue ;
	sw:term_status    "stable" .

gs1:nutrientBasisQuantityType
	rdf:type          rdf:Property , owl:ObjectProperty ;
	rdfs:comment      "The type of quantity specified in the nutrientBasisQuantity for example measurement, serving size, or container. This is used in conjunction with the nutrientBasisQuantity."@en ;
	rdfs:domain       gs1:FoodBeverageTobaccoProduct ;
	rdfs:isDefinedBy  gs1: ;
	rdfs:label        "Nutrient Basis Quantity Type Code"@en ;
	rdfs:range        gs1:NutrientBasisQuantityCode ;
	sw:term_status    "stable" .

gs1:nutrientMeasurementPrecision
	rdf:type          owl:ObjectProperty , rdf:Property ;
	rdfs:comment      "The Code indicating whether the specified nutrient content is exact or approximate."@en ;
	rdfs:domain       gs1:FoodBeverageTobaccoProduct ;
	rdfs:isDefinedBy  gs1: ;
	rdfs:label        "Nutrient Measurement Precision"@en ;
	rdfs:range        gs1:MeasurementPrecisionCode ;
	sw:term_status    "stable" .

gs1:nutritionalClaim
	rdf:type  rdf:Property , owl:ObjectProperty ;
	rdfs:comment      "Code indicating a nutritional claim applicable to the product, for example FAT_FREE."@en ;
	rdfs:domain       gs1:FoodBeverageTobaccoProduct ;
	rdfs:isDefinedBy  gs1: ;
	rdfs:label        "Nutritional Claim Code"@en ;
	rdfs:range        gs1:NutritionalClaimTypeCode ;
	sw:term_status    "stable" .

gs1:nutritionalClaimStatement
	rdf:type          rdf:Property , owl:DatatypeProperty ;
	rdfs:comment      "Free text field for any additional nutritional claims."@en ;
	rdfs:domain       gs1:FoodBeverageTobaccoProduct ;
	rdfs:isDefinedBy  gs1: ;
	rdfs:label        "Nutritional Claim Statement"@en ;
	rdfs:range        rdf:langString ;
	sw:term_status    "stable" .

gs1:nutritionalInfo
	rdf:type  owl:ObjectProperty , rdf:Property ;
	rdfs:comment        "A link to nutritional facts."@en ;
	rdfs:domain         owl:Thing ;
	rdfs:label          "Nutritional Information"@en ;
	rdfs:range          xsd:anyURI ;
	rdfs:subPropertyOf  gs1:linkType ;
	sw:term_status      "stable" .

gs1:occupiedBy
	rdf:type  rdf:Property , owl:ObjectProperty ;
	rdfs:comment      "Links to the organisation(s) that occupy this place. Property SHOULD be applied to a specific sub-location, rather than a main location, wherever possible."@en ;
	rdfs:domain       gs1:Place ;
	rdfs:isDefinedBy  gs1: ;
	rdfs:label        "Occupied by"@en ;
	rdfs:range        gs1:Organization ;
	sw:term_status    "stable" .

gs1:occupies
	rdf:type    rdf:Property , owl:ObjectProperty ;
	rdfs:comment      "Links to the place(s) that this organisation occupies."@en ;
	rdfs:domain       gs1:Organization ;
	rdfs:isDefinedBy  gs1: ;
	rdfs:label        "Occupies location"@en ;
	rdfs:range        gs1:Place ;
	sw:term_status    "stable" .

gs1:offerDescription
	rdf:type  owl:DatatypeProperty , rdf:Property ;
	rdfs:comment        "A description of the offer including goods or services offered for sale or use."@en ;
	rdfs:domain         gs1:Offer ;
	rdfs:isDefinedBy    gs1: ;
	rdfs:label          "Offer Description"@en ;
	rdfs:range          rdf:langString ;
	rdfs:subPropertyOf  schema:description ;
	sw:term_status      "stable" ;
	skos:related        schema:Offer .

gs1:offerDiscount
	rdf:type  owl:ObjectProperty , rdf:Property ;
	rdfs:comment      "A discount associated with an offer."@en ;
	rdfs:domain       gs1:Offer ;
	rdfs:isDefinedBy  gs1: ;
	rdfs:label        "Offer Discount"@en ;
	rdfs:range        gs1:Discount ;
	sw:term_status    "stable" .

gs1:offerRedemptionType
	rdf:type          owl:DatatypeProperty , rdf:Property ;
	rdfs:comment      "A code indicating the type of redemptions that apply to the offer, for example single use."@en ;
	rdfs:domain       gs1:Discount ;
	rdfs:isDefinedBy  gs1: ;
	rdfs:label        "Offer Redemption Type"@en ;
	rdfs:range        gs1:OfferRedemptionTypeCode ;
	sw:term_status    "unstable" .

gs1:offerRedemptionURL
	rdf:type          rdf:Property , owl:ObjectProperty ;
	rdfs:comment      "The URL where the offer seeker will need to go in order to redeem the offer for an online redemption."@en ;
	rdfs:domain       gs1:Offer ;
	rdfs:isDefinedBy  gs1: ;
	rdfs:label        "Offer Redemption URL"@en ;
	rdfs:range        gs1:ReferencedFileDetails ;
	sw:term_status    "unstable" ;
	skos:exactMatch   schema:itemOffered .

gs1:offerRestrictionDescription
	rdf:type            rdf:Property , owl:DatatypeProperty ;
	rdfs:comment        "A description of what the offer is restricted to, relative to all other offerings by the issuer, for example payment restrictions, subscription required, new customers only."@en ;
	rdfs:domain         gs1:Discount ;
	rdfs:isDefinedBy    gs1: ;
	rdfs:label          "Offer Restriction Description"@en ;
	rdfs:range          rdf:langString ;
	rdfs:subPropertyOf  schema:name ;
	sw:term_status      "unstable" ;
	skos:related        schema:Offer .

gs1:openingHoursInfo
	rdf:type  owl:ObjectProperty , rdf:Property ;
	rdfs:comment        "A link to details on hours of operation."@en ;
	rdfs:domain         owl:Thing ;
	rdfs:label          "Opening hours information"@en ;
	rdfs:range          xsd:anyURI ;
	rdfs:subPropertyOf  gs1:linkType ;
	sw:term_status      "stable" .

gs1:organicClaim
	rdf:type  owl:ObjectProperty , rdf:Property ;
	rdfs:comment      "Relates to an organic claim about the product"@en ;
	rdfs:domain       gs1:Product ;
	rdfs:isDefinedBy  gs1: ;
	rdfs:label        "Has Organic Claim"@en ;
	rdfs:range        gs1:OrganicClaimDetails ;
	sw:term_status    "stable" .

gs1:organicClaimAgency
	rdf:type          owl:FunctionalProperty , owl:ObjectProperty , rdf:Property ;
	rdfs:comment      "A governing body that creates and maintains standards related to organic products."@en ;
	rdfs:domain       gs1:OrganicClaimDetails ;
	rdfs:isDefinedBy  gs1: ;
	rdfs:label        "Organic Claim Agency Code"@en ;
	rdfs:range        gs1:OrganicClaimAgencyCode ;
	sw:term_status    "stable" .

gs1:organicPercentClaim
	rdf:type          rdf:Property , owl:DatatypeProperty ;
	rdfs:comment      "The percent of actual organic materials per weight of the product. This is usually claimed on the product."@en ;
	rdfs:domain       gs1:OrganicClaimDetails ;
	rdfs:isDefinedBy  gs1: ;
	rdfs:label        "Organic Percent Claim"@en ;
	rdfs:range        xsd:float ;
	sw:term_status    "stable" .

gs1:organizationHistory
	rdf:type          owl:ObjectProperty , rdf:Property ;
	rdfs:comment      "Provides details on if and when an organisation/party is active or inactive."@en ;
	rdfs:domain       gs1:Organization ;
	rdfs:isDefinedBy  gs1: ;
	rdfs:label        "Has Organization History"@en ;
	rdfs:range        gs1:OrganizationStatusHistory ;
	sw:term_status    "stable" .

gs1:organizationID
	rdf:type  owl:DatatypeProperty , rdf:Property ;
	rdfs:comment      "Identifier value associated to an organisation/party. This value SHALL follow rules set forth by the administrating organisation designated in gs1:OrganizationID_Type."@en ;
	rdfs:domain       gs1:OrganizationID_Details ;
	rdfs:isDefinedBy  gs1: ;
	rdfs:label        "Organisation ID"@en ;
	rdfs:range        xsd:string ;
	sw:term_status    "stable" .

gs1:organizationID_Qualifier
	rdf:type          owl:DatatypeProperty , rdf:Property ;
	rdfs:comment      "Secondary qualifier to supplement gs1:organizationID_Type meaning. May be used with proprietary ID code values to define identifier administrator."@en ;
	rdfs:domain       gs1:OrganizationID_Details ;
	rdfs:isDefinedBy  gs1: ;
	rdfs:label        "Organisation ID Qualifier"@en ;
	rdfs:range        xsd:string ;
	sw:term_status    "stable" .

gs1:organizationID_Type
	rdf:type          owl:ObjectProperty , rdf:Property ;
	rdfs:comment      "Organisation that administers the gs1:organizationID or the name of the ID itself.  Value from gs1:OrganizationID_Type code list."@en ;
	rdfs:domain       gs1:OrganizationID_Details ;
	rdfs:isDefinedBy  gs1: ;
	rdfs:label        "Organisation ID"@en ;
	rdfs:range        gs1:OrganizationID_Type ;
	sw:term_status    "stable" .

gs1:organizationID_URI
	rdf:type          owl:ObjectProperty , rdf:Property ;
	rdfs:comment      "A URI that links to information about the gs1:organizationID."@en ;
	rdfs:domain       gs1:OrganizationID_Details ;
	rdfs:isDefinedBy  gs1: ;
	rdfs:label        "Organisation ID URI"@en ;
	rdfs:range        xsd:anyURI ;
	sw:term_status    "stable" .

gs1:organizationName
	rdf:type  owl:DatatypeProperty , rdf:Property ;
	rdfs:comment        "The name of the organization expressed in text."@en ;
	rdfs:domain         [ rdf:type     owl:Class ;
	owl:unionOf  ( gs1:PostalAddress gs1:Organization )
	] ;
	rdfs:isDefinedBy    gs1: ;
	rdfs:label          "Organization Name"@en ;
	rdfs:range          rdf:langString ;
	rdfs:subPropertyOf  schema:name ;
	sw:term_status      "stable" ;
	skos:related        schema:Organization , schema:PostalAddress .

gs1:organizationRole
	rdf:type  owl:ObjectProperty , rdf:Property ;
	rdfs:comment      "The role and/or purpose of a party (i.e. legal entity or function).  Multiple values from gs1:OrganizationRoleType code list may be associated to a single organisation/party."@en ;
	rdfs:domain       gs1:Organization ;
	rdfs:isDefinedBy  gs1: ;
	rdfs:label        "Has Organization Role"@en ;
	rdfs:range        gs1:OrganizationRoleType ;
	sw:term_status    "stable" .

gs1:organizationStatus
	rdf:type          owl:ObjectProperty , rdf:Property ;
	rdfs:comment      "Designation of active/inactive status of an organisation/party."@en ;
	rdfs:domain       gs1:OrganizationStatusHistory ;
	rdfs:isDefinedBy  gs1: ;
	rdfs:label        "Organisation Status"@en ;
	rdfs:range        gs1:StatusType ;
	sw:term_status    "stable" .

gs1:originalCodeValue
	rdf:type          owl:DatatypeProperty , rdf:Property ;
	rdfs:comment      "Links to the alphanumeric code value defined elsewhere in GS1 or the GS1 Global Data Dictionary"@en ;
	rdfs:domain       gs1:TypeCode ;
	rdfs:isDefinedBy  gs1: ;
	rdfs:label        "Original Code Value"@en ;
	rdfs:range        xsd:string ;
	sw:term_status    "stable" .

gs1:outOfPackageDepth
	rdf:type          rdf:Property , owl:ObjectProperty ;
	rdfs:comment      "The depth of the product out of its packaging, as measured according to the GS1 Package Measurement Rules. See https://www.gs1.org/package-measurement-rules-implementation-guide for more details."@en ;
	rdfs:domain       gs1:Product ;
	rdfs:isDefinedBy  gs1: ;
	rdfs:label        "Out of Package Depth"@en ;
	rdfs:range        gs1:QuantitativeValue ;
	sw:term_status    "stable" ;
	skos:broadMatch   schema:depth .

gs1:outOfPackageDiameter
	rdf:type          owl:ObjectProperty , rdf:Property ;
	rdfs:comment      "The measurement of the diameter of the product out of its package at its largest point. For example, 165 MMT."@en ;
	rdfs:domain       gs1:Product ;
	rdfs:isDefinedBy  gs1: ;
	rdfs:label        "Out of Package Diameter"@en ;
	rdfs:range        gs1:QuantitativeValue ;
	sw:term_status    "stable" .

gs1:outOfPackageHeight
	rdf:type          owl:ObjectProperty , rdf:Property ;
	rdfs:comment      "The height of the product out of the package, as measured according to the GS1 Package Measurement Rules. See https://www.gs1.org/package-measurement-rules-implementation-guide for more details."@en ;
	rdfs:domain       gs1:Product ;
	rdfs:isDefinedBy  gs1: ;
	rdfs:label        "Out of Package Height"@en ;
	rdfs:range        gs1:QuantitativeValue ;
	sw:term_status    "stable" ;
	skos:broadMatch   schema:height .

gs1:outOfPackageWidth
	rdf:type          owl:ObjectProperty , rdf:Property ;
	rdfs:comment      "The width of the product out of the package, as measured according to the GS1 Package Measurement Rules. See https://www.gs1.org/package-measurement-rules-implementation-guide for more details."@en ;
	rdfs:domain       gs1:Product ;
	rdfs:isDefinedBy  gs1: ;
	rdfs:label        "Out of Package Width"@en ;
	rdfs:range        gs1:QuantitativeValue ;
	sw:term_status    "stable" ;
	skos:broadMatch   schema:width .

gs1:ownedBy
	rdf:type     rdf:Property , owl:ObjectProperty ;
	rdfs:comment      "Links to the organisation(s) that own this place, in full or in part. This includes joint ventures. For leased locations, see gs1:lessorFor and gs1:isLeasedFrom."@en ;
	rdfs:domain       _:b0 ;
	rdfs:isDefinedBy  gs1: ;
	rdfs:label        "Owned by"@en ;
	rdfs:range        gs1:Organization ;
	sw:term_status    "stable" .

gs1:owns
	rdf:type        rdf:Property , owl:ObjectProperty ;
	rdfs:comment      "Links to the place(s) or organisation(s) that this organisation owns."@en ;
	rdfs:domain       gs1:Organization ;
	rdfs:isDefinedBy  gs1: ;
	rdfs:label        "Owns"@en ;
	rdfs:range        _:b0 ;
	sw:term_status    "stable" .

gs1:packaging
	rdf:type   rdf:Property , owl:ObjectProperty ;
	rdfs:comment      "Details on the packaging for a product including type, weight and materials."@en ;
	rdfs:domain       gs1:Product ;
	rdfs:isDefinedBy  gs1: ;
	rdfs:label        "Has Packaging"@en ;
	rdfs:range        gs1:PackagingDetails ;
	sw:term_status    "stable" .

gs1:packagingDate
	rdf:type  rdf:Property , owl:ObjectProperty ;
	rdfs:comment      "The packaging date is the date when the goods were packed as determined by the packager. The date may refer to the trade item itself or to items contained."@en ;
	rdfs:domain       schema:Product , gs1:Product ;
	rdfs:isDefinedBy  gs1: ;
	rdfs:label        "Packaging Date"@en ;
	rdfs:range        xsd:date ;
	sw:term_status    "stable" ;
	skos:altLabel     "Packaging Date"@en ;
	skos:notation     "13"^^gs1:AI ;
	skos:prefLabel    "13" .

gs1:packagingFeature
	rdf:type  rdf:Property , owl:ObjectProperty ;
	rdfs:comment      "Code indicating a feature that facilitates the usage of the product by the consumer, for example a handle. Packaging features do not affect the core composition of the packaging type nor modify its usage."@en ;
	rdfs:domain       gs1:PackagingDetails ;
	rdfs:isDefinedBy  gs1: ;
	rdfs:label        "Packaging Feature"@en ;
	rdfs:range        gs1:PackagingFeatureCode ;
	sw:term_status    "stable" .

gs1:packagingFunction
	rdf:type          owl:ObjectProperty , rdf:Property ;
	rdfs:comment      "Code indicating specific functionality for packaging resulting from specific processes or features present in the packaging type,for example, ANTI_TAMPERING."@en ;
	rdfs:domain       gs1:PackagingDetails ;
	rdfs:isDefinedBy  gs1: ;
	rdfs:label        "Packaging Function"@en ;
	rdfs:range        gs1:PackagingFunctionCode ;
	sw:term_status    "stable" .

gs1:packagingMarkedDietAllergenType
	rdf:type          rdf:Property , owl:ObjectProperty ;
	rdfs:comment      "Indication of which dietary or allergen marks are on the package."@en ;
	rdfs:domain       gs1:FoodBeverageTobaccoProduct ;
	rdfs:isDefinedBy  gs1: ;
	rdfs:label        "Packaging Marked Diet Allergen Type Code"@en ;
	rdfs:range        gs1:PackagingMarkedDietAllergenCode ;
	sw:term_status    "stable" .

gs1:packagingMarkedFreeFrom
	rdf:type          owl:ObjectProperty , rdf:Property ;
	rdfs:comment      "Indication of the food ingredients that the package is marked free from."@en ;
	rdfs:domain       gs1:FoodBeverageTobaccoProduct ;
	rdfs:isDefinedBy  gs1: ;
	rdfs:label        "Packaging Marked Free From Code"@en ;
	rdfs:range        gs1:PackagingMarkedFreeFromCode ;
	sw:term_status    "stable" .

gs1:packagingMarkedLabelAccreditation
	rdf:type          owl:ObjectProperty , rdf:Property ;
	rdfs:comment      "A marking that the product received recognition, endorsement, certification by following guidelines by the label issuing agency. This does not represent claims for regulatory purposes on products such as free from markings."@en ;
	rdfs:domain       gs1:Product ;
	rdfs:isDefinedBy  gs1: ;
	rdfs:label        "Accreditation Code"@en ;
	rdfs:range        gs1:PackagingMarkedLabelAccreditationCode ;
	sw:term_status    "stable" .

gs1:packagingMaterial
	rdf:type          rdf:Property , owl:ObjectProperty ;
	rdfs:comment      "links to details about packaging material type, quantity and thickness"@en ;
	rdfs:domain       gs1:PackagingDetails ;
	rdfs:isDefinedBy  gs1: ;
	rdfs:label        "Has Packaging Material Details"@en ;
	rdfs:range        gs1:PackagingMaterialDetails ;
	sw:term_status    "stable" .

gs1:packagingMaterialCompositionQuantity
	rdf:type          rdf:Property , owl:ObjectProperty ;
	rdfs:comment      "The quantity of the packaging material of the product. Can be weight, volume or surface, can vary by country."@en ;
	rdfs:domain       gs1:PackagingMaterialDetails ;
	rdfs:isDefinedBy  gs1: ;
	rdfs:label        "Packaging Material Composition Quantity"@en ;
	rdfs:range        gs1:QuantitativeValue ;
	sw:term_status    "stable" .

gs1:packagingMaterialThickness
	rdf:type          owl:ObjectProperty , rdf:Property ;
	rdfs:comment      "The thickness of a packaging material."@en ;
	rdfs:domain       gs1:PackagingMaterialDetails ;
	rdfs:isDefinedBy  gs1: ;
	rdfs:label        "Packaging Material Thickness"@en ;
	rdfs:range        gs1:QuantitativeValue ;
	sw:term_status    "stable" .

gs1:packagingMaterialType
	rdf:type          rdf:Property , owl:ObjectProperty ;
	rdfs:comment      "The materials used for the packaging of the product for example glass or plastic."@en ;
	rdfs:domain       gs1:PackagingMaterialDetails ;
	rdfs:isDefinedBy  gs1: ;
	rdfs:label        "Packaging Material Type"@en ;
	rdfs:range        gs1:PackagingMaterialTypeCode ;
	sw:term_status    "stable" .

gs1:packagingRecyclingProcessType
	rdf:type          owl:ObjectProperty , rdf:Property ;
	rdfs:comment      "The process the packaging could undertake for recyclable & sustainability programs. Examples COMPOSTABLE, ENERGY_RECOVERABLE, REUSABLE."@en ;
	rdfs:domain       gs1:PackagingDetails ;
	rdfs:isDefinedBy  gs1: ;
	rdfs:label        "Packaging Recycling Process Type"@en ;
	rdfs:range        gs1:PackagingRecyclingProcessTypeCode ;
	sw:term_status    "stable" .

gs1:packagingRecyclingScheme
	rdf:type          rdf:Property , owl:ObjectProperty ;
	rdfs:comment      "A code indicating the recycling scheme the packaging of this product will fall within when recycled. Applies to recyclable packaging with or without deposit."@en ;
	rdfs:domain       gs1:PackagingDetails ;
	rdfs:isDefinedBy  gs1: ;
	rdfs:label        "Packaging Recycling Scheme"@en ;
	rdfs:range        gs1:PackagingRecyclingSchemeCode ;
	sw:term_status    "stable" .

gs1:packagingShape
	rdf:type  owl:ObjectProperty , rdf:Property ;
	rdfs:comment      "A code depicting the shape of a package for example CONE."@en ;
	rdfs:domain       gs1:PackagingDetails ;
	rdfs:isDefinedBy  gs1: ;
	rdfs:label        "Packaging Shape"@en ;
	rdfs:range        gs1:PackagingShapeCode ;
	sw:term_status    "stable" .

gs1:packagingType
	rdf:type  rdf:Property , owl:DatatypeProperty ;
	rdfs:comment      "The dominant means used to transport, store, handle or display the product as defined by the data source. This packaging is not used to describe any manufacturing process.Recommend to use UNECE Rec 21 codes."@en ;
	rdfs:domain       gs1:PackagingDetails ;
	rdfs:isDefinedBy  gs1: ;
	rdfs:label        "Packaging Type"@en ;
	rdfs:range        xsd:string ;
	sw:term_status    "stable" .

gs1:pantothenicAcidPerNutrientBasis
	rdf:type          owl:ObjectProperty , rdf:Property ;
	rdfs:comment      "Pantothenic Acid per specified nutrient basis quantity."@en ;
	rdfs:domain       gs1:FoodBeverageTobaccoProduct ;
	rdfs:isDefinedBy  gs1: ;
	rdfs:label        "Pantothenic Acid Per Nutrient Basis Quantity"@en ;
	rdfs:range        gs1:NutritionMeasurementType ;
	sw:term_status    "stable" .

gs1:parentOrganization
	rdf:type          owl:ObjectProperty , rdf:Property ;
	rdfs:comment      "Designates the legal entity or function directly above the organisation/party being identified in a hierarchy. This is not defaulted to the highest-level entity in the hierarchy. Only one parent organisation SHALL be associated to a single GLN. To specify other affiliated organisations, see gs1:affiliatedTo, gs1:managedBy, gs1:franchiseeOf, gs1:ownedBy. To specify an organisation/party lower in the hierarchy, see gs1:subOrganization."@en ;
	rdfs:domain       gs1:Organization ;
	rdfs:isDefinedBy  gs1: ;
	rdfs:label        "Parent Organization"@en ;
	rdfs:range        gs1:Organization ;
	sw:term_status    "stable" .

gs1:partyGLN
	rdf:type    owl:DatatypeProperty , rdf:Property ;
	rdfs:comment      "13-digit GLN that is being used to identify a legal entity or function. If gs1:glnType is present, gs1:partyGLN SHALL only be used when gs1:GLN_TypeCode includes LEGAL_ENTITY and/or FUNCTION"@en ;
	rdfs:domain       gs1:Organization ;
	rdfs:isDefinedBy  gs1: ;
	rdfs:label        "Party GLN"@en ;
	rdfs:range        xsd:string ;
	sw:term_status    "stable" .

gs1:paymentLink
	rdf:type   owl:ObjectProperty , rdf:Property ;
	rdfs:comment        "A link to a place where payments details are provided and/or payments can be made by the user."@en ;
	rdfs:domain         owl:Thing ;
	rdfs:label          "Make Payment"@en ;
	rdfs:range          xsd:anyURI ;
	rdfs:subPropertyOf  gs1:linkType ;
	sw:term_status      "stable" .

gs1:paymentTerms
	rdf:type  rdf:Property , owl:DatatypeProperty ;
	rdfs:comment      "The type of payment term expressed as a code, for example Discount."@en ;
	rdfs:domain       gs1:Offer ;
	rdfs:isDefinedBy  gs1: ;
	rdfs:label        "Payment Terms"@en ;
	rdfs:range        xsd:string ;
	sw:term_status    "stable" .

gs1:percentageOfAlcoholByVolume
	rdf:type          rdf:Property , owl:DatatypeProperty ;
	rdfs:comment      "The percentage of alcohol contained in product."@en ;
	rdfs:domain       gs1:Beverage ;
	rdfs:isDefinedBy  gs1: ;
	rdfs:label        "Percentage of Alcohol Per Volume"@en ;
	rdfs:range        xsd:float ;
	sw:term_status    "stable" .

gs1:phosphorusPerNutrientBasis
	rdf:type          owl:ObjectProperty , rdf:Property ;
	rdfs:comment      "Phosphorus per specified nutrient basis quantity."@en ;
	rdfs:domain       gs1:FoodBeverageTobaccoProduct ;
	rdfs:isDefinedBy  gs1: ;
	rdfs:label        "Phosphorus Per Nutrient Basis Quantity"@en ;
	rdfs:range        gs1:NutritionMeasurementType ;
	sw:term_status    "stable" .

gs1:physicalLocationName
	rdf:type          owl:DatatypeProperty , rdf:Property ;
	rdfs:comment      "The name of a physical place. To specify the name of a digital location, see gs1:digitalLocationName."@en ;
	rdfs:domain       gs1:Place ;
	rdfs:isDefinedBy  gs1: ;
	rdfs:label        "Physical Location Name"@en ;
	rdfs:range        rdf:langString ;
	sw:term_status    "stable" .

gs1:pip
	rdf:type           owl:ObjectProperty , rdf:Property ;
	rdfs:comment        "A link to information specifically about the identified item, typically operated by the brand owner or a retailer of the product and aimed at consumers. It may include links to further information, product description, specifications etc."@en ;
	rdfs:domain         owl:Thing ;
	rdfs:label          "Product Information Page"@en ;
	rdfs:range          xsd:anyURI ;
	rdfs:subPropertyOf  gs1:linkType ;
	sw:term_status      "stable" .

gs1:polygon
	rdf:type     rdf:Property , owl:DatatypeProperty ;
	rdfs:comment      "A polygon is the area enclosed by a point-to-point path for which the starting and ending points are the same. A polygon is expressed as a series of four or more space delimited points where the first and final points are identical."@en ;
	rdfs:domain       gs1:GeoShape ;
	rdfs:isDefinedBy  gs1: ;
	rdfs:label        "Polygon"@en ;
	rdfs:range        xsd:string ;
	sw:term_status    "stable" ;
	skos:exactMatch   schema:polygon .

gs1:polyolsPerNutrientBasis
	rdf:type          owl:ObjectProperty , rdf:Property ;
	rdfs:comment      "Polyols per specified nutrient basis quantity."@en ;
	rdfs:domain       gs1:FoodBeverageTobaccoProduct ;
	rdfs:isDefinedBy  gs1: ;
	rdfs:label        "Polyols Per Nutrient Basis Quantity"@en ;
	rdfs:range        gs1:NutritionMeasurementType ;
	sw:term_status    "stable" .

gs1:polyunsaturatedFatPerNutrientBasis
	rdf:type          owl:ObjectProperty , rdf:Property ;
	rdfs:comment      "Polyunsaturated fat per specified nutrient basis quantity."@en ;
	rdfs:domain       gs1:FoodBeverageTobaccoProduct ;
	rdfs:isDefinedBy  gs1: ;
	rdfs:label        "Polyunsaturated Fat Per Nutrient Basis Quantity"@en ;
	rdfs:range        gs1:NutritionMeasurementType ;
	sw:term_status    "stable" .

gs1:postOfficeBoxNumber
	rdf:type          rdf:Property , owl:DatatypeProperty ;
	rdfs:comment      "The number that identifies a PO box. A PO box is a box in a post office or other postal service location assigned to an organization where postal items may be kept."@en ;
	rdfs:domain       gs1:PostalAddress ;
	rdfs:isDefinedBy  gs1: ;
	rdfs:label        "PO Box Number"@en ;
	rdfs:range        xsd:string ;
	sw:term_status    "stable" ;
	skos:exactMatch   schema:postOfficeBoxNumber .

gs1:postalCode
	rdf:type  owl:DatatypeProperty , rdf:Property ;
	rdfs:comment      "Text specifying the postal code for an address."@en ;
	rdfs:domain       gs1:PostalAddress ;
	rdfs:isDefinedBy  gs1: ;
	rdfs:label        "Postal Code"@en ;
	rdfs:range        xsd:string ;
	sw:term_status    "stable" ;
	skos:exactMatch   vcard:postal-code , schema:postalCode .

gs1:postalName
	rdf:type  rdf:Property , owl:DatatypeProperty ;
	rdfs:comment      "The name of the recipient expressed in text. Note that this may be different than gs1:OrganizationName."@en ;
	rdfs:domain       gs1:PostalAddress ;
	rdfs:isDefinedBy  gs1: ;
	rdfs:label        "Postal Name"@en ;
	rdfs:range        rdf:langString ;
	sw:term_status    "stable" .

gs1:potassiumPerNutrientBasis
	rdf:type          rdf:Property , owl:ObjectProperty ;
	rdfs:comment      "Potassium per specified nutrient basis quantity."@en ;
	rdfs:domain       gs1:FoodBeverageTobaccoProduct ;
	rdfs:isDefinedBy  gs1: ;
	rdfs:label        "Potassium Per Nutrient Basis Quantity"@en ;
	rdfs:range        gs1:NutritionMeasurementType ;
	sw:term_status    "stable" .

gs1:preparationCode
	rdf:type  rdf:Property , owl:ObjectProperty ;
	rdfs:comment      "Code specifying the preparation state of the product for which the nutrient information is valid. PREPARED, UNPREPARED."@en ;
	rdfs:domain       gs1:FoodAndBeveragePreparationInformation ;
	rdfs:isDefinedBy  gs1: ;
	rdfs:label        "Preparation Type Code"@en ;
	rdfs:range        gs1:PreparationTypeCode ;
	sw:term_status    "stable" .

gs1:preparationConsumptionPrecautions
	rdf:type          owl:DatatypeProperty , rdf:Property ;
	rdfs:comment      "Specifies additional precautions to be taken before preparation or consumption of the product."@en ;
	rdfs:domain       gs1:FoodAndBeveragePreparationInformation ;
	rdfs:isDefinedBy  gs1: ;
	rdfs:label        "Preparation Consumption Precautions"@en ;
	rdfs:range        rdf:langString ;
	sw:term_status    "stable" .

gs1:preparationInformation
	rdf:type          rdf:Property , owl:ObjectProperty ;
	rdfs:comment      "Links to information about how to prepare a specific Food/Beverage/Tobacco product."@en ;
	rdfs:domain       gs1:FoodBeverageTobaccoProduct ;
	rdfs:isDefinedBy  gs1: ;
	rdfs:label        "Has Food And Beverage Preparation Information"@en ;
	rdfs:range        gs1:FoodAndBeveragePreparationInformation ;
	sw:term_status    "stable" .

gs1:preparationInstructions
	rdf:type          rdf:Property , owl:DatatypeProperty ;
	rdfs:comment      "Free text providing instructions on how to prepare the product before serving."@en ;
	rdfs:domain       gs1:FoodAndBeveragePreparationInformation ;
	rdfs:isDefinedBy  gs1: ;
	rdfs:label        "Preparation Instructions"@en ;
	rdfs:range        rdf:langString ;
	sw:term_status    "stable" .

gs1:preservationTechnique
	rdf:type          owl:ObjectProperty , rdf:Property ;
	rdfs:comment      "Code indicating the preservation technique used to preserve the product from deterioration, for example, BRINING."@en ;
	rdfs:domain       gs1:FoodBeverageTobaccoProduct ;
	rdfs:isDefinedBy  gs1: ;
	rdfs:label        "Preservation Technique"@en ;
	rdfs:range        gs1:PreservationTechniqueCode ;
	sw:term_status    "stable" .

gs1:price
	rdf:type       rdf:Property , owl:DatatypeProperty ;
	rdfs:comment      "Provides a price value as a floating-point numeric value that is qualified by the corresponding currency. See also gs1:priceCurrency. The price value indicates the unit price unless the property gs1:eligibleQuantity is specified and indicates multiple units"@en ;
	rdfs:domain       gs1:PriceSpecification ;
	rdfs:isDefinedBy  gs1: ;
	rdfs:label        "Price Value"@en ;
	rdfs:range        xsd:float ;
	rdfs:seeAlso      gs1:priceCurrency ;
	sw:term_status    "stable" ;
	skos:exactMatch   schema:price .

gs1:priceCurrency
	rdf:type  owl:DatatypeProperty , rdf:Property ;
	rdfs:comment      "A string value indicating a currency from ISO 4217 for example USD ."@en ;
	rdfs:domain       gs1:PriceSpecification ;
	rdfs:isDefinedBy  gs1: ;
	rdfs:label        "Price Currency"@en ;
	rdfs:range        xsd:string ;
	sw:term_status    "stable" ;
	skos:exactMatch   schema:priceCurrency .

gs1:priceSpecification
	rdf:type          owl:ObjectProperty , rdf:Property ;
	rdfs:comment      "The price related to an offer. If the offer is a multi-buy offer for a quantity of product greater than one unit, this should be indicated using the property gs1:eligibleQuantity"@en ;
	rdfs:domain       gs1:Offer ;
	rdfs:isDefinedBy  gs1: ;
	rdfs:label        "Price Specification"@en ;
	rdfs:range        gs1:PriceSpecification ;
	sw:term_status    "stable" ;
	skos:exactMatch   schema:priceSpecification .

gs1:primaryAlternateProduct
	rdf:type            rdf:Property , owl:ObjectProperty ;
	rdfs:comment        "A product that is similar to the current product but is not exact match. Same form fit function, e.g. same product different colour, different package size, better quality."@en ;
	rdfs:domain         gs1:Product ;
	rdfs:isDefinedBy    gs1: ;
	rdfs:label          "Has Primary Alternate Product"@en ;
	rdfs:range          gs1:Product ;
	rdfs:subPropertyOf  schema:isSimilarTo ;
	sw:term_status      "stable" .

gs1:primaryLocationOf
	rdf:type          rdf:Property , owl:ObjectProperty ;
	rdfs:comment      "Links to the organisation(s) that designate this place as its/their primary location. Property SHOULD be applied to a specific sub-location, rather than a main location, wherever possible."@en ;
	rdfs:domain       gs1:Place ;
	rdfs:isDefinedBy  gs1: ;
	rdfs:label        "Primary location of"@en ;
	rdfs:range        gs1:Organization ;
	sw:term_status    "stable" .

gs1:productDescription
	rdf:type            rdf:Property , owl:DatatypeProperty ;
	rdfs:comment        "An understandable and useable description of a product using brand and other descriptors. This attribute is filled with as little abbreviation as possible, while keeping to a reasonable length.  This should be a meaningful description of the product with full spelling to facilitate message processing. Retailers can use this description as the base to fully understand the brand, flavour, scent etc. of the specific product, in order to accurately create a product description as needed for their internal systems. Examples: XYZ Brand Base Invisible Solid Deodorant AP Stick Spring Breeze."@en ;
	rdfs:domain         gs1:Product ;
	rdfs:isDefinedBy    gs1: ;
	rdfs:label          "Product Description"@en ;
	rdfs:range          rdf:langString ;
	rdfs:subPropertyOf  schema:description ;
	sw:term_status      "stable" ;
	skos:related        schema:Product .

gs1:productFeatureBenefit
	rdf:type          rdf:Property , owl:DatatypeProperty ;
	rdfs:comment      "Element for consumer facing marketing content to describe the key features or benefits of the style suitable for display purposes."@en ;
	rdfs:domain       gs1:Product ;
	rdfs:isDefinedBy  gs1: ;
	rdfs:label        "Product Feature Benefit"@en ;
	rdfs:range        rdf:langString ;
	sw:term_status    "stable" .

gs1:productFormDescription
	rdf:type          rdf:Property , owl:DatatypeProperty ;
	rdfs:comment      "The physical form or shape of the product. Used, for example, in pharmaceutical industry to indicate the formulation of the product. Defines the form the product takes and is distinct from the form of the packaging."@en ;
	rdfs:domain       gs1:Product ;
	rdfs:isDefinedBy  gs1: ;
	rdfs:label        "Product Form Description"@en ;
	rdfs:range        rdf:langString ;
	sw:term_status    "stable" .

gs1:productID
	rdf:type   owl:FunctionalProperty , owl:DatatypeProperty , rdf:Property ;
	rdfs:comment      "Additional means to the Global Trade Item Number to identify a product."@en ;
	rdfs:domain       gs1:Product ;
	rdfs:isDefinedBy  gs1: ;
	rdfs:label        "Product ID"@en ;
	rdfs:range        xsd:string ;
	sw:term_status    "stable" ;
	skos:exactMatch   schema:productID .

gs1:productMarketingMessage
	rdf:type          owl:DatatypeProperty , rdf:Property ;
	rdfs:comment      "Marketing message associated with the product. Consumer-friendly marketing detailed description of the product."@en ;
	rdfs:domain       gs1:Product ;
	rdfs:isDefinedBy  gs1: ;
	rdfs:label        "Product Marketing Message"@en ;
	rdfs:range        rdf:langString ;
	sw:term_status    "stable" .

gs1:productName
	rdf:type   owl:DatatypeProperty , rdf:Property ;
	rdfs:comment        "Consumer friendly short description of the product suitable for compact presentation."@en ;
	rdfs:domain         gs1:Product ;
	rdfs:isDefinedBy    gs1: ;
	rdfs:label          "Product Name"@en ;
	rdfs:range          rdf:langString ;
	rdfs:subPropertyOf  schema:name ;
	sw:term_status      "stable" ;
	skos:related        schema:Product .

gs1:productRange
	rdf:type  owl:DatatypeProperty , rdf:Property ;
	rdfs:comment      "A name, used by a Brand Owner, that span multiple consumer categories or uses. E.g. (Waist Watchers)."@en ;
	rdfs:domain       gs1:Product ;
	rdfs:isDefinedBy  gs1: ;
	rdfs:label        "Product Range"@en ;
	rdfs:range        rdf:langString ;
	sw:term_status    "stable" ;
	skos:related      schema:brand .

gs1:productSustainabilityInfo
	rdf:type            owl:ObjectProperty , rdf:Property ;
	rdfs:comment        "This term has been deprecated. Please use gs1:sustainabilityInfo instead."@en ;
	rdfs:domain         gs1:Product , schema:Product ;
	rdfs:label          "Sustainability and recycling (deprecated)"@en ;
	rdfs:range          xsd:anyURI ;
	rdfs:subPropertyOf  gs1:linkType ;
	sw:term_status      "deprecated" .

gs1:productYield
	rdf:type  rdf:Property , owl:ObjectProperty ;
	rdfs:comment      "Product quantity after preparation. This can differ based on productYieldType"@en ;
	rdfs:domain       gs1:ProductYieldDetails ;
	rdfs:isDefinedBy  gs1: ;
	rdfs:label        "Product Yield"@en ;
	rdfs:range        gs1:QuantitativeValue ;
	sw:term_status    "stable" .

gs1:productYieldType
	rdf:type  rdf:Property , owl:ObjectProperty ;
	rdfs:comment      "Code indicating the type of yield measurement specified in productYield. Examples: AFTER_DILUTION, DRAINED_WEIGHT."@en ;
	rdfs:domain       gs1:ProductYieldDetails ;
	rdfs:isDefinedBy  gs1: ;
	rdfs:label        "Product Yield Type Code"@en ;
	rdfs:range        gs1:ProductYieldTypeCode ;
	sw:term_status    "stable" .

gs1:productYieldVariationPercentage
	rdf:type          rdf:Property , owl:DatatypeProperty ;
	rdfs:comment      "Indication of range in percent of the given cooking / roasting loss. Percentage that the actual weight of the product differs upward or downward from the average or estimated product yield."@en ;
	rdfs:domain       gs1:ProductYieldDetails ;
	rdfs:isDefinedBy  gs1: ;
	rdfs:label        "Product Yield Variation Percentage"@en ;
	rdfs:range        xsd:float ;
	sw:term_status    "stable" .

gs1:productionDate
	rdf:type  owl:ObjectProperty , rdf:Property ;
	rdfs:comment      "The production date is the production or assembly date determined by the manufacturer. The date may refer to the trade item itself or to items contained."@en ;
	rdfs:domain       gs1:Product , schema:Product ;
	rdfs:isDefinedBy  gs1: ;
	rdfs:label        "Production Date"@en ;
	rdfs:range        xsd:date ;
	sw:term_status    "stable" ;
	skos:altLabel     "Production Date"@en ;
	skos:notation     "11"^^gs1:AI ;
	skos:prefLabel    "11" .

gs1:productionDateTime
	rdf:type          owl:ObjectProperty , rdf:Property ;
	rdfs:comment      "The date and time of production (or assembly). The date and time of production is determined by the manufacturer. The date and time may refer to the trade item itself or to the items contained."@en ;
	rdfs:domain       schema:Product , gs1:Product ;
	rdfs:isDefinedBy  gs1: ;
	rdfs:label        "Production Date and Time"@en ;
	rdfs:range        xsd:date ;
	sw:term_status    "stable" ;
	skos:altLabel     "Production Date and Time"@en ;
	skos:notation     "8008"^^gs1:AI ;
	skos:prefLabel    "8008" .

gs1:productionVariantDescription
	rdf:type          rdf:Property , owl:DatatypeProperty ;
	rdfs:comment      "Free text assigned by the manufacturer to describe the production variant. Examples are: package series X, package series Y."@en ;
	rdfs:domain       gs1:Product ;
	rdfs:isDefinedBy  gs1: ;
	rdfs:label        "Production Variant Description"@en ;
	rdfs:range        rdf:langString ;
	sw:term_status    "stable" .

gs1:productionVariantEffectiveDateTime
	rdf:type          owl:DatatypeProperty , rdf:Property ;
	rdfs:comment      "The start date of a production variant. The variant applies to products having a date mark (a best before date or expiration date) on the package that comes on or after the effective date."@en ;
	rdfs:domain       gs1:Product ;
	rdfs:isDefinedBy  gs1: ;
	rdfs:label        "Production Variant Effective Date Time"@en ;
	rdfs:range        xsd:dateTime ;
	sw:term_status    "stable" .

gs1:promotion
	rdf:type     owl:ObjectProperty , rdf:Property ;
	rdfs:comment        "A link to a promotion."@en ;
	rdfs:domain         owl:Thing ;
	rdfs:label          "Promotion"@en ;
	rdfs:range          xsd:anyURI ;
	rdfs:subPropertyOf  gs1:linkType ;
	sw:term_status      "stable" .

gs1:proteinPerNutrientBasis
	rdf:type          rdf:Property , owl:ObjectProperty ;
	rdfs:comment      "Protein per specified nutrient basis quantity."@en ;
	rdfs:domain       gs1:FoodBeverageTobaccoProduct ;
	rdfs:isDefinedBy  gs1: ;
	rdfs:label        "Protein Per Nutrient Basis Quantity"@en ;
	rdfs:range        gs1:NutritionMeasurementType ;
	sw:term_status    "stable" .

gs1:provenanceStatement
	rdf:type          rdf:Property , owl:DatatypeProperty ;
	rdfs:comment      "Free text description of the region or place the product originates from. This is to be specifically used to specify areas such as cities, mountain ranges, regions. Examples: Made in the Thuringen Mountains, Made in Paris, From the Napa Valley."@en ;
	rdfs:domain       gs1:Product ;
	rdfs:isDefinedBy  gs1: ;
	rdfs:label        "Provenance Statement"@en ;
	rdfs:range        rdf:langString ;
	sw:term_status    "stable" .

gs1:purchaseSuppliesOrAccessories
	rdf:type            owl:ObjectProperty , rdf:Property ;
	rdfs:comment        "A link to information about where supplies or accessories for the item can be purchased or ordered."@en ;
	rdfs:domain         owl:Thing ;
	rdfs:label          "Purchase supplies or accessories"@en ;
	rdfs:range          xsd:anyURI ;
	rdfs:subPropertyOf  gs1:linkType ;
	sw:term_status      "stable" .

gs1:qualifyingBrandName
	rdf:type          owl:DatatypeProperty , rdf:Property ;
	rdfs:comment      "If specified, the discount is only available when purchasing a product from one of the brand names specified via this property."@en ;
	rdfs:domain       gs1:Discount ;
	rdfs:isDefinedBy  gs1: ;
	rdfs:label        "Qualifying Brand Name"@en ;
	rdfs:range        rdf:langString ;
	sw:term_status    "unstable" .

gs1:qualifyingGPCs
	rdf:type  rdf:Property , owl:DatatypeProperty ;
	rdfs:comment      "If specified, the discount is only available when purchasing a product whose Global Product Classification (GPC) brick value appears in the list specified via this property."@en ;
	rdfs:domain       gs1:Discount ;
	rdfs:isDefinedBy  gs1: ;
	rdfs:label        "Qualifying Product GPC codes"@en ;
	rdfs:range        xsd:string ;
	sw:term_status    "unstable" .

gs1:qualifyingProductCategoryDescription
	rdf:type          rdf:Property , owl:DatatypeProperty ;
	rdfs:comment      "If specified, the discount is only available when purchasing a product from categories specified in this free-form text field."@en ;
	rdfs:domain       gs1:Discount ;
	rdfs:isDefinedBy  gs1: ;
	rdfs:label        "Qualifying Product Category Description"@en ;
	rdfs:range        rdf:langString ;
	sw:term_status    "unstable" .

gs1:qualifyingProductClassificationCode
	rdf:type          owl:DatatypeProperty , rdf:Property , owl:FunctionalProperty ;
	rdfs:comment      "If specified, the discount is only available when purchasing a product whose product classification (other than GPC) appears in the list specified via this property. This property specifies a product classification other than GPC."@en ;
	rdfs:domain       gs1:Discount ;
	rdfs:isDefinedBy  gs1: ;
	rdfs:label        "Qualifying Product Classification Code"@en ;
	rdfs:range        gs1:AdditionalProductClassificationDetails ;
	sw:term_status    "unstable" .

gs1:qualifyingProductGTINs
	rdf:type          owl:DatatypeProperty , rdf:Property ;
	rdfs:comment      "If specified, the discount is only available when purchasing a product whose GTIN appears in the list specified via this property."@en ;
	rdfs:domain       gs1:Discount ;
	rdfs:isDefinedBy  gs1: ;
	rdfs:label        "Qualifying Product GTINs"@en ;
	rdfs:range        xsd:string ;
	sw:term_status    "unstable" .

gs1:qualifyingSubBrandName
	rdf:type          owl:DatatypeProperty , rdf:Property ;
	rdfs:comment      "If specified, the discount is only available when purchasing a product from one of the sub-brand names (specified product ranges for a given brand) specified via this property."@en ;
	rdfs:domain       gs1:Discount ;
	rdfs:isDefinedBy  gs1: ;
	rdfs:label        "Qualifying Sub-brand Name"@en ;
	rdfs:range        rdf:langString ;
	sw:term_status    "unstable" .

gs1:quickStartGuide
	rdf:type  owl:ObjectProperty , rdf:Property ;
	rdfs:comment        "A link to a description of the key features needed to be understood to begin using the item or interacting with something new."@en ;
	rdfs:domain         owl:Thing ;
	rdfs:label          "Quick start guide"@en ;
	rdfs:range          xsd:anyURI ;
	rdfs:subPropertyOf  gs1:linkType ;
	sw:term_status      "stable" .

gs1:recallStatus
	rdf:type  owl:ObjectProperty , rdf:Property ;
	rdfs:comment        "A link to information about whether the product has been recalled or not, typically an API."@en ;
	rdfs:domain         owl:Thing ;
	rdfs:label          "Recall status"@en ;
	rdfs:range          xsd:anyURI ;
	rdfs:subPropertyOf  gs1:linkType ;
	sw:term_status      "stable" .

gs1:recipeInfo
	rdf:type    owl:ObjectProperty , rdf:Property ;
	rdfs:comment        "A link to a recipe website."@en ;
	rdfs:domain         owl:Thing ;
	rdfs:label          "Recipe website"@en ;
	rdfs:range          xsd:anyURI ;
	rdfs:subPropertyOf  gs1:linkType ;
	sw:term_status      "stable" .

gs1:referencedFile
	rdf:type  owl:ObjectProperty , rdf:Property ;
	rdfs:comment      "Link to a file or website containing additional information on product."@en ;
	rdfs:domain       gs1:Product ;
	rdfs:isDefinedBy  gs1: ;
	rdfs:label        "Has Referenced File"@en ;
	rdfs:range        gs1:ReferencedFileDetails ;
	sw:term_status    "stable" .

gs1:referencedFileEffectiveEndDateTime
	rdf:type            owl:DatatypeProperty , rdf:Property ;
	rdfs:comment        "The date upon which the target of this external link ceases to be effective for use."@en ;
	rdfs:domain         gs1:ReferencedFileDetails ;
	rdfs:isDefinedBy    gs1: ;
	rdfs:label          "Referenced File Effective End Date"@en ;
	rdfs:range          xsd:dateTime ;
	rdfs:subPropertyOf  schema:expires ;
	sw:term_status      "stable" .

gs1:referencedFileEffectiveStartDateTime
	rdf:type          owl:DatatypeProperty , rdf:Property ;
	rdfs:comment      "The date upon which the target of this external link begins to be effective for use."@en ;
	rdfs:domain       gs1:ReferencedFileDetails ;
	rdfs:isDefinedBy  gs1: ;
	rdfs:label        "Referenced File Effective Start Date"@en ;
	rdfs:range        xsd:dateTime ;
	rdfs:seeAlso      schema:datePublished ;
	sw:term_status    "stable" .

gs1:referencedFileSize
	rdf:type            owl:ObjectProperty , rdf:Property ;
	rdfs:comment        "The size of the file as it is stored in an uncompressed format."@en ;
	rdfs:domain         gs1:ReferencedFileDetails ;
	rdfs:isDefinedBy    gs1: ;
	rdfs:label          "Referenced File Size"@en ;
	rdfs:range          gs1:QuantitativeValue ;
	rdfs:subPropertyOf  schema:contentSize ;
	sw:term_status      "stable" .

gs1:referencedFileType
	rdf:type          owl:ObjectProperty , rdf:Property ;
	rdfs:comment      "A code indicating the purpose or role of file (not a MIME type) that is being referenced, for example PRODUCT_LABEL_IMAGE. This code is used when the purpose of a file is not specified in the property."@en ;
	rdfs:domain       gs1:ReferencedFileDetails ;
	rdfs:isDefinedBy  gs1: ;
	rdfs:label        "Referenced File Type"@en ;
	rdfs:range        gs1:ReferencedFileTypeCode ;
	rdfs:seeAlso      schema:description ;
	sw:term_status    "stable" .

gs1:referencedFileURL
	rdf:type            rdf:Property , owl:DatatypeProperty ;
	rdfs:comment        "Simple text string that refers to a resource on the internet, URLs may refer to documents, resources, people, etc."@en ;
	rdfs:domain         gs1:ReferencedFileDetails ;
	rdfs:isDefinedBy    gs1: ;
	rdfs:label          "Website"@en ;
	rdfs:range          xsd:anyURI ;
	rdfs:subPropertyOf  schema:url ;
	sw:term_status      "stable" .

gs1:registerProduct
	rdf:type  owl:ObjectProperty , rdf:Property ;
	rdfs:comment        "A link to an entry point for registering ownership of a product including for warranty purposes."@en ;
	rdfs:domain         owl:Thing ;
	rdfs:label          "Register purchase"@en ;
	rdfs:range          xsd:anyURI ;
	rdfs:subPropertyOf  gs1:linkType ;
	sw:term_status      "stable" .

gs1:registryEntry
	rdf:type  owl:ObjectProperty , rdf:Property ;
	rdfs:comment        "A link to an entry in a register, such as a business register or register of locations. Such registers may act as alternative identifiers, such as official company numbers, LEIs, other location identifiers etc."@en ;
	rdfs:domain         owl:Thing ;
	rdfs:label          "Entry in a register"@en ;
	rdfs:range          xsd:anyURI ;
	rdfs:subPropertyOf  gs1:linkType ;
	sw:term_status      "stable" .

gs1:regulatedProductName
	rdf:type          owl:DatatypeProperty , rdf:Property ;
	rdfs:comment      "The prescribed, regulated or generic product name or denomination that describes the true nature of the product. For example for a food product in order to distinguish it from other foods according to country specific regulations."@en ;
	rdfs:domain       gs1:Product ;
	rdfs:isDefinedBy  gs1: ;
	rdfs:label        "Regulated Product Name"@en ;
	rdfs:range        rdf:langString ;
	sw:term_status    "stable" ;
	skos:broadMatch   schema:name ;
	skos:related      schema:Product .

gs1:reheatingClaim
	rdf:type  rdf:Property , owl:ObjectProperty ;
	rdfs:comment      "Indicates, with reference to the product branding, labelling or packaging whether a food product which is ready to eat can be reheated if required prior to consumption."@en ;
	rdfs:domain       gs1:FoodBeverageTobaccoProduct ;
	rdfs:isDefinedBy  gs1: ;
	rdfs:label        "Reheating Claim"@en ;
	rdfs:range        gs1:NonbinaryLogicCode ;
	sw:term_status    "stable" .

gs1:relatedImage
	rdf:type  owl:ObjectProperty , rdf:Property ;
	rdfs:comment        "A link to any image that depicts or relates to the identified entity (e.g., trade item, assets, business process, patient record, location, organisation, etc.)"@en ;
	rdfs:domain         owl:Thing ;
	rdfs:label          "Related image"@en ;
	rdfs:range          xsd:anyURI ;
	rdfs:subPropertyOf  gs1:linkType ;
	sw:term_status      "stable" .

gs1:relatedOrganization
	rdf:type          rdf:Property , owl:ObjectProperty ;
	rdfs:comment      "The organisation(s) associated with a place."@en ;
	rdfs:domain       gs1:Place ;
	rdfs:isDefinedBy  gs1: ;
	rdfs:label        "Has Organisation"@en ;
	rdfs:range        gs1:Organization ;
	sw:term_status    "stable" .

gs1:relatedVideo
	rdf:type  owl:ObjectProperty , rdf:Property ;
	rdfs:comment        "A link to any video, or document that has an embedded video, that describes or relates to the identified item, organisation, or location in some way."@en ;
	rdfs:domain         owl:Thing ;
	rdfs:label          "Related  video"@en ;
	rdfs:range          xsd:anyURI ;
	rdfs:subPropertyOf  gs1:linkType ;
	sw:term_status      "stable" .

gs1:replacedByOrganization
	rdf:type          owl:ObjectProperty , rdf:Property ;
	rdfs:comment      "Links to the successor organisation that is used in place of a previous organisation"@en ;
	rdfs:domain       gs1:Organization ;
	rdfs:isDefinedBy  gs1: ;
	rdfs:label        "Replaced by organization"@en ;
	rdfs:range        gs1:Organization ;
	sw:term_status    "stable" .

gs1:replacedByPlace
	rdf:type  owl:ObjectProperty , rdf:Property ;
	rdfs:comment      "Links to the successor location that is used in place of a previous location"@en ;
	rdfs:domain       gs1:Place ;
	rdfs:isDefinedBy  gs1: ;
	rdfs:label        "Replaced by Place"@en ;
	rdfs:range        gs1:Place ;
	sw:term_status    "stable" .

gs1:replacedByProduct
	rdf:type            owl:ObjectProperty , rdf:Property ;
	rdfs:comment        "The product which permanently replaces the current product. This product is sent in the record for the original item that is being replaced."@en ;
	rdfs:domain         gs1:Product ;
	rdfs:isDefinedBy    gs1: ;
	rdfs:label          "Has Replaced By Product"@en ;
	rdfs:range          gs1:Product ;
	rdfs:subPropertyOf  schema:isSimilarTo ;
	sw:term_status      "stable" .

gs1:replacedOrganization
	rdf:type          owl:ObjectProperty , rdf:Property ;
	rdfs:comment      "Links to the previous organisation that this organisation replaces"@en ;
	rdfs:domain       gs1:Organization ;
	rdfs:isDefinedBy  gs1: ;
	rdfs:label        "Replaced organization"@en ;
	rdfs:range        gs1:Organization ;
	sw:term_status    "stable" .

gs1:replacedPlace
	rdf:type  owl:ObjectProperty , rdf:Property ;
	rdfs:comment      "Links to the previous location that this location replaces"@en ;
	rdfs:domain       gs1:Place ;
	rdfs:isDefinedBy  gs1: ;
	rdfs:label        "Replaced Place"@en ;
	rdfs:range        gs1:Place ;
	sw:term_status    "stable" .

gs1:replacedProduct
	rdf:type  owl:ObjectProperty , rdf:Property ;
	rdfs:comment        "Indicates the product identification of an item that is being permanently replaced by this product."@en ;
	rdfs:domain         gs1:Product ;
	rdfs:isDefinedBy    gs1: ;
	rdfs:label          "Has Replaced Product"@en ;
	rdfs:range          gs1:Product ;
	rdfs:subPropertyOf  schema:isSimilarTo ;
	sw:term_status      "stable" .

gs1:responsibility
	rdf:type  rdf:Property , owl:DatatypeProperty ;
	rdfs:comment      "Text further specifying the area of responsibility of the trade contact."@en ;
	rdfs:domain       gs1:ContactPoint ;
	rdfs:isDefinedBy  gs1: ;
	rdfs:label        "Responsibility"@en ;
	rdfs:range        rdf:langString ;
	sw:term_status    "stable" .

gs1:responsibleForLocation
	rdf:type          rdf:Property , owl:ObjectProperty ;
	rdfs:comment      "Links to the place(s) for which this organisation is responsible."@en ;
	rdfs:domain       gs1:Organization ;
	rdfs:isDefinedBy  gs1: ;
	rdfs:label        "Responsible for location"@en ;
	rdfs:range        gs1:Place ;
	sw:term_status    "stable" .

gs1:responsibleOrganization
	rdf:type          rdf:Property , owl:ObjectProperty ;
	rdfs:comment      "Links to the organisation that is directly responsible for this place."@en ;
	rdfs:domain       gs1:Place ;
	rdfs:isDefinedBy  gs1: ;
	rdfs:label        "Organisation responsible for the location"@en ;
	rdfs:range        gs1:Organization ;
	sw:term_status    "stable" .

gs1:returnablePackageDepositAmount
	rdf:type          owl:ObjectProperty , rdf:Property ;
	rdfs:comment      "The monetary amount for the individual returnable package."@en ;
	rdfs:domain       gs1:ReturnablePackageDepositDetails ;
	rdfs:isDefinedBy  gs1: ;
	rdfs:label        "Returnable Package Deposit Amount"@en ;
	rdfs:range        gs1:PriceSpecification ;
	sw:term_status    "stable" .

gs1:returnablePackageDepositRegion
	rdf:type          rdf:Property , owl:ObjectProperty ;
	rdfs:comment      "The geographic region associated with the returnable package deposit amount."@en ;
	rdfs:domain       gs1:ReturnablePackageDepositDetails ;
	rdfs:isDefinedBy  gs1: ;
	rdfs:label        "Returnable Package Deposit Region"@en ;
	rdfs:range        gs1:Country ;
	sw:term_status    "stable" .

gs1:review
	rdf:type        owl:ObjectProperty , rdf:Property ;
	rdfs:comment        "A link to reviews."@en ;
	rdfs:domain         owl:Thing ;
	rdfs:label          "Reviews"@en ;
	rdfs:range          xsd:anyURI ;
	rdfs:subPropertyOf  gs1:linkType ;
	sw:term_status      "stable" .

gs1:riboflavinPerNutrientBasis
	rdf:type          rdf:Property , owl:ObjectProperty ;
	rdfs:comment      "Riboflavin per specified nutrient basis quantity."@en ;
	rdfs:domain       gs1:FoodBeverageTobaccoProduct ;
	rdfs:isDefinedBy  gs1: ;
	rdfs:label        "Riboflavin Per Nutrient Basis Quantity"@en ;
	rdfs:range        gs1:NutritionMeasurementType ;
	sw:term_status    "stable" .

gs1:safetyInfo
	rdf:type    owl:ObjectProperty , rdf:Property ;
	rdfs:comment        "A link to safety information."@en ;
	rdfs:domain         owl:Thing ;
	rdfs:label          "Safety information"@en ;
	rdfs:range          xsd:anyURI ;
	rdfs:subPropertyOf  gs1:linkType ;
	sw:term_status      "stable" .

gs1:saltPerNutrientBasis
	rdf:type          rdf:Property , owl:ObjectProperty ;
	rdfs:comment      "Salt per specified nutrient basis quantity."@en ;
	rdfs:domain       gs1:FoodBeverageTobaccoProduct ;
	rdfs:isDefinedBy  gs1: ;
	rdfs:label        "Salt Per Nutrient Basis Quantity"@en ;
	rdfs:range        gs1:NutritionMeasurementType ;
	sw:term_status    "stable" .

gs1:saturatedFatPerNutrientBasis
	rdf:type          owl:ObjectProperty , rdf:Property ;
	rdfs:comment      "Saturated fat per specified nutrient basis quantity."@en ;
	rdfs:domain       gs1:FoodBeverageTobaccoProduct ;
	rdfs:isDefinedBy  gs1: ;
	rdfs:label        "Saturated Fat Per Nutrient Basis Quantity"@en ;
	rdfs:range        gs1:NutritionMeasurementType ;
	sw:term_status    "stable" .

gs1:scheduleTime
	rdf:type  owl:ObjectProperty , rdf:Property ;
	rdfs:comment        "A link to a site that offers information on scheduling, appointments, or reservations. This may or may not allow the user to book the reservation."@en ;
	rdfs:domain         owl:Thing ;
	rdfs:label          "Scheduling/Reservation"@en ;
	rdfs:range          xsd:anyURI ;
	rdfs:subPropertyOf  gs1:linkType ;
	sw:term_status      "stable" .

gs1:seasonCalendarYear
	rdf:type          owl:DatatypeProperty , rdf:Property ;
	rdfs:comment      "The calendar year in which the product is seasonally available."@en ;
	rdfs:domain       gs1:WearableProduct ;
	rdfs:isDefinedBy  gs1: ;
	rdfs:label        "Season Calendar Year"@en ;
	rdfs:range        xsd:gYear ;
	sw:term_status    "stable" .

gs1:seasonName
	rdf:type  owl:DatatypeProperty , rdf:Property ;
	rdfs:comment      "Element defines the season applicable to the item for example Winter."@en ;
	rdfs:domain       gs1:WearableProduct ;
	rdfs:isDefinedBy  gs1: ;
	rdfs:label        "Season Name"@en ;
	rdfs:range        rdf:langString ;
	sw:term_status    "stable" .

gs1:seasonParameter
	rdf:type  rdf:Property , owl:ObjectProperty ;
	rdfs:comment      "Code indicating the season in which the product is available, e.g. SPRING, WINTER"@en ;
	rdfs:domain       gs1:WearableProduct ;
	rdfs:isDefinedBy  gs1: ;
	rdfs:label        "Season Parameter"@en ;
	rdfs:range        gs1:SeasonParameterCode ;
	sw:term_status    "stable" .

gs1:seeker
	rdf:type      rdf:Property , owl:ObjectProperty ;
	rdfs:comment      "The organization seeking an offer."@en ;
	rdfs:domain       gs1:Offer ;
	rdfs:isDefinedBy  gs1: ;
	rdfs:label        "Seeker"@en ;
	rdfs:range        gs1:Organization ;
	sw:term_status    "stable" .

gs1:selectedProductsOnly
	rdf:type          owl:DatatypeProperty , rdf:Property ;
	rdfs:comment      "If specified and set to true, the discount only applies to specific products selected by the retailer or offer promoter - not to all items in that product category.  This property should be asserted and set to true for offers that say 'on selected products'."@en ;
	rdfs:domain       gs1:Discount ;
	rdfs:isDefinedBy  gs1: ;
	rdfs:label        "Selected Products Only"@en ;
	rdfs:range        xsd:boolean ;
	sw:term_status    "unstable" .

gs1:seleniumPerNutrientBasis
	rdf:type          owl:ObjectProperty , rdf:Property ;
	rdfs:comment      "Selenium per specified nutrient basis quantity."@en ;
	rdfs:domain       gs1:FoodBeverageTobaccoProduct ;
	rdfs:isDefinedBy  gs1: ;
	rdfs:label        "Selenium Per Nutrient Basis Quantity"@en ;
	rdfs:range        gs1:NutritionMeasurementType ;
	sw:term_status    "stable" .

gs1:sellByDate
	rdf:type  owl:ObjectProperty , rdf:Property ;
	rdfs:comment      "The date specified by the manufacturer as the last date the retailer is to offer the product for sale to the consumer. The product should not be merchandised after this date."@en ;
	rdfs:domain       schema:Product , gs1:Product ;
	rdfs:isDefinedBy  gs1: ;
	rdfs:label        "Sell By Date"@en ;
	rdfs:range        xsd:date ;
	sw:term_status    "stable" ;
	skos:altLabel     "Sell By Date"@en ;
	skos:notation     "16"^^gs1:AI ;
	skos:prefLabel    "16" .

gs1:seller
	rdf:type      rdf:Property , owl:ObjectProperty ;
	rdfs:comment      "The organization seeking to sell a product or service."@en ;
	rdfs:domain       gs1:Offer ;
	rdfs:isDefinedBy  gs1: ;
	rdfs:label        "Seller"@en ;
	rdfs:range        gs1:Organization ;
	sw:term_status    "stable" ;
	skos:exactMatch   schema:seller .

gs1:serviceInfo
	rdf:type   owl:ObjectProperty , rdf:Property ;
	rdfs:comment        "A link to service or maintenance instructions."@en ;
	rdfs:domain         owl:Thing ;
	rdfs:label          "Service information"@en ;
	rdfs:range          xsd:anyURI ;
	rdfs:subPropertyOf  gs1:linkType ;
	sw:term_status      "stable" .

gs1:servingSize
	rdf:type  owl:ObjectProperty , rdf:Property ;
	rdfs:comment      "Measurement value specifying the serving size in which the information per nutrient has been stated. Example: Per 100 GRM."@en ;
	rdfs:domain       gs1:FoodBeverageTobaccoProduct ;
	rdfs:isDefinedBy  gs1: ;
	rdfs:label        "Serving Size"@en ;
	rdfs:range        gs1:QuantitativeValue ;
	sw:term_status    "stable" .

gs1:servingSizeDescription
	rdf:type          rdf:Property , owl:DatatypeProperty ;
	rdfs:comment      "A free text field specifying the serving size for which the nutrient information has been stated for example: per 1/3 cup (42 g)."@en ;
	rdfs:domain       gs1:FoodBeverageTobaccoProduct ;
	rdfs:isDefinedBy  gs1: ;
	rdfs:label        "Serving Size Description"@en ;
	rdfs:range        rdf:langString ;
	sw:term_status    "stable" .

gs1:servingSuggestion
	rdf:type          rdf:Property , owl:DatatypeProperty ;
	rdfs:comment      "Free text field for serving suggestion."@en ;
	rdfs:domain       gs1:FoodBeverageTobaccoProduct ;
	rdfs:isDefinedBy  gs1: ;
	rdfs:label        "Serving Suggestion"@en ;
	rdfs:range        rdf:langString ;
	sw:term_status    "stable" .

gs1:sharpnessOfCheese
	rdf:type          rdf:Property , owl:ObjectProperty ;
	rdfs:comment      "The descriptive term that is used by the product manufacturer to identify the sharpness of the taste of the product for example EXTRA_SHARP. Usually the longer the aging of the product, the sharper the taste."@en ;
	rdfs:domain       gs1:MilkButterCreamYogurtCheeseEggsSubstitutes ;
	rdfs:isDefinedBy  gs1: ;
	rdfs:label        "Sharpness Of Cheese"@en ;
	rdfs:range        gs1:SharpnessOfCheeseCode ;
	sw:term_status    "stable" .

gs1:size
	rdf:type        owl:ObjectProperty , rdf:Property ;
	rdfs:comment      "Links a wearable product to one or more groupings of gs1:SizeDetails representing size systems, size groups, size type and size dimensions."@en ;
	rdfs:domain       gs1:WearableProduct ;
	rdfs:isDefinedBy  gs1: ;
	rdfs:label        "Size"@en ;
	rdfs:range        gs1:SizeDetails ;
	sw:term_status    "stable" .

gs1:sizeCode
	rdf:type    owl:ObjectProperty , rdf:Property ;
	rdfs:comment      "Links a product to one or more groupings of gs1:SizeCodeDetails representing the size value from a specified code list."@en ;
	rdfs:domain       gs1:Product ;
	rdfs:isDefinedBy  gs1: ;
	rdfs:label        "Size Code"@en ;
	rdfs:range        gs1:SizeCodeDetails ;
	sw:term_status    "stable" .

gs1:sizeCodeListCode
	rdf:type  owl:DatatypeProperty , rdf:Property ;
	rdfs:comment      "Code specifying a size code list. Allowed code values are specified in GS1 Code List SizeCodeListCode ."@en ;
	rdfs:domain       gs1:SizeCodeDetails ;
	rdfs:isDefinedBy  gs1: ;
	rdfs:label        "Size Code List Code"@en ;
	rdfs:range        xsd:string ;
	sw:term_status    "stable" .

gs1:sizeCodeValue
	rdf:type  owl:DatatypeProperty , rdf:Property ;
	rdfs:comment      "A code indicating the size of an object according to a specific code list. The applied code list is specified as additional information together with the size code."@en ;
	rdfs:domain       gs1:SizeCodeDetails ;
	rdfs:isDefinedBy  gs1: ;
	rdfs:label        "Size Code"@en ;
	rdfs:range        xsd:string ;
	sw:term_status    "stable" .

gs1:sizeDimension
	rdf:type  rdf:Property , owl:ObjectProperty ;
	rdfs:comment      "The numerical size measurement relating to the size type."@en ;
	rdfs:domain       gs1:SizeDetails ;
	rdfs:isDefinedBy  gs1: ;
	rdfs:label        "Size Dimension"@en ;
	rdfs:range        gs1:QuantitativeValue ;
	sw:term_status    "stable" .

gs1:sizeGroup
	rdf:type   owl:ObjectProperty , rdf:Property ;
	rdfs:comment      "Code indicating the type of size that is necessary to uniquely specify the size of the item, for example, BOYS."@en ;
	rdfs:domain       gs1:SizeDetails ;
	rdfs:isDefinedBy  gs1: ;
	rdfs:label        "Size Group"@en ;
	rdfs:range        gs1:SizeGroupCode ;
	sw:term_status    "stable" .

gs1:sizeSystem
	rdf:type  owl:ObjectProperty , rdf:Property ;
	rdfs:comment      "The system that is being used to define the size for example EUROPE. Size system is used in conjunction with size group to define the size dimension."@en ;
	rdfs:domain       gs1:SizeDetails ;
	rdfs:isDefinedBy  gs1: ;
	rdfs:label        "Size System"@en ;
	rdfs:range        gs1:SizeSystemCode ;
	sw:term_status    "stable" .

gs1:sizeType
	rdf:type    rdf:Property , owl:ObjectProperty ;
	rdfs:comment      "The type of size dimension being specified for example SLEEVE."@en ;
	rdfs:domain       gs1:SizeDetails ;
	rdfs:isDefinedBy  gs1: ;
	rdfs:label        "Size Type"@en ;
	rdfs:range        gs1:SizeTypeCode ;
	sw:term_status    "stable" .

gs1:smartLabel
	rdf:type    owl:ObjectProperty , rdf:Property ;
	rdfs:comment        "A link to the product's SmartLabel page."@en ;
	rdfs:domain         owl:Thing ;
	rdfs:label          "SmartLabel"@en ;
	rdfs:range          xsd:anyURI ;
	rdfs:subPropertyOf  gs1:linkType ;
	sw:term_status      "stable" .

gs1:smpc
	rdf:type          owl:ObjectProperty , rdf:Property ;
	rdfs:comment        "A link to Summary Product Characteristics. To be used specifically when linking to information for healthcare professionals."@en ;
	rdfs:domain         owl:Thing ;
	rdfs:label          "Summary Product Characteristics (SmPC)"@en ;
	rdfs:range          xsd:anyURI ;
	rdfs:subPropertyOf  gs1:linkType ;
	sw:term_status      "stable" .

gs1:socialMedia
	rdf:type   owl:ObjectProperty , rdf:Property ;
	rdfs:comment        "A link to a social media channel. The title will typically be replaced by the name of the channel."@en ;
	rdfs:domain         owl:Thing ;
	rdfs:label          "Social media"@en ;
	rdfs:range          xsd:anyURI ;
	rdfs:subPropertyOf  gs1:linkType ;
	sw:term_status      "stable" .

gs1:sodiumPerNutrientBasis
	rdf:type          rdf:Property , owl:ObjectProperty ;
	rdfs:comment      "Sodium per specified nutrient basis quantity."@en ;
	rdfs:domain       gs1:FoodBeverageTobaccoProduct ;
	rdfs:isDefinedBy  gs1: ;
	rdfs:label        "Sodium Per Nutrient Basis Quantity"@en ;
	rdfs:range        gs1:NutritionMeasurementType ;
	sw:term_status    "stable" .

gs1:sourceAnimal
	rdf:type  owl:ObjectProperty , rdf:Property ;
	rdfs:comment      "Code indicating the source of raw material used to produce the food product, for example a GOAT for milk."@en ;
	rdfs:domain       gs1:FoodBeverageTobaccoProduct ;
	rdfs:isDefinedBy  gs1: ;
	rdfs:label        "Source Animal Code"@en ;
	rdfs:range        gs1:SourceAnimalCode ;
	sw:term_status    "stable" .

gs1:sportingActivityType
	rdf:type          owl:ObjectProperty , rdf:Property ;
	rdfs:comment      "Code indicating the type of sporting activity for which the product is intended to be worn, for example FOOTBALL."@en ;
	rdfs:domain       gs1:WearableProduct ;
	rdfs:isDefinedBy  gs1: ;
	rdfs:label        "Sporting Activity Type"@en ;
	rdfs:range        gs1:SportingActivityTypeCode ;
	sw:term_status    "stable" .

gs1:starchPerNutrientBasis
	rdf:type          owl:ObjectProperty , rdf:Property ;
	rdfs:comment      "Starch per specified nutrient basis quantity."@en ;
	rdfs:domain       gs1:FoodBeverageTobaccoProduct ;
	rdfs:isDefinedBy  gs1: ;
	rdfs:label        "Starch Per Nutrient Basis Quantity"@en ;
	rdfs:range        gs1:NutritionMeasurementType ;
	sw:term_status    "stable" .

gs1:statisticInfo
	rdf:type  owl:ObjectProperty , rdf:Property ;
	rdfs:comment        "A link to information about statistics regarding an organisation, location, or other entity."@en ;
	rdfs:domain         owl:Thing ;
	rdfs:label          "Statistics"@en ;
	rdfs:range          xsd:anyURI ;
	rdfs:subPropertyOf  gs1:linkType ;
	sw:term_status      "stable" .

gs1:statusTimestamp
	rdf:type  owl:DatatypeProperty , rdf:Property ;
	rdfs:comment      "Date and time (including optional timezone) associated to status designations. Timestamps may be future dated to provide advance notice of status changes. For further information about the required lexical representation of date, time, and timezone please see https://www.w3.org/TR/xmlschema-2/#dateTime"@en ;
	rdfs:domain       [ rdf:type     owl:Class ;
	owl:unionOf  ( gs1:OrganizationStatusHistory gs1:LocationStatusHistory )
	] ;
	rdfs:isDefinedBy  gs1: ;
	rdfs:label        "Status Timestamp"@en ;
	rdfs:range        xsd:dateTime ;
	sw:term_status    "stable" .

gs1:streetAddress
	rdf:type  owl:DatatypeProperty , rdf:Property ;
	rdfs:comment      "The street address expressed as free form text. The street address is printed on paper as the first lines below the name. For example, the name of the street and the number in the street or the name of a building. A total of four street address lines are available. gs1:streetAddress SHOULD be used before populating lines two through four. For a PO Box gs1:postOfficeBoxNumber SHOULD be used instead."@en ;
	rdfs:domain       gs1:PostalAddress ;
	rdfs:isDefinedBy  gs1: ;
	rdfs:label        "Street Address"@en ;
	rdfs:range        rdf:langString ;
	sw:term_status    "stable" ;
	skos:exactMatch   schema:streetAddress , vcard:street-address .

gs1:streetAddressLine2
	rdf:type          owl:DatatypeProperty , rdf:Property ;
	rdfs:comment      "The second line of the street address, expressed as free form text. The street address is printed on paper as the first lines below the name. For example, the name of the street and the number in the street or the name of a building. A total of four street address lines are available. gs1:streetAddress SHOULD be used before populating lines two through four. These SHALL NOT be used as alternatives to the dedicated address properties gs1:addressSuburb, gs1:addressLocality and gs1:addressRegion."@en ;
	rdfs:domain       gs1:PostalAddress ;
	rdfs:isDefinedBy  gs1: ;
	rdfs:label        "Street Address Line 2"@en ;
	rdfs:range        rdf:langString ;
	sw:term_status    "stable" .

gs1:streetAddressLine3
	rdf:type          owl:DatatypeProperty , rdf:Property ;
	rdfs:comment      "The third line of the street address, expressed as free form text. The street address is printed on paper as the first lines below the name. For example, the name of the street and the number in the street or the name of a building. A total of four street address lines are available. gs1:streetAddress and gs1:streetaddressLine2 SHOULD be used before populating lines three and four. These SHALL NOT be used as alternatives to the dedicated address properties gs1:addressSuburb, gs1:addressLocality and gs1:addressRegion."@en ;
	rdfs:domain       gs1:PostalAddress ;
	rdfs:isDefinedBy  gs1: ;
	rdfs:label        "Street Address Line 3"@en ;
	rdfs:range        rdf:langString ;
	sw:term_status    "stable" .

gs1:streetAddressLine4
	rdf:type          owl:DatatypeProperty , rdf:Property ;
	rdfs:comment      "The fourth line of the street address, expressed as free form text. The street address is printed on paper as the first lines below the name. For example, the name of the street and the number in the street or the name of a building. gs1:streetAddress, gs1:streetaddressLine2 and gs1:streetaddressLine3 SHOULD be used before populating line four. These SHALL NOT be used as alternatives to the dedicated address properties gs1:addressSuburb, gs1:addressLocality and gs1:addressRegion."@en ;
	rdfs:domain       gs1:PostalAddress ;
	rdfs:isDefinedBy  gs1: ;
	rdfs:label        "Street Address Line 4"@en ;
	rdfs:range        rdf:langString ;
	sw:term_status    "stable" .

gs1:styleDescription
	rdf:type  owl:DatatypeProperty , rdf:Property ;
	rdfs:comment      "An attribute that classifies products that share many of the same characteristics (attribute values) that does NOT vary by GTIN, and are presented by the supplier as a single merchandise selection for the buyer."@en ;
	rdfs:domain       gs1:WearableProduct ;
	rdfs:isDefinedBy  gs1: ;
	rdfs:label        "Style Description"@en ;
	rdfs:range        rdf:langString ;
	sw:term_status    "stable" .

gs1:subBrandName
	rdf:type  owl:DatatypeProperty , rdf:Property ;
	rdfs:comment        "Second level of brand. Can be a trademark. It is the primary differentiating factor that a brand owner wants to communicate to the consumer or buyer. E.g. Yummy-Cola Classic. In this example Yummy-Cola is the brand and Classic is the sub-brand."@en ;
	rdfs:domain         gs1:Brand ;
	rdfs:isDefinedBy    gs1: ;
	rdfs:label          "Sub-brand Name"@en ;
	rdfs:range          rdf:langString ;
	rdfs:subPropertyOf  schema:name ;
	sw:term_status      "stable" ;
	skos:related        schema:Brand .

gs1:subOrganization
	rdf:type  owl:ObjectProperty , rdf:Property ;
	rdfs:comment      "Designates a legal entity or function directly below the organisation/party being identified in a hierarchy. There may be multiple sub-organisations associated to a single GLN. To specify other affiliated organisations, see gs1:manages, gs1:franchisorOf, gs1:owns. To specify a parent organisation, see gs1:parentOrganization."@en ;
	rdfs:domain       gs1:Organization ;
	rdfs:isDefinedBy  gs1: ;
	rdfs:label        "Sub-Organization"@en ;
	rdfs:range        gs1:Organization ;
	sw:term_status    "stable" .

gs1:subscribe
	rdf:type     owl:ObjectProperty , rdf:Property ;
	rdfs:comment        "A link to a subscription form"@en ;
	rdfs:domain         owl:Thing ;
	rdfs:label          "Subscribe"@en ;
	rdfs:range          xsd:anyURI ;
	rdfs:subPropertyOf  gs1:linkType ;
	sw:term_status      "stable" .

gs1:sugarsPerNutrientBasis
	rdf:type          rdf:Property , owl:ObjectProperty ;
	rdfs:comment      "Sugars per specified nutrient basis quantity."@en ;
	rdfs:domain       gs1:FoodBeverageTobaccoProduct ;
	rdfs:isDefinedBy  gs1: ;
	rdfs:label        "Sugars Per Nutrient Basis Quantity"@en ;
	rdfs:range        gs1:NutritionMeasurementType ;
	sw:term_status    "stable" .

gs1:supplierSpecifiedMinimumConsumerStorageDays
	rdf:type          owl:DatatypeProperty , rdf:Property ;
	rdfs:comment      "Represents the number of days between a product's sell by date and its use by date."@en ;
	rdfs:domain       gs1:Product ;
	rdfs:isDefinedBy  gs1: ;
	rdfs:label        "Supplier Specified Minimum Consumer Storage Days"@en ;
	rdfs:range        xsd:integer ;
	sw:term_status    "stable" .

gs1:support
	rdf:type       owl:ObjectProperty , rdf:Property ;
	rdfs:comment        "A link to a source of support such as a helpdesk, chat support, email etc."@en ;
	rdfs:domain         owl:Thing ;
	rdfs:label          "Support"@en ;
	rdfs:range          xsd:anyURI ;
	rdfs:subPropertyOf  gs1:linkType ;
	sw:term_status      "stable" .

gs1:sustainabilityInfo
	rdf:type            owl:ObjectProperty , rdf:Property ;
	rdfs:comment        "A link to information relating to sustainability and recycling requirements or processes."@en ;
	rdfs:domain         owl:Thing ;
	rdfs:label          "Sustainability and recycling"@en ;
	rdfs:range          xsd:anyURI ;
	rdfs:subPropertyOf  gs1:linkType ;
	sw:term_status      "stable" .

gs1:targetConsumerAge
	rdf:type          rdf:Property , owl:DatatypeProperty ;
	rdfs:comment      "Identifies the target consumer age range for which a product has been designed."@en ;
	rdfs:domain       gs1:WearableProduct ;
	rdfs:isDefinedBy  gs1: ;
	rdfs:label        "Target Consumer Age"@en ;
	rdfs:range        xsd:string ;
	sw:term_status    "stable" .

gs1:targetConsumerGender
	rdf:type          rdf:Property , owl:ObjectProperty ;
	rdfs:comment      "Identifies the target consumer gender for which a product has been designed for example MALE"@en ;
	rdfs:domain       gs1:WearableProduct ;
	rdfs:isDefinedBy  gs1: ;
	rdfs:label        "Target Consumer Gender"@en ;
	rdfs:range        gs1:TargetConsumerGenderCode ;
	sw:term_status    "stable" .

gs1:targetMarket
	rdf:type  rdf:Property , owl:ObjectProperty ;
	rdfs:comment      "Relates to a set of target market details (product release date and associated countries)"@en ;
	rdfs:domain       gs1:Product ;
	rdfs:isDefinedBy  gs1: ;
	rdfs:label        "Has Target Market"@en ;
	rdfs:range        gs1:TargetMarketDetails ;
	sw:term_status    "stable" .

gs1:targetMarketCountries
	rdf:type          owl:ObjectProperty , rdf:Property ;
	rdfs:comment      "List of countries representing the target market for a particular release date indicated by gs1:consumerFirstAvailabilityDateTime"@en ;
	rdfs:domain       gs1:TargetMarketDetails ;
	rdfs:isDefinedBy  gs1: ;
	rdfs:label        "Target Market Countries"@en ;
	rdfs:range        gs1:Country ;
	sw:term_status    "stable" .

gs1:telephone
	rdf:type   owl:DatatypeProperty , rdf:Property ;
	rdfs:comment      "A telephone number for example +44 217 992 9999."@en ;
	rdfs:domain       gs1:ContactPoint ;
	rdfs:isDefinedBy  gs1: ;
	rdfs:label        "Telephone"@en ;
	rdfs:range        xsd:string ;
	sw:term_status    "stable" ;
	skos:exactMatch   schema:telephone , vcard:hasTelephone .

gs1:textileMaterial
	rdf:type  rdf:Property , owl:ObjectProperty ;
	rdfs:comment      "One or more links to information about the materials used in a wearable product."@en ;
	rdfs:domain       gs1:Clothing ;
	rdfs:isDefinedBy  gs1: ;
	rdfs:label        "Has Textile Material"@en ;
	rdfs:range        gs1:TextileMaterialDetails ;
	sw:term_status    "stable" .

gs1:textileMaterialContent
	rdf:type          owl:DatatypeProperty , rdf:Property ;
	rdfs:comment      "A description of the material composition used in conjunction with the material percentage."@en ;
	rdfs:domain       gs1:WearableProduct ;
	rdfs:isDefinedBy  gs1: ;
	rdfs:label        "Textile Material Content"@en ;
	rdfs:range        rdf:langString ;
	sw:term_status    "stable" .

gs1:textileMaterialDescription
	rdf:type          rdf:Property , owl:FunctionalProperty , owl:DatatypeProperty ;
	rdfs:comment      "This provides a name or brief description of one material contained within the product, for example Rayon."@en ;
	rdfs:domain       gs1:TextileMaterialDetails ;
	rdfs:isDefinedBy  gs1: ;
	rdfs:label        "Textile Description"@en ;
	rdfs:range        rdf:langString ;
	sw:term_status    "stable" .

gs1:textileMaterialPercentage
	rdf:type          owl:DatatypeProperty , owl:FunctionalProperty , rdf:Property ;
	rdfs:comment      "Corresponding net weight percentage of the product material specified via gs1:textileMaterialDescription, e.g. 70."@en ;
	rdfs:domain       gs1:TextileMaterialDetails ;
	rdfs:isDefinedBy  gs1: ;
	rdfs:label        "Textile Material Percentage"@en ;
	rdfs:range        xsd:float ;
	sw:term_status    "stable" .

gs1:textileMaterialThreadCount
	rdf:type          owl:DatatypeProperty , owl:FunctionalProperty , rdf:Property ;
	rdfs:comment      "The quality of material (fabric) of a product based on the total number of vertical and horizontal threads in one square inch."@en ;
	rdfs:domain       gs1:TextileMaterialDetails ;
	rdfs:isDefinedBy  gs1: ;
	rdfs:label        "Textile Material Thread Count"@en ;
	rdfs:range        rdf:langString ;
	sw:term_status    "stable" .

gs1:textileMaterialWeight
	rdf:type          rdf:Property , owl:ObjectProperty , owl:FunctionalProperty ;
	rdfs:comment      "The measured weight of the material expressed in ounces per square yard or grams per square meter."@en ;
	rdfs:domain       gs1:TextileMaterialDetails ;
	rdfs:isDefinedBy  gs1: ;
	rdfs:label        "Textile Material Weight"@en ;
	rdfs:range        gs1:QuantitativeValue ;
	sw:term_status    "stable" .

gs1:thiaminPerNutrientBasis
	rdf:type          owl:ObjectProperty , rdf:Property ;
	rdfs:comment      "Thiamin per specified nutrient basis quantity."@en ;
	rdfs:domain       gs1:FoodBeverageTobaccoProduct ;
	rdfs:isDefinedBy  gs1: ;
	rdfs:label        "Thiamin Per Nutrient Basis Quantity"@en ;
	rdfs:range        gs1:NutritionMeasurementType ;
	sw:term_status    "stable" .

gs1:traceability
	rdf:type  owl:ObjectProperty , rdf:Property ;
	rdfs:comment        "A link to traceability information (includes track and trace).  Traceability information may be provided for consumption by humans or computers. If the target is an EPCIS repository, use gs1:epcis instead."@en ;
	rdfs:domain         owl:Thing ;
	rdfs:label          "Traceability information"@en ;
	rdfs:range          xsd:anyURI ;
	rdfs:subPropertyOf  gs1:linkType ;
	sw:term_status      "stable" .

gs1:transFatPerNutrientBasis
	rdf:type          owl:ObjectProperty , rdf:Property ;
	rdfs:comment      "Trans Fat per specified nutrient basis quantity."@en ;
	rdfs:domain       gs1:FoodBeverageTobaccoProduct ;
	rdfs:isDefinedBy  gs1: ;
	rdfs:label        "Trans Fat Per Nutrient Basis Quantity"@en ;
	rdfs:range        gs1:NutritionMeasurementType ;
	sw:term_status    "stable" .

gs1:tutorial
	rdf:type      owl:ObjectProperty , rdf:Property ;
	rdfs:comment        "A link to a tutorial or set of tutorials, such as online classes, how-to videos etc."@en ;
	rdfs:domain         owl:Thing ;
	rdfs:label          "Tutorial"@en ;
	rdfs:range          xsd:anyURI ;
	rdfs:subPropertyOf  gs1:linkType ;
	sw:term_status      "stable" .

gs1:unitCode
	rdf:type    owl:DatatypeProperty , rdf:Property ;
	rdfs:comment      "A string value indicating a Measurement Unit from UN/ECE Recommendation 20, Units of Measure used in International Trade e.g. GRM = gram - see http://www.unece.org/fileadmin/DAM/cefact/recommendations/rec20/rec20_rev3_Annex3e.pdf"@en ;
	rdfs:domain       gs1:QuantitativeValue ;
	rdfs:isDefinedBy  gs1: ;
	rdfs:label        "Measurement Unit"@en ;
	rdfs:range        xsd:string ;
	sw:term_status    "stable" ;
	skos:exactMatch   schema:unitCode .

gs1:upperMaterialType
	rdf:type          rdf:Property , owl:ObjectProperty ;
	rdfs:comment      "The material(s) used for the upper part of the footwear product. The upper is the part of a shoe, boot, slipper or other item of footwear that is above the sole."@en ;
	rdfs:domain       gs1:Footwear ;
	rdfs:isDefinedBy  gs1: ;
	rdfs:label        "Has Upper Material"@en ;
	rdfs:range        gs1:TextileMaterialDetails ;
	sw:term_status    "stable" .

gs1:userAgreement
	rdf:type  owl:ObjectProperty , rdf:Property ;
	rdfs:comment        "A link to an agreement or waiver."@en ;
	rdfs:domain         owl:Thing ;
	rdfs:label          "Sign waiver/agreement/document"@en ;
	rdfs:range          xsd:anyURI ;
	rdfs:subPropertyOf  gs1:linkType ;
	sw:term_status      "stable" .

gs1:usesManagedLocation
	rdf:type          rdf:Property , owl:ObjectProperty ;
	rdfs:comment      "Links to the place(s) that this organisation uses as a managed space."@en ;
	rdfs:domain       gs1:Organization ;
	rdfs:isDefinedBy  gs1: ;
	rdfs:label        "Uses managed location"@en ;
	rdfs:range        gs1:Place ;
	sw:term_status    "stable" .

gs1:validFrom
	rdf:type   owl:DatatypeProperty , rdf:Property ;
	rdfs:comment      "The effective start date of the price ."@en ;
	rdfs:domain       gs1:PriceSpecification ;
	rdfs:isDefinedBy  gs1: ;
	rdfs:label        "Valid From"@en ;
	rdfs:range        xsd:dateTime ;
	sw:term_status    "stable" ;
	skos:exactMatch   schema:validFrom .

gs1:validThrough
	rdf:type  owl:DatatypeProperty , rdf:Property ;
	rdfs:comment      "The effective end date of the price ."@en ;
	rdfs:domain       gs1:PriceSpecification ;
	rdfs:isDefinedBy  gs1: ;
	rdfs:label        "Valid Through"@en ;
	rdfs:range        xsd:dateTime ;
	sw:term_status    "stable" ;
	skos:exactMatch   schema:validThrough .

gs1:value
	rdf:type       owl:DatatypeProperty , rdf:Property ;
	rdfs:comment      "A floating-point numeric value that is qualified by the corresponding measurement unit code - see gs1:unitCode"@en ;
	rdfs:domain       gs1:QuantitativeValue ;
	rdfs:isDefinedBy  gs1: ;
	rdfs:label        "Measurement Value"@en ;
	rdfs:range        xsd:float ;
	sw:term_status    "stable" ;
	skos:exactMatch   schema:value .

gs1:variantDescription
	rdf:type          rdf:Property , owl:DatatypeProperty ;
	rdfs:comment      "Free text field used to identify the variant of the product. Variants are the distinguishing characteristics that differentiate products with the same brand and size including such things as the particular flavour, fragrance, taste."@en ;
	rdfs:domain       gs1:Product ;
	rdfs:isDefinedBy  gs1: ;
	rdfs:label        "Variant Description"@en ;
	rdfs:range        rdf:langString ;
	sw:term_status    "stable" .

gs1:verificationService
	rdf:type            owl:ObjectProperty , rdf:Property ;
	rdfs:comment        "A link to a GS1 Lightweight Messaging Service for verifying the status of a product, organisation, or location and its identifier."@en ;
	rdfs:domain         owl:Thing ;
	rdfs:label          "Verification Service"@en ;
	rdfs:range          xsd:anyURI ;
	rdfs:subPropertyOf  gs1:linkType ;
	sw:term_status      "stable" .

gs1:vintner
	rdf:type     owl:DatatypeProperty , rdf:Property ;
	rdfs:comment      "The person hired by a winery or wine company who is responsible for many of the processes in the preparation, taste and quality of the wine produced. The science of wine making is referred to as oenology. The vintner is the oenologist."@en ;
	rdfs:domain       gs1:Beverage ;
	rdfs:isDefinedBy  gs1: ;
	rdfs:label        "Vintner"@en ;
	rdfs:range        rdf:langString ;
	sw:term_status    "stable" .

gs1:vitaminAPerNutrientBasis
	rdf:type          rdf:Property , owl:ObjectProperty ;
	rdfs:comment      "Vitamin A per specified nutrient basis quantity."@en ;
	rdfs:domain       gs1:FoodBeverageTobaccoProduct ;
	rdfs:isDefinedBy  gs1: ;
	rdfs:label        "Vitamin A Per Nutrient Basis Quantity"@en ;
	rdfs:range        gs1:NutritionMeasurementType ;
	sw:term_status    "stable" .

gs1:vitaminB12PerNutrientBasis
	rdf:type          rdf:Property , owl:ObjectProperty ;
	rdfs:comment      "Vitamin B12 per specified nutrient basis quantity."@en ;
	rdfs:domain       gs1:FoodBeverageTobaccoProduct ;
	rdfs:isDefinedBy  gs1: ;
	rdfs:label        "Vitamin B12 Per Nutrient Basis Quantity"@en ;
	rdfs:range        gs1:NutritionMeasurementType ;
	sw:term_status    "stable" .

gs1:vitaminB6PerNutrientBasis
	rdf:type          owl:ObjectProperty , rdf:Property ;
	rdfs:comment      "Vitamin B6 per specified nutrient basis quantity."@en ;
	rdfs:domain       gs1:FoodBeverageTobaccoProduct ;
	rdfs:isDefinedBy  gs1: ;
	rdfs:label        "Vitamin B6 Per Nutrient Basis Quantity"@en ;
	rdfs:range        gs1:NutritionMeasurementType ;
	sw:term_status    "stable" .

gs1:vitaminCPerNutrientBasis
	rdf:type          owl:ObjectProperty , rdf:Property ;
	rdfs:comment      "Vitamin C per specified nutrient basis quantity."@en ;
	rdfs:domain       gs1:FoodBeverageTobaccoProduct ;
	rdfs:isDefinedBy  gs1: ;
	rdfs:label        "Vitamin C Per Nutrient Basis Quantity"@en ;
	rdfs:range        gs1:NutritionMeasurementType ;
	sw:term_status    "stable" .

gs1:vitaminDPerNutrientBasis
	rdf:type          owl:ObjectProperty , rdf:Property ;
	rdfs:comment      "Vitamin D per specified nutrient basis quantity."@en ;
	rdfs:domain       gs1:FoodBeverageTobaccoProduct ;
	rdfs:isDefinedBy  gs1: ;
	rdfs:label        "Vitamin D Per Nutrient Basis Quantity"@en ;
	rdfs:range        gs1:NutritionMeasurementType ;
	sw:term_status    "stable" .

gs1:vitaminEPerNutrientBasis
	rdf:type          rdf:Property , owl:ObjectProperty ;
	rdfs:comment      "Vitamin E per specified nutrient basis quantity."@en ;
	rdfs:domain       gs1:FoodBeverageTobaccoProduct ;
	rdfs:isDefinedBy  gs1: ;
	rdfs:label        "Vitamin E Per Nutrient Basis Quantity"@en ;
	rdfs:range        gs1:NutritionMeasurementType ;
	sw:term_status    "stable" .

gs1:vitaminKPerNutrientBasis
	rdf:type          rdf:Property , owl:ObjectProperty ;
	rdfs:comment      "Vitamin K per specified nutrient basis quantity."@en ;
	rdfs:domain       gs1:FoodBeverageTobaccoProduct ;
	rdfs:isDefinedBy  gs1: ;
	rdfs:label        "Vitamin K Per Nutrient Basis Quantity"@en ;
	rdfs:range        gs1:NutritionMeasurementType ;
	sw:term_status    "stable" .

gs1:warningCopyDescription
	rdf:type          rdf:Property , owl:DatatypeProperty ;
	rdfs:comment      "Warning information is additional information that outlines special requirements, warning and caution information printed on the package."@en ;
	rdfs:domain       gs1:Product ;
	rdfs:isDefinedBy  gs1: ;
	rdfs:label        "Warning Copy Description"@en ;
	rdfs:range        rdf:langString ;
	sw:term_status    "stable" .

gs1:warranty
	rdf:type      owl:ObjectProperty , rdf:Property ;
	rdfs:comment        "The warranty associated with the product, as provided by the manufacturer."@en ;
	rdfs:domain         gs1:Offer ;
	rdfs:isDefinedBy    gs1: ;
	rdfs:label          "Has Offer Warranty"@en ;
	rdfs:range          gs1:WarrantyPromise ;
	rdfs:subPropertyOf  schema:warranty ;
	sw:term_status      "stable" ;
	skos:exactMatch     schema:warranty .

gs1:warrantyScopeDescription
	rdf:type            owl:DatatypeProperty , rdf:Property ;
	rdfs:comment        "The description of warranty available for the product. Allows for the representation of the same value in different languages but not for multiple values."@en ;
	rdfs:domain         gs1:WarrantyPromise ;
	rdfs:isDefinedBy    gs1: ;
	rdfs:label          "Warranty Scope"@en ;
	rdfs:range          rdf:langString ;
	rdfs:seeAlso        schema:WarrantyPromise ;
	rdfs:subPropertyOf  schema:description ;
	sw:term_status      "stable" .

gs1:whatsInTheBox
	rdf:type  owl:ObjectProperty , rdf:Property ;
	rdfs:comment        "A link to a description of all the individual items in a packaged item."@en ;
	rdfs:domain         owl:Thing ;
	rdfs:label          "What's in the box?"@en ;
	rdfs:range          xsd:anyURI ;
	rdfs:subPropertyOf  gs1:linkType ;
	sw:term_status      "stable" .

gs1:yield
	rdf:type       owl:ObjectProperty , rdf:Property ;
	rdfs:comment      "Product quantity after preparation."@en ;
	rdfs:domain       gs1:FoodAndBeveragePreparationInformation ;
	rdfs:isDefinedBy  gs1: ;
	rdfs:label        "Yield"@en ;
	rdfs:range        gs1:ProductYieldDetails ;
	sw:term_status    "stable" .

gs1:zincPerNutrientBasis
	rdf:type          rdf:Property , owl:ObjectProperty ;
	rdfs:comment      "Zinc per specified nutrient basis quantity."@en ;
	rdfs:domain       gs1:FoodBeverageTobaccoProduct ;
	rdfs:isDefinedBy  gs1: ;
	rdfs:label        "Zinc Per Nutrient Basis Quantity"@en ;
	rdfs:range        gs1:NutritionMeasurementType ;
	sw:term_status    "stable" .


gs1:AllergenTypeCode
	rdfs:isDefinedBy  <http://apps.gs1.org/GDD/bms/Version2_8/Pages/clDetails.aspx?semanticURN=urn:gs1:gdd:cl:AllergenTypeCodeList&release=1> ;
	rdfs:label        "Allergen Type Code"@en ;
	rdfs:subClassOf   gs1:TypeCode .

gs1:AnatomicalFormCode
	rdfs:label       "Anatomical Form Code"@en ;
	rdfs:subClassOf  gs1:TypeCode .

gs1:CertificationStatus
	rdfs:comment      "A set of codes for the status of a certification instance"@en ;
	rdfs:isDefinedBy  gs1: ;
	rdfs:label        "Certification Status Code"@en ;
	rdfs:subClassOf   gs1:TypeCode .

gs1:CheeseFirmnessCode
	rdfs:label       "Cheese Firmness Code"@en ;
	rdfs:subClassOf  gs1:TypeCode .

gs1:ColourCodeListCode
	rdfs:label       "Colour Code List Code"@en ;
	rdfs:subClassOf  gs1:TypeCode .

gs1:ConsumerLifestageCode
	rdfs:label       "Consumer Lifestage Code"@en ;
	rdfs:subClassOf  gs1:TypeCode .

gs1:ConsumerSalesConditionsCode
	rdfs:isDefinedBy  <http://apps.gs1.org/GDD/bms/Version2_8/Pages/clDetails.aspx?semanticURN=urn:gs1:gdd:cl:ConsumerSalesConditionCodeList&release=2> ;
	rdfs:label        "Consumer Sales Conditions Code"@en ;
	rdfs:subClassOf   gs1:TypeCode .

gs1:DietTypeCode
	rdfs:label  "Diet Type Code"@en ;
	rdfs:subClassOf  gs1:TypeCode .

gs1:DiscountTypeCode
	rdfs:label  "Discount Type Code"@en ;
	rdfs:subClassOf  gs1:TypeCode .

gs1:FoodBeverageRefrigerationClaimCode
	rdfs:label       "Food Beverage Refrigeration Claim Code"@en ;
	rdfs:subClassOf  gs1:TypeCode .

gs1:FoodBeverageTargetUseCode
	rdfs:label       "Food Beverage Target Use Code"@en ;
	rdfs:subClassOf  gs1:TypeCode .

gs1:FootwearFasteningTypeCode
	rdfs:label       "Footwear Fastening Type Code"@en ;
	rdfs:subClassOf  gs1:TypeCode .

gs1:FreshOrSeawaterFarmedCode
	rdfs:label       "Fresh Or Seawater Farmed Code"@en ;
	rdfs:subClassOf  gs1:TypeCode .

gs1:GLN_TypeCode
	rdfs:comment  "GLN Type Code indicates what type of thing is being identified by a GLN. gs1:GLN_TypeCode value selections SHALL NOT contain both gs1:GLN_TypeCode-FIXED_PHYSICAL_LOCATION and gs1:GLN_TypeCode-MOBILE_PHYSICAL_LOCATION."@en ;
	rdfs:isDefinedBy  gs1: ;
	rdfs:label        "GLN Type Code"@en ;
	rdfs:subClassOf   gs1:TypeCode .

gs1:GrowingMethodCode
	rdfs:isDefinedBy  <http://apps.gs1.org/GDD/Pages/clDetails.aspx?semanticURN=urn:gs1:gdd:cl:GrowingMethodCode&release=1> ;
	rdfs:label        "Growing Method Code"@en ;
	rdfs:subClassOf   gs1:TypeCode .

gs1:LevelOfContainmentCode
	rdfs:isDefinedBy  <http://apps.gs1.org/GDD/bms/Version2_8/Pages/clDetails.aspx?semanticURN=urn:gs1:gdd:cl:LevelOfContainmentCodeList&release=1> ;
	rdfs:label        "Level Of Containment Code"@en ;
	rdfs:subClassOf   gs1:TypeCode .

gs1:LocationID_Type
	rdfs:isDefinedBy  gs1: ;
	rdfs:label        "Location ID Type"@en ;
	rdfs:subClassOf   gs1:TypeCode .

gs1:MaturationMethodCode
	rdfs:isDefinedBy  <http://apps.gs1.org/GDD/Pages/clDetails.aspx?semanticURN=urn:gs1:gdd:cl:MaturationMethodCode&release=1> ;
	rdfs:label        "Maturation Method Code"@en ;
	rdfs:subClassOf   gs1:TypeCode .

gs1:MeasurementPrecisionCode
	rdfs:isDefinedBy  <http://apps.gs1.org/GDD/Pages/clDetails.aspx?semanticURN=urn:gs1:gdd:cl:MeasurementPrecisionCode&release=1> ;
	rdfs:label        "Measurement Precision Code"@en ;
	rdfs:subClassOf   gs1:TypeCode .

gs1:MeasurementType
	rdfs:comment  "A set of measurement types for properties that can be measured or sensed by appropriate measuring devices or sensors"@en ;
	rdfs:isDefinedBy  gs1: ;
	rdfs:label        "Measurement type"@en ;
	rdfs:subClassOf   gs1:TypeCode .

gs1:NonbinaryLogicCode
	rdfs:isDefinedBy  <http://apps.gs1.org/GDD/Pages/clDetails.aspx?semanticURN=urn:gs1:gdd:cl:NonBinaryLogicEnumeration&release=1> ;
	rdfs:label        "Nonbinary Logic Code"@en ;
	rdfs:subClassOf   gs1:TypeCode .

gs1:NutrientBasisQuantityCode
	rdfs:isDefinedBy  <http://apps.gs1.org/GDD/Pages/clDetails.aspx?semanticURN=urn:gs1:gdd:cl:NutrientBasisQuantityTypeCode&release=1> ;
	rdfs:label        "Nutrient Basis Quantity Code"@en ;
	rdfs:subClassOf   gs1:TypeCode .

gs1:NutritionalClaimTypeCode
	rdfs:isDefinedBy  <http://apps.gs1.org/GDD/Pages/clDetails.aspx?semanticURN=urn:gs1:gdd:cl:NutritionalClaimTypeCode&release=1> ;
	rdfs:label        "Nutritional Claim Type Code"@en ;
	rdfs:subClassOf   gs1:TypeCode .

gs1:OfferRedemptionTypeCode
	rdfs:label       "Offer Redemption Type Code"@en ;
	rdfs:subClassOf  gs1:TypeCode .

gs1:OrganicClaimAgencyCode
	rdfs:isDefinedBy  <http://apps.gs1.org/GDD/Pages/clDetails.aspx?semanticURN=urn:gs1:gdd:cl:OrganicClaimAgencyCode&release=1> ;
	rdfs:label        "Organic Claim Agency Code"@en ;
	rdfs:subClassOf   gs1:TypeCode .

gs1:OrganizationID_Type
	rdfs:isDefinedBy  gs1: ;
	rdfs:label        "Organization ID Type"@en ;
	rdfs:subClassOf   gs1:TypeCode .

gs1:OrganizationRoleType
	rdfs:isDefinedBy  <http://apps.gs1.org/GDD/Pages/clDetails.aspx?semanticURN=urn:gs1:gdd:cl:PartyRoleCode&release=2> ;
	rdfs:label        "Organization Role Code"@en ;
	rdfs:subClassOf   gs1:TypeCode .

gs1:PackagingFeatureCode
	rdfs:isDefinedBy  <http://apps.gs1.org/GDD/Pages/clDetails.aspx?semanticURN=urn:gs1:gdd:cl:PackagingFeatureCode&release=1> ;
	rdfs:label        "Packaging Feature Code"@en ;
	rdfs:subClassOf   gs1:TypeCode .

gs1:PackagingFunctionCode
	rdfs:isDefinedBy  <http://apps.gs1.org/GDD/Pages/clDetails.aspx?semanticURN=urn:gs1:gdd:cl:PackagingFunctionCode&release=1> ;
	rdfs:label        "Packaging Function Code"@en ;
	rdfs:subClassOf   gs1:TypeCode .

gs1:PackagingMarkedDietAllergenCode
	rdfs:isDefinedBy  <http://apps.gs1.org/GDD/bms/Version2_8/Pages/clDetails.aspx?semanticURN=urn:gs1:gdd:cl:PackageMarksDietAllergenCodeList&release=1> ;
	rdfs:label        "Packaging Marked Diet Allergen Code"@en ;
	rdfs:subClassOf   gs1:TypeCode .

gs1:PackagingMarkedFreeFromCode
	rdfs:isDefinedBy  <http://apps.gs1.org/GDD/Pages/clDetails.aspx?semanticURN=urn:gs1:gdd:cl:PackagingMarkedFreeFromCode&release=1> ;
	rdfs:label        "Packaging Marked Free From Code"@en ;
	rdfs:subClassOf   gs1:TypeCode .

gs1:PackagingMarkedLabelAccreditationCode
	rdfs:isDefinedBy  <http://apps.gs1.org/GDD/Pages/clDetails.aspx?semanticURN=urn:gs1:gdd:cl:PackagingMarkedLabelAccreditationCode&release=1> ;
	rdfs:label        "Packaging Marked Label Accreditation Code"@en ;
	rdfs:subClassOf   gs1:TypeCode .

gs1:PackagingMaterialTypeCode
	rdfs:isDefinedBy  <http://apps.gs1.org/GDD/Pages/clDetails.aspx?semanticURN=urn:gs1:gdd:cl:PackagingMaterialTypeCode&release=1> ;
	rdfs:label        "Packaging Material Type Code"@en ;
	rdfs:subClassOf   gs1:TypeCode .

gs1:PackagingRecyclingProcessTypeCode
	rdfs:isDefinedBy  <http://apps.gs1.org/GDD/Pages/clDetails.aspx?semanticURN=urn:gs1:gdd:cl:PackagingRecyclingProcessTypeCode&release=1> ;
	rdfs:label        "Packaging Recycling Process Type Code"@en ;
	rdfs:subClassOf   gs1:TypeCode .

gs1:PackagingRecyclingSchemeCode
	rdfs:isDefinedBy  <http://apps.gs1.org/GDD/Pages/clDetails.aspx?semanticURN=urn:gs1:gdd:cl:PackagingRecyclingSchemeCode&release=1> ;
	rdfs:label        "Packaging Recycling Scheme Code"@en ;
	rdfs:subClassOf   gs1:TypeCode .

gs1:PackagingShapeCode
	rdfs:isDefinedBy  <http://apps.gs1.org/GDD/Pages/clDetails.aspx?semanticURN=urn:gs1:gdd:cl:PackagingShapeCode&release=1> ;
	rdfs:label        "Packaging Shape Code"@en ;
	rdfs:subClassOf   gs1:TypeCode .

gs1:PaymentMethod
	rdfs:comment  "A code indicating an accepted method of payment"@en ;
	rdfs:isDefinedBy  <http://apps.gs1.org/GDD/Pages/clDetails.aspx?semanticURN=urn:gs1:gdd:cl:PaymentMethod&release=1> ;
	rdfs:label        "Payment Method Code"@en ;
	rdfs:subClassOf   gs1:TypeCode .

gs1:PreparationTypeCode
	rdfs:comment      "A code indicating a method of preparation of a food or beverage product"@en ;
	rdfs:isDefinedBy  <http://apps.gs1.org/GDD/Pages/clDetails.aspx?semanticURN=urn:gs1:gdd:cl:PreparationTypeCode&release=1> ;
	rdfs:label        "Preparation Type Code"@en ;
	rdfs:subClassOf   gs1:TypeCode .

gs1:PreservationTechniqueCode
	rdfs:isDefinedBy  <http://apps.gs1.org/GDD/Pages/clDetails.aspx?semanticURN=urn:gs1:gdd:cl:PreservationTechniqueTypeCode&release=1> ;
	rdfs:label        "Preservation Technique Code"@en ;
	rdfs:subClassOf   gs1:TypeCode .

gs1:ProductYieldTypeCode
	rdfs:isDefinedBy  <http://apps.gs1.org/GDD/Pages/clDetails.aspx?semanticURN=urn:gs1:gdd:cl:ProductYieldTypeCode&release=1> ;
	rdfs:label        "Product Yield Type Code"@en ;
	rdfs:subClassOf   gs1:TypeCode .

gs1:ReferencedFileTypeCode
	rdfs:isDefinedBy  <http://apps.gs1.org/GDD/Pages/clDetails.aspx?semanticURN=urn:gs1:gdd:cl:ReferencedFileTypeCode&release=1> ;
	rdfs:label        "Referenced File Type Code"@en ;
	rdfs:subClassOf   gs1:TypeCode .

gs1:SeasonParameterCode
	rdfs:isDefinedBy  <http://apps.gs1.org/GDD/Pages/clDetails.aspx?semanticURN=urn:gs1:gdd:cl:SeasonParameterCode&release=1> ;
	rdfs:label        "Season Parameter Code"@en ;
	rdfs:subClassOf   gs1:TypeCode .

gs1:SecurityMarking
	rdfs:isDefinedBy  gs1: ;
	rdfs:label        "Security Marking code list"@en ;
	rdfs:subClassOf   gs1:TypeCode .

gs1:SensorAlertType
	rdfs:comment  "A code list for reasons for generating a sensor alert, including an alarm condition or an error condition"@en ;
	rdfs:isDefinedBy  gs1: ;
	rdfs:label        "Sensor Alert Type"@en ;
	rdfs:subClassOf   gs1:TypeCode .

gs1:SharpnessOfCheeseCode
	rdfs:isDefinedBy  gs1: ;
	rdfs:label        "Sharpness of Cheese Code"@en ;
	rdfs:subClassOf   gs1:TypeCode .

gs1:SizeGroupCode
	rdfs:isDefinedBy  <http://apps.gs1.org/GDD/Pages/clDetails.aspx?semanticURN=urn:gs1:gdd:cl:SizeGroupCode&release=1> ;
	rdfs:label        "Size Group Code"@en ;
	rdfs:subClassOf   gs1:TypeCode .

gs1:SizeSystemCode
	rdfs:isDefinedBy  <http://apps.gs1.org/GDD/Pages/clDetails.aspx?semanticURN=urn:gs1:gdd:cl:SizeSystemCode&release=1> ;
	rdfs:label        "Size System Code"@en ;
	rdfs:subClassOf   gs1:TypeCode .

gs1:SizeTypeCode
	rdfs:isDefinedBy  <http://apps.gs1.org/GDD/Pages/clDetails.aspx?semanticURN=urn:gs1:gdd:cl:SizeTypeCode&release=1> ;
	rdfs:label        "Size Type Code"@en ;
	rdfs:subClassOf   gs1:TypeCode .

gs1:SourceAnimalCode
	rdfs:isDefinedBy  <http://apps.gs1.org/GDD/Pages/clDetails.aspx?semanticURN=urn:gs1:gdd:cl:SourceAnimalCode&release=1> ;
	rdfs:label        "Source Animal Code"@en ;
	rdfs:subClassOf   gs1:TypeCode .

gs1:SportingActivityTypeCode
	rdfs:label       "Sporting Activity Type Code"@en ;
	rdfs:subClassOf  gs1:TypeCode .

gs1:StatusType
	rdfs:isDefinedBy  gs1: ;
	rdfs:label        "Status Type"@en ;
	rdfs:subClassOf   gs1:TypeCode .

gs1:TargetConsumerGenderCode
	rdfs:isDefinedBy  <http://apps.gs1.org/GDD/bms/Version2_8/Pages/clDetails.aspx?semanticURN=urn:gs1:gdd:cl:TargetConsumerGenderList&release=1> ;
	rdfs:label        "Target Consumer Gender Code"@en ;
	rdfs:subClassOf   gs1:TypeCode .

gs1:TradeChannelCode
	rdfs:label  "Trade Channel Code"@en ;
	rdfs:subClassOf  gs1:TypeCode .

gs1:UpperTypeCode
	rdfs:label  "Upper Type Code"@en ;
	rdfs:subClassOf  gs1:TypeCode .


<https://gs1.org/voc/AllergenTypeCode-1%2C3-BIS-%282%2C4-DIAMINOPHENOXY%29PROPANE>
	rdf:type               gs1:AllergenTypeCode ;
	rdfs:comment           "Refers to the presence of 1,3-Bis-(2,4-diaminophenoxy)propane as listed in the regulations specified in AllergenSpecificationAgency and AllergenSpecificationName."@en ;
	rdfs:label             "1,3-Bis-(2,4-diaminophenoxy)propane"@en ;
	skos:prefLabel         "1,3-BIS-(2,4-DIAMINOPHENOXY)PROPANE" ;
	gs1:originalCodeValue  "BR" .

<https://gs1.org/voc/AllergenTypeCode-2%2C6-DIMETHOXY-3%2C5-PYRIDINEDIAMINE_HCL>
	rdf:type               gs1:AllergenTypeCode ;
	rdfs:comment           "Refers to the presence of 2,6-Dimethoxy-3,5-pyridinediamine HCl as listed in the regulations specified in AllergenSpecificationAgency and AllergenSpecificationName."@en ;
	rdfs:label             "2,6-Dimethoxy-3,5-pyridinediamine HCl"@en ;
	skos:prefLabel         "2,6-DIMETHOXY-3,5-PYRIDINEDIAMINE_HCL" ;
	gs1:originalCodeValue  "DA" .

<https://gs1.org/voc/AllergenTypeCode-3-AMINO-2%2C4-DICHLOROPHENOL>
	rdf:type               gs1:AllergenTypeCode ;
	rdfs:comment           "Refers to the presence of 3-Amino-2,4-dichlorophenol as listed in the regulations specified in AllergenSpecificationAgency and AllergenSpecificationName."@en ;
	rdfs:label             "3-Amino-2,4-dichlorophenol"@en ;
	skos:prefLabel         "3-AMINO-2,4-DICHLOROPHENOL" ;
	gs1:originalCodeValue  "AD" .

<https://gs1.org/voc/AllergenTypeCode-HYDROXYPROPYL_BIS%28N-HYDROXYETHYL-P-PHENYLDIAMINE%29_HCL>
	rdf:type               gs1:AllergenTypeCode ;
	rdfs:comment           "Refers to the presence of Hydroxypropyl bis(N-hydroxyethyl-p-phenyldiamine) HCl as listed in the regulations specified in AllergenSpecificationAgency and AllergenSpecificationName."@en ;
	rdfs:label             "Hydroxypropyl bis(N-hydroxyethyl-p-phenyldiamine) HCl"@en ;
	skos:prefLabel         "HYDROXYPROPYL_BIS(N-HYDROXYETHYL-P-PHENYLDIAMINE)_HCL" ;
	gs1:originalCodeValue  "HH" .

<https://gs1.org/voc/AllergenTypeCode-MONKFISH_%28ANGLERFISH%2C_LOTTE%29>
	rdf:type               gs1:AllergenTypeCode ;
	rdfs:comment           "Refers to the presence of Monkfish (Anglerfish, Lotte) and its derivatives in the product, as listed in the regulations specified in AllergenSpecificationAgency and AllergenSpecificationName."@en ;
	rdfs:label             "Monkfish (Anglerfish, Lotte) and its Derivatives"@en ;
	skos:prefLabel         "MONKFISH_(ANGLERFISH,_LOTTE)" ;
	gs1:originalCodeValue  "MKF" .

<https://gs1.org/voc/AllergenTypeCode-SQUID_%28CALAMARI%29>
	rdf:type               gs1:AllergenTypeCode ;
	rdfs:comment           "Refers to the presence of Squid (Calamari) and its derivatives in the product, as listed in the regulations specified in AllergenSpecificationAgency and AllergenSpecificationName."@en ;
	rdfs:label             "Squid (Calamari) and its Derivatives"@en ;
	skos:prefLabel         "SQUID_(CALAMARI)" ;
	gs1:originalCodeValue  "SQU" .

<https://gs1.org/voc/AllergenTypeCode-TOLUENE-2%2C5-DIAMINE>
	rdf:type               gs1:AllergenTypeCode ;
	rdfs:comment           "Refers to the presence of Toluene-2,5-diamine as listed in the regulations specified in AllergenSpecificationAgency and AllergenSpecificationName."@en ;
	rdfs:label             "Toluene-2,5-diamine"@en ;
	skos:prefLabel         "TOLUENE-2,5-DIAMINE" ;
	gs1:originalCodeValue  "TD" .

gs1:ALARM_CONDITION
	rdf:type  gs1:SensorAlertType ;
	rdfs:comment    "Indicates the reporting of an alarm condition detected by a sensor device"@en ;
	rdfs:label      "Alarm condition"@en ;
	skos:prefLabel  "ALARM_CONDITION" .

gs1:AbsoluteHumidity
	rdf:type  gs1:MeasurementType ;
	rdfs:comment    "The ratio of the mass of water vapour in a sample of moist air to the volume of the sample.  SI Units: kilogram per cubic metre"@en ;
	rdfs:label      "Absolute humidity"@en ;
	skos:prefLabel  "AbsoluteHumidity" .

gs1:AbsorbedDose
	rdf:type  gs1:MeasurementType ;
	rdfs:comment    "The energy absorbed per unit mass of the patient from the decay of a radionuclide given to a patient for diagnostic or therapeutic purposes.  SI Units: gray"@en ;
	rdfs:label      "Absorbed dose"@en ;
	skos:prefLabel  "AbsorbedDose" .

gs1:AbsorbedDoseRate
	rdf:type  gs1:MeasurementType ;
	rdfs:comment    "The energy absorbed per unit time per unit mass of the patient from the decay of a radionuclide given to a patient for diagnostic or therapeutic purposes.  SI Units: gray per second"@en ;
	rdfs:label      "Absorbed dose rate"@en ;
	skos:prefLabel  "AbsorbedDoseRate" .

gs1:Acceleration
	rdf:type  gs1:MeasurementType ;
	rdfs:comment    "The rate of change of velocity, a vector quantity with magnitude and direction.  SI Units: metre per second per second"@en ;
	rdfs:label      "Acceleration"@en ;
	skos:prefLabel  "Acceleration" .

gs1:AllergenTypeCode-1-NAPHTHOL
	rdf:type               gs1:AllergenTypeCode ;
	rdfs:comment           "Refers to the presence of 1-Naphthol as listed in the regulations specified in AllergenSpecificationAgency and AllergenSpecificationName."@en ;
	rdfs:label             "1-Naphthol"@en ;
	skos:prefLabel         "1-NAPHTHOL" ;
	gs1:originalCodeValue  "ON" .

gs1:AllergenTypeCode-2-HYDROXYETHYL-PICRAMIC_ACID
	rdf:type               gs1:AllergenTypeCode ;
	rdfs:comment           "Refers to the presence of 2-Hydroxyethyl-picramic acid as listed in the regulations specified in AllergenSpecificationAgency and AllergenSpecificationName."@en ;
	rdfs:label             "2-Hydroxyethyl-picramic Acid"@en ;
	skos:prefLabel         "2-HYDROXYETHYL-PICRAMIC_ACID" ;
	gs1:originalCodeValue  "HP" .

gs1:AllergenTypeCode-2-METHYL-5-HYDROXYETHYLAMINOPHENOL
	rdf:type               gs1:AllergenTypeCode ;
	rdfs:comment           "Refers to the presence of 2-Methyl-5-hydroxyethylaminophenol as listed in the regulations specified in AllergenSpecificationAgency and AllergenSpecificationName."@en ;
	rdfs:label             "2-Methyl-5-hydroxyethylaminophenol"@en ;
	skos:prefLabel         "2-METHYL-5-HYDROXYETHYLAMINOPHENOL" ;
	gs1:originalCodeValue  "MH" .

gs1:AllergenTypeCode-3-AMINOPHENOL
	rdf:type               gs1:AllergenTypeCode ;
	rdfs:comment           "Refers to the presence of 3-Aminophenol as listed in the regulations specified in AllergenSpecificationAgency and AllergenSpecificationName."@en ;
	rdfs:label             "3-Aminophenol"@en ;
	skos:prefLabel         "3-AMINOPHENOL" ;
	gs1:originalCodeValue  "TA" .

gs1:AllergenTypeCode-4-AMINO-3-NITROPHENOL
	rdf:type               gs1:AllergenTypeCode ;
	rdfs:comment           "Refers to the presence of 4-Amino-3-nitrophenol as listed in the regulations specified in AllergenSpecificationAgency and AllergenSpecificationName."@en ;
	rdfs:label             "4-Amino-3-nitrophenol"@en ;
	skos:prefLabel         "4-AMINO-3-NITROPHENOL" ;
	gs1:originalCodeValue  "FT" .

gs1:AllergenTypeCode-4-HYDROXY-PROPYLAMINO-3-NITROPHENOL
	rdf:type               gs1:AllergenTypeCode ;
	rdfs:comment           "Refers to the presence of 4-Hydroxy-propylamino-3-nitrophenol as listed in the regulations specified in AllergenSpecificationAgency and AllergenSpecificationName."@en ;
	rdfs:label             "4-Hydroxy-propylamino-3-nitrophenol"@en ;
	skos:prefLabel         "4-HYDROXY-PROPYLAMINO-3-NITROPHENOL" ;
	gs1:originalCodeValue  "FH" .

gs1:AllergenTypeCode-ABALONE
	rdf:type               gs1:AllergenTypeCode ;
	rdfs:comment           "Refers to the presence of Abalone and its derivatives in the product, as listed in the regulations specified in AllergenSpecificationAgency and AllergenSpecificationName."@en ;
	rdfs:label             "Abalone and its Derivatives"@en ;
	skos:prefLabel         "ABALONE" ;
	gs1:originalCodeValue  "ABN" .

gs1:AllergenTypeCode-ALMONDS
	rdf:type               gs1:AllergenTypeCode ;
	rdfs:comment           "Refers to the presence of almond and almond products as listed in the regulations specified in AllergenSpecificationAgency and AllergenSpecificationName."@en ;
	rdfs:label             "Almond and Almond Products"@en ;
	skos:prefLabel         "ALMONDS" ;
	gs1:originalCodeValue  "SA" .

gs1:AllergenTypeCode-ALPHA_ISOMETHYL_IONONE
	rdf:type               gs1:AllergenTypeCode ;
	rdfs:comment           "Refers to the presence of Alpha-Isomethyl Ionone as listed in the regulations specified in AllergenSpecificationAgency and AllergenSpecificationName."@en ;
	rdfs:label             "Alpha-Isomethyl Ionone"@en ;
	skos:prefLabel         "ALPHA_ISOMETHYL_IONONE" ;
	gs1:originalCodeValue  "AI" .

gs1:AllergenTypeCode-AMYLCINNAMYL_ALCOHOL
	rdf:type               gs1:AllergenTypeCode ;
	rdfs:comment           "Refers to the presence of Amylcinnamyl Alcohol as listed in the regulations specified in AllergenSpecificationAgency and AllergenSpecificationName."@en ;
	rdfs:label             "Amylcinnamyl Alcohol"@en ;
	skos:prefLabel         "AMYLCINNAMYL_ALCOHOL" ;
	gs1:originalCodeValue  "AA" .

gs1:AllergenTypeCode-AMYL_CINNAMAL
	rdf:type               gs1:AllergenTypeCode ;
	rdfs:comment           "Refers to the presence of Amyl Cinnamal as listed in the regulations specified in AllergenSpecificationAgency and AllergenSpecificationName."@en ;
	rdfs:label             "Amyl Cinnamal"@en ;
	skos:prefLabel         "AMYL_CINNAMAL" ;
	gs1:originalCodeValue  "AL" .

gs1:AllergenTypeCode-ANCHOVY
	rdf:type               gs1:AllergenTypeCode ;
	rdfs:comment           "Refers to the presence of anchovies and their derivatives in the product, as listed as listed in the regulations specified in AllergenSpecificationAgency and AllergenSpecificationName."@en ;
	rdfs:label             "Anchovy and its Derivatives"@en ;
	skos:prefLabel         "ANCHOVY" ;
	gs1:originalCodeValue  "ADC" .

gs1:AllergenTypeCode-ANISE_ALCOHOL
	rdf:type               gs1:AllergenTypeCode ;
	rdfs:comment           "Refers to the presence of Anise Alcohol as listed in the regulations specified in AllergenSpecificationAgency and AllergenSpecificationName."@en ;
	rdfs:label             "Anise Alcohol"@en ;
	skos:prefLabel         "ANISE_ALCOHOL" ;
	gs1:originalCodeValue  "AH" .

gs1:AllergenTypeCode-BARLEY
	rdf:type               gs1:AllergenTypeCode ;
	rdfs:comment           "Refers to the presence of Barley and barley products (glutencontaining grain) as listed in the regulations specified in AllergenSpecificationAgency and AllergenSpecificationName."@en ;
	rdfs:label             "Barley and Barley Products"@en ;
	skos:prefLabel         "BARLEY" ;
	gs1:originalCodeValue  "GB" .

gs1:AllergenTypeCode-BARNACLE
	rdf:type               gs1:AllergenTypeCode ;
	rdfs:comment           "Refers to the presence of Barnacles and their derivatives in the product, as listed as listed in the regulations specified in AllergenSpecificationAgency and AllergenSpecificationName."@en ;
	rdfs:label             "Barnacle and its Derivatives"@en ;
	skos:prefLabel         "BARNACLE" ;
	gs1:originalCodeValue  "ABF" .

gs1:AllergenTypeCode-BASA
	rdf:type               gs1:AllergenTypeCode ;
	rdfs:comment           "Refers to the presence of Basa and its derivatives in the product, as listed in the regulations specified in AllergenSpecificationAgency and AllergenSpecificationName."@en ;
	rdfs:label             "Basa and its Derivatives"@en ;
	skos:prefLabel         "BASA" ;
	gs1:originalCodeValue  "BAS" .

gs1:AllergenTypeCode-BASS
	rdf:type               gs1:AllergenTypeCode ;
	rdfs:comment           "Refers to the presence of bass and their derivatives in the product, as listed as listed in the regulations specified in AllergenSpecificationAgency and AllergenSpecificationName."@en ;
	rdfs:label             "Bass and its Derivatives"@en ;
	skos:prefLabel         "BASS" ;
	gs1:originalCodeValue  "ADB" .

gs1:AllergenTypeCode-BEECH_NUTS
	rdf:type               gs1:AllergenTypeCode ;
	rdfs:comment           "Refers to the presence of Beech nuts [Fagus spp. (Fagaceae)] and their derivatives in the product, as listed as listed in the regulations specified in AllergenSpecificationAgency and AllergenSpecificationName."@en ;
	rdfs:label             "Beech Nuts and Their Derivatives"@en ;
	skos:prefLabel         "BEECH_NUTS" ;
	gs1:originalCodeValue  "SD" .

gs1:AllergenTypeCode-BEEF
	rdf:type               gs1:AllergenTypeCode ;
	rdfs:comment           "Refers to the presence of beef and its derivative in the product, as listed in the regulations specified in AllergenSpecificationAgency and AllergenSpecificationName."@en ;
	rdfs:label             "Beef and its Derivatives"@en ;
	skos:prefLabel         "BEEF" ;
	gs1:originalCodeValue  "BF" .

gs1:AllergenTypeCode-BENZYL_ALCOHOL
	rdf:type               gs1:AllergenTypeCode ;
	rdfs:comment           "Refers to the presence of Benzyl Alcohol as listed in the regulations specified in AllergenSpecificationAgency and AllergenSpecificationName."@en ;
	rdfs:label             "Benzyl Alcohol"@en ;
	skos:prefLabel         "BENZYL_ALCOHOL" ;
	gs1:originalCodeValue  "BA" .

gs1:AllergenTypeCode-BENZYL_BENZOATE
	rdf:type               gs1:AllergenTypeCode ;
	rdfs:comment           "Refers to the presence of Benzyl Benzoate as listed in the regulations specified in AllergenSpecificationAgency and AllergenSpecificationName."@en ;
	rdfs:label             "Benzyl Benzoate"@en ;
	skos:prefLabel         "BENZYL_BENZOATE" ;
	gs1:originalCodeValue  "BB" .

gs1:AllergenTypeCode-BENZYL_CINNAMATE
	rdf:type               gs1:AllergenTypeCode ;
	rdfs:comment           "Refers to the presence of Benzyl Cinnamate as listed in the regulations specified in AllergenSpecificationAgency and AllergenSpecificationName."@en ;
	rdfs:label             "Benzyl Cinnamate."@en ;
	skos:prefLabel         "BENZYL_CINNAMATE" ;
	gs1:originalCodeValue  "BI" .

gs1:AllergenTypeCode-BENZYL_SALICYLATE
	rdf:type               gs1:AllergenTypeCode ;
	rdfs:comment           "Refers to the presence of Benzyl Salicylate as listed in the regulations specified in AllergenSpecificationAgency and AllergenSpecificationName."@en ;
	rdfs:label             "Benzyl Salicylate"@en ;
	skos:prefLabel         "BENZYL_SALICYLATE" ;
	gs1:originalCodeValue  "BS" .

gs1:AllergenTypeCode-BLUEFISH
	rdf:type               gs1:AllergenTypeCode ;
	rdfs:comment           "Refers to the presence of Bluefish and its derivatives in the product, as listed in the regulations specified in AllergenSpecificationAgency and AllergenSpecificationName."@en ;
	rdfs:label             "Bluefish and its Derivatives"@en ;
	skos:prefLabel         "BLUEFISH" ;
	gs1:originalCodeValue  "BLF" .

gs1:AllergenTypeCode-BRAZIL_NUTS
	rdf:type               gs1:AllergenTypeCode ;
	rdfs:comment           "Refers to the presence of brazil nut and brazil nut products as listed in the regulations specified in AllergenSpecificationAgency and AllergenSpecificationName."@en ;
	rdfs:label             "Brazil Nut and Brazil Nut Products"@en ;
	skos:prefLabel         "BRAZIL_NUTS" ;
	gs1:originalCodeValue  "SR" .

gs1:AllergenTypeCode-BREAM
	rdf:type               gs1:AllergenTypeCode ;
	rdfs:comment           "Refers to the presence of Bream and its derivatives in the product, as listed in the regulations specified in AllergenSpecificationAgency and AllergenSpecificationName."@en ;
	rdfs:label             "Bream and its Derivatives"@en ;
	skos:prefLabel         "BREAM" ;
	gs1:originalCodeValue  "BRM" .

gs1:AllergenTypeCode-BUTTERNUTS
	rdf:type               gs1:AllergenTypeCode ;
	rdfs:comment           "Refers to the presence of Butternuts [Juglans cinerea (Juglandaceae)] and their derivatives in the product, as listed as listed in the regulations specified in AllergenSpecificationAgency and AllergenSpecificationName."@en ;
	rdfs:label             "Butternuts and Their Derivatives"@en ;
	skos:prefLabel         "BUTTERNUTS" ;
	gs1:originalCodeValue  "SE" .

gs1:AllergenTypeCode-BUTYLPHENYL_METHYLPROPIONATE
	rdf:type               gs1:AllergenTypeCode ;
	rdfs:comment           "Refers to the presence of Butylphenyl Methylpropionate as listed in the regulations specified in AllergenSpecificationAgency and AllergenSpecificationName."@en ;
	rdfs:label             "Butylphenyl Methylpropionate."@en ;
	skos:prefLabel         "BUTYLPHENYL_METHYLPROPIONATE" ;
	gs1:originalCodeValue  "BE" .

gs1:AllergenTypeCode-CARP
	rdf:type               gs1:AllergenTypeCode ;
	rdfs:comment           "Refers to the presence of Carp and their derivatives in the product, as listed as listed in the regulations specified in AllergenSpecificationAgency and AllergenSpecificationName."@en ;
	rdfs:label             "Carp and its Derivatives"@en ;
	skos:prefLabel         "CARP" ;
	gs1:originalCodeValue  "ACP" .

gs1:AllergenTypeCode-CARROTS
	rdf:type               gs1:AllergenTypeCode ;
	rdfs:comment           "Refers to the presence of carrot and their derivatives in the product, as listed in as listed in the regulations specified in AllergenSpecificationAgency and AllergenSpecificationName"@en ;
	rdfs:label             "Carrot and Derivatives"@en ;
	skos:prefLabel         "CARROTS" ;
	gs1:originalCodeValue  "NW" .

gs1:AllergenTypeCode-CASHEW_NUTS
	rdf:type               gs1:AllergenTypeCode ;
	rdfs:comment           "Refers to the presence of cashew and cashew products as listed in the regulations specified in AllergenSpecificationAgency and AllergenSpecificationName."@en ;
	rdfs:label             "Cashew and Cashew Products"@en ;
	skos:prefLabel         "CASHEW_NUTS" ;
	gs1:originalCodeValue  "SC" .

gs1:AllergenTypeCode-CATFISH
	rdf:type               gs1:AllergenTypeCode ;
	rdfs:comment           "Refers to the presence of catfish and their derivatives in the product, as listed as listed in the regulations specified in AllergenSpecificationAgency and AllergenSpecificationName."@en ;
	rdfs:label             "Catfish and its Derivatives"@en ;
	skos:prefLabel         "CATFISH" ;
	gs1:originalCodeValue  "ADE" .

gs1:AllergenTypeCode-CELERY
	rdf:type               gs1:AllergenTypeCode ;
	rdfs:comment           "Refers to the presence of celery or their derivatives in the product, as listed in as listed in the regulations specified in AllergenSpecificationAgency and AllergenSpecificationName"@en ;
	rdfs:label             "Celery or Derivatives"@en ;
	skos:prefLabel         "CELERY" ;
	gs1:originalCodeValue  "BC" .

gs1:AllergenTypeCode-CEREALS_CONTAINING_GLUTEN
	rdf:type               gs1:AllergenTypeCode ;
	rdfs:comment           "Refers to the presence of Cereals containing gluten and their derivatives in the product, as listed in the regulations specified in AllergenSpecificationAgency and AllergenSpecificationName"@en ;
	rdfs:label             "Cereals Containing Gluten and Their Derivatives"@en ;
	skos:prefLabel         "CEREALS_CONTAINING_GLUTEN" ;
	gs1:originalCodeValue  "AW" .

gs1:AllergenTypeCode-CHAR
	rdf:type               gs1:AllergenTypeCode ;
	rdfs:comment           "Refers to the presence of Char and its derivatives in the product, as listed in the regulations specified in AllergenSpecificationAgency and AllergenSpecificationName."@en ;
	rdfs:label             "Char and its Derivatives"@en ;
	skos:prefLabel         "CHAR" ;
	gs1:originalCodeValue  "CHR" .

gs1:AllergenTypeCode-CHESTNUTS
	rdf:type               gs1:AllergenTypeCode ;
	rdfs:comment           "Refers to the presence of Chestnuts [Castanea spp. (Fagaceae)] and their derivatives in the product, as listed as listed in the regulations specified in AllergenSpecificationAgency and AllergenSpecificationName."@en ;
	rdfs:label             "Chestnuts and Their Derivatives"@en ;
	skos:prefLabel         "CHESTNUTS" ;
	gs1:originalCodeValue  "SN" .

gs1:AllergenTypeCode-CHICKEN_MEAT
	rdf:type               gs1:AllergenTypeCode ;
	rdfs:comment           "Refers to the presence of chicken meat and its derivative in the product, as listed in the regulations specified in AllergenSpecificationAgency and AllergenSpecificationName."@en ;
	rdfs:label             "Chicken Meat and its Derivatives"@en ;
	skos:prefLabel         "CHICKEN_MEAT" ;
	gs1:originalCodeValue  "CM" .

gs1:AllergenTypeCode-CHINQUAPINS
	rdf:type               gs1:AllergenTypeCode ;
	rdfs:comment           "Refers to the presence of Chinquapins [Castanea pumila (Fagaceae)] and their derivatives in the product, as listed as listed in the regulations specified in AllergenSpecificationAgency and AllergenSpecificationName."@en ;
	rdfs:label             "Chinquapins and Their Derivatives"@en ;
	skos:prefLabel         "CHINQUAPINS" ;
	gs1:originalCodeValue  "SF" .

gs1:AllergenTypeCode-CHUB
	rdf:type               gs1:AllergenTypeCode ;
	rdfs:comment           "Refers to the presence of Chub and its derivatives in the product, as listed in the regulations specified in AllergenSpecificationAgency and AllergenSpecificationName."@en ;
	rdfs:label             "Chub and its Derivatives"@en ;
	skos:prefLabel         "CHUB" ;
	gs1:originalCodeValue  "CHB" .

gs1:AllergenTypeCode-CINNAMAL
	rdf:type               gs1:AllergenTypeCode ;
	rdfs:comment           "Refers to the presence of Cinnamal as listed in the regulations specified in AllergenSpecificationAgency and AllergenSpecificationName."@en ;
	rdfs:label             "Cinnamal"@en ;
	skos:prefLabel         "CINNAMAL" ;
	gs1:originalCodeValue  "CL" .

gs1:AllergenTypeCode-CINNAMYL_ALCOHOL
	rdf:type               gs1:AllergenTypeCode ;
	rdfs:comment           "Refers to the presence of Cinnamyl Alcohol as listed in the regulations specified in AllergenSpecificationAgency and AllergenSpecificationName."@en ;
	rdfs:label             "Cinnamyl Alcohol"@en ;
	skos:prefLabel         "CINNAMYL_ALCOHOL" ;
	gs1:originalCodeValue  "CA" .

gs1:AllergenTypeCode-CISCO
	rdf:type               gs1:AllergenTypeCode ;
	rdfs:comment           "Refers to the presence of Cisco and its derivatives in the product, as listed in the regulations specified in AllergenSpecificationAgency and AllergenSpecificationName."@en ;
	rdfs:label             "Cisco and its Derivatives"@en ;
	skos:prefLabel         "CISCO" ;
	gs1:originalCodeValue  "CSC" .

gs1:AllergenTypeCode-CITRAL
	rdf:type               gs1:AllergenTypeCode ;
	rdfs:comment           "Refers to the presence of Citral as listed in the regulations specified in AllergenSpecificationAgency and AllergenSpecificationName."@en ;
	rdfs:label             "Citral"@en ;
	skos:prefLabel         "CITRAL" ;
	gs1:originalCodeValue  "CT" .

gs1:AllergenTypeCode-CITRONELLOL
	rdf:type               gs1:AllergenTypeCode ;
	rdfs:comment           "Refers to the presence of Citronellol as listed in the regulations specified in AllergenSpecificationAgency and AllergenSpecificationName."@en ;
	rdfs:label             "Citronellol"@en ;
	skos:prefLabel         "CITRONELLOL" ;
	gs1:originalCodeValue  "CN" .

gs1:AllergenTypeCode-CLAM
	rdf:type               gs1:AllergenTypeCode ;
	rdfs:comment           "Refers to the presence of Clam and its derivatives in the product, as listed in the regulations specified in AllergenSpecificationAgency and AllergenSpecificationName."@en ;
	rdfs:label             "Clam and its Derivatives"@en ;
	skos:prefLabel         "CLAM" ;
	gs1:originalCodeValue  "CLM" .

gs1:AllergenTypeCode-COCKLE
	rdf:type               gs1:AllergenTypeCode ;
	rdfs:comment           "Refers to the presence of Cockle and its derivatives in the product, as listed in the regulations specified in AllergenSpecificationAgency and AllergenSpecificationName."@en ;
	rdfs:label             "Cockle and its Derivatives"@en ;
	skos:prefLabel         "COCKLE" ;
	gs1:originalCodeValue  "COK" .

gs1:AllergenTypeCode-COCOA
	rdf:type               gs1:AllergenTypeCode ;
	rdfs:comment           "Refers to the presence of cocoa and their derivatives in the product, as listed in as listed in the regulations specified in AllergenSpecificationAgency and AllergenSpecificationName"@en ;
	rdfs:label             "Cocoa and Derivatives"@en ;
	skos:prefLabel         "COCOA" ;
	gs1:originalCodeValue  "NC" .

gs1:AllergenTypeCode-COCONUTS
	rdf:type               gs1:AllergenTypeCode ;
	rdfs:comment           "Refers to the presence of Coconuts [Cocos (Arecaceae)] and their derivatives in the product, as listed as listed in the regulations specified in AllergenSpecificationAgency and AllergenSpecificationName."@en ;
	rdfs:label             "Coconuts and Their Derivatives"@en ;
	skos:prefLabel         "COCONUTS" ;
	gs1:originalCodeValue  "SO" .

gs1:AllergenTypeCode-COD
	rdf:type               gs1:AllergenTypeCode ;
	rdfs:comment           "Refers to the presence of Cod and their derivatives in the product, as listed as listed in the regulations specified in AllergenSpecificationAgency and AllergenSpecificationName."@en ;
	rdfs:label             "Cod and its Derivatives"@en ;
	skos:prefLabel         "COD" ;
	gs1:originalCodeValue  "ADF" .

gs1:AllergenTypeCode-CONCH
	rdf:type               gs1:AllergenTypeCode ;
	rdfs:comment           "Refers to the presence of Conch and its derivatives in the product, as listed in the regulations specified in AllergenSpecificationAgency and AllergenSpecificationName."@en ;
	rdfs:label             "Conch and its Derivatives"@en ;
	skos:prefLabel         "CONCH" ;
	gs1:originalCodeValue  "CON" .

gs1:AllergenTypeCode-CORIANDER
	rdf:type               gs1:AllergenTypeCode ;
	rdfs:comment           "Refers to the presence of coriander and their derivatives in the product, as listed in as listed in the regulations specified in AllergenSpecificationAgency and AllergenSpecificationName"@en ;
	rdfs:label             "Coriander Derivatives"@en ;
	skos:prefLabel         "CORIANDER" ;
	gs1:originalCodeValue  "NK" .

gs1:AllergenTypeCode-CORN
	rdf:type               gs1:AllergenTypeCode ;
	rdfs:comment           "Refers to the presence of corn and their derivatives in the product, as listed in as listed in the regulations specified in AllergenSpecificationAgency and AllergenSpecificationName"@en ;
	rdfs:label             "Corn and Derivatives"@en ;
	skos:prefLabel         "CORN" ;
	gs1:originalCodeValue  "NM" .

gs1:AllergenTypeCode-COTTON_SEEDS
	rdf:type               gs1:AllergenTypeCode ;
	rdfs:comment           "Refers to the presence of Cotton Seeds or their derivatives in the product as listed in the regulations specified in AllergenSpecificationAgency and AllergenSpecificationName"@en ;
	rdfs:label             "Cotton Seeds and Their Derivatives"@en ;
	skos:prefLabel         "COTTON_SEEDS" ;
	gs1:originalCodeValue  "CS" .

gs1:AllergenTypeCode-COUMARIN
	rdf:type               gs1:AllergenTypeCode ;
	rdfs:comment           "Refers to the presence of Coumarin as listed in the regulations specified in AllergenSpecificationAgency and AllergenSpecificationName."@en ;
	rdfs:label             "Coumarin"@en ;
	skos:prefLabel         "COUMARIN" ;
	gs1:originalCodeValue  "CO" .

gs1:AllergenTypeCode-CRAB
	rdf:type               gs1:AllergenTypeCode ;
	rdfs:comment           "Refers to the presence of Crab and their derivatives in the product, as listed as listed in the regulations specified in AllergenSpecificationAgency and AllergenSpecificationName."@en ;
	rdfs:label             "Crab and its Derivatives"@en ;
	skos:prefLabel         "CRAB" ;
	gs1:originalCodeValue  "ABG" .

gs1:AllergenTypeCode-CRAWFISH
	rdf:type               gs1:AllergenTypeCode ;
	rdfs:comment           "Refers to the presence of Crawfish and their derivatives in the product, as listed as listed in the regulations specified in AllergenSpecificationAgency and AllergenSpecificationName."@en ;
	rdfs:label             "Crawfish and its Derivatives"@en ;
	skos:prefLabel         "CRAWFISH" ;
	gs1:originalCodeValue  "ABH" .

gs1:AllergenTypeCode-CRUSTACEANS
	rdf:type               gs1:AllergenTypeCode ;
	rdfs:comment           "Refers to the presence of Crustaceans and their derivatives in the product, as listed as listed in the regulations specified in AllergenSpecificationAgency and AllergenSpecificationName"@en ;
	rdfs:label             "Crustaceans and Their Derivatives"@en ;
	skos:prefLabel         "CRUSTACEANS" ;
	gs1:originalCodeValue  "AC" .

gs1:AllergenTypeCode-D-LIMONENE
	rdf:type               gs1:AllergenTypeCode ;
	rdfs:comment           "Refers to the presence of d-Limonene as listed in the regulations specified in AllergenSpecificationAgency and AllergenSpecificationName"@en ;
	rdfs:label             "d-Limonene"@en ;
	skos:prefLabel         "D-LIMONENE" ;
	gs1:originalCodeValue  "BO" .

gs1:AllergenTypeCode-DIAMINOPHENOLS
	rdf:type               gs1:AllergenTypeCode ;
	rdfs:comment           "Refers to the presence of Diaminophenols as listed in the regulations specified in AllergenSpecificationAgency and AllergenSpecificationName."@en ;
	rdfs:label             "Diaminophenols"@en ;
	skos:prefLabel         "DIAMINOPHENOLS" ;
	gs1:originalCodeValue  "DP" .

gs1:AllergenTypeCode-EEL
	rdf:type               gs1:AllergenTypeCode ;
	rdfs:comment           "Refers to the presence of Eel and its derivatives in the product, as listed in the regulations specified in AllergenSpecificationAgency and AllergenSpecificationName."@en ;
	rdfs:label             "Eel and its Derivatives"@en ;
	skos:prefLabel         "EEL" ;
	gs1:originalCodeValue  "EEL" .

gs1:AllergenTypeCode-EGGS
	rdf:type               gs1:AllergenTypeCode ;
	rdfs:comment           "Refers to the presence of eggs and their derivatives in the product, as listed as listed in the regulations specified in AllergenSpecificationAgency and AllergenSpecificationName"@en ;
	rdfs:label             "Eggs and Their Derivatives"@en ;
	skos:prefLabel         "EGGS" ;
	gs1:originalCodeValue  "AE" .

gs1:AllergenTypeCode-EUGENOL
	rdf:type               gs1:AllergenTypeCode ;
	rdfs:comment           "Refers to the presence of Eugenol as listed in the regulations specified in AllergenSpecificationAgency and AllergenSpecificationName."@en ;
	rdfs:label             "Eugenol"@en ;
	skos:prefLabel         "EUGENOL" ;
	gs1:originalCodeValue  "EG" .

gs1:AllergenTypeCode-EVERNIA_FURFURACEA
	rdf:type               gs1:AllergenTypeCode ;
	rdfs:comment           "Refers to the presence of Evernia Furfuracea as listed in the regulations specified in AllergenSpecificationAgency and AllergenSpecificationName."@en ;
	rdfs:label             "Evernia Furfuracea"@en ;
	skos:prefLabel         "EVERNIA_FURFURACEA" ;
	gs1:originalCodeValue  "EV" .

gs1:AllergenTypeCode-EVERNIA_PRUNASTRI
	rdf:type               gs1:AllergenTypeCode ;
	rdfs:comment           "Refers to the presence of Evernia Prunastri as listed in the regulations specified in AllergenSpecificationAgency and AllergenSpecificationName."@en ;
	rdfs:label             "Evernia Prunastri"@en ;
	skos:prefLabel         "EVERNIA_PRUNASTRI" ;
	gs1:originalCodeValue  "EP" .

gs1:AllergenTypeCode-FARNESOL
	rdf:type               gs1:AllergenTypeCode ;
	rdfs:comment           "Refers to the presence of Farnesol as listed in the regulations specified in AllergenSpecificationAgency and AllergenSpecificationName."@en ;
	rdfs:label             "Farnesol"@en ;
	skos:prefLabel         "FARNESOL" ;
	gs1:originalCodeValue  "FA" .

gs1:AllergenTypeCode-FISH
	rdf:type               gs1:AllergenTypeCode ;
	rdfs:comment           "Refers to the presence of Fish and their derivatives in the product, as listed in as listed in the regulations specified in AllergenSpecificationAgency and AllergenSpecificationName"@en ;
	rdfs:label             "Fish and Their Derivatives"@en ;
	skos:prefLabel         "FISH" ;
	gs1:originalCodeValue  "AF" .

gs1:AllergenTypeCode-FLOUNDER
	rdf:type               gs1:AllergenTypeCode ;
	rdfs:comment           "Refers to the presence of Flounder and their derivatives in the product, as listed as listed in the regulations specified in AllergenSpecificationAgency and AllergenSpecificationName."@en ;
	rdfs:label             "Flounder and its Derivatives"@en ;
	skos:prefLabel         "FLOUNDER" ;
	gs1:originalCodeValue  "ADG" .

gs1:AllergenTypeCode-GERANIOL
	rdf:type               gs1:AllergenTypeCode ;
	rdfs:comment           "Refers to the presence of Geraniol as listed in the regulations specified in AllergenSpecificationAgency and AllergenSpecificationName."@en ;
	rdfs:label             "Geraniol"@en ;
	skos:prefLabel         "GERANIOL" ;
	gs1:originalCodeValue  "GE" .

gs1:AllergenTypeCode-GINKGO_NUTS
	rdf:type               gs1:AllergenTypeCode ;
	rdfs:comment           "Refers to the presence of Ginkgo nuts [Ginkgo biloba L. (Ginkgoaceae)] and their derivatives in the product, as listed as listed in the regulations specified in AllergenSpecificationAgency and AllergenSpecificationName."@en ;
	rdfs:label             "Ginkgo Nuts and Their Derivatives"@en ;
	skos:prefLabel         "GINKGO_NUTS" ;
	gs1:originalCodeValue  "SG" .

gs1:AllergenTypeCode-GLUTAMATE
	rdf:type               gs1:AllergenTypeCode ;
	rdfs:comment           "Refers to the presence of glutamate and its derivative in the product, as listed in the regulations specified in AllergenSpecificationAgency and AllergenSpecificationName."@en ;
	rdfs:label             "Glutamate and Their Derivatives"@en ;
	skos:prefLabel         "GLUTAMATE" ;
	gs1:originalCodeValue  "GL" .

gs1:AllergenTypeCode-GLUTEN
	rdf:type               gs1:AllergenTypeCode ;
	rdfs:comment           "Refers to the presense of other gluten containing grain and gluten containing grain products as listed in the regulations specified in AllergenSpecificationAgency and AllergenSpecificationName."@en ;
	rdfs:label             "Gluten"@en ;
	skos:prefLabel         "GLUTEN" ;
	gs1:originalCodeValue  "AX" .

gs1:AllergenTypeCode-GROUPER
	rdf:type               gs1:AllergenTypeCode ;
	rdfs:comment           "Refers to the presence of Grouper and their derivatives in the product, as listed as listed in the regulations specified in AllergenSpecificationAgency and AllergenSpecificationName."@en ;
	rdfs:label             "Grouper and its Derivatives"@en ;
	skos:prefLabel         "GROUPER" ;
	gs1:originalCodeValue  "ADH" .

gs1:AllergenTypeCode-HADDOCK
	rdf:type               gs1:AllergenTypeCode ;
	rdfs:comment           "Refers to the presence of Haddock and their derivatives in the product, as listed as listed in the regulations specified in AllergenSpecificationAgency and AllergenSpecificationName."@en ;
	rdfs:label             "Haddock and its Derivatives"@en ;
	skos:prefLabel         "HADDOCK" ;
	gs1:originalCodeValue  "ADI" .

gs1:AllergenTypeCode-HAKE
	rdf:type               gs1:AllergenTypeCode ;
	rdfs:comment           "Refers to the presence of Hake and their derivatives in the product, as listed as listed in the regulations specified in AllergenSpecificationAgency and AllergenSpecificationName."@en ;
	rdfs:label             "Hake and its Derivatives"@en ;
	skos:prefLabel         "HAKE" ;
	gs1:originalCodeValue  "ADJ" .

gs1:AllergenTypeCode-HALIBUT
	rdf:type               gs1:AllergenTypeCode ;
	rdfs:comment           "Refers to the presence of Halibut and their derivatives in the product, as listed as listed in the regulations specified in AllergenSpecificationAgency and AllergenSpecificationName."@en ;
	rdfs:label             "Halibut and its Derivatives"@en ;
	skos:prefLabel         "HALIBUT" ;
	gs1:originalCodeValue  "ADK" .

gs1:AllergenTypeCode-HAZELNUTS
	rdf:type               gs1:AllergenTypeCode ;
	rdfs:comment           "Refers to the presence of hazelnut and hazelnut products as listed in the regulations specified in AllergenSpecificationAgency and AllergenSpecificationName."@en ;
	rdfs:label             "Hazelnut and Hazelnut Products"@en ;
	skos:prefLabel         "HAZELNUTS" ;
	gs1:originalCodeValue  "SH" .

gs1:AllergenTypeCode-HC_BLUE_NO_11
	rdf:type               gs1:AllergenTypeCode ;
	rdfs:comment           "Refers to the presence of HC Blue No 11 as listed in the regulations specified in AllergenSpecificationAgency and AllergenSpecificationName."@en ;
	rdfs:label             "HC Blue No 11"@en ;
	skos:prefLabel         "HC_BLUE_NO_11" ;
	gs1:originalCodeValue  "HD" .

gs1:AllergenTypeCode-HC_BLUE_NO_12
	rdf:type               gs1:AllergenTypeCode ;
	rdfs:comment           "Refers to the presence of HC Blue No 12 as listed in the regulations specified in AllergenSpecificationAgency and AllergenSpecificationName."@en ;
	rdfs:label             "HC Blue No 12"@en ;
	skos:prefLabel         "HC_BLUE_NO_12" ;
	gs1:originalCodeValue  "HB" .

gs1:AllergenTypeCode-HERRING
	rdf:type               gs1:AllergenTypeCode ;
	rdfs:comment           "Refers to the presence of Herring and their derivatives in the product, as listed as listed in the regulations specified in AllergenSpecificationAgency and AllergenSpecificationName."@en ;
	rdfs:label             "Herring and its Derivatives"@en ;
	skos:prefLabel         "HERRING" ;
	gs1:originalCodeValue  "ADL" .

gs1:AllergenTypeCode-HEXYL_CINNAMAL
	rdf:type               gs1:AllergenTypeCode ;
	rdfs:comment           "Refers to the presence of Hexyl Cinnamal as listed in the regulations specified in AllergenSpecificationAgency and AllergenSpecificationName."@en ;
	rdfs:label             "Hexyl Cinnamal"@en ;
	skos:prefLabel         "HEXYL_CINNAMAL" ;
	gs1:originalCodeValue  "HX" .

gs1:AllergenTypeCode-HICKORY_NUTS
	rdf:type               gs1:AllergenTypeCode ;
	rdfs:comment           "Refers to the presence of hickory nuts [Carya spp. (Junglandacease)] and their derivatives in the product, as listed as listed in the regulations specified in AllergenSpecificationAgency and AllergenSpecificationName."@en ;
	rdfs:label             "Hickory Nuts and Their Derivatives"@en ;
	skos:prefLabel         "HICKORY_NUTS" ;
	gs1:originalCodeValue  "SI" .

gs1:AllergenTypeCode-HYDROXYBENZOMORPHOLINE
	rdf:type               gs1:AllergenTypeCode ;
	rdfs:comment           "Refers to the presence of Hydroxybenzomorpholine as listed in the regulations specified in AllergenSpecificationAgency and AllergenSpecificationName."@en ;
	rdfs:label             "Hydroxybenzomorpholine"@en ;
	skos:prefLabel         "HYDROXYBENZOMORPHOLINE" ;
	gs1:originalCodeValue  "HE" .

gs1:AllergenTypeCode-HYDROXYCITRONELLAL
	rdf:type               gs1:AllergenTypeCode ;
	rdfs:comment           "Refers to the presence of Hydroxycitronellal as listed in the regulations specified in AllergenSpecificationAgency and AllergenSpecificationName."@en ;
	rdfs:label             "Hydroxycitronellal"@en ;
	skos:prefLabel         "HYDROXYCITRONELLAL" ;
	gs1:originalCodeValue  "HY" .

gs1:AllergenTypeCode-HYDROXYETHYL-2-NITRO-P-TOLUIDINE
	rdf:type               gs1:AllergenTypeCode ;
	rdfs:comment           "Refers to the presence of Hydroxyethyl-2-nitro-p-toluidine as listed in the regulations specified in AllergenSpecificationAgency and AllergenSpecificationName."@en ;
	rdfs:label             "Hydroxyethyl-2-nitro-p-toluidine"@en ;
	skos:prefLabel         "HYDROXYETHYL-2-NITRO-P-TOLUIDINE" ;
	gs1:originalCodeValue  "HN" .

gs1:AllergenTypeCode-HYDROXYISOHEXYL_3-CYCLOHEXENE_CARBOXALDEHYDE_ISOEUGENOL_LIMONENE_LINAL
	rdf:type               gs1:AllergenTypeCode ;
	rdfs:comment           "Refers to the presence of Hydroxyisohexyl 3-Cyclohexene Carboxaldehyde Isoeugenol Limonene Linal as listed in the regulations specified in AllergenSpecificationAgency and llergenSpecificationName."@en ;
	rdfs:label             "Hydroxyisohexyl 3-Cyclohexene Carboxaldehyde Isoeugenol Limonene Linal"@en ;
	skos:prefLabel         "HYDROXYISOHEXYL_3-CYCLOHEXENE_CARBOXALDEHYDE_ISOEUGENOL_LIMONENE_LINAL" ;
	gs1:originalCodeValue  "HC" .

gs1:AllergenTypeCode-ISOEUGENOL
	rdf:type               gs1:AllergenTypeCode ;
	rdfs:comment           "Refers to the presence of Isoeugenol as listed in the regulations specified in AllergenSpecificationAgency and AllergenSpecificationName"@en ;
	rdfs:label             "Isoeugenol"@en ;
	skos:prefLabel         "ISOEUGENOL" ;
	gs1:originalCodeValue  "BN" .

gs1:AllergenTypeCode-KAMUT
	rdf:type               gs1:AllergenTypeCode ;
	rdfs:comment           "Refers to the presence of kamut and kamut products (glutencontaining grain) as listed in the regulations specified in AllergenSpecificationAgency and AllergenSpecificationName."@en ;
	rdfs:label             "Kamut and Kamut Products"@en ;
	skos:prefLabel         "KAMUT" ;
	gs1:originalCodeValue  "GK" .

gs1:AllergenTypeCode-KRILL
	rdf:type               gs1:AllergenTypeCode ;
	rdfs:comment           "Refers to the presence of Krill and their derivatives in the product, as listed as listed in the regulations specified in AllergenSpecificationAgency and AllergenSpecificationName."@en ;
	rdfs:label             "Krill and its Derivatives"@en ;
	skos:prefLabel         "KRILL" ;
	gs1:originalCodeValue  "ABI" .

gs1:AllergenTypeCode-LACTOSE
	rdf:type               gs1:AllergenTypeCode ;
	rdfs:comment           "Refers to the presence of lactose as listed in the regulations specified in AllergenSpecificationAgency and AllergenSpecificationName."@en ;
	rdfs:label             "Lactose"@en ;
	skos:prefLabel         "LACTOSE" ;
	gs1:originalCodeValue  "ML" .

gs1:AllergenTypeCode-LAND
	rdf:type               gs1:AllergenTypeCode ;
	rdfs:comment           "Refers to the presence of Land and sea snails (Escargot) and its derivatives in the product, as listed in the regulations specified in AllergenSpecificationAgency and AllergenSpecificationName."@en ;
	rdfs:label             "Land and sea snails (Escargot) and its Derivatives"@en ;
	skos:prefLabel         "LAND" ;
	gs1:originalCodeValue  "LSN" .

gs1:AllergenTypeCode-LICHEE_NUTS
	rdf:type               gs1:AllergenTypeCode ;
	rdfs:comment           "Refers to the presence of Lichee nuts [Litchi chinensis Sonn. (Sapindaceae)] and their derivatives in the product, as listed as listed in the regulations specified in AllergenSpecificationAgency and AllergenSpecificationName."@en ;
	rdfs:label             "Lichee Nuts and Their Derivatives"@en ;
	skos:prefLabel         "LICHEE_NUTS" ;
	gs1:originalCodeValue  "SL" .

gs1:AllergenTypeCode-LIMPETS
	rdf:type               gs1:AllergenTypeCode ;
	rdfs:comment           "Refers to the presence of Limpets and its derivatives in the product, as listed in the regulations specified in AllergenSpecificationAgency and AllergenSpecificationName."@en ;
	rdfs:label             "Limpets and its Derivatives"@en ;
	skos:prefLabel         "LIMPETS" ;
	gs1:originalCodeValue  "LMT" .

gs1:AllergenTypeCode-LINALOOL
	rdf:type               gs1:AllergenTypeCode ;
	rdfs:comment           "Refers to the presence of Linalool as listed in the regulations specified in AllergenSpecificationAgency and AllergenSpecificationName"@en ;
	rdfs:label             "Linalool"@en ;
	skos:prefLabel         "LINALOOL" ;
	gs1:originalCodeValue  "BP" .

gs1:AllergenTypeCode-LOBSTER
	rdf:type               gs1:AllergenTypeCode ;
	rdfs:comment           "Refers to the presence of Lobster and their derivatives in the product, as listed as listed in the regulations specified in AllergenSpecificationAgency and AllergenSpecificationName."@en ;
	rdfs:label             "Lobster and its Derivatives"@en ;
	skos:prefLabel         "LOBSTER" ;
	gs1:originalCodeValue  "ABJ" .

gs1:AllergenTypeCode-LUPINE
	rdf:type               gs1:AllergenTypeCode ;
	rdfs:comment           "Refers to the presence of Lupine and their derivatives in the product, as listed in as listed in the regulations specified in AllergenSpecificationAgency and AllergenSpecificationName"@en ;
	rdfs:label             "Lupine and Derivatives"@en ;
	skos:prefLabel         "LUPINE" ;
	gs1:originalCodeValue  "NL" .

gs1:AllergenTypeCode-MACADAMIA_NUTS
	rdf:type               gs1:AllergenTypeCode ;
	rdfs:comment           "Refers to the presence of macadamia nut and macadamia nut products as listed in the regulations specified in AllergenSpecificationAgency and AllergenSpecificationName"@en ;
	rdfs:label             "Macadamia Nut and Macadamia Nut Products"@en ;
	skos:prefLabel         "MACADAMIA_NUTS" ;
	gs1:originalCodeValue  "SM" .

gs1:AllergenTypeCode-MACKEREL
	rdf:type               gs1:AllergenTypeCode ;
	rdfs:comment           "Refers to the presence of Mackerel and its derivatives in the product, as listed in the regulations specified in AllergenSpecificationAgency and AllergenSpecificationName."@en ;
	rdfs:label             "Mackerel and its Derivatives"@en ;
	skos:prefLabel         "MACKEREL" ;
	gs1:originalCodeValue  "MAC" .

gs1:AllergenTypeCode-MAHI_MAHI
	rdf:type               gs1:AllergenTypeCode ;
	rdfs:comment           "Refers to the presence of Mahi Mahi and their derivatives in the product, as listed as listed in the regulations specified in AllergenSpecificationAgency and AllergenSpecificationName."@en ;
	rdfs:label             "Mahi mahi and its Derivatives"@en ;
	skos:prefLabel         "MAHI_MAHI" ;
	gs1:originalCodeValue  "ADM" .

gs1:AllergenTypeCode-MARLIN
	rdf:type               gs1:AllergenTypeCode ;
	rdfs:comment           "Refers to the presence of Marlin and its derivatives in the product, as listed in the regulations specified in AllergenSpecificationAgency and AllergenSpecificationName."@en ;
	rdfs:label             "Marlin and its Derivatives"@en ;
	skos:prefLabel         "MARLIN" ;
	gs1:originalCodeValue  "MAL" .

gs1:AllergenTypeCode-MELATONIN
	rdf:type               gs1:AllergenTypeCode ;
	rdfs:comment           "Refers to the presence of Melatonin, a hormone secreted by the pineal gland that inhibits melanin formation and is thought to be concerned with regulating the reproductive cycle."@en ;
	rdfs:label             "Melatonin"@en ;
	skos:prefLabel         "MELATONIN" ;
	gs1:originalCodeValue  "MM" .

gs1:AllergenTypeCode-METHYL_2_OCTYNOATE
	rdf:type               gs1:AllergenTypeCode ;
	rdfs:comment           "Refers to the presence of Methyl 2-Octynoate as listed in the regulations specified in AllergenSpecificationAgency and AllergenSpecificationName."@en ;
	rdfs:label             "Methyl 2-Octynoate"@en ;
	skos:prefLabel         "METHYL_2_OCTYNOATE" ;
	gs1:originalCodeValue  "MO" .

gs1:AllergenTypeCode-METHYL_HEPTIN_CARBONATE
	rdf:type               gs1:AllergenTypeCode ;
	rdfs:comment           "Refers to the presence of Methyl heptin carbonate as listed in the regulations specified in AllergenSpecificationAgency and AllergenSpecificationName"@en ;
	rdfs:label             "Methyl Heptin Carbonate"@en ;
	skos:prefLabel         "METHYL_HEPTIN_CARBONATE" ;
	gs1:originalCodeValue  "BQ" .

gs1:AllergenTypeCode-MILK
	rdf:type               gs1:AllergenTypeCode ;
	rdfs:comment           "Refers to the presence of milk and their derivatives in the product, as listed in as listed in the regulations specified in AllergenSpecificationAgency and AllergenSpecificationName"@en ;
	rdfs:label             "Milk and Derivatives"@en ;
	skos:prefLabel         "MILK" ;
	gs1:originalCodeValue  "AM" .

gs1:AllergenTypeCode-MOLLUSCS
	rdf:type               gs1:AllergenTypeCode ;
	rdfs:comment           "Refers to the presence of molluscs and their derivatives in the product, as listed in as listed in the regulations specified in AllergenSpecificationAgency and AllergenSpecificationName"@en ;
	rdfs:label             "Molluscs and Their Derivatives"@en ;
	skos:prefLabel         "MOLLUSCS" ;
	gs1:originalCodeValue  "UM" .

gs1:AllergenTypeCode-MUSSELS
	rdf:type               gs1:AllergenTypeCode ;
	rdfs:comment           "Refers to the presence of Mussels and its derivatives in the product, as listed in the regulations specified in AllergenSpecificationAgency and AllergenSpecificationName."@en ;
	rdfs:label             "Mussels and its Derivatives"@en ;
	skos:prefLabel         "MUSSELS" ;
	gs1:originalCodeValue  "MSS" .

gs1:AllergenTypeCode-MUSTARD
	rdf:type               gs1:AllergenTypeCode ;
	rdfs:comment           "Refers to the presence of mustard or their derivatives in the product, as listed in as listed in the regulations specified in AllergenSpecificationAgency and AllergenSpecificationName"@en ;
	rdfs:label             "Mustard and Derivatives"@en ;
	skos:prefLabel         "MUSTARD" ;
	gs1:originalCodeValue  "BM" .

gs1:AllergenTypeCode-NO_DECLARED_ALLERGENS
	rdf:type               gs1:AllergenTypeCode ;
	rdfs:comment           "Does not contain declaration obligatory allergens as listed in the regulations specified in AllergenSpecificationAgency and AllergenSpecificationName."@en ;
	rdfs:label             "No Declaration Obligatory Allergens"@en ;
	skos:prefLabel         "NO_DECLARED_ALLERGENS" ;
	gs1:originalCodeValue  "X99" .

gs1:AllergenTypeCode-OAT
	rdf:type               gs1:AllergenTypeCode ;
	rdfs:comment           "Refers to the presence of oat and oat products (gluten containing grain) as listed in the regulations specified in AllergenSpecificationAgency and AllergenSpecificationName."@en ;
	rdfs:label             "Oat and Oat Products"@en ;
	skos:prefLabel         "OAT" ;
	gs1:originalCodeValue  "GO" .

gs1:AllergenTypeCode-OCTOPUS
	rdf:type               gs1:AllergenTypeCode ;
	rdfs:comment           "Refers to the presence of Octopus and its derivatives in the product, as listed in the regulations specified in AllergenSpecificationAgency and AllergenSpecificationName."@en ;
	rdfs:label             "Octopus and its Derivatives"@en ;
	skos:prefLabel         "OCTOPUS" ;
	gs1:originalCodeValue  "OCT" .

gs1:AllergenTypeCode-ORANGE_ROUGHY
	rdf:type               gs1:AllergenTypeCode ;
	rdfs:comment           "Refers to the presence of Orange roughy and its derivatives in the product, as listed in the regulations specified in AllergenSpecificationAgency and AllergenSpecificationName."@en ;
	rdfs:label             "Orange roughy and its Derivatives"@en ;
	skos:prefLabel         "ORANGE_ROUGHY" ;
	gs1:originalCodeValue  "ORR" .

gs1:AllergenTypeCode-OYSTERS
	rdf:type               gs1:AllergenTypeCode ;
	rdfs:comment           "Refers to the presence Oysters and its derivatives in the product, as listed in the regulations specified in AllergenSpecificationAgency and AllergenSpecificationName."@en ;
	rdfs:label             "Oysters and its Derivatives"@en ;
	skos:prefLabel         "OYSTERS" ;
	gs1:originalCodeValue  "OYS" .

gs1:AllergenTypeCode-P-METHYLAMINOPHENOL
	rdf:type               gs1:AllergenTypeCode ;
	rdfs:comment           "Refers to the presence of p-Methylaminophenol as listed in the regulations specified in AllergenSpecificationAgency and AllergenSpecificationName."@en ;
	rdfs:label             "p-Methylaminophenol"@en ;
	skos:prefLabel         "P-METHYLAMINOPHENOL" ;
	gs1:originalCodeValue  "PM" .

gs1:AllergenTypeCode-P-PHENYLENEDIAMINE
	rdf:type               gs1:AllergenTypeCode ;
	rdfs:comment           "Refers to the presence of p-Phenylenediamine in the product as listed in the regulations specified in AllergenSpecificationAgency and AllergenSpecificationName."@en ;
	rdfs:label             "p-Phenylenediamine"@en ;
	skos:prefLabel         "P-PHENYLENEDIAMINE" ;
	gs1:originalCodeValue  "PP" .

gs1:AllergenTypeCode-PEANUTS
	rdf:type               gs1:AllergenTypeCode ;
	rdfs:comment           "Refers to the presence of peanuts and their derivatives in the product, as listed in as listed in the regulations specified in AllergenSpecificationAgency and AllergenSpecificationName"@en ;
	rdfs:label             "Peanuts and Their Derivatives"@en ;
	skos:prefLabel         "PEANUTS" ;
	gs1:originalCodeValue  "AP" .

gs1:AllergenTypeCode-PEAS
	rdf:type               gs1:AllergenTypeCode ;
	rdfs:comment           "Refers to the presence of peas and pea products as listed in the regulations specified in AllergenSpecificationAgency and AllergenSpecificationName."@en ;
	rdfs:label             "Peas and Pea Products"@en ;
	skos:prefLabel         "PEAS" ;
	gs1:originalCodeValue  "NE" .

gs1:AllergenTypeCode-PECAN_NUTS
	rdf:type               gs1:AllergenTypeCode ;
	rdfs:comment           "Refers to the presence of pecan nut and pecan nut products as listed in the regulations specified in AllergenSpecificationAgency and AllergenSpecificationName."@en ;
	rdfs:label             "Pecan Nut and Pecan Nut"@en ;
	skos:prefLabel         "PECAN_NUTS" ;
	gs1:originalCodeValue  "SP" .

gs1:AllergenTypeCode-PERCH
	rdf:type               gs1:AllergenTypeCode ;
	rdfs:comment           "Refers to the presence of Perch and their derivatives in the product, as listed as listed in the regulations specified in AllergenSpecificationAgency and AllergenSpecificationName."@en ;
	rdfs:label             "Perch and its Derivatives"@en ;
	skos:prefLabel         "PERCH" ;
	gs1:originalCodeValue  "ANO" .

gs1:AllergenTypeCode-PERIWINKLE
	rdf:type               gs1:AllergenTypeCode ;
	rdfs:comment           "Refers to the presence of Periwinkle and its derivatives in the product, as listed in the regulations specified in AllergenSpecificationAgency and AllergenSpecificationName."@en ;
	rdfs:label             "Periwinkle and its Derivatives"@en ;
	skos:prefLabel         "PERIWINKLE" ;
	gs1:originalCodeValue  "PER" .

gs1:AllergenTypeCode-PIKE
	rdf:type               gs1:AllergenTypeCode ;
	rdfs:comment           "Refers to the presence of Pike and their derivatives in the product, as listed as listed in the regulations specified in AllergenSpecificationAgency and AllergenSpecificationName."@en ;
	rdfs:label             "Pike and its Derivatives"@en ;
	skos:prefLabel         "PIKE" ;
	gs1:originalCodeValue  "ADP" .

gs1:AllergenTypeCode-PILI_NUTS
	rdf:type               gs1:AllergenTypeCode ;
	rdfs:comment           "Refers to the presence of Pili nuts [Canarium ovatum (Burseraceae)] and their derivatives in the product, as listed as listed in the regulations specified in AllergenSpecificationAgency and AllergenSpecificationName."@en ;
	rdfs:label             "Pili Nuts and Their Derivatives"@en ;
	skos:prefLabel         "PILI_NUTS" ;
	gs1:originalCodeValue  "SK" .

gs1:AllergenTypeCode-PINE_NUTS
	rdf:type               gs1:AllergenTypeCode ;
	rdfs:comment           "Refers to the presence of Pine Nuts and their derivatives as listed in the regulations specified in AllergenSpecificationAgency and AllergenSpecificationName."@en ;
	rdfs:label             "Pine Nut and Their Derivatives"@en ;
	skos:prefLabel         "PINE_NUTS" ;
	gs1:originalCodeValue  "PN" .

gs1:AllergenTypeCode-PISTACHIOS
	rdf:type               gs1:AllergenTypeCode ;
	rdfs:comment           "Refers to the presence of pistachio and pistachio products as listed in the regulations specified in AllergenSpecificationAgency and AllergenSpecificationName."@en ;
	rdfs:label             "Pistachio and Pistachio Products"@en ;
	skos:prefLabel         "PISTACHIOS" ;
	gs1:originalCodeValue  "ST" .

gs1:AllergenTypeCode-PLAICE
	rdf:type               gs1:AllergenTypeCode ;
	rdfs:comment           "Refers to the presence of Plaice and its derivatives in the product, as listed in the regulations specified in AllergenSpecificationAgency and AllergenSpecificationName."@en ;
	rdfs:label             "Plaice and its Derivatives"@en ;
	skos:prefLabel         "PLAICE" ;
	gs1:originalCodeValue  "PLC" .

gs1:AllergenTypeCode-POD_FRUITS
	rdf:type               gs1:AllergenTypeCode ;
	rdfs:comment           "Refers to the presence of pod fruits and their derivatives in the product, as listed in as listed in the regulations specified in AllergenSpecificationAgency and AllergenSpecificationName"@en ;
	rdfs:label             "Pod Fruits Derivatives"@en ;
	skos:prefLabel         "POD_FRUITS" ;
	gs1:originalCodeValue  "NP" .

gs1:AllergenTypeCode-POLLOCK
	rdf:type               gs1:AllergenTypeCode ;
	rdfs:comment           "Refers to the presence of Pollock and their derivatives in the product, as listed as listed in the regulations specified in AllergenSpecificationAgency and AllergenSpecificationName."@en ;
	rdfs:label             "Pollock and its Derivatives"@en ;
	skos:prefLabel         "POLLOCK" ;
	gs1:originalCodeValue  "ADQ" .

gs1:AllergenTypeCode-POMPANO
	rdf:type               gs1:AllergenTypeCode ;
	rdfs:comment           "Refers to the presence of Pompano and its derivatives in the product, as listed in the regulations specified in AllergenSpecificationAgency and AllergenSpecificationName."@en ;
	rdfs:label             "Pompano and its Derivatives"@en ;
	skos:prefLabel         "POMPANO" ;
	gs1:originalCodeValue  "POM" .

gs1:AllergenTypeCode-POPPY_SEEDS
	rdf:type               gs1:AllergenTypeCode ;
	rdfs:comment           "Refers to the presence of Poppy Seeds or their derivatives in the product as listed in the regulations specified in AllergenSpecificationAgency and AllergenSpecificationName."@en ;
	rdfs:label             "Poppy Seeds and Their Derivatives"@en ;
	skos:prefLabel         "POPPY_SEEDS" ;
	gs1:originalCodeValue  "PS" .

gs1:AllergenTypeCode-PORGY
	rdf:type               gs1:AllergenTypeCode ;
	rdfs:comment           "Refers to the presence of Porgy and its derivatives in the product, as listed in the regulations specified in AllergenSpecificationAgency and AllergenSpecificationName."@en ;
	rdfs:label             "Porgy and its Derivatives"@en ;
	skos:prefLabel         "PORGY" ;
	gs1:originalCodeValue  "PRG" .

gs1:AllergenTypeCode-PORK
	rdf:type               gs1:AllergenTypeCode ;
	rdfs:comment           "Refers to the presence of pork and its derivative in the product, as listed in the regulations specified in AllergenSpecificationAgency and AllergenSpecificationName."@en ;
	rdfs:label             "Pork and its Derivatives"@en ;
	skos:prefLabel         "PORK" ;
	gs1:originalCodeValue  "PO" .

gs1:AllergenTypeCode-PRAWNS
	rdf:type               gs1:AllergenTypeCode ;
	rdfs:comment           "Refers to the presence of Prawns and their derivatives in the product, as listed as listed in the regulations specified in AllergenSpecificationAgency and AllergenSpecificationName."@en ;
	rdfs:label             "Prawns and their Derivatives"@en ;
	skos:prefLabel         "PRAWNS" ;
	gs1:originalCodeValue  "ABK" .

gs1:AllergenTypeCode-PULSES
	rdf:type               gs1:AllergenTypeCode ;
	rdfs:comment           "Refers to the presence of pulses. An annual leguminous crop yielding from one to twelve seeds of variable size, shape, and colour within a pod. Pulses are used for food and animal feed. The term 'pulse', as used by the Food and Agricultural Organization (FAO), is reserved for crops harvested solely for the dry seed. This excludes green beans and green peas, which are considered vegetable crops. Also excluded are crops that are mainly grown for oil extraction"@en ;
	rdfs:label             "Pulses"@en ;
	skos:prefLabel         "PULSES" ;
	gs1:originalCodeValue  "SX" .

gs1:AllergenTypeCode-QUAHAUGS
	rdf:type               gs1:AllergenTypeCode ;
	rdfs:comment           "Refers to the presence of Quahaugs and its derivatives in the product, listed as listed in the regulations specified in AllergenSpecificationAgency and AllergenSpecificationName."@en ;
	rdfs:label             "Quahaugs and its Derivatives"@en ;
	skos:prefLabel         "QUAHAUGS" ;
	gs1:originalCodeValue  "QUA" .

gs1:AllergenTypeCode-QUEENSLAND_NUTS
	rdf:type               gs1:AllergenTypeCode ;
	rdfs:comment           "Refers to the presence of queensland nut and queensland nut products as listed in the regulations specified in AllergenSpecificationAgency and AllergenSpecificationName."@en ;
	rdfs:label             "Queensland Nut and Queensland Nut Products"@en ;
	skos:prefLabel         "QUEENSLAND_NUTS" ;
	gs1:originalCodeValue  "SQ" .

gs1:AllergenTypeCode-ROCKFISH
	rdf:type               gs1:AllergenTypeCode ;
	rdfs:comment           "Refers to the presence of Rockfish and its derivatives in the product, as listed in the regulations specified in AllergenSpecificationAgency and AllergenSpecificationName."@en ;
	rdfs:label             "Rockfish and its Derivatives"@en ;
	skos:prefLabel         "ROCKFISH" ;
	gs1:originalCodeValue  "ROF" .

gs1:AllergenTypeCode-RYE
	rdf:type               gs1:AllergenTypeCode ;
	rdfs:comment           "Refers to the presence of rye and their derivatives in the product, as listed in as listed in the regulations specified in AllergenSpecificationAgency and AllergenSpecificationName"@en ;
	rdfs:label             "Rye and Derivatives"@en ;
	skos:prefLabel         "RYE" ;
	gs1:originalCodeValue  "NR" .

gs1:AllergenTypeCode-SALICYLATE
	rdf:type               gs1:AllergenTypeCode ;
	rdfs:comment           "Refers to the presence of Salicylate, a salt or ester of salicylic acid."@en ;
	rdfs:label             "Salicylate"@en ;
	skos:prefLabel         "SALICYLATE" ;
	gs1:originalCodeValue  "SU" .

gs1:AllergenTypeCode-SALMON
	rdf:type               gs1:AllergenTypeCode ;
	rdfs:comment           "Refers to the presence of Salmon and their derivatives in the product, as listed as listed in the regulations specified in AllergenSpecificationAgency and AllergenSpecificationName."@en ;
	rdfs:label             "Salmon and its Derivatives"@en ;
	skos:prefLabel         "SALMON" ;
	gs1:originalCodeValue  "ADR" .

gs1:AllergenTypeCode-SARDINE
	rdf:type               gs1:AllergenTypeCode ;
	rdfs:comment           "Refers to the presence of Sardine and its derivatives in the product, as listed in the regulations specified in AllergenSpecificationAgency and AllergenSpecificationName."@en ;
	rdfs:label             "Sardine and its Derivatives"@en ;
	skos:prefLabel         "SARDINE" ;
	gs1:originalCodeValue  "SAR" .

gs1:AllergenTypeCode-SCALLOPS
	rdf:type               gs1:AllergenTypeCode ;
	rdfs:comment           "Refers to the presence of Scallops and its derivatives in the product, as listed in the regulations specified in AllergenSpecificationAgency and AllergenSpecificationName."@en ;
	rdfs:label             "Scallops and its Derivatives"@en ;
	skos:prefLabel         "SCALLOPS" ;
	gs1:originalCodeValue  "SCA" .

gs1:AllergenTypeCode-SEED_PRODUCTS
	rdf:type               gs1:AllergenTypeCode ;
	rdfs:comment           "Refers to the presence of seed products as listed in the regulations specified in AllergenSpecificationAgency and AllergenSpecificationName"@en ;
	rdfs:label             "Seed Products"@en ;
	skos:prefLabel         "SEED_PRODUCTS" ;
	gs1:originalCodeValue  "SB" .

gs1:AllergenTypeCode-SESAME_SEEDS
	rdf:type               gs1:AllergenTypeCode ;
	rdfs:comment           "Refers to the presence of sesame seeds or their derivatives in the product, as listed in as listed in the regulations specified in AllergenSpecificationAgency and AllergenSpecificationName"@en ;
	rdfs:label             "Sesame Seeds or Their Derivatives"@en ;
	skos:prefLabel         "SESAME_SEEDS" ;
	gs1:originalCodeValue  "AS" .

gs1:AllergenTypeCode-SHARK
	rdf:type               gs1:AllergenTypeCode ;
	rdfs:comment           "Refers to the presence of Shark and its derivatives in the product, as listed in the regulations specified in AllergenSpecificationAgency and AllergenSpecificationName."@en ;
	rdfs:label             "Shark and its Derivatives"@en ;
	skos:prefLabel         "SHARK" ;
	gs1:originalCodeValue  "SHK" .

gs1:AllergenTypeCode-SHEA_NUTS
	rdf:type               gs1:AllergenTypeCode ;
	rdfs:comment           "Refers to the presence of Shea nuts [Vitellaria paradoxa C.F. Gaertn. (Sapotaceae)] and their derivatives in the product, as listed as listed in the regulations specified in AllergenSpecificationAgency and AllergenSpecificationName."@en ;
	rdfs:label             "Shea Nuts and Their Derivatives"@en ;
	skos:prefLabel         "SHEA_NUTS" ;
	gs1:originalCodeValue  "SJ" .

gs1:AllergenTypeCode-SHELLFISH
	rdf:type               gs1:AllergenTypeCode ;
	rdfs:comment           "Refers to the presence of shellfish and its derivatives as listed in the regulations specified in AllergenSpecificationAgency and AllergenSpecificationName."@en ;
	rdfs:label             "Shellfish and its Derivatives"@en ;
	skos:prefLabel         "SHELLFISH" ;
	gs1:originalCodeValue  "UN" .

gs1:AllergenTypeCode-SHRIMP
	rdf:type               gs1:AllergenTypeCode ;
	rdfs:comment           "Refers to the presence of Shrimp and their derivatives in the product, as listed as listed in the regulations specified in AllergenSpecificationAgency and AllergenSpecificationName."@en ;
	rdfs:label             "Shrimp and its Derivatives"@en ;
	skos:prefLabel         "SHRIMP" ;
	gs1:originalCodeValue  "ABL" .

gs1:AllergenTypeCode-SMELT
	rdf:type               gs1:AllergenTypeCode ;
	rdfs:comment           "Refers to the presence of Smelt and its derivatives in the product, as listed in the regulations specified in AllergenSpecificationAgency and AllergenSpecificationName."@en ;
	rdfs:label             "Smelt and its Derivatives"@en ;
	skos:prefLabel         "SMELT" ;
	gs1:originalCodeValue  "SMT" .

gs1:AllergenTypeCode-SNAPPER
	rdf:type               gs1:AllergenTypeCode ;
	rdfs:comment           "Refers to the presence of Snapper and their derivatives in the product, as listed as listed in the regulations specified in AllergenSpecificationAgency and AllergenSpecificationName."@en ;
	rdfs:label             "Snapper and its Derivatives"@en ;
	skos:prefLabel         "SNAPPER" ;
	gs1:originalCodeValue  "ADS" .

gs1:AllergenTypeCode-SOLE
	rdf:type               gs1:AllergenTypeCode ;
	rdfs:comment           "Refers to the presence of Sole and their derivatives in the product, as listed as listed in the regulations specified in AllergenSpecificationAgency and AllergenSpecificationName."@en ;
	rdfs:label             "Sole and its Derivatives"@en ;
	skos:prefLabel         "SOLE" ;
	gs1:originalCodeValue  "ADT" .

gs1:AllergenTypeCode-SOYBEANS
	rdf:type               gs1:AllergenTypeCode ;
	rdfs:comment           "Refers to the presence of soybeans and their derivatives in the product, as listed in as listed in the regulations specified in AllergenSpecificationAgency and AllergenSpecificationName"@en ;
	rdfs:label             "Soybeans and Their Derivatives"@en ;
	skos:prefLabel         "SOYBEANS" ;
	gs1:originalCodeValue  "AY" .

gs1:AllergenTypeCode-SPELT
	rdf:type               gs1:AllergenTypeCode ;
	rdfs:comment           "Refers to the presence of spelt and spelt products (gluten containing grain) as listed in the regulations specified in AllergenSpecificationAgency and AllergenSpecificationName."@en ;
	rdfs:label             "Spelt and Spelt Products"@en ;
	skos:prefLabel         "SPELT" ;
	gs1:originalCodeValue  "GS" .

gs1:AllergenTypeCode-STURGEON
	rdf:type               gs1:AllergenTypeCode ;
	rdfs:comment           "Refers to the presence of Sturgeon and its derivatives in the product, as listed in the regulations specified in AllergenSpecificationAgency and AllergenSpecificationName."@en ;
	rdfs:label             "Sturgeon and its Derivatives"@en ;
	skos:prefLabel         "STURGEON" ;
	gs1:originalCodeValue  "STG" .

gs1:AllergenTypeCode-SULPHUR_DIOXIDE
	rdf:type               gs1:AllergenTypeCode ;
	rdfs:comment           "Refers to the presence of sulphur dioxide and sulphites as listed in the regulations specified in AllergenSpecificationAgency and AllergenSpecificationName."@en ;
	rdfs:label             "Sulphur Dioxide and Sulphites"@en ;
	skos:prefLabel         "SULPHUR_DIOXIDE" ;
	gs1:originalCodeValue  "AU" .

gs1:AllergenTypeCode-SUNFLOWER_SEEDS
	rdf:type               gs1:AllergenTypeCode ;
	rdfs:comment           "Refers to the presence of Sunflower Seeds or their derivatives in the product as listed in the regulations specified in AllergenSpecificationAgency and AllergenSpecificationName."@en ;
	rdfs:label             "Sunflower Seeds and Their Derivatives"@en ;
	skos:prefLabel         "SUNFLOWER_SEEDS" ;
	gs1:originalCodeValue  "SS" .

gs1:AllergenTypeCode-SWORDFISH
	rdf:type               gs1:AllergenTypeCode ;
	rdfs:comment           "Refers to the presence of Swordfish and their derivatives in the product, as listed as listed in the regulations specified in AllergenSpecificationAgency and AllergenSpecificationName."@en ;
	rdfs:label             "Swordfish and its Derivatives"@en ;
	skos:prefLabel         "SWORDFISH" ;
	gs1:originalCodeValue  "ADU" .

gs1:AllergenTypeCode-TILAPIA
	rdf:type               gs1:AllergenTypeCode ;
	rdfs:comment           "Refers to the presence of Tilapia and their derivatives in the product, as listed as listed in the regulations specified in AllergenSpecificationAgency and AllergenSpecificationName."@en ;
	rdfs:label             "Tilapia and its Derivatives"@en ;
	skos:prefLabel         "TILAPIA" ;
	gs1:originalCodeValue  "ADV" .

gs1:AllergenTypeCode-TREE_NUTS
	rdf:type               gs1:AllergenTypeCode ;
	rdfs:comment           "Refers to the presence of tree nuts and their derivatives in the product, as listed in the regulations specified in AllergenSpecificationAgency and AllergenSpecificationName. Tree nuts can include almonds, hazelnut, walnut, cashews, etc."@en ;
	rdfs:label             "Tree Nuts and Their Derivatives"@en ;
	skos:prefLabel         "TREE_NUTS" ;
	gs1:originalCodeValue  "AN" .

gs1:AllergenTypeCode-TREE_NUT_TRACES
	rdf:type               gs1:AllergenTypeCode ;
	rdfs:comment           "Contains Traces of Tree Nuts, i.e. almonds, various kinds of tree nuts."@en ;
	rdfs:label             "Traces of Tree Nuts"@en ;
	skos:prefLabel         "TREE_NUT_TRACES" ;
	gs1:originalCodeValue  "TN" .

gs1:AllergenTypeCode-TRITICALE
	rdf:type               gs1:AllergenTypeCode ;
	rdfs:comment           "Refers to the presence of Triticale and their derivatives as listed in the regulations specified in AllergenSpecificationAgency and AllergenSpecificationName."@en ;
	rdfs:label             "Triticale and Their Derivatives"@en ;
	skos:prefLabel         "TRITICALE" ;
	gs1:originalCodeValue  "TR" .

gs1:AllergenTypeCode-TROUT
	rdf:type               gs1:AllergenTypeCode ;
	rdfs:comment           "Refers to the presence of Trout and their derivatives in the product, as listed as listed in the regulations specified in AllergenSpecificationAgency and AllergenSpecificationName."@en ;
	rdfs:label             "Trout and its Derivatives"@en ;
	skos:prefLabel         "TROUT" ;
	gs1:originalCodeValue  "ADW" .

gs1:AllergenTypeCode-TUNA
	rdf:type               gs1:AllergenTypeCode ;
	rdfs:comment           "Refers to the presence of Tuna and their derivatives in the product, as listed as listed in the regulations specified in AllergenSpecificationAgency and AllergenSpecificationName."@en ;
	rdfs:label             "Tuna and its Derivatives"@en ;
	skos:prefLabel         "TUNA" ;
	gs1:originalCodeValue  "ABD" .

gs1:AllergenTypeCode-TURBOT
	rdf:type               gs1:AllergenTypeCode ;
	rdfs:comment           "Refers to the presence of Turbot and its derivatives in the product, as listed in the regulations specified in AllergenSpecificationAgency and AllergenSpecificationName."@en ;
	rdfs:label             "Turbot and its Derivatives"@en ;
	skos:prefLabel         "TURBOT" ;
	gs1:originalCodeValue  "TUR" .

gs1:AllergenTypeCode-WALLEYE
	rdf:type               gs1:AllergenTypeCode ;
	rdfs:comment           "Refers to the presence of Walleye and their derivatives in the product, as listed as listed in the regulations specified in AllergenSpecificationAgency and AllergenSpecificationName."@en ;
	rdfs:label             "Walleye and its Derivatives"@en ;
	skos:prefLabel         "WALLEYE" ;
	gs1:originalCodeValue  "ABE" .

gs1:AllergenTypeCode-WALNUTS
	rdf:type               gs1:AllergenTypeCode ;
	rdfs:comment           "Refers to the presence of walnut and walnut products as listed in the regulations specified in AllergenSpecificationAgency and AllergenSpecificationName"@en ;
	rdfs:label             "Walnut and Walnut Products"@en ;
	skos:prefLabel         "WALNUTS" ;
	gs1:originalCodeValue  "SW" .

gs1:AllergenTypeCode-WHEAT
	rdf:type               gs1:AllergenTypeCode ;
	rdfs:comment           "Refers to the presence of wheat and their derivatives in the product, as listed in the regulations specified in AllergenSpecificationAgency and AllergenSpecificationName"@en ;
	rdfs:label             "Wheat and Their Derivatives"@en ;
	skos:prefLabel         "WHEAT" ;
	gs1:originalCodeValue  "UW" .

gs1:AllergenTypeCode-WHELKS
	rdf:type               gs1:AllergenTypeCode ;
	rdfs:comment           "Refers to the presence of Whelks and its derivatives in the product, as listed in the regulations specified in AllergenSpecificationAgency and AllergenSpecificationName."@en ;
	rdfs:label             "Whelks and its Derivatives"@en ;
	skos:prefLabel         "WHELKS" ;
	gs1:originalCodeValue  "WHK" .

gs1:AllergenTypeCode-WHITEFISH
	rdf:type               gs1:AllergenTypeCode ;
	rdfs:comment           "Refers to the presence of Whitefish and their derivatives in the product, as listed as listed in the regulations specified in AllergenSpecificationAgency and AllergenSpecificationName."@en ;
	rdfs:label             "Whitefish and its Derivatives"@en ;
	skos:prefLabel         "WHITEFISH" ;
	gs1:originalCodeValue  "AWF" .

gs1:AllergenTypeCode-WHITING
	rdf:type               gs1:AllergenTypeCode ;
	rdfs:comment           "Refers to the presence of Whiting and its derivatives in the product, as listed in the regulations specified in AllergenSpecificationAgency and AllergenSpecificationName."@en ;
	rdfs:label             "Whiting and its Derivatives"@en ;
	skos:prefLabel         "WHITING" ;
	gs1:originalCodeValue  "WHT" .

gs1:Altitude
	rdf:type  gs1:MeasurementType ;
	rdfs:comment    "The height above the surface of a defined geoid, typically the World Geodetic System (WGS 84) geoid for measurements from location sensors using satellite technology (e.g. GPS, Glonass, Galileo) , which approximates to the surface of the earth at sea level.  Positive values indicate height above the geoid surface. Negative values indicate depth below the geoid surface.  SI Units: metres"@en ;
	rdfs:label      "Altitude or Elevation"@en ;
	skos:prefLabel  "Altitude" .

gs1:AmountOfSubstance
	rdf:type        gs1:MeasurementType ;
	rdfs:comment    "The amount of substance that contains a number of atoms, molecules etc. that is equal to the Avogadro constant.  SI Units: mole"@en ;
	rdfs:label      "Amount of substance"@en ;
	skos:prefLabel  "AmountOfSubstance" .

gs1:AmountOfSubstancePerUnitVolume
	rdf:type        gs1:MeasurementType ;
	rdfs:comment    "The concentration of a solution expressed as the number of moles of dissolved substance per unit volume of solution.  SI Units: mole per cubic metre"@en ;
	rdfs:label      "Amount of substance per unit volume"@en ;
	skos:prefLabel  "AmountOfSubstancePerUnitVolume" .

gs1:AnatomicalFormCode-BELLY
	rdf:type        gs1:AnatomicalFormCode ;
	rdfs:label      "Belly"@en ;
	skos:prefLabel  "BELLY" .

gs1:AnatomicalFormCode-BLOOD
	rdf:type        gs1:AnatomicalFormCode ;
	rdfs:label      "Blood"@en ;
	skos:prefLabel  "BLOOD" .

gs1:AnatomicalFormCode-BONE
	rdf:type        gs1:AnatomicalFormCode ;
	rdfs:label      "Bone"@en ;
	skos:prefLabel  "BONE" .

gs1:AnatomicalFormCode-BRAIN
	rdf:type        gs1:AnatomicalFormCode ;
	rdfs:label      "Brain"@en ;
	skos:prefLabel  "BRAIN" .

gs1:AnatomicalFormCode-CARCASS_NONPOULTRY
	rdf:type        gs1:AnatomicalFormCode ;
	rdfs:label      "Carcass Nonpoultry"@en ;
	skos:prefLabel  "CARCASS_NONPOULTRY" .

gs1:AnatomicalFormCode-DIAPHRAM
	rdf:type        gs1:AnatomicalFormCode ;
	rdfs:label      "Diaphram"@en ;
	skos:prefLabel  "DIAPHRAM" .

gs1:AnatomicalFormCode-ESOPHAGUS
	rdf:type        gs1:AnatomicalFormCode ;
	rdfs:label      "Esophagus"@en ;
	skos:prefLabel  "ESOPHAGUS" .

gs1:AnatomicalFormCode-FAT
	rdf:type        gs1:AnatomicalFormCode ;
	rdfs:label      "Fat"@en ;
	skos:prefLabel  "FAT" .

gs1:AnatomicalFormCode-FEET
	rdf:type        gs1:AnatomicalFormCode ;
	rdfs:label      "Feet"@en ;
	skos:prefLabel  "FEET" .

gs1:AnatomicalFormCode-FOREQUARTER
	rdf:type        gs1:AnatomicalFormCode ;
	rdfs:label      "Forequarter"@en ;
	skos:prefLabel  "FOREQUARTER" .

gs1:AnatomicalFormCode-GIZZARD
	rdf:type        gs1:AnatomicalFormCode ;
	rdfs:label      "Gizzard"@en ;
	skos:prefLabel  "GIZZARD" .

gs1:AnatomicalFormCode-HEAD
	rdf:type        gs1:AnatomicalFormCode ;
	rdfs:label      "Head"@en ;
	skos:prefLabel  "HEAD" .

gs1:AnatomicalFormCode-HEADMEAT_CHEEKMEAT
	rdf:type        gs1:AnatomicalFormCode ;
	rdfs:label      "Headmeat Cheekmeat"@en ;
	skos:prefLabel  "HEADMEAT_CHEEKMEAT" .

gs1:AnatomicalFormCode-HEART
	rdf:type        gs1:AnatomicalFormCode ;
	rdfs:label      "Heart"@en ;
	skos:prefLabel  "HEART" .

gs1:AnatomicalFormCode-HINDQUARTER
	rdf:type        gs1:AnatomicalFormCode ;
	rdfs:label      "Hindquarter"@en ;
	skos:prefLabel  "HINDQUARTER" .

gs1:AnatomicalFormCode-HORN
	rdf:type        gs1:AnatomicalFormCode ;
	rdfs:label      "Horn"@en ;
	skos:prefLabel  "HORN" .

gs1:AnatomicalFormCode-INTESTINE_LARGE
	rdf:type        gs1:AnatomicalFormCode ;
	rdfs:label      "Intestine Large"@en ;
	skos:prefLabel  "INTESTINE_LARGE" .

gs1:AnatomicalFormCode-INTESTINE_SMALL
	rdf:type        gs1:AnatomicalFormCode ;
	rdfs:label      "Intenstine Small"@en ;
	skos:prefLabel  "INTESTINE_SMALL" .

gs1:AnatomicalFormCode-KIDNEY
	rdf:type        gs1:AnatomicalFormCode ;
	rdfs:label      "Kidney"@en ;
	skos:prefLabel  "KIDNEY" .

gs1:AnatomicalFormCode-LIPS
	rdf:type        gs1:AnatomicalFormCode ;
	rdfs:label      "Lips"@en ;
	skos:prefLabel  "LIPS" .

gs1:AnatomicalFormCode-LIVER
	rdf:type        gs1:AnatomicalFormCode ;
	rdfs:label      "Liver"@en ;
	skos:prefLabel  "LIVER" .

gs1:AnatomicalFormCode-LUNGS
	rdf:type        gs1:AnatomicalFormCode ;
	rdfs:label      "Lungs"@en ;
	skos:prefLabel  "LUNGS" .

gs1:AnatomicalFormCode-MIXED_OFFAL
	rdf:type        gs1:AnatomicalFormCode ;
	rdfs:label      "Mixed Offal"@en ;
	skos:prefLabel  "MIXED_OFFAL" .

gs1:AnatomicalFormCode-MIXED_PARTS_FOR_GROUNDING_MINCING
	rdf:type        gs1:AnatomicalFormCode ;
	rdfs:label      "Mixed Parts For Grounding or Mincing"@en ;
	skos:prefLabel  "MIXED_PARTS_FOR_GROUNDING_MINCING" .

gs1:AnatomicalFormCode-NECK
	rdf:type        gs1:AnatomicalFormCode ;
	rdfs:label      "Neck"@en ;
	skos:prefLabel  "NECK" .

gs1:AnatomicalFormCode-PANCREAS
	rdf:type        gs1:AnatomicalFormCode ;
	rdfs:label      "Pancreas"@en ;
	skos:prefLabel  "PANCREAS" .

gs1:AnatomicalFormCode-SKIN
	rdf:type        gs1:AnatomicalFormCode ;
	rdfs:label      "Skin"@en ;
	skos:prefLabel  "SKIN" .

gs1:AnatomicalFormCode-STOMACH
	rdf:type        gs1:AnatomicalFormCode ;
	rdfs:label      "Stomach"@en ;
	skos:prefLabel  "STOMACH" .

gs1:AnatomicalFormCode-TAIL
	rdf:type        gs1:AnatomicalFormCode ;
	rdfs:label      "Tail"@en ;
	skos:prefLabel  "TAIL" .

gs1:AnatomicalFormCode-TENDONS
	rdf:type        gs1:AnatomicalFormCode ;
	rdfs:label      "Tendons"@en ;
	skos:prefLabel  "TENDONS" .

gs1:AnatomicalFormCode-TESTICLES
	rdf:type        gs1:AnatomicalFormCode ;
	rdfs:label      "Testicles"@en ;
	skos:prefLabel  "TESTICLES" .

gs1:AnatomicalFormCode-THYMUS
	rdf:type        gs1:AnatomicalFormCode ;
	rdfs:label      "Thymus"@en ;
	skos:prefLabel  "THYMUS" .

gs1:AnatomicalFormCode-TONGUE
	rdf:type        gs1:AnatomicalFormCode ;
	rdfs:label      "Tongue"@en ;
	skos:prefLabel  "TONGUE" .

gs1:AnatomicalFormCode-TRIPE
	rdf:type        gs1:AnatomicalFormCode ;
	rdfs:label      "Tripe"@en ;
	skos:prefLabel  "TRIPE" .

gs1:AnatomicalFormCode-UNCLASSIFIED
	rdf:type        gs1:AnatomicalFormCode ;
	rdfs:label      "Unclassified"@en ;
	skos:prefLabel  "UNCLASSIFIED" .

gs1:AnatomicalFormCode-UNIDENTIFIED
	rdf:type        gs1:AnatomicalFormCode ;
	rdfs:label      "Unidentified"@en ;
	skos:prefLabel  "UNIDENTIFIED" .

gs1:AnatomicalFormCode-WHOLE_BIRD
	rdf:type        gs1:AnatomicalFormCode ;
	rdfs:label      "Whole Bird"@en ;
	skos:prefLabel  "WHOLE_BIRD" .

gs1:AnatomicalFormCode-WHOLE_MUSCLE_NONPOULTRY_MEATPART_PIECE
	rdf:type        gs1:AnatomicalFormCode ;
	rdfs:label      "Whole Muscle Nonpoultry Meatpart Piece"@en ;
	skos:prefLabel  "WHOLE_MUSCLE_NONPOULTRY_MEATPART_PIECE" .

gs1:AnatomicalFormCode-WHOLE_MUSCLE_POULTRY_PART
	rdf:type        gs1:AnatomicalFormCode ;
	rdfs:label      "Whole Muscle Poultry Part"@en ;
	skos:prefLabel  "WHOLE_MUSCLE_POULTRY_PART" .

gs1:AnatomicalFormCode-WHOLE_MUSCLE_PRIMAL
	rdf:type        gs1:AnatomicalFormCode ;
	rdfs:label      "Whole Muscle Primal"@en ;
	skos:prefLabel  "WHOLE_MUSCLE_PRIMAL" .

gs1:AnatomicalFormCode-WHOLE_MUSCLE_RIBCUT
	rdf:type        gs1:AnatomicalFormCode ;
	rdfs:label      "Whole Muscle Ribcut"@en ;
	skos:prefLabel  "WHOLE_MUSCLE_RIBCUT" .

gs1:AnatomicalFormCode-WHOLE_MUSCLE_ROASTCUT
	rdf:type        gs1:AnatomicalFormCode ;
	rdfs:label      "Whole Muscle Roast Cut"@en ;
	skos:prefLabel  "WHOLE_MUSCLE_ROASTCUT" .

gs1:AnatomicalFormCode-WHOLE_MUSCLE_SLICE_CHOPCUT
	rdf:type        gs1:AnatomicalFormCode ;
	rdfs:label      "Whole Muscle Slice Chopcut"@en ;
	skos:prefLabel  "WHOLE_MUSCLE_SLICE_CHOPCUT" .

gs1:AnatomicalFormCode-WHOLE_MUSCLE_SLICE_CUTLET
	rdf:type        gs1:AnatomicalFormCode ;
	rdfs:label      "Whole Muscle Slice Cutlet"@en ;
	skos:prefLabel  "WHOLE_MUSCLE_SLICE_CUTLET" .

gs1:AnatomicalFormCode-WHOLE_MUSCLE_STEAK_CHOPCUT
	rdf:type        gs1:AnatomicalFormCode ;
	rdfs:label      "Whole Muscle Steak Chop-cut"@en ;
	skos:prefLabel  "WHOLE_MUSCLE_STEAK_CHOPCUT" .

gs1:AnatomicalFormCode-WHOLE_MUSCLE_SUBPRIMAL
	rdf:type        gs1:AnatomicalFormCode ;
	rdfs:label      "Whole Muscle Subprimal"@en ;
	skos:prefLabel  "WHOLE_MUSCLE_SUBPRIMAL" .

gs1:Angle
	rdf:type     gs1:MeasurementType ;
	rdfs:comment    "The inclination of one line or plane to another.  Units: degrees, radians, etc."@en ;
	rdfs:label      "Angle"@en ;
	skos:prefLabel  "Angle" .

gs1:AngularAcceleration
	rdf:type        gs1:MeasurementType ;
	rdfs:comment    "The rate of change of angular velocity with respect to time.  SI Units: radian per second per second"@en ;
	rdfs:label      "Angular acceleration"@en ;
	skos:prefLabel  "AngularAcceleration" .

gs1:AngularMomentum
	rdf:type  gs1:MeasurementType ;
	rdfs:comment    "The integral over time of the torque acting on a body that is free to rotate, resulting in a corresponding change in its angular momentum.  SI Units: newton metre second, kilogram metre squared per second"@en ;
	rdfs:label      "Angular impulse or Angular momentum"@en ;
	skos:prefLabel  "AngularMomentum" .

gs1:AngularVelocity
	rdf:type  gs1:MeasurementType ;
	rdfs:comment    "The rate of change of angle with respect to time; a measure of the number of revolutions per unit time.  SI Units: radian per second"@en ;
	rdfs:label      "Angular velocity"@en ;
	skos:prefLabel  "AngularVelocity" .

gs1:Area
	rdf:type      gs1:MeasurementType ;
	rdfs:comment    "The amount of two-dimensional space occupied, measured in units of length squared.  SI Units: square metre"@en ;
	rdfs:label      "Area"@en ;
	skos:prefLabel  "Area" .

gs1:Capacitance
	rdf:type  gs1:MeasurementType ;
	rdfs:comment    "The capacitance of an isolated conductor is defined as the ratio of the total charge on it to its electric potential.  SI Units: farad"@en ;
	rdfs:label      "Capacitance"@en ;
	skos:prefLabel  "Capacitance" .

gs1:CertificationStatus-ACTIVE
	rdf:type        gs1:CertificationStatus ;
	rdfs:comment    "This certification instance is declared to be in effect for the certified subject."@en ;
	rdfs:label      "Active"@en ;
	skos:prefLabel  "ACTIVE" .

gs1:CertificationStatus-INACTIVE
	rdf:type        gs1:CertificationStatus ;
	rdfs:comment    "This certification instance is declared to be no longer in effect."@en ;
	rdfs:label      "Inactive"@en ;
	skos:prefLabel  "INACTIVE" .

gs1:CheeseFirmnessCode-EXTRA_HARD
	rdf:type        gs1:CheeseFirmnessCode ;
	rdfs:label      "Extra Hard"@en ;
	skos:prefLabel  "EXTRA_HARD" .

gs1:CheeseFirmnessCode-FIRM_SEMIHARD
	rdf:type        gs1:CheeseFirmnessCode ;
	rdfs:label      "Firm Semi Hard"@en ;
	skos:prefLabel  "FIRM_SEMIHARD" .

gs1:CheeseFirmnessCode-HARD
	rdf:type        gs1:CheeseFirmnessCode ;
	rdfs:label      "Hard"@en ;
	skos:prefLabel  "HARD" .

gs1:CheeseFirmnessCode-SOFT
	rdf:type        gs1:CheeseFirmnessCode ;
	rdfs:label      "Soft"@en ;
	skos:prefLabel  "SOFT" .

gs1:CheeseFirmnessCode-UNIDENTIFIED
	rdf:type        gs1:CheeseFirmnessCode ;
	rdfs:label      "Unidentified"@en ;
	skos:prefLabel  "UNIDENTIFIED" .

gs1:ColourCodeList-BUYER
	rdf:type               gs1:ColourCodeListCode ;
	rdfs:comment           "Assigned by buyer."@en ;
	rdfs:label             "Assigned by Buyer"@en ;
	skos:prefLabel         "BUYER" ;
	gs1:originalCodeValue  "6" .

gs1:ColourCodeList-IFPS
	rdf:type               gs1:ColourCodeListCode ;
	rdfs:comment           "International Federation for Produce Standards."@en ;
	rdfs:label             "International Federation for Produce Standards"@en ;
	skos:prefLabel         "IFPS" ;
	gs1:originalCodeValue  "11" .

gs1:ColourCodeList-NCS
	rdf:type               gs1:ColourCodeListCode ;
	rdfs:comment           "Natural Colour System."@en ;
	rdfs:label             "Natural Colour System"@en ;
	skos:prefLabel         "NCS" ;
	gs1:originalCodeValue  "10" .

gs1:ColourCodeList-NRF
	rdf:type               gs1:ColourCodeListCode ;
	rdfs:comment           "National Retail Federation."@en ;
	rdfs:label             "National Retail Federation."@en ;
	skos:prefLabel         "NRF" ;
	gs1:originalCodeValue  "1" .

gs1:ColourCodeList-PANTONE_HEXACHROME
	rdf:type               gs1:ColourCodeListCode ;
	rdfs:comment           "Pantone Hexachrome."@en ;
	rdfs:label             "Pantone Hexachrome"@en ;
	skos:prefLabel         "PANTONE_HEXACHROME" ;
	gs1:originalCodeValue  "4" .

gs1:ColourCodeList-PANTONE_MATCHING
	rdf:type               gs1:ColourCodeListCode ;
	rdfs:comment           "Pantone Matching System."@en ;
	rdfs:label             "Pantone Matching System"@en ;
	skos:prefLabel         "PANTONE_MATCHING" ;
	gs1:originalCodeValue  "2" .

gs1:ColourCodeList-PANTONE_PROCESS_COLOUR
	rdf:type               gs1:ColourCodeListCode ;
	rdfs:comment           "Pantone Process Colour System."@en ;
	rdfs:label             "Pantone Process Colour System"@en ;
	skos:prefLabel         "PANTONE_PROCESS_COLOUR" ;
	gs1:originalCodeValue  "3" .

gs1:ColourCodeList-PANTONE_TEXTILE
	rdf:type               gs1:ColourCodeListCode ;
	rdfs:comment           "Pantone Textile. Same as GS1 ColourCodeList Code 5"@en ;
	rdfs:label             "Pantone Textile"@en ;
	skos:prefLabel         "PANTONE_TEXTILE" ;
	gs1:originalCodeValue  "5" .

gs1:ColourCodeList-RAL
	rdf:type               gs1:ColourCodeListCode ;
	rdfs:comment           "Farbsystem RAL Colour System."@en ;
	rdfs:label             "Farbsystem RAL Colour System"@en ;
	skos:prefLabel         "RAL" ;
	gs1:originalCodeValue  "9" .

gs1:ColourCodeList-SELLER
	rdf:type               gs1:ColourCodeListCode ;
	rdfs:comment           "Assigned by seller."@en ;
	rdfs:label             "Assigned by Seller"@en ;
	skos:prefLabel         "SELLER" ;
	gs1:originalCodeValue  "7" .

gs1:ColourCodeList-WWS
	rdf:type               gs1:ColourCodeListCode ;
	rdfs:comment           "Waren Wirtschafts System."@en ;
	rdfs:label             "Waren Wirtschafts System"@en ;
	skos:prefLabel         "WWS" ;
	gs1:originalCodeValue  "8" .

gs1:Conductance
	rdf:type  gs1:MeasurementType ;
	rdfs:comment    "The ratio of the current in the conductor to the potential difference between its ends; reciprocal of resistance.  SI Units: siemen"@en ;
	rdfs:label      "Conductance"@en ;
	skos:prefLabel  "Conductance" .

gs1:Conductivity
	rdf:type  gs1:MeasurementType ;
	rdfs:comment    "A measure of how strongly a material conducts electric current. The ratio of the current density to the electric field that causes the current to flow.  SI Units: siemen per metre"@en ;
	rdfs:label      "Conductivity"@en ;
	skos:prefLabel  "Conductivity" .

gs1:ConsumerLifestageCode-ADULT
	rdf:type        gs1:ConsumerLifestageCode ;
	rdfs:label      "Suitable for Adults"@en ;
	skos:prefLabel  "ADULT" .

gs1:ConsumerLifestageCode-ALL_AGES
	rdf:type        gs1:ConsumerLifestageCode ;
	rdfs:label      "Suitable for All Ages"@en ;
	skos:prefLabel  "ALL_AGES" .

gs1:ConsumerLifestageCode-BABY_INFANT
	rdf:type        gs1:ConsumerLifestageCode ;
	rdfs:label      "Suitable for Babies/Infants"@en ;
	skos:prefLabel  "BABY_INFANT" .

gs1:ConsumerLifestageCode-CHILD_1_To_2_YEARS
	rdf:type        gs1:ConsumerLifestageCode ;
	rdfs:label      "Suitable for Children One to Two Years Old"@en ;
	skos:prefLabel  "CHILD_1_To_2_YEARS" .

gs1:ConsumerLifestageCode-CHILD_2_YEARS_ONWARDS
	rdf:type        gs1:ConsumerLifestageCode ;
	rdfs:label      "Suitable for Children 2 Plus Years of Age"@en ;
	skos:prefLabel  "CHILD_2_YEARS_ONWARDS" .

gs1:ConsumerLifestageCode-UNCLASSIFIED
	rdf:type        gs1:ConsumerLifestageCode ;
	rdfs:label      "Unclassified"@en ;
	skos:prefLabel  "UNCLASSIFIED" .

gs1:ConsumerLifestageCode-UNIDENTIFIED
	rdf:type        gs1:ConsumerLifestageCode ;
	rdfs:label      "Unidentified"@en ;
	skos:prefLabel  "UNIDENTIFIED" .

gs1:ConsumerSalesConditionsCode-BTC
	rdf:type        gs1:ConsumerSalesConditionsCode ;
	rdfs:comment    "Products that are sold without a prescription but must be distributed through a pharmacy."@en ;
	rdfs:label      "Behind the Counter"@en ;
	skos:prefLabel  "BTC" .

gs1:ConsumerSalesConditionsCode-OTC
	rdf:type        gs1:ConsumerSalesConditionsCode ;
	rdfs:comment    "Products that may be sold without a prescription. These products are generally available without restrictions."@en ;
	rdfs:label      "Over the Counter"@en ;
	skos:prefLabel  "OTC" .

gs1:ConsumerSalesConditionsCode-PRESCRIPTION_REQUIRED
	rdf:type        gs1:ConsumerSalesConditionsCode ;
	rdfs:comment    "Product may only be sold or dispensed under the direction of a prescription."@en ;
	rdfs:label      "Prescription Required"@en ;
	skos:prefLabel  "PRESCRIPTION_REQUIRED" .

gs1:ConsumerSalesConditionsCode-RESTRICTED_TO_SELL_16
	rdf:type        gs1:ConsumerSalesConditionsCode ;
	rdfs:comment    "Based upon legal regulatory restrictions it is illegal to sell the product to anyone under the age of 16 years old."@en ;
	rdfs:label      "Restricted To Sell 16"@en ;
	skos:prefLabel  "RESTRICTED_TO_SELL_16" .

gs1:ConsumerSalesConditionsCode-RESTRICTED_TO_SELL_18
	rdf:type        gs1:ConsumerSalesConditionsCode ;
	rdfs:comment    "Based upon legal regulatory restrictions it is illegal to sell the product to anyone under the age of 18 years old."@en ;
	rdfs:label      "Restricted To Sell 18"@en ;
	skos:prefLabel  "RESTRICTED_TO_SELL_18" .

gs1:ConsumerSalesConditionsCode-RESTRICTED_TO_SELL_21
	rdf:type        gs1:ConsumerSalesConditionsCode ;
	rdfs:comment    "Based upon legal regulatory restrictions it is illegal to sell the product to anyone under the age of 21 years old."@en ;
	rdfs:label      "Restricted To Sell 21"@en ;
	skos:prefLabel  "RESTRICTED_TO_SELL_21" .

gs1:Count
	rdf:type     gs1:MeasurementType ;
	rdfs:comment    "A measure of the total quantity of something; the number of individual units present.  Typically dimensionless (no units)"@en ;
	rdfs:label      "Count"@en ;
	skos:prefLabel  "Count" .

gs1:Density
	rdf:type   gs1:MeasurementType ;
	rdfs:comment    "The mass per unit volume of a substance.  SI Units: kilogram per cubic metre"@en ;
	rdfs:label      "Density"@en ;
	skos:prefLabel  "Density" .

gs1:DietTypeCode-COELIAC
	rdf:type        gs1:DietTypeCode ;
	rdfs:comment    "Denotes a product that can be safely consumed by a person with coeliac disease. Coeliac disease is caused by a reaction to gladin (a gluten protein found in wheat) and similar proteins found in other crops."@en ;
	rdfs:label      "Coeliac"@en ;
	skos:prefLabel  "COELIAC" .

gs1:DietTypeCode-DIETETIC
	rdf:type        gs1:DietTypeCode ;
	rdfs:comment    "Denotes a product that is specially prepared or processed for people on restrictive diets."@en ;
	rdfs:label      "Dietetic"@en ;
	skos:prefLabel  "DIETETIC" .

gs1:DietTypeCode-FREE_FROM_GLUTEN
	rdf:type        gs1:DietTypeCode ;
	rdfs:comment    "Denotes a product that can be used in a gluten free diet, as specified by the appropriate authority within a target market."@en ;
	rdfs:label      "Free From Gluten"@en ;
	skos:prefLabel  "FREE_FROM_GLUTEN" .

gs1:DietTypeCode-HALAL
	rdf:type        gs1:DietTypeCode ;
	rdfs:comment    "Denotes selling or serving food ritually fit according to Islamic dietary laws."@en ;
	rdfs:label      "Halal"@en ;
	skos:prefLabel  "HALAL" .

gs1:DietTypeCode-KOSHER
	rdf:type        gs1:DietTypeCode ;
	rdfs:comment    "Denotes selling or serving food ritually fit according to Jewish dietary laws."@en ;
	rdfs:label      "Kosher"@en ;
	skos:prefLabel  "KOSHER" .

gs1:DietTypeCode-ORGANIC
	rdf:type        gs1:DietTypeCode ;
	rdfs:comment    "Denotes a food product that was produced with the use of feed or fertiliser of plant or animal origin, without employment of chemically formulated fertilisers, growth stimulants, antibiotics or pesticides."@en ;
	rdfs:label      "Organic"@en ;
	skos:prefLabel  "ORGANIC" .

gs1:DietTypeCode-VEGAN
	rdf:type        gs1:DietTypeCode ;
	rdfs:comment    "Denotes a food product which contains no animal food or dairy products."@en ;
	rdfs:label      "Vegan"@en ;
	skos:prefLabel  "VEGAN" .

gs1:DietTypeCode-VEGETARIAN
	rdf:type        gs1:DietTypeCode ;
	rdfs:comment    "Denotes a product that contains no meat, fish or other animal products."@en ;
	rdfs:label      "Vegetarian"@en ;
	skos:prefLabel  "VEGETARIAN" .

gs1:DietTypeCode-WITHOUT_BEEF
	rdf:type        gs1:DietTypeCode ;
	rdfs:comment    "Denotes a product that contains no beef or beef-products. Beef is considered to be a taboo food product by some religions most notable Hinduism, Buddhism and Jainism."@en ;
	rdfs:label      "Without Beef"@en ;
	skos:prefLabel  "WITHOUT_BEEF" .

gs1:DietTypeCode-WITHOUT_PORK
	rdf:type        gs1:DietTypeCode ;
	rdfs:comment    "Denotes a product that contains no pork meat."@en ;
	rdfs:label      "Without Pork"@en ;
	skos:prefLabel  "WITHOUT_PORK" .

gs1:Dimensionless
	rdf:type  gs1:MeasurementType ;
	rdfs:comment    "A measurement whose units are dimensionless.  gs1:Count or gs1:VolumeFraction or gs1:RelativeHumidity should be used in preference if appropriate."@en ;
	rdfs:label      "Dimensionless"@en ;
	skos:prefLabel  "Dimensionless" .

gs1:DiscountTypeCode-BOGO
	rdf:type        gs1:DiscountTypeCode ;
	rdfs:comment    "Buy one item and get the second item free of charge"@en ;
	rdfs:label      "BOGO"@en ;
	skos:prefLabel  "BOGO" .

gs1:DiscountTypeCode-DISCOUNTED_ITEM
	rdf:type        gs1:DiscountTypeCode ;
	rdfs:comment    "A discount on the item expressed as an amount (value and currency)"@en ;
	rdfs:label      "Discounted Item"@en ;
	skos:prefLabel  "DISCOUNTED_ITEM" .

gs1:DiscountTypeCode-FREE_GIFT
	rdf:type        gs1:DiscountTypeCode ;
	rdfs:comment    "A gift given to a consumer as part of a promotional contingent on the consumer making a purchase of another item or items."@en ;
	rdfs:label      "Free Gift"@en ;
	skos:prefLabel  "FREE_GIFT" .

gs1:DiscountTypeCode-FREE_SHIPPING
	rdf:type        gs1:DiscountTypeCode ;
	rdfs:comment    "No charge for shipping."@en ;
	rdfs:label      "Free Shipping"@en ;
	skos:prefLabel  "FREE_SHIPPING" .

gs1:DiscountTypeCode-OTHER
	rdf:type        gs1:DiscountTypeCode ;
	rdfs:comment    "A discount other than the ones on this list."@en ;
	rdfs:label      "Other"@en ;
	skos:prefLabel  "OTHER" .

gs1:DiscountTypeCode-PERCENTAGE_OFF
	rdf:type        gs1:DiscountTypeCode ;
	rdfs:comment    "A percentage off the product price."@en ;
	rdfs:label      "Percentage Off"@en ;
	skos:prefLabel  "PERCENTAGE_OFF" .

gs1:DoseEquivalent
	rdf:type  gs1:MeasurementType ;
	rdfs:comment    "The product of the absorbed dose multiplied by a Q factor (relating to the type of radiation) and a factor relating to all relevant aspects of the body being irradiated, multiplied by the exposure time.  SI Units: sievert"@en ;
	rdfs:label      "Dose Equivalent"@en ;
	skos:prefLabel  "DoseEquivalent" .

gs1:DoseEquivalentRate
	rdf:type        gs1:MeasurementType ;
	rdfs:comment    "The product of the absorbed dose rate multiplied by a Q factor (relating to the type of radiation) and a factor relating to all relevant aspects of the body being irradiated.  SI Units: sievert per second"@en ;
	rdfs:label      "Dose equivalent rate"@en ;
	skos:prefLabel  "DoseEquivalentRate" .

gs1:DynamicViscosity
	rdf:type  gs1:MeasurementType ;
	rdfs:comment    "The value of the tangential force per unit area which is necessary to maintain unit relative velocty between two parallel planes unit distance apart in a fluid.  SI Units: pascal"@en ;
	rdfs:label      "Dynamic viscosity"@en ;
	skos:prefLabel  "DynamicViscosity" .

gs1:ERROR_CONDITION
	rdf:type  gs1:SensorAlertType ;
	rdfs:comment    "Indicates the reporting of an error condition detected by a sensor device"@en ;
	rdfs:label      "Error condition"@en ;
	skos:prefLabel  "ERROR_CONDITION" .

gs1:ElectricCharge
	rdf:type  gs1:MeasurementType ;
	rdfs:comment    "Quantity of unbalanced electricity in an object, i.e. excess or deficiency of electrons, resulting in negative or positive electrification, respectively.  SI Units: coulomb"@en ;
	rdfs:label      "Electric Charge"@en ;
	skos:prefLabel  "ElectricCharge" .

gs1:ElectricCurrent
	rdf:type  gs1:MeasurementType ;
	rdfs:comment    "Rate of flow of charge in a substance, whether solid, liquid or gas.  SI Units: ampere"@en ;
	rdfs:label      "Electric Current"@en ;
	skos:prefLabel  "ElectricCurrent" .

gs1:ElectricCurrentDensity
	rdf:type        gs1:MeasurementType ;
	rdfs:comment    "Rate of flow of charge in a substance per unit area perpendicular to the current.  SI Units: ampere per square metre"@en ;
	rdfs:label      "Electric current density"@en ;
	skos:prefLabel  "ElectricCurrentDensity" .

gs1:ElectricFieldStrength
	rdf:type        gs1:MeasurementType ;
	rdfs:comment    "The electric force acting on a unit charge. The linear gradient of the electrostatic potential.  SI Units: volt per metre = newton / coulomb"@en ;
	rdfs:label      "Electric field strength"@en ;
	skos:prefLabel  "ElectricFieldStrength" .

gs1:Energy
	rdf:type    gs1:MeasurementType ;
	rdfs:comment    "A measure of a the capacity of a system or body to do work.  SI Units: joule"@en ;
	rdfs:label      "Energy"@en ;
	skos:prefLabel  "Energy" .

gs1:Exposure
	rdf:type  gs1:MeasurementType ;
	rdfs:comment    "The product of light intensity and time duration of the exposure.  SI Units: lux second"@en ;
	rdfs:label      "Exposure"@en ;
	skos:prefLabel  "Exposure" .

gs1:FoodBeverageRefrigerationClaimCode-CAN_BE_REFRIGERATED
	rdf:type        gs1:FoodBeverageRefrigerationClaimCode ;
	rdfs:label      "Can Be Refrigerated."@en ;
	skos:prefLabel  "CAN_BE_REFRIGERATED" .

gs1:FoodBeverageRefrigerationClaimCode-MUST_BE_REFRIGERATED
	rdf:type        gs1:FoodBeverageRefrigerationClaimCode ;
	rdfs:label      "Must Be Refrigerated."@en ;
	skos:prefLabel  "MUST_BE_REFRIGERATED" .

gs1:FoodBeverageRefrigerationClaimCode-SHELF_STABLE
	rdf:type        gs1:FoodBeverageRefrigerationClaimCode ;
	rdfs:label      "Shelf Stable."@en ;
	skos:prefLabel  "SHELF_STABLE" .

gs1:FoodBeverageRefrigerationClaimCode-UNIDENTIFIED
	rdf:type        gs1:FoodBeverageRefrigerationClaimCode ;
	rdfs:label      "Unidentified."@en ;
	skos:prefLabel  "UNIDENTIFIED" .

gs1:FoodBeverageTargetUseCode-ANY_MEAL
	rdf:type        gs1:FoodBeverageTargetUseCode ;
	rdfs:label      "Any Meal"@en ;
	skos:prefLabel  "ANY_MEAL" .

gs1:FoodBeverageTargetUseCode-BREAKFAST
	rdf:type        gs1:FoodBeverageTargetUseCode ;
	rdfs:label      "Breakfast"@en ;
	skos:prefLabel  "BREAKFAST" .

gs1:FoodBeverageTargetUseCode-MAIN_MEAL
	rdf:type        gs1:FoodBeverageTargetUseCode ;
	rdfs:label      "Main Meal"@en ;
	skos:prefLabel  "MAIN_MEAL" .

gs1:FoodBeverageTargetUseCode-PORTABLE_MEAL
	rdf:type        gs1:FoodBeverageTargetUseCode ;
	rdfs:label      "Portable Meal"@en ;
	skos:prefLabel  "PORTABLE_MEAL" .

gs1:FoodBeverageTargetUseCode-SNACK
	rdf:type        gs1:FoodBeverageTargetUseCode ;
	rdfs:label      "Snack"@en ;
	skos:prefLabel  "SNACK" .

gs1:FoodBeverageTargetUseCode-UNCLASSIFIED
	rdf:type        gs1:FoodBeverageTargetUseCode ;
	rdfs:label      "Unclassified"@en ;
	skos:prefLabel  "UNCLASSIFIED" .

gs1:FootwearFasteningTypeCode-MULTIPLE_FASTENING
	rdf:type        gs1:FootwearFasteningTypeCode ;
	rdfs:label      "Multiple Fastenings"@en ;
	skos:prefLabel  "MULTIPLE_FASTENING" .

gs1:FootwearFasteningTypeCode-SHOE_LACE
	rdf:type        gs1:FootwearFasteningTypeCode ;
	rdfs:label      "Shoe Lace"@en ;
	skos:prefLabel  "SHOE_LACE" .

gs1:FootwearFasteningTypeCode-SLIP_ON_WITHOUT_ELASTIC
	rdf:type        gs1:FootwearFasteningTypeCode ;
	rdfs:label      "Slip On Without Elastic"@en ;
	skos:prefLabel  "SLIP_ON_WITHOUT_ELASTIC" .

gs1:FootwearFasteningTypeCode-SLIP_ON_WITH_ELASTIC
	rdf:type        gs1:FootwearFasteningTypeCode ;
	rdfs:label      "Slip On With Elastic"@en ;
	skos:prefLabel  "SLIP_ON_WITH_ELASTIC" .

gs1:FootwearFasteningTypeCode-STRAP
	rdf:type        gs1:FootwearFasteningTypeCode ;
	rdfs:label      "Strap"@en ;
	skos:prefLabel  "STRAP" .

gs1:FootwearFasteningTypeCode-UNCLASSIFIED
	rdf:type        gs1:FootwearFasteningTypeCode ;
	rdfs:label      "Unclassified"@en ;
	skos:prefLabel  "UNCLASSIFIED" .

gs1:FootwearFasteningTypeCode-UNIDENTIFIED
	rdf:type        gs1:FootwearFasteningTypeCode ;
	rdfs:label      "Unidentified"@en ;
	skos:prefLabel  "UNIDENTIFIED" .

gs1:FootwearFasteningTypeCode-VELCRO
	rdf:type        gs1:FootwearFasteningTypeCode ;
	rdfs:label      "Velcro"@en ;
	skos:prefLabel  "VELCRO" .

gs1:Force
	rdf:type     gs1:MeasurementType ;
	rdfs:comment    "The rate of change of linear momentum of a body on which a force acts. A force acting on a body which is free to move produces an acceleration in the motion of the body.  SI Units: newton"@en ;
	rdfs:label      "Force"@en ;
	skos:prefLabel  "Force" .

gs1:Frequency
	rdf:type  gs1:MeasurementType ;
	rdfs:comment    "The rate of repetition of a periodic oscillation or disturbance; the number of cycles per unit time.  SI Units: hertz"@en ;
	rdfs:label      "Frequency"@en ;
	skos:prefLabel  "Frequency" .

gs1:FreshOrSeawaterFarmedCode-FRESHWATER_FARMED
	rdf:type        gs1:FreshOrSeawaterFarmedCode ;
	rdfs:label      "Freshwater Farmed"@en ;
	skos:prefLabel  "FRESHWATER_FARMED" .

gs1:FreshOrSeawaterFarmedCode-SEAWATER_FARMED
	rdf:type        gs1:FreshOrSeawaterFarmedCode ;
	rdfs:label      "Seawater Farmed"@en ;
	skos:prefLabel  "SEAWATER_FARMED" .

gs1:FreshOrSeawaterFarmedCode-UNCLASSIFIED
	rdf:type        gs1:FreshOrSeawaterFarmedCode ;
	rdfs:label      "Unclassified"@en ;
	skos:prefLabel  "UNCLASSIFIED" .

gs1:FreshOrSeawaterFarmedCode-UNIDENTIFIED
	rdf:type        gs1:FreshOrSeawaterFarmedCode ;
	rdfs:label      "Unidentified"@en ;
	skos:prefLabel  "UNIDENTIFIED" .

gs1:GLN_TypeCode-DIGITAL_LOCATION
	rdf:type        gs1:GLN_TypeCode ;
	rdfs:comment    "An electronic (non-physical) address that is used for communication between computer systems."@en ;
	rdfs:label      "Digital Location"@en ;
	skos:prefLabel  "DIGITAL_LOCATION" .

gs1:GLN_TypeCode-FIXED_PHYSICAL_LOCATION
	rdf:type        gs1:GLN_TypeCode ;
	rdfs:comment    "Fixed physical location - a tangible place that does not change locations and may be represented by an address, coordinates, or other means."@en ;
	rdfs:label      "Fixed Physical Location"@en ;
	skos:prefLabel  "FIXED_PHYSICAL_LOCATION" .

gs1:GLN_TypeCode-FUNCTION
	rdf:type        gs1:GLN_TypeCode ;
	rdfs:comment    "An organisational subdivision or department."@en ;
	rdfs:label      "Function"@en ;
	skos:prefLabel  "FUNCTION" .

gs1:GLN_TypeCode-LEGAL_ENTITY
	rdf:type        gs1:GLN_TypeCode ;
	rdfs:comment    "Any business, government body, department, charity, individual, or institution that has standing in the eyes of the law and has the capacity to enter into agreements or contracts."@en ;
	rdfs:label      "Legal Entity"@en ;
	skos:prefLabel  "LEGAL_ENTITY" .

gs1:GLN_TypeCode-MOBILE_PHYSICAL_LOCATION
	rdf:type        gs1:GLN_TypeCode ;
	rdfs:comment    "Mobile physical location - a tangible place that is expected to change locations and may be represented by an address, coordinates, or other means."@en ;
	rdfs:label      "Mobile Physical Location"@en ;
	skos:prefLabel  "MOBILE_PHYSICAL_LOCATION" .

gs1:GrowingMethodCode-CAGE_FREE
	rdf:type        gs1:GrowingMethodCode ;
	rdfs:comment    "Animal is not confined to a cage."@en ;
	rdfs:label      "Cage Free"@en ;
	skos:prefLabel  "CAGE_FREE" .

gs1:GrowingMethodCode-CLONED_FOODS
	rdf:type        gs1:GrowingMethodCode ;
	rdfs:comment    "Product is a result of genetic engineering."@en ;
	rdfs:label      "Cloned Food"@en ;
	skos:prefLabel  "CLONED_FOODS" .

gs1:GrowingMethodCode-CONVENTIONAL
	rdf:type        gs1:GrowingMethodCode ;
	rdfs:comment    "Foods grown non-organically, either indoors or outdoors without any special processes."@en ;
	rdfs:label      "Conventional"@en ;
	skos:prefLabel  "CONVENTIONAL" .

gs1:GrowingMethodCode-FARM_RAISED
	rdf:type        gs1:GrowingMethodCode ;
	rdfs:comment    "Animal is raised on a farm."@en ;
	rdfs:label      "Farm Raised"@en ;
	skos:prefLabel  "FARM_RAISED" .

gs1:GrowingMethodCode-FIELD_GROWN
	rdf:type        gs1:GrowingMethodCode ;
	rdfs:comment    "Plants Grown Outdoors"@en ;
	rdfs:label      "Field Grown"@en ;
	skos:prefLabel  "FIELD_GROWN" .

gs1:GrowingMethodCode-FLY_FREE
	rdf:type        gs1:GrowingMethodCode ;
	rdfs:comment    "Citrus Grown in an area certified to be free of all Caribbean Fruit Flies based on trappings"@en ;
	rdfs:label      "Fly Free"@en ;
	skos:prefLabel  "FLY_FREE" .

gs1:GrowingMethodCode-FREE_RANGE
	rdf:type        gs1:GrowingMethodCode ;
	rdfs:comment    "A method that animals are allowed to roam with little restriction to their movements."@en ;
	rdfs:label      "Free Range"@en ;
	skos:prefLabel  "FREE_RANGE" .

gs1:GrowingMethodCode-GRASS_FED
	rdf:type        gs1:GrowingMethodCode ;
	rdfs:comment    "Animal is predominately fed grass or forage."@en ;
	rdfs:label      "Grass Fed"@en ;
	skos:prefLabel  "GRASS_FED" .

gs1:GrowingMethodCode-GREENHOUSE
	rdf:type        gs1:GrowingMethodCode ;
	rdfs:comment    "Plants that are grown and cultivated in an indoor covered place."@en ;
	rdfs:label      "Greenhouse"@en ;
	skos:prefLabel  "GREENHOUSE" .

gs1:GrowingMethodCode-HUMANELY_RAISED
	rdf:type        gs1:GrowingMethodCode ;
	rdfs:comment    "A process where animals are raised such that the welfare of the animal is a foremost concern."@en ;
	rdfs:label      "Humanely Raised"@en ;
	skos:prefLabel  "HUMANELY_RAISED" .

gs1:GrowingMethodCode-HYDROPONIC
	rdf:type        gs1:GrowingMethodCode ;
	rdfs:comment    "Plants grown using mineral nutrient solutions instead of soil."@en ;
	rdfs:label      "Hydroponic"@en ;
	skos:prefLabel  "HYDROPONIC" .

gs1:GrowingMethodCode-INTEGRATED_PEST_MANAGEMENT
	rdf:type        gs1:GrowingMethodCode ;
	rdfs:comment    "(IPM) Plants grown using a pest control strategy that uses an array of complimentary methods: mechanical devices, physical devices, genetic, biological, legal, cultural management and chemical management. These methods are done in three stages: prevention, observation, and intervention. It is an ecological approach with a main goal of significantly reducing or eliminating the use of pesticides."@en ;
	rdfs:label      "Integrated Pest Management"@en ;
	skos:prefLabel  "INTEGRATED_PEST_MANAGEMENT" .

gs1:GrowingMethodCode-ORGANIC
	rdf:type        gs1:GrowingMethodCode ;
	rdfs:comment    "Foods grown organically, either indoors or outdoors."@en ;
	rdfs:label      "Organic"@en ;
	skos:prefLabel  "ORGANIC" .

gs1:GrowingMethodCode-SHADE_GROWN
	rdf:type        gs1:GrowingMethodCode ;
	rdfs:comment    "Produce which has been grown under shade or grown under cloth."@en ;
	rdfs:label      "Shade Grown"@en ;
	skos:prefLabel  "SHADE_GROWN" .

gs1:GrowingMethodCode-SUSTAINABLE
	rdf:type        gs1:GrowingMethodCode ;
	rdfs:comemnt    "A method of growing a resource so that the resource is not depleted or permanently damaged" ;
	rdfs:label      "Sustainable"@en ;
	skos:prefLabel  "SUSTAINABLE" .

gs1:GrowingMethodCode-WILD
	rdf:type        gs1:GrowingMethodCode ;
	rdfs:comment    "The animal or plant was not inhibited or prohibited from roving, wandering, and not tamed or domesticated."@en ;
	rdfs:label      "Wild"@en ;
	skos:prefLabel  "WILD" .

gs1:Illuminance
	rdf:type  gs1:MeasurementType ;
	rdfs:comment    "The energy in the form of visible radiation reaching a surface per unit area in unit time; the amount of luminous flux per unit area.  SI Units: lux = 1 lumen per square metre"@en ;
	rdfs:label      "Illuminance"@en ;
	skos:prefLabel  "Illuminance" .

gs1:Inductance
	rdf:type  gs1:MeasurementType ;
	rdfs:comment    "The magnitude of the property of an element or circuit to form a magnetic field and store magnetic energy when carrying a current. The property of an electric circuit or component that causes an electromotive force to be generated in it as a result of a change in the current flowing through the circuit (self inductance) or of a change in the current flowing through a neighbouring circuit with which it is magnetically linked (mutual inductance).  SI Units: henry"@en ;
	rdfs:label      "Inductance"@en ;
	skos:prefLabel  "Inductance" .

gs1:Irradiance
	rdf:type  gs1:MeasurementType ;
	rdfs:comment    "The flux of radiant energy per unit area, especially an area perpendicular to the direction of travel through a medium. A measure of the radiant power per unit area that flows across a surface.  SI Units: watt per square metre"@en ;
	rdfs:label      "Irradiance"@en ;
	skos:prefLabel  "Irradiance" .

gs1:KinematicViscosity
	rdf:type        gs1:MeasurementType ;
	rdfs:comment    "The ratio of the viscosity of a liquid to its density.  SI Units: square metres per second"@en ;
	rdfs:label      "Kinematic viscosity"@en ;
	skos:prefLabel  "KinematicViscosity" .

gs1:Length
	rdf:type    gs1:MeasurementType ;
	rdfs:comment    "The linear magnitude of any thing, as measured end to end.  Length, width, depth, height, diameter are all measured in units of length.  SI Units: metre"@en ;
	rdfs:label      "Length"@en ;
	skos:prefLabel  "Length" .

gs1:LevelOfContainmentCode-CONTAINS
	rdf:type        gs1:LevelOfContainmentCode ;
	rdfs:comment    "Intentionally included in the product."@en ;
	rdfs:label      "Contains"@en ;
	skos:prefLabel  "CONTAINS" .

gs1:LevelOfContainmentCode-FREE_FROM
	rdf:type        gs1:LevelOfContainmentCode ;
	rdfs:comment    "The product is free from the indicated substance."@en ;
	rdfs:label      "Free From"@en ;
	skos:prefLabel  "FREE_FROM" .

gs1:LevelOfContainmentCode-MAY_CONTAIN
	rdf:type        gs1:LevelOfContainmentCode ;
	rdfs:comment    "The substance is not intentionally included, but due to shared production facilities or other reasons, the product may contain the substance."@en ;
	rdfs:label      "May Contain"@en ;
	skos:prefLabel  "MAY_CONTAIN" .

gs1:LinearMomentum
	rdf:type  gs1:MeasurementType ;
	rdfs:comment    "The impulse is the integral over time of the force acting between two colliding bodies. Linear momentum of a body is the product of its mass and its velocity.  SI Units: newton seconds"@en ;
	rdfs:label      "Impulse or linear momentum"@en ;
	skos:prefLabel  "LinearMomentum" .

gs1:LocationID_Type-BIC_FACILITY
	rdf:type        gs1:LocationID_Type ;
	rdfs:comment    "The BIC Facility Code (BFC) began life in the 1980s as the 'LoCode' identifier under ISO 9897. Now a 'child code' of the UN/Locode, the BIC Facility Code is used to identify container facilities such as depots, container yards, container freight stations, M&R vendors and other facilities in the container supply chain. The BIC Facility Code is complementary to the SMDG Ocean Terminal Code, which is also a child code of the UN/Locode. The BIC Facility Code covers container facility types other than ocean terminals."@en ;
	rdfs:label      "BIC Facility Code (BFC) "@en ;
	skos:prefLabel  "BIC_FACILITY" .

gs1:LocationID_Type-CRD_LOCATION_CODE
	rdf:type        gs1:LocationID_Type ;
	rdfs:comment    "The Central Reference File Database (CRD) (formerly known as Central Repository Domain) is a centralised database that stores Location Codes and Company Codes required by European regulation, and makes them available to users. CRD contains the following reference files: - List of Countries (ISO 3166) - The Location Reference File which uniquely identifies physical rail points (e.g. stations, customer sidings, loading places) containing the Location Code (which includes the Country Code) - The Partner Reference File uniquely identifies all rail actors who exchange information (Company Codes); Each company actor must have a unique Company Code assigned by UIC"@en ;
	rdfs:label      "Central Reference File Database (CRD) covers both Locations and Organisations. The Location Reference File uniquely identifies physical rail points (e.g. stations, customer sidings, loading places)"@en ;
	skos:prefLabel  "CRD_LOCATION_CODE" .

gs1:LocationID_Type-ENI_NUMBER
	rdf:type        gs1:LocationID_Type ;
	rdfs:comment    "An ENI number (European Number of Identification or European Vessel Identification Number) is a registration for ships capable of navigating on inland European waters. It is a unique, eight-digit identifier that is attached to a hull for its entire lifetime, independent of the vessel's current name or flag. ENI was introduced by the Inland Transport Committee of the United Nations Economic Commission for Europe in their meeting on 11-13 October 2006 in Geneva. It is based on the Rhine Vessel certification system previously used for ships navigating the Rhine, and is comparable to the IMO ship identification number. "@en ;
	rdfs:label      "An ENI number (European Number of Identification or European Vessel Identification Number)."@en ;
	skos:prefLabel  "ENI_NUMBER" .

gs1:LocationID_Type-FR_SIRET
	rdf:type        gs1:LocationID_Type ;
	rdfs:comment    "The SIRET number, issued by Insee (the National Institute of Statistics and Economic Studies) identifies each establishment that is part of a company in France. There are as many SIRET numbers as there are establishments in the company. An establishment is a geographically located operating or production unit, separated but legally dependent on a company. It is the place where the company's activity is carried out. It is composed of 14 digits: the 9 digits of the SIREN number + the 5 digits of the NIC (internal classification number specific to each establishment)."@en ;
	rdfs:label      "Systme d'identification du rpertoire des tablissements"@en ;
	skos:prefLabel  "FR_SIRET" .

gs1:LocationID_Type-IATA_CODE
	rdf:type        gs1:LocationID_Type ;
	rdfs:comment    "Three-letter geocode designating many airports and metropolitan areas around the world, defined by the International Air Transport Association (IATA). The IATA three-letter codes are a subset of the UN/LOCODE codelist."@en ;
	rdfs:label      "International Air Transport Association (IATA) code"@en ;
	skos:prefLabel  "IATA_CODE" .

gs1:LocationID_Type-IMO_NUMBER
	rdf:type        gs1:LocationID_Type ;
	rdfs:comment    "IMO number is an important identifier given to oil/gas vessels, shipping vessels, and fishing vessels that is painted visibly across the vessel and bolted to the hull"@en ;
	rdfs:label      "International Maritime Organization Number"@en ;
	skos:prefLabel  "IMO_NUMBER" .

gs1:LocationID_Type-ISPS_CODE
	rdf:type        gs1:LocationID_Type ;
	rdfs:comment    "The International Ship and Port Facility Security Code (ISPS Code) is an International code that was conceived following the September 11th 2001 terrorists attacks in the USA.  Its primary purpose is to identify and counter any terrorist threat to the Maritime Industry particularly against ships and ports. The code also serves to improve security against armed robbery, theft and piracy. The code came into force in 2004 and prescribes responsibilities to: 1) Governments 2) Shipping companies 3) Shipboard personnel 4) Port/facility personnel"@en ;
	rdfs:label      "International Ship and Port Facility Security Code (ISPS Code)"@en ;
	skos:prefLabel  "ISPS_CODE" .

gs1:LocationID_Type-ISRS_LOCATION_CODE
	rdf:type        gs1:LocationID_Type ;
	rdfs:comment    "The International Ship Reporting Standard (ISRS) location code is a 20 character alphanumeric code consisting of: - UN country code (2 characters) e.g., NL = Netherlands, - UN location code (3 characters) e.g., RTM = Rotterdam, - Fairway section code (5 characters) e.g., 00102 = Nieuwe Maas, - Object reference code (5 characters) e.g., 66666 = ID administration or terminal code, - Fairway section hectometre e.g., 00050 = hectometres from zero point of Fairway section 00102.  The ISRS Location Code is created once and shall not be changed throughout the lifetime of the object. The Standard / Commission Regulation for Electronic Ship Reporting requires the ISRS Location Code of all objects relevant for reporting of voyages, e.g. ports, terminals, passage points, etc."@en ;
	rdfs:label      "International Ship Reporting Standard or ISRS location code "@en ;
	skos:prefLabel  "ISRS_LOCATION_CODE" .

gs1:LocationID_Type-LOCATION_FOR_INTERNAL_USE_1
	rdf:type        gs1:LocationID_Type ;
	rdfs:comment    "Identification used for internal mapping purposes."@en ;
	rdfs:label      "Location For Internal Use 1"@en ;
	skos:prefLabel  "LOCATION_FOR_INTERNAL_USE_1" .

gs1:LocationID_Type-LOCATION_FOR_INTERNAL_USE_10
	rdf:type        gs1:LocationID_Type ;
	rdfs:comment    "Identification used for internal mapping purposes."@en ;
	rdfs:label      "Location For Internal Use 10"@en ;
	skos:prefLabel  "LOCATION_FOR_INTERNAL_USE_10" .

gs1:LocationID_Type-LOCATION_FOR_INTERNAL_USE_2
	rdf:type        gs1:LocationID_Type ;
	rdfs:comment    "Identification used for internal mapping purposes."@en ;
	rdfs:label      "Location For Internal Use 2"@en ;
	skos:prefLabel  "LOCATION_FOR_INTERNAL_USE_2" .

gs1:LocationID_Type-LOCATION_FOR_INTERNAL_USE_3
	rdf:type        gs1:LocationID_Type ;
	rdfs:comment    "Identification used for internal mapping purposes."@en ;
	rdfs:label      "Location For Internal Use 3"@en ;
	skos:prefLabel  "LOCATION_FOR_INTERNAL_USE_3" .

gs1:LocationID_Type-LOCATION_FOR_INTERNAL_USE_4
	rdf:type        gs1:LocationID_Type ;
	rdfs:comment    "Identification used for internal mapping purposes."@en ;
	rdfs:label      "Location For Internal Use 4"@en ;
	skos:prefLabel  "LOCATION_FOR_INTERNAL_USE_4" .

gs1:LocationID_Type-LOCATION_FOR_INTERNAL_USE_5
	rdf:type        gs1:LocationID_Type ;
	rdfs:comment    "Identification used for internal mapping purposes."@en ;
	rdfs:label      "Location For Internal Use 5"@en ;
	skos:prefLabel  "LOCATION_FOR_INTERNAL_USE_5" .

gs1:LocationID_Type-LOCATION_FOR_INTERNAL_USE_6
	rdf:type        gs1:LocationID_Type ;
	rdfs:comment    "Identification used for internal mapping purposes."@en ;
	rdfs:label      "Location For Internal Use 6"@en ;
	skos:prefLabel  "LOCATION_FOR_INTERNAL_USE_6" .

gs1:LocationID_Type-LOCATION_FOR_INTERNAL_USE_7
	rdf:type        gs1:LocationID_Type ;
	rdfs:comment    "Identification used for internal mapping purposes."@en ;
	rdfs:label      "Location For Internal Use 7"@en ;
	skos:prefLabel  "LOCATION_FOR_INTERNAL_USE_7" .

gs1:LocationID_Type-LOCATION_FOR_INTERNAL_USE_8
	rdf:type        gs1:LocationID_Type ;
	rdfs:comment    "Identification used for internal mapping purposes."@en ;
	rdfs:label      "Location For Internal Use 8"@en ;
	skos:prefLabel  "LOCATION_FOR_INTERNAL_USE_8" .

gs1:LocationID_Type-LOCATION_FOR_INTERNAL_USE_9
	rdf:type        gs1:LocationID_Type ;
	rdfs:comment    "Identification used for internal mapping purposes."@en ;
	rdfs:label      "Location For Internal Use 9"@en ;
	skos:prefLabel  "LOCATION_FOR_INTERNAL_USE_9" .

gs1:LocationID_Type-MMSI_NUMBER
	rdf:type        gs1:LocationID_Type ;
	rdfs:comment    "Maritime Mobile Service Identities (MMSIs) are nine-digit numbers used by maritime digital selective calling (DSC), automatic identification systems (AIS), and certain other equipment to uniquely identify a ship or a coast radio station."@en ;
	rdfs:label      "Maritime Mobile Service Identity number"@en ;
	skos:prefLabel  "MMSI_NUMBER" .

gs1:LocationID_Type-OAR_ID
	rdf:type        gs1:LocationID_Type ;
	rdfs:comment    "Open Apparel Registry ID. A sixteen-digit numbering system which uniquely identities global apparel facilities. The ID consists of a Country code, Origin date (the date the facility first appeared in the registry), a General ID and Check ID. OAR IDs are allocated by the Open Apparel Registry to all facilities contributed to the database for the purposes of enabling industry collaboration and improved identification of factories, as well as powering interoperability between industry databases."@en ;
	rdfs:label      "Open Apparel Registry ID"@en ;
	skos:prefLabel  "OAR_ID" .

gs1:LocationID_Type-OPEN_LOCATION_CODE
	rdf:type        gs1:LocationID_Type ;
	rdfs:comment    "The Open Location Code is a geocode system for identifying an area anywhere on the Earth. It was developed at Google's Zrich engineering office, and released late October 2014. Location codes created by the OLC system are referred to as 'plus codes'."@en ;
	rdfs:label      "Open Location Code"@en ;
	skos:prefLabel  "OPEN_LOCATION_CODE" .

gs1:LocationID_Type-SMDG_CODE
	rdf:type        gs1:LocationID_Type ;
	rdfs:comment    "The SMDG Terminal Code List (TCL) contains codes for container handling terminal facilities that are called by seagoing cargo vessels in maritime transport."@en ;
	rdfs:label      "SMDG Container terminal code"@en ;
	skos:prefLabel  "SMDG_CODE" .

gs1:LocationID_Type-UN_LOCODE
	rdf:type        gs1:LocationID_Type ;
	rdfs:comment    "UN/LOCODE, the United Nations Code for Trade and Transport Locations, is a geographic coding scheme developed and maintained by United Nations Economic Commission for Europe."@en ;
	rdfs:label      "UN/LOCODE"@en ;
	skos:prefLabel  "UN_LOCODE" .

gs1:LocationID_Type-US_CIF_CODE
	rdf:type        gs1:LocationID_Type ;
	rdfs:comment    "The Customer Identification File (CIF) is an industry reference file (for the USA), managed by Railinc, that contains the name, physical mailing and billing address, corporate parent information and a unique 13-character identification code for each location and sub-location of a transportation-carrier customer. Railroads use the identification code to accurately identify customers and their locations, ensuring each party in the transaction is referencing the same physical customer location."@en ;
	rdfs:label      "Customer Identification File (CIF) for RAIL "@en ;
	skos:prefLabel  "US_CIF_CODE" .

gs1:LocationID_Type-US_EST_NUMBER
	rdf:type        gs1:LocationID_Type ;
	rdfs:comment    "All containers of meat, poultry, and egg products must be labeled with a USDA mark of inspection and establishment (EST number), which is assigned to the plant where the product was produced."@en ;
	rdfs:label      "USDA Establishment Number"@en ;
	skos:prefLabel  "US_EST_NUMBER" .

gs1:LocationID_Type-US_FEI
	rdf:type        gs1:LocationID_Type ;
	rdfs:comment    "An FDA Establishment Identification (FEI) number is a unique identifier issued by FDA to track inspections of the regulated establishment or facility. FEI numbers are also used to track GDUFA facility fee payments."@en ;
	rdfs:label      "FDA Establishment Identifier (Facility FEI)"@en ;
	skos:prefLabel  "US_FEI" .

gs1:LocationID_Type-US_HIN_IDENTIFICATION
	rdf:type        gs1:LocationID_Type ;
	rdfs:comment    "The HIN is a unique combination of letters and/or numbers permanently affixed to the vessel. All boats must be registered with the USCG (United States Coast Guard ) in order to track accidents and history of boats. Information about a boat's records may be found by using a vessel documentation search by Hull ID Number (HIN)."@en ;
	rdfs:label      "Hull Identification Number "@en ;
	skos:prefLabel  "US_HIN_IDENTIFICATION" .

gs1:LocationID_Type-US_MINE_ID
	rdf:type        gs1:LocationID_Type ;
	rdfs:comment    "All mines are required to apply for an MSHA mine identification number. An MSHA ID is required for each mine site and must be issued before any operations may begin. A mine ID may be requested by completing the online form or by contacting U.S. district office."@en ;
	rdfs:label      "U.S. Mine ID"@en ;
	skos:prefLabel  "US_MINE_ID" .

gs1:LocationID_Type-US_TCN_CODE
	rdf:type        gs1:LocationID_Type ;
	rdfs:comment    "The Terminal Control Locations Directory lists all approved terminals registered as part of the taxable fuel bulk delivery system. Terminals are listed by the terminal number."@en ;
	rdfs:label      "Terminal Control Number (TCN) / Terminal Locations Directory. USA - IRS."@en ;
	skos:prefLabel  "US_TCN_CODE" .

gs1:Luminance
	rdf:type  gs1:MeasurementType ;
	rdfs:comment    "A measure of the light-emitting intensity of a light source, in a specific direction per unit area of the emitting surface. For a very narrow cone containing the direction, it is the ratio of the luminous flux emitted within that cone to the solid angle of the cone per unit area of the emitting surface.  SI Units: candela per square metre"@en ;
	rdfs:label      "Luminance"@en ;
	skos:prefLabel  "Luminance" .

gs1:LuminousFlux
	rdf:type  gs1:MeasurementType ;
	rdfs:comment    "A measure of the perceived power of light emitted by a source or received by a surface and irrespective of direction, taking into account the sensitivity of the human eye to different wavelengths of light.  SI Units: lumen = 1 candela per steradian"@en ;
	rdfs:label      "Luminous flux"@en ;
	skos:prefLabel  "LuminousFlux" .

gs1:LuminousIntensity
	rdf:type        gs1:MeasurementType ;
	rdfs:comment    "A measure of the light-emitting intensity of a light source, in a specific direction. For a very narrow cone containing the direction, it is the ratio of the luminous flex emitted within that cone to the solid angle of the cone.  SI Units: candela"@en ;
	rdfs:label      "Luminous intensity"@en ;
	skos:prefLabel  "LuminousIntensity" .

gs1:MagneticFlux
	rdf:type  gs1:MeasurementType ;
	rdfs:comment    "A measure of the total magnetic field that passes through a specific area. The surface integral of the product of the permeability of the medium and the magnetic field intensity perpendicular to the surface.  SI Units: weber"@en ;
	rdfs:label      "Magnetic flux"@en ;
	skos:prefLabel  "MagneticFlux" .

gs1:MagneticFluxDensity
	rdf:type        gs1:MeasurementType ;
	rdfs:comment    "The product of the magnetic field strength and the permeability of a material.  SI Units: tesla = weber per square metre"@en ;
	rdfs:label      "Magnetic flux density"@en ;
	skos:prefLabel  "MagneticFluxDensity" .

gs1:MagneticVectorPotential
	rdf:type        gs1:MeasurementType ;
	rdfs:comment    "The potential energy per unit element of current (current multiplied by length).    SI Units: weber per metre  (Joules per ampere metre)"@en ;
	rdfs:label      "Magnetic vector potential"@en ;
	skos:prefLabel  "MagneticVectorPotential" .

gs1:Mass
	rdf:type      gs1:MeasurementType ;
	rdfs:comment    "The quantity of matter in a body. Inertial mass is the measure of the inertia of a body; its resistance to acceleration.  SI Units: kilogram"@en ;
	rdfs:label      "Mass"@en ;
	skos:prefLabel  "Mass" .

gs1:MassConcentration
	rdf:type        gs1:MeasurementType ;
	rdfs:comment    "The mass of the consistutent (or solute) divided by the volume of the mixture (or solvent).  SI Units: kilogram per cubic metre"@en ;
	rdfs:label      "Mass concentration"@en ;
	skos:prefLabel  "MassConcentration" .

gs1:MassFlowRate
	rdf:type  gs1:MeasurementType ;
	rdfs:comment    "The mass of fluid that passes per unit of time.  SI Units: kilogram per second"@en ;
	rdfs:label      "Mass flow rate"@en ;
	skos:prefLabel  "MassFlowRate" .

gs1:MassPerAreaTime
	rdf:type  gs1:MeasurementType ;
	rdfs:comment    "The mass of fluid that passes per unit of time per unit area perpendicular to the flow direction.  SI Units: kilogram per second per square metre"@en ;
	rdfs:label      "Mass flux / Mass per area per time"@en ;
	skos:prefLabel  "MassPerAreaTime" .

gs1:MaturationMethodCode-JET_FRESH
	rdf:type        gs1:MaturationMethodCode ;
	rdfs:comment    "Freshly picked and immediately packed and shipped at mature stage and flown to destination for adequate distribution (i.e. imports from South America, Africa or Europe). Flown by jet to market; the carton will be labelled Jet Fresh, when applicable, stickered Jet Fresh. For the produce industry, most common with berries, stone fruits and pineapples."@en ;
	rdfs:label      "Jet Fresh"@en ;
	skos:prefLabel  "JET_FRESH" .

gs1:MaturationMethodCode-PRECONDITIONED
	rdf:type        gs1:MaturationMethodCode ;
	rdfs:comment    "Product stored at proper temperature prior to shipment to allow ripening and/or colouring, adequate for distribution and/or consumption. Pre-conditioned product is matured to a specific maturity level as a result of ripening through either temperature, gas treatment, humidity or any combination thereof."@en ;
	rdfs:label      "Preconditioned"@en ;
	skos:prefLabel  "PRECONDITIONED" .

gs1:MaturationMethodCode-TREE_VINE_RIPE
	rdf:type        gs1:MaturationMethodCode ;
	rdfs:comment    "Product that is picked at optimum maturity or just shy of. It is almost ripe or ready to eat. This fruit will be shipped immediately (imported = flown) from the pack-house and stickered as Tree or Vine Ripe."@en ;
	rdfs:label      "Tree Vine Ripe"@en ;
	skos:prefLabel  "TREE_VINE_RIPE" .

gs1:MeasurementPrecisionCode-APPROXIMATELY
	rdf:type        gs1:MeasurementPrecisionCode ;
	rdfs:comment    "The method used to analyse the products resulted in approximate value of the nutritional content."@en ;
	rdfs:label      "Approximately"@en ;
	skos:prefLabel  "APPROXIMATELY" .

gs1:MeasurementPrecisionCode-EXACT
	rdf:type        gs1:MeasurementPrecisionCode ;
	rdfs:comment    "The method used to analyse the products resulted in exact value of the nutritional content."@en ;
	rdfs:label      "Exact"@en ;
	skos:prefLabel  "EXACT" .

gs1:MeasurementPrecisionCode-LESS_THAN
	rdf:type        gs1:MeasurementPrecisionCode ;
	rdfs:comment    "To indicate presence when the measurement value is too small to be measured precisely (rule states less than 0.5)."@en ;
	rdfs:label      "Less Than"@en ;
	skos:prefLabel  "LESS_THAN" .

gs1:MemoryCapacity
	rdf:type  gs1:MeasurementType ;
	rdfs:comment    "A measure of the size of a data structure or capacity of a data carrier, typically measured in bits (binary digits), bytes or octets (8 bits) or multiples thereof.  Units: byte"@en ;
	rdfs:label      "Memory capacity"@en ;
	skos:prefLabel  "MemoryCapacity" .

gs1:MolalityOfSolute
	rdf:type  gs1:MeasurementType ;
	rdfs:comment    "The concentration of a solution expressed as the number of moles of dissolved substance per unit mass of solvent.  SI Units: mole per kg"@en ;
	rdfs:label      "Molality of solute"@en ;
	skos:prefLabel  "MolalityOfSolute" .

gs1:MolarEnergy
	rdf:type  gs1:MeasurementType ;
	rdfs:comment    "The ratio of the thermodynamic energy of a chemical compound to the amount of substance (atoms or molecules) contained within it, the amount of substance being measured in moles.  SI Units: joule per mole"@en ;
	rdfs:label      "Molar thermodynamic energy"@en ;
	skos:prefLabel  "MolarEnergy" .

gs1:MolarMass
	rdf:type  gs1:MeasurementType ;
	rdfs:comment    "The ratio of the mass of a chemical compound to the amount of substance (atoms or molecules) contained within it, the amount of substance being measured in moles.  SI Units: kilogram per mole"@en ;
	rdfs:label      "Molar mass"@en ;
	skos:prefLabel  "MolarMass" .

gs1:MolarVolume
	rdf:type  gs1:MeasurementType ;
	rdfs:comment    "The volume occupied by a substance per unit amount of substance at a specified temperature and pressure.  SI Units: cubic metre per mole"@en ;
	rdfs:label      "Molar volume"@en ;
	skos:prefLabel  "MolarVolume" .

gs1:NonbinaryLogicCode-FALSE
	rdf:type        gs1:NonbinaryLogicCode ;
	rdfs:label      "False"@en ;
	skos:prefLabel  "FALSE" .

gs1:NonbinaryLogicCode-NOT_APPLICABLE
	rdf:type        gs1:NonbinaryLogicCode ;
	rdfs:label      "Not Applicable"@en ;
	skos:prefLabel  "NOT_APPLICABLE" .

gs1:NonbinaryLogicCode-TRUE
	rdf:type        gs1:NonbinaryLogicCode ;
	rdfs:label      "True"@en ;
	skos:prefLabel  "TRUE" .

gs1:NonbinaryLogicCode-UNSPECIFIED
	rdf:type        gs1:NonbinaryLogicCode ;
	rdfs:label      "Unspecified"@en ;
	skos:prefLabel  "UNSPECIFIED" .

gs1:NutrientBasisQuantityCode-BY_MEASURE
	rdf:type        gs1:NutrientBasisQuantityCode ;
	rdfs:comment    "Nutrient measurement is based on a measurement value for example grams or ounces."@en ;
	rdfs:label      "By Measure"@en ;
	skos:prefLabel  "BY_MEASURE" .

gs1:NutrientBasisQuantityCode-BY_SERVING
	rdf:type        gs1:NutrientBasisQuantityCode ;
	rdfs:comment    "Nutrient measurement is based on a specified serving amount."@en ;
	rdfs:label      "By Serving"@en ;
	skos:prefLabel  "BY_SERVING" .

gs1:NutritionalClaimTypeCode-ADDITIVE_FREE
	rdf:type        gs1:NutritionalClaimTypeCode ;
	rdfs:comment    "A claim that a food is free from additives. Note the amount that determines containment or lack of containment is based on target market regulations."@en ;
	rdfs:label      "Additive Free"@en ;
	skos:prefLabel  "ADDITIVE_FREE" .

gs1:NutritionalClaimTypeCode-ARTIFICIALLY_SWEETENED
	rdf:type        gs1:NutritionalClaimTypeCode ;
	rdfs:comment    "A claim that a food contains artificial sweeteners. Artificial sweeteners are sugar substitutes that are synthetic."@en ;
	rdfs:label      "Artificially Sweetened"@en ;
	skos:prefLabel  "ARTIFICIALLY_SWEETENED" .

gs1:NutritionalClaimTypeCode-CHOLESTEROL_FREE
	rdf:type        gs1:NutritionalClaimTypeCode ;
	rdfs:comment    "A claim that a food is free from Cholesterol. Note the amount that determines containment or lack of containment is based on target market regulations."@en ;
	rdfs:label      "Cholesterol Free"@en ;
	skos:prefLabel  "CHOLESTEROL_FREE" .

gs1:NutritionalClaimTypeCode-COLOURING_AGENT_FREE
	rdf:type        gs1:NutritionalClaimTypeCode ;
	rdfs:comment    "A claim that a food is free from colouring agents. Note the amount that determines containment or lack of containment is based on target market regulations."@en ;
	rdfs:label      "Colouring Agent Free"@en ;
	skos:prefLabel  "COLOURING_AGENT_FREE" .

gs1:NutritionalClaimTypeCode-CONTAINS_GLYZYRRHIZIN
	rdf:type        gs1:NutritionalClaimTypeCode ;
	rdfs:comment    "A claim that a food contains glyzyrrhizin. Note the amount that determines containment or lack of containment is based on target market regulations."@en ;
	rdfs:label      "Contains Glyzyrrhizin"@en ;
	skos:prefLabel  "CONTAINS_GLYZYRRHIZIN" .

gs1:NutritionalClaimTypeCode-CONTAINS_LIQUORICE
	rdf:type        gs1:NutritionalClaimTypeCode ;
	rdfs:comment    "A claim that a food is contains liquorice. Note the amount that determines containment or lack of containment is based on target market regulations."@en ;
	rdfs:label      "Contains Liquorice"@en ;
	skos:prefLabel  "CONTAINS_LIQUORICE" .

gs1:NutritionalClaimTypeCode-CONTAINS_SOY
	rdf:type        gs1:NutritionalClaimTypeCode ;
	rdfs:comment    "A claim that a food contains soy. Note the amount that determines containment or lack of containment is based on target market regulations."@en ;
	rdfs:label      "Contains Soy"@en ;
	skos:prefLabel  "CONTAINS_SOY" .

gs1:NutritionalClaimTypeCode-EGG_FREE
	rdf:type        gs1:NutritionalClaimTypeCode ;
	rdfs:comment    "A claim that a food is free from egg. Note the amount that determines containment or lack of containment is based on target market regulations."@en ;
	rdfs:label      "Egg Free"@en ;
	skos:prefLabel  "EGG_FREE" .

gs1:NutritionalClaimTypeCode-ENERGY_FREE
	rdf:type        gs1:NutritionalClaimTypeCode ;
	rdfs:comment    "A claim that a food is energy-free, and any claim likely to have the same meaning for the consumer, may only be made where the product contains less than 4kcal (17kj)/100ml. In the case of energy-free foods, the term naturally may be used as a prefix to this claim."@en ;
	rdfs:label      "Energy Free"@en ;
	skos:prefLabel  "ENERGY_FREE" .

gs1:NutritionalClaimTypeCode-ENERGY_REDUCED
	rdf:type        gs1:NutritionalClaimTypeCode ;
	rdfs:comment    "A claim that a food is energy-reduced, and any claim likely to have the same meaning for the consumer, may only be made where the energy value is reduced by at least 30%, with an indication of the characteristic(s), which make(s) the food reduced in its total energy value."@en ;
	rdfs:label      "Energy Reduced"@en ;
	skos:prefLabel  "ENERGY_REDUCED" .

gs1:NutritionalClaimTypeCode-ENRICHED_OR_FORTIFIED_IN_VITAMINS_AND_OR_MINERALS
	rdf:type        gs1:NutritionalClaimTypeCode ;
	rdfs:comment    "A claim that a food is enriched or fortified in vitamins and/or minerals, and any claim likely to have the same meaning for the consumer, may only be made where the product contains the vitamins and/or minerals in at least a significant amount as defined in the Annex of Directive 90/496/EEC."@en ;
	rdfs:label      "Enriched or Fortified in Vitamins Minerals"@en ;
	skos:prefLabel  "ENRICHED_OR_FORTIFIED_IN_VITAMINS_AND_OR_MINERALS" .

gs1:NutritionalClaimTypeCode-FAT_FREE
	rdf:type        gs1:NutritionalClaimTypeCode ;
	rdfs:comment    "A claim that a food is fat-free, and any claim likely to have the same meaning for the consumer, may only be made where the product contains no more than 0.5g of fat per 100g or 100ml. However, claims expressed as X% fat-free shall be prohibited. In the case of foods naturally fat-free, the term naturally may be used as a prefix to this claim."@en ;
	rdfs:label      "Fat Free"@en ;
	skos:prefLabel  "FAT_FREE" .

gs1:NutritionalClaimTypeCode-FREE_FROM_GLUTEN
	rdf:type        gs1:NutritionalClaimTypeCode ;
	rdfs:comment    "A claim that a food is free from Gluten. Any claim likely to have the same meaning for the consumer, may only be made where the product contains an amount less than or equal to 20 mg/kg gluten according to the Commission Regulation (EC) No 41/2009"@en ;
	rdfs:label      "Free From Gluten"@en ;
	skos:prefLabel  "FREE_FROM_GLUTEN" .

gs1:NutritionalClaimTypeCode-GUARANTEED_LACTOSE_FREE
	rdf:type        gs1:NutritionalClaimTypeCode ;
	rdfs:comment    "A claim that a food is regularly analysed to guarantee that the product is free from lactose."@en ;
	rdfs:label      "Guarantee Lactose Free"@en ;
	skos:prefLabel  "GUARANTEED_LACTOSE_FREE" .

gs1:NutritionalClaimTypeCode-HIGH_FIBRE
	rdf:type        gs1:NutritionalClaimTypeCode ;
	rdfs:comment    "A claim that a food is high in fibre, and any claim likely to have the same meaning for the consumer, may only be made where the product contains at least 6g of fibre per 100g or at least 3g of fibre per 100 kcal. In the case of foods naturally high in fibre, the term naturally may be used as a prefix to this claim."@en ;
	rdfs:label      "High Fibre"@en ;
	skos:prefLabel  "HIGH_FIBRE" .

gs1:NutritionalClaimTypeCode-HIGH_PROTEIN
	rdf:type        gs1:NutritionalClaimTypeCode ;
	rdfs:comment    "A claim that a food is high in protein, and any claim likely to have the same meaning for the consumer, may only be made where at least 20% of the energy value of the food is provided by protein. In the case of foods naturally high in protein, the term naturally may be used as a prefix to this claim."@en ;
	rdfs:label      "High Protein"@en ;
	skos:prefLabel  "HIGH_PROTEIN" .

gs1:NutritionalClaimTypeCode-HIGH_VITAMINS_AND_OR_MINERALS
	rdf:type        gs1:NutritionalClaimTypeCode ;
	rdfs:comment    "A claim that a food is high in vitamins and or minerals, and any claim likely to have the same meaning for the consumer, may only be made where the product contains at least twice the value of source of vitamins and minerals. In case of foods naturally high in vitamins and/or minerals, the term naturally may be used as a prefix to this claim."@en ;
	rdfs:label      "High in Vitamins Minerals"@en ;
	skos:prefLabel  "HIGH_VITAMINS_AND_OR_MINERALS" .

gs1:NutritionalClaimTypeCode-LACTOSE_FREE
	rdf:type        gs1:NutritionalClaimTypeCode ;
	rdfs:comment    "A claim that a food is free of lactose. Note the amount that determines containment or lack of containment is based on target market regulations."@en ;
	rdfs:label      "Lactose Free"@en ;
	skos:prefLabel  "LACTOSE_FREE" .

gs1:NutritionalClaimTypeCode-LIGHT_LITE
	rdf:type        gs1:NutritionalClaimTypeCode ;
	rdfs:comment    "A claim stating that a product is light or lite, and any claim likely to have the same meaning for the consumer, shall follow the same conditions as those set for the term reduced; the claim shall also be accompanied by an indication of the characteristic(s) which make the food light or lite."@en ;
	rdfs:label      "Light or Lite"@en ;
	skos:prefLabel  "LIGHT_LITE" .

gs1:NutritionalClaimTypeCode-LOW_ENERGY
	rdf:type        gs1:NutritionalClaimTypeCode ;
	rdfs:comment    "A claim that a food is low in energy, and any claim likely to have the same meaning for the consumer, may only be made where the product contains less than 40 kcal (170 kj)/100g and less than 20kcal (80kj)/100ml. In the case of foods naturally low in energy, the term naturally may be used as a prefix to this claim."@en ;
	rdfs:label      "Low Energy"@en ;
	skos:prefLabel  "LOW_ENERGY" .

gs1:NutritionalClaimTypeCode-LOW_FAT
	rdf:type        gs1:NutritionalClaimTypeCode ;
	rdfs:comment    "A claim that a food is low in fat, and any claim likely to have the same meaning for the consumer, may only be made where the product contains no more than 3g of fat per 100g or 1.5g of fat per 100ml. In the case of foods naturally low in fat, the term naturally may be used as a prefix to this claim."@en ;
	rdfs:label      "Low in Fat"@en ;
	skos:prefLabel  "LOW_FAT" .

gs1:NutritionalClaimTypeCode-LOW_LACTOSE
	rdf:type        gs1:NutritionalClaimTypeCode ;
	rdfs:comment    "A claim that a food is low in lactose. Note the amount that determines containment or lack of containment is based on target market regulations."@en ;
	rdfs:label      "Low in Lactose"@en ;
	skos:prefLabel  "LOW_LACTOSE" .

gs1:NutritionalClaimTypeCode-LOW_PROTEIN
	rdf:type        gs1:NutritionalClaimTypeCode ;
	rdfs:comment    "A claim that a food contains low levels of protein. Note the amount that determines containment or lack of containment is based on target market regulations."@en ;
	rdfs:label      "Low Protein"@en ;
	skos:prefLabel  "LOW_PROTEIN" .

gs1:NutritionalClaimTypeCode-LOW_SATURATED_FAT
	rdf:type        gs1:NutritionalClaimTypeCode ;
	rdfs:comment    "A claim that a food is low in saturated fat, and any claim likely to have the same meaning for the consumer, may only be made where the product contains no more than 1.5g of saturates per 100g for solids or, 0.75g of saturates per 100ml for liquids and in either case saturated fat must not provide more than 10% of energy. In the case of foods naturally low in saturated fat, the term naturally may be used as a prefix to this claim."@en ;
	rdfs:label      "Low in Saturated Fat"@en ;
	skos:prefLabel  "LOW_SATURATED_FAT" .

gs1:NutritionalClaimTypeCode-LOW_SODIUM_SALT
	rdf:type        gs1:NutritionalClaimTypeCode ;
	rdfs:comment    "A claim that a food is low in sodium, and any claim likely to have the same meaning for the consumer, may only be made where the product contains no more than 0.12g of sodium, or the equivalent value for salt, per 100g or per 100ml. In the case of foods naturally low in sodium, the term naturally may be used as a prefix to this claim."@en ;
	rdfs:label      "Low in Sodium"@en ;
	skos:prefLabel  "LOW_SODIUM_SALT" .

gs1:NutritionalClaimTypeCode-LOW_SUGARS
	rdf:type        gs1:NutritionalClaimTypeCode ;
	rdfs:comment    "A claim that a food is low in sugars, and any claim likely to have the same meaning for the consumer, may only be made where the product contains no more than 5g of sugars per 100g or 100ml. In the case of foods naturally low in sugars, the term naturally may be used as a prefix to this claim."@en ;
	rdfs:label      "Low in sugars"@en ;
	skos:prefLabel  "LOW_SUGARS" .

gs1:NutritionalClaimTypeCode-MILK_FREE
	rdf:type        gs1:NutritionalClaimTypeCode ;
	rdfs:comment    "A claim that a food is free from milk. Note the amount that determines containment or lack of containment is based on target market regulations."@en ;
	rdfs:label      "Milk Free"@en ;
	skos:prefLabel  "MILK_FREE" .

gs1:NutritionalClaimTypeCode-MILK_PROTEIN_FREE
	rdf:type        gs1:NutritionalClaimTypeCode ;
	rdfs:comment    "A claim that a food is free from milk proteins. Note the amount that determines containment or lack of containment is based on target market regulations."@en ;
	rdfs:label      "Milk Protein Free"@en ;
	skos:prefLabel  "MILK_PROTEIN_FREE" .

gs1:NutritionalClaimTypeCode-NATURAL_SOURCE_OF_VITAMINS_AND_OR_MINERALS
	rdf:type        gs1:NutritionalClaimTypeCode ;
	rdfs:comment    "A claim that a food is a natural source of vitamins and/or minerals, and any claim likely to have the same meaning for the consumer, may only be made where the product contains at least 15% of the recommended daily allowance specified in the Annex of Council Directive 90/496/EEC per 100 g or 100 ml."@en ;
	rdfs:label      "Natural Source of Vitamins Minerals"@en ;
	skos:prefLabel  "NATURAL_SOURCE_OF_VITAMINS_AND_OR_MINERALS" .

gs1:NutritionalClaimTypeCode-NON_ALCOHOLIC
	rdf:type        gs1:NutritionalClaimTypeCode ;
	rdfs:comment    "A claim that a food contains no alcohol. Note the amount that determines containment or lack of containment is based on target market regulations."@en ;
	rdfs:label      "Non-alcoholic"@en ;
	skos:prefLabel  "NON_ALCOHOLIC" .

gs1:NutritionalClaimTypeCode-NUT_FREE
	rdf:type        gs1:NutritionalClaimTypeCode ;
	rdfs:comment    "A claim that a food is free from nuts. Note the amount that determines containment or lack of containment is based on target market regulations."@en ;
	rdfs:label      "Nut Free"@en ;
	skos:prefLabel  "NUT_FREE" .

gs1:NutritionalClaimTypeCode-PEANUT_FREE
	rdf:type        gs1:NutritionalClaimTypeCode ;
	rdfs:comment    "A claim that a food is free from peanuts. Note the amount that determines containment or lack of containment is based on target market regulations."@en ;
	rdfs:label      "Peanut Free"@en ;
	skos:prefLabel  "PEANUT_FREE" .

gs1:NutritionalClaimTypeCode-PRESERVATIVE_FREE
	rdf:type        gs1:NutritionalClaimTypeCode ;
	rdfs:comment    "A claim that a food is free from preservatives. A preservative is a natural or synthetic substance or chemical that is added to products to prevent decomposition by microbial growth or by undesirable chemical changes. Note the amount that determines containment or lack of containment is based on target market regulations."@en ;
	rdfs:label      "Preservative Free"@en ;
	skos:prefLabel  "PRESERVATIVE_FREE" .

gs1:NutritionalClaimTypeCode-SATURATED_FAT_FREE
	rdf:type        gs1:NutritionalClaimTypeCode ;
	rdfs:comment    "A claim that a food does not contain saturated fat, and any claim likely to have the same meaning for the consumer, may only be made where the product contains no more than 0.1g of saturated fat per 100g or 100ml. In the case of foods naturally saturated fat-free, the term naturally may be used as a prefix to this claim."@en ;
	rdfs:label      "Saturated Fat Free"@en ;
	skos:prefLabel  "SATURATED_FAT_FREE" .

gs1:NutritionalClaimTypeCode-SODIUM_FREE_OR_SALT_FREE
	rdf:type        gs1:NutritionalClaimTypeCode ;
	rdfs:comment    "A claim that a food is sodium-free, and any claim likely to have the same meaning for the consumer, may only be made where the product contains no more than 0.005g of sodium, or the equivalent value for salt, per 100g. In the case of foods naturally sodium-free, the term naturally may be used as a prefix to this claim."@en ;
	rdfs:label      "Sodium of Salt Free"@en ;
	skos:prefLabel  "SODIUM_FREE_OR_SALT_FREE" .

gs1:NutritionalClaimTypeCode-SOURCE_OF_FIBRE
	rdf:type        gs1:NutritionalClaimTypeCode ;
	rdfs:comment    "A claim that a food is a source of fibre, and any claim likely to have the same meaning for the consumer, may only be made where the product contains at least 3g of fibre per 100g or at least 1.5g of fibre per 100kcal. In the case of foods that are naturally sources of fibre, the term naturally may be used as a prefix to this claim."@en ;
	rdfs:label      "Source of Fibre"@en ;
	skos:prefLabel  "SOURCE_OF_FIBRE" .

gs1:NutritionalClaimTypeCode-SOURCE_OF_PROTEIN
	rdf:type        gs1:NutritionalClaimTypeCode ;
	rdfs:comment    "A claim that a food is a source of protein, and any claim likely to have the same meaning for the consumer, may only be made where at least 12% of the energy value of the food is provided by protein. In the case of foods that are naturally sources of protein, the term naturally may be used as a prefix to this claim."@en ;
	rdfs:label      "Source of Protein"@en ;
	skos:prefLabel  "SOURCE_OF_PROTEIN" .

gs1:NutritionalClaimTypeCode-SOY_FREE
	rdf:type        gs1:NutritionalClaimTypeCode ;
	rdfs:comment    "A claim that a food is free from Soy. Note the amount that determines containment or lack of containment is based on target market regulations."@en ;
	rdfs:label      "Soy Free"@en ;
	skos:prefLabel  "SOY_FREE" .

gs1:NutritionalClaimTypeCode-STRONGLY_SALTED
	rdf:type        gs1:NutritionalClaimTypeCode ;
	rdfs:comment    "A claim that a food has a high sodium content. Note the amount that determines containment or lack of containment is based on target market regulations."@en ;
	rdfs:label      "Strongly Salted"@en ;
	skos:prefLabel  "STRONGLY_SALTED" .

gs1:NutritionalClaimTypeCode-SUGARS_FREE
	rdf:type        gs1:NutritionalClaimTypeCode ;
	rdfs:comment    "A claim that a food is sugars-free, and any claim likely to have the same meaning for the consumer, may only be made where the product contains no more than 0.5g of sugars per 100g or 100ml. In the case of foods naturally sugars-free, the term naturally may be used as a prefix to this claim."@en ;
	rdfs:label      "Sugar Free"@en ;
	skos:prefLabel  "SUGARS_FREE" .

gs1:NutritionalClaimTypeCode-SWEETENED_WITH_AGAVE_SYRUP
	rdf:type        gs1:NutritionalClaimTypeCode ;
	rdfs:comment    "A claim that a food is sweetened with syrup from the Agave plant."@en ;
	rdfs:label      "Sweetened With Agave Syrup"@en ;
	skos:prefLabel  "SWEETENED_WITH_AGAVE_SYRUP" .

gs1:NutritionalClaimTypeCode-SWEETENED_WITH_CANE_SUGAR
	rdf:type        gs1:NutritionalClaimTypeCode ;
	rdfs:comment    "A claim that a food is sweetened with sugar from sugar cane."@en ;
	rdfs:label      "Sweetened With Came Sugar"@en ;
	skos:prefLabel  "SWEETENED_WITH_CANE_SUGAR" .

gs1:NutritionalClaimTypeCode-SWEETENED_WITH_CORN_SYRUP
	rdf:type        gs1:NutritionalClaimTypeCode ;
	rdfs:comment    "A claim that a food is sweetened with corn syrup."@en ;
	rdfs:label      "Sweetened With Corn Syrup"@en ;
	skos:prefLabel  "SWEETENED_WITH_CORN_SYRUP" .

gs1:NutritionalClaimTypeCode-SWEETENED_WITH_FRUCTOSE
	rdf:type        gs1:NutritionalClaimTypeCode ;
	rdfs:comment    "A claim that a food is sweetened with fructose."@en ;
	rdfs:label      "Sweetened With Fructose"@en ;
	skos:prefLabel  "SWEETENED_WITH_FRUCTOSE" .

gs1:NutritionalClaimTypeCode-SWEETENED_WITH_FRUIT_JUICE
	rdf:type        gs1:NutritionalClaimTypeCode ;
	rdfs:comment    "A claim that a food is sweetened with fruit juice."@en ;
	rdfs:label      "Sweetened With Fruit Juice"@en ;
	skos:prefLabel  "SWEETENED_WITH_FRUIT_JUICE" .

gs1:NutritionalClaimTypeCode-SWEETENED_WITH_FRUIT_SYRUP
	rdf:type        gs1:NutritionalClaimTypeCode ;
	rdfs:comment    "A claim that a food is sweetened with fruit syrup. Fruit syrup is made from fruit and other ingredients such as sugar, corn syrup and water."@en ;
	rdfs:label      "Sweetened With Fruit Syrup"@en ;
	skos:prefLabel  "SWEETENED_WITH_FRUIT_SYRUP" .

gs1:NutritionalClaimTypeCode-SWEETENED_WITH_HONEY
	rdf:type        gs1:NutritionalClaimTypeCode ;
	rdfs:comment    "A claim that a food is sweetened with honey."@en ;
	rdfs:label      "Sweetened With Honey"@en ;
	skos:prefLabel  "SWEETENED_WITH_HONEY" .

gs1:NutritionalClaimTypeCode-SWEETENED_WITH_MALT
	rdf:type        gs1:NutritionalClaimTypeCode ;
	rdfs:comment    "A claim that a food is sweetened with malt."@en ;
	rdfs:label      "Sweetened With Malt"@en ;
	skos:prefLabel  "SWEETENED_WITH_MALT" .

gs1:NutritionalClaimTypeCode-SWEETENED_WITH_RAW_BEET_SUGAR
	rdf:type        gs1:NutritionalClaimTypeCode ;
	rdfs:comment    "A claim that a food is sweetened with raw sugar derived from the sugar beet."@en ;
	rdfs:label      "Sweetened With Raw Beet Sugar"@en ;
	skos:prefLabel  "SWEETENED_WITH_RAW_BEET_SUGAR" .

gs1:NutritionalClaimTypeCode-SWEETENED_WITH_WHITE_SUGAR
	rdf:type        gs1:NutritionalClaimTypeCode ;
	rdfs:comment    "A claim that a food is sweetened with white sugar. White or granulated sugar is refined sugar (pure white crystalline sucrose) ground to granules or grains."@en ;
	rdfs:label      "Sweetened With White Sugar"@en ;
	skos:prefLabel  "SWEETENED_WITH_WHITE_SUGAR" .

gs1:NutritionalClaimTypeCode-VERY_LOW_GLUTEN
	rdf:type        gs1:NutritionalClaimTypeCode ;
	rdfs:comment    "A claim that a food contains a low level of gluten which is defined as 21 - 100 mg/kg gluten according to the Commission Regulation (EC) No 41/2009"@en ;
	rdfs:label      "Very Low Gluten"@en ;
	skos:prefLabel  "VERY_LOW_GLUTEN" .

gs1:NutritionalClaimTypeCode-VERY_LOW_SODIUM_SALT
	rdf:type        gs1:NutritionalClaimTypeCode ;
	rdfs:comment    "A claim that a food is very low in sodium, and any claim likely to have the same meaning for the consumer, may only be made where the product contains no more than 0.04g of sodium, or the equivalent value for salt, per 100g or per 100 ml. In the case of foods naturally very low in sodium, the term naturally may be used as a prefix to this claim."@en ;
	rdfs:label      "Very Low in Sodium Salt"@en ;
	skos:prefLabel  "VERY_LOW_SODIUM_SALT" .

gs1:NutritionalClaimTypeCode-WHEAT_FREE
	rdf:type        gs1:NutritionalClaimTypeCode ;
	rdfs:comment    "A claim that a food is free from wheat. Note the amount that determines containment or lack of containment is based on target market regulations."@en ;
	rdfs:label      "Wheat Free"@en ;
	skos:prefLabel  "WHEAT_FREE" .

gs1:NutritionalClaimTypeCode-WITH_NO_ADDED_SUGARS
	rdf:type        gs1:NutritionalClaimTypeCode ;
	rdfs:comment    "A claim stating that sugar has not been added to a food, and any claim likely to have the same meaning for the consumer, may only be made where the product does not contain any added mono- or disaccharides or any other food used for its sweetening properties."@en ;
	rdfs:label      "No Added Sugar"@en ;
	skos:prefLabel  "WITH_NO_ADDED_SUGARS" .

gs1:OfferRedemptionTypeCode-COUPON_CODE
	rdf:type        gs1:OfferRedemptionTypeCode ;
	rdfs:comment    "Offer available as a code that can be entered to redeem the coupon or voucher."@en ;
	rdfs:label      "Coupon Code"@en ;
	skos:prefLabel  "COUPON_CODE" .

gs1:OfferRedemptionTypeCode-GIFT_CARD
	rdf:type        gs1:OfferRedemptionTypeCode ;
	rdfs:comment    "A prepaid stored-value money card."@en ;
	rdfs:label      "Gift Card"@en ;
	skos:prefLabel  "GIFT_CARD" .

gs1:OfferRedemptionTypeCode-REBATE
	rdf:type        gs1:OfferRedemptionTypeCode ;
	rdfs:comment    "A partial refund upon purchase of a product."@en ;
	rdfs:label      "Rebate"@en ;
	skos:prefLabel  "REBATE" .

gs1:OfferRedemptionTypeCode-SALE
	rdf:type        gs1:OfferRedemptionTypeCode ;
	rdfs:comment    "Offer available as a reduced sales price on a product."@en ;
	rdfs:label      "Sale"@en ;
	skos:prefLabel  "SALE" .

gs1:OfferRedemptionTypeCode-SINGLE_USE_CODE
	rdf:type        gs1:OfferRedemptionTypeCode ;
	rdfs:comment    "Offer available as a code that can be entered once to redeem the coupon."@en ;
	rdfs:label      "Single Use Code"@en ;
	skos:prefLabel  "SINGLE_USE_CODE" .

gs1:OrganicClaimAgencyCode-BFA
	rdf:type        gs1:OrganicClaimAgencyCode ;
	rdfs:comment    "Biological Farmers of Australia"@en ;
	rdfs:label      "Biological Farmers of Australia"@en ;
	skos:prefLabel  "BFA" .

gs1:OrganicClaimAgencyCode-BIOLAND
	rdf:type        gs1:OrganicClaimAgencyCode ;
	rdfs:comment    "Bioland: The leading organic farmers' association in Germany for the economy of organic-based businesses without synthetic pesticides and synthetic chemical nitrogen fertilizer. The animals are kept humanely and processed food carefully. This provides an environmentally sound and sustainable food production. http://www.bioland.de."@en ;
	rdfs:label      "Bioland"@en ;
	skos:prefLabel  "BIOLAND" .

gs1:OrganicClaimAgencyCode-DEMETER_BUND
	rdf:type        gs1:OrganicClaimAgencyCode ;
	rdfs:comment    "The Demeter movement as an entrepreneurial network promotes the development of bio-dynamic economy, to secure the livelihoods of the world and to strengthen the positive people in his ministry. In cooperation contribute producers, processors, traders and consumers in partnership to shape the market."@en ;
	rdfs:label      "Demeter-Bund"@en ;
	skos:prefLabel  "DEMETER_BUND" .

gs1:OrganicClaimAgencyCode-DEMETER_INTERNATIONAL
	rdf:type        gs1:OrganicClaimAgencyCode ;
	rdfs:comment    "Demeter International Demeter-International e. V. is a non profit organisation and its member organisations work together in the spirit of an international confederation with democratic principles. Membership requires a functioning Demeter certification programme. Same as GS1 Code 16"@en ;
	rdfs:label      "Demeter International"@en ;
	skos:prefLabel  "DEMETER_INTERNATIONAL" .

gs1:OrganicClaimAgencyCode-ECOLAND
	rdf:type        gs1:OrganicClaimAgencyCode ;
	rdfs:comment    "Ecoland is a membership organisation whose members elect a governing Board which is responsible for the design and implementation of the organic certification system."@en ;
	rdfs:label      "Ecoland"@en ;
	skos:prefLabel  "ECOLAND" .

gs1:OrganicClaimAgencyCode-ECOVIN
	rdf:type        gs1:OrganicClaimAgencyCode ;
	rdfs:comment    "ECOVIN Federation Organic Viticulture Association: ECOVIN largest merger in 1985 as ecologically-working wine estates in Germany was founded. Approximately 220 member companies currently manage 1,600 hectares of vineyards in 11 German wine-growing areas. Same as GS1 code 14"@en ;
	rdfs:label      "Ecovin"@en ;
	skos:prefLabel  "ECOVIN" .

gs1:OrganicClaimAgencyCode-EPA
	rdf:type        gs1:OrganicClaimAgencyCode ;
	rdfs:comment    "US Environmental Protection Agency. Same as GS1 Code 1"@en ;
	rdfs:label      "US Environmental Protection Agency"@en ;
	skos:prefLabel  "EPA" .

gs1:OrganicClaimAgencyCode-FDA
	rdf:type        gs1:OrganicClaimAgencyCode ;
	rdfs:comment    "FDA US Food and Drug Agency"@en ;
	rdfs:label      "FDA US Food and Drug Agency"@en ;
	skos:prefLabel  "FDA" .

gs1:OrganicClaimAgencyCode-FSA
	rdf:type        gs1:OrganicClaimAgencyCode ;
	rdfs:comment    "UK Food Standards Agency"@en ;
	rdfs:label      "FSA"@en ;
	skos:prefLabel  "FSA" .

gs1:OrganicClaimAgencyCode-GAA
	rdf:type        gs1:OrganicClaimAgencyCode ;
	rdfs:comment    "GAA is a diverse farming association for farmers, processors and traders inside.Focal point is Germany. GAA is a special design for the structure of the organic farming. Biokreis- The Biokreis is an association for organic farming. Currently more than 800 farms, 80 and 200 processors, consumers are members of Biokreis, committed to working together on more than 33,000 for organic and sustainable farming."@en ;
	rdfs:label      "GAA"@en ;
	skos:prefLabel  "GAA" .

gs1:OrganicClaimAgencyCode-IFOA
	rdf:type        gs1:OrganicClaimAgencyCode ;
	rdfs:comment    "International Foundation for Organic Agriculture"@en ;
	rdfs:label      "International Foundation for Organic Agriculture"@en ;
	skos:prefLabel  "IFOA" .

gs1:OrganicClaimAgencyCode-IFOAM
	rdf:type        gs1:OrganicClaimAgencyCode ;
	rdfs:comment    "The International Federation of Organic Agriculture Movements (IFOAM) is a grassroots and democratic organization that currently unites 750 member organizations in 116 countries. Same as GS1 code 15"@en ;
	rdfs:label      "International Federation of Organic Agriculture Movements."@en ;
	skos:prefLabel  "IFOAM" .

gs1:OrganicClaimAgencyCode-NATURLAND
	rdf:type        gs1:OrganicClaimAgencyCode ;
	rdfs:comment    "Naturland - Naturland is active the world over in promoting organic agriculture. Its members are farmers who produce a wide range of valuable products: coffee from Mexico and Peru, olive oil from Greece, tea from the slopes of India's mountains, pineapple and other tropical fruit from Uganda, spices from Sri Lanka. Organic agriculture safeguards the existence of smallholders and helps with the sustainable management of what are often fragile ecosystems. On a global scale, over 50,000 Naturland farmers are cultivating an area of over 142,000 hectares.Same as GS1 Code 12"@en ;
	rdfs:label      "Naturland"@en ;
	skos:prefLabel  "NATURLAND" .

gs1:OrganicClaimAgencyCode-QAI
	rdf:type        gs1:OrganicClaimAgencyCode ;
	rdfs:comment    "Quality Assurance International. QAI is a leading USDA-accredited organic product certifying agency."@en ;
	rdfs:label      "Quality Assurance International"@en ;
	skos:prefLabel  "QAI" .

gs1:OrganicClaimAgencyCode-SUDITIROL
	rdf:type        gs1:OrganicClaimAgencyCode ;
	rdfs:comment    "Bioland Association of South Tyrol The Association of South Tyrol is the largest organic association for organic farmers having to farmers in South Tyrol and the only active in association with a national association office Terlan."@en ;
	rdfs:label      "Sudtirol Bioland"@en ;
	skos:prefLabel  "SUDITIROL" .

gs1:OrganicClaimAgencyCode-USDA
	rdf:type        gs1:OrganicClaimAgencyCode ;
	rdfs:comment    "US Department of Agriculture."@en ;
	rdfs:label      "US Department of Agriculture"@en ;
	skos:prefLabel  "USDA" .

gs1:OrganizationID_Type-AU_ABN
	rdf:type        gs1:OrganizationID_Type ;
	rdfs:comment    "The Australian Business Number is a unique 11-digit identifier issued by the Australian Business Register which is operated by the Australian Taxation Office."@en ;
	rdfs:label      "Australian Business Number"@en ;
	skos:prefLabel  "AU_ABN" .

gs1:OrganizationID_Type-AU_ACN
	rdf:type        gs1:OrganizationID_Type ;
	rdfs:comment    "An Australian Company Number is a unique identifier required by every company registered under Australia's Corporations Act 2001. The ACN is a nine-digit number issued by the Australian Securities & Investments Commission to every Australian company."@en ;
	rdfs:label      "Australian Company Number"@en ;
	skos:prefLabel  "AU_ACN" .

gs1:OrganizationID_Type-CRD_PARTNER_CODE
	rdf:type        gs1:OrganizationID_Type ;
	rdfs:comment    "The Central Reference File Database (CRD), formerly known as Central Repository Domain is a centralised database that stores Location Codes and Company Codes required by European regulation, and makes them available to users. CRD contains the following reference files: - List of Countries (ISO 3166) - The Location Reference File which uniquely identifies physical rail points (e.g. stations, customer sidings, loading places) containing the Location Code (which includes the Country Code) - The Partner Reference File uniquely identifies all rail actors who exchange information (Company Codes); Each company actor must have a unique Company Code assigned by UIC"@en ;
	rdfs:label      "Central Reference File Database (CRD) covers both Locations and Organisations. The Partner Reference File uniquely identifies all rail actors who exchange information (Company Codes).  Rail context"@en ;
	skos:prefLabel  "CRD_PARTNER_CODE" .

gs1:OrganizationID_Type-CRN
	rdf:type        gs1:OrganizationID_Type ;
	rdfs:comment    "A company registration number is a unique combination of numbers and/or letters. The company registration number (also known as the company number, registration number or simply in its abbreviated form) is used to identify a company and verify that it is an entity registered within the national registry for companies or enterprises. This value is generic and is not associated to any specific region."@en ;
	rdfs:label      "Company Registration Number (CRN)"@en ;
	skos:prefLabel  "CRN" .

gs1:OrganizationID_Type-DID
	rdf:type        gs1:OrganizationID_Type ;
	rdfs:comment    "A globally unique persistent identifier that does not require a centralized registration authority because it is generated and/or registered cryptographically. The generic format of a DID is defined in the DID Core specification [DID-CORE]. A specific DID scheme is defined in a DID method specification. Many (but not all) DID methods make use of distributed ledger technology (DLT) or some other form of decentralized network."@en ;
	rdfs:label      "Decentralized identifier"@en ;
	skos:prefLabel  "DID" .

gs1:OrganizationID_Type-DUNS
	rdf:type        gs1:OrganizationID_Type ;
	rdfs:comment    "Data Universal Numbering System. It is a nine-digit numbering system which uniquely identifies an individual business. The DUNS number is a nine-digit number issued by Dun & Bradstreet assigned to each business location in the D&B database having a unique, separate, and distinct operation for the purpose of identifying them. A DUNS number is also a way in which separate corporate entities, having no official relationship, can be branded as one by sharing one DUNS number among the affiliated comp"@en ;
	rdfs:label      "DUNS"@en ;
	skos:prefLabel  "DUNS" .

gs1:OrganizationID_Type-DUNS_PLUS_FOUR
	rdf:type        gs1:OrganizationID_Type ;
	rdfs:comment    "The DUNS+4 refers to the DUNS number assigned by Dun and Bradstreet, plus a 4-character suffix that is assigned by the vendor to establish additional Central Contractor Registration (CCR) database records for identifying alternative electronic funds transfer (EFT) accounts for the same vendor located at the same physical address. Dun and Bradstreet has no affiliation with the 4-character suffix."@en ;
	rdfs:label      "DUNS+4"@en ;
	skos:prefLabel  "DUNS_PLUS_FOUR" .

gs1:OrganizationID_Type-EORI
	rdf:type        gs1:OrganizationID_Type ;
	rdfs:comment    "Businesses and people wishing to trade with the EU must, use the EORI number as an identification number in all customs procedures when exchanging information with Customs - https://ec.europa.eu/taxation_customs/dds2/eos/eori_home.jsp?Lang=en"@en ;
	rdfs:label      "Economic Operators Registration and Identification number"@en ;
	skos:prefLabel  "EORI" .

gs1:OrganizationID_Type-EO_ID
	rdf:type        gs1:OrganizationID_Type ;
	rdfs:comment    "A type of identifier in the format of the invariant set of ISO646:1991 used in accordance with the EU Implementing Regulation 2018/574 to identify an economic operator."@en ;
	rdfs:label      "Economic Operator Identifier"@en ;
	skos:prefLabel  "EO_ID" .

gs1:OrganizationID_Type-EU_VAT_IDENTIFICATION_NUMBER
	rdf:type        gs1:OrganizationID_Type ;
	rdfs:comment    "An identifier used to identify companies for value added tax purposes in the European Union. Link: https://ec.europa.eu/taxation_customs/vies/faqvies.do#item_11"@en ;
	rdfs:label      "EU VAT Identification Number"@en ;
	skos:prefLabel  "EU_VAT_IDENTIFICATION_NUMBER" .

gs1:OrganizationID_Type-FR_RCS
	rdf:type        gs1:OrganizationID_Type ;
	rdfs:comment    "The RCS (Registre du commerce et des socits), otherwise known as the Greffe, is the registry for the company accounts and by-laws of all companies in France."@en ;
	rdfs:label      "Registre du commerce et des socits"@en ;
	skos:prefLabel  "FR_RCS" .

gs1:OrganizationID_Type-FR_SIREN
	rdf:type        gs1:OrganizationID_Type ;
	rdfs:comment    "The SIREN number, issued by Insee (the National Institute of Statistics and Economic Studies) is the unique identification number of each company. It is a number that allows each company to be identified by the administrations in France. The SIREN number also constitutes the first 9 digits of the SIRET number."@en ;
	rdfs:label      "Systme d'identification du rpertoire des entreprises"@en ;
	skos:prefLabel  "FR_SIREN" .

gs1:OrganizationID_Type-IMO_COMPANY_NUMBER
	rdf:type        gs1:OrganizationID_Type ;
	rdfs:comment    "IMO registers all vessels subject to the SOLAS convention. IMO also records the Owner, Operator, Manager and Group Beneficial Owner. For that purpose they also record the Companies acting in these roles using the IMO Company Number"@en ;
	rdfs:label      "International Maritime Organisation (IMO) Company Number"@en ;
	skos:prefLabel  "IMO_COMPANY_NUMBER" .

gs1:OrganizationID_Type-LEI
	rdf:type        gs1:OrganizationID_Type ;
	rdfs:comment    "The Legal Entity Identifier (LEI) is a 20-character, alpha-numeric code based on the ISO 17442 standard developed by the International Organization for Standardization (ISO). It connects to key reference information that enables clear and unique identification of legal entities participating in financial transactions"@en ;
	rdfs:label      " Legal Entity Identifier (LEI)"@en ;
	skos:prefLabel  "LEI" .

gs1:OrganizationID_Type-NL_KVK_NUMBER
	rdf:type        gs1:OrganizationID_Type ;
	rdfs:comment    "When registering with the Netherlands Chamber of Commerce KVK, a business is listed in the Dutch Commercial Register or Handelsregister (HR) as it is called in the Netherlands. The businesses are then given a 8-digit KVK number. This number serves to prove an organisation is a registered business."@en ;
	rdfs:label      "Kamer van Koophandel (KVK) number"@en ;
	skos:prefLabel  "NL_KVK_NUMBER" .

gs1:OrganizationID_Type-NL_OIN_NUMBER
	rdf:type        gs1:OrganizationID_Type ;
	rdfs:comment    "The Organization Identification Number (OIN) is a unique number assigned to organizations by Logius, the digital government service of the Netherlands Ministry of the Interior and Kingdom Relations, to identify, authenticate and/or authorise themselves in digital messaging within and with the government."@en ;
	rdfs:label      "Organisatie-identificatienummer (OIN number)"@en ;
	skos:prefLabel  "NL_OIN_NUMBER" .

gs1:OrganizationID_Type-NZ_GST_NUMBER
	rdf:type        gs1:OrganizationID_Type ;
	rdfs:comment    "An identifier used to identify companies for goods and services tax purposes in New Zealand."@en ;
	rdfs:label      "New Zealand GST Number"@en ;
	skos:prefLabel  "NZ_GST_NUMBER" .

gs1:OrganizationID_Type-NZ_IRD_NUMBER
	rdf:type        gs1:OrganizationID_Type ;
	rdfs:comment    "An identifier used to identify companies for tax purposes in New Zealand."@en ;
	rdfs:label      "New Zealand Inland Revenue Identification Number"@en ;
	skos:prefLabel  "NZ_IRD_NUMBER" .

gs1:OrganizationID_Type-ORG_FOR_INTERNAL_USE_1
	rdf:type        gs1:OrganizationID_Type ;
	rdfs:comment    "Identification used for internal mapping purposes."@en ;
	rdfs:label      "Organization For Internal Use 1"@en ;
	skos:prefLabel  "ORG_FOR_INTERNAL_USE_1" .

gs1:OrganizationID_Type-ORG_FOR_INTERNAL_USE_10
	rdf:type        gs1:OrganizationID_Type ;
	rdfs:comment    "Identification used for internal mapping purposes."@en ;
	rdfs:label      "Organization For Internal Use 10"@en ;
	skos:prefLabel  "ORG_FOR_INTERNAL_USE_10" .

gs1:OrganizationID_Type-ORG_FOR_INTERNAL_USE_2
	rdf:type        gs1:OrganizationID_Type ;
	rdfs:comment    "Identification used for internal mapping purposes."@en ;
	rdfs:label      "Organization For Internal Use 2"@en ;
	skos:prefLabel  "ORG_FOR_INTERNAL_USE_2" .

gs1:OrganizationID_Type-ORG_FOR_INTERNAL_USE_3
	rdf:type        gs1:OrganizationID_Type ;
	rdfs:comment    "Identification used for internal mapping purposes."@en ;
	rdfs:label      "Organization For Internal Use 3"@en ;
	skos:prefLabel  "ORG_FOR_INTERNAL_USE_3" .

gs1:OrganizationID_Type-ORG_FOR_INTERNAL_USE_4
	rdf:type        gs1:OrganizationID_Type ;
	rdfs:comment    "Identification used for internal mapping purposes."@en ;
	rdfs:label      "Organization For Internal Use 4"@en ;
	skos:prefLabel  "ORG_FOR_INTERNAL_USE_4" .

gs1:OrganizationID_Type-ORG_FOR_INTERNAL_USE_5
	rdf:type        gs1:OrganizationID_Type ;
	rdfs:comment    "Identification used for internal mapping purposes."@en ;
	rdfs:label      "Organization For Internal Use 5"@en ;
	skos:prefLabel  "ORG_FOR_INTERNAL_USE_5" .

gs1:OrganizationID_Type-ORG_FOR_INTERNAL_USE_6
	rdf:type        gs1:OrganizationID_Type ;
	rdfs:comment    "Identification used for internal mapping purposes."@en ;
	rdfs:label      "Organization For Internal Use 6"@en ;
	skos:prefLabel  "ORG_FOR_INTERNAL_USE_6" .

gs1:OrganizationID_Type-ORG_FOR_INTERNAL_USE_7
	rdf:type        gs1:OrganizationID_Type ;
	rdfs:comment    "Identification used for internal mapping purposes."@en ;
	rdfs:label      "Organization For Internal Use 7"@en ;
	skos:prefLabel  "ORG_FOR_INTERNAL_USE_7" .

gs1:OrganizationID_Type-ORG_FOR_INTERNAL_USE_8
	rdf:type        gs1:OrganizationID_Type ;
	rdfs:comment    "Identification used for internal mapping purposes."@en ;
	rdfs:label      "Organization For Internal Use 8"@en ;
	skos:prefLabel  "ORG_FOR_INTERNAL_USE_8" .

gs1:OrganizationID_Type-ORG_FOR_INTERNAL_USE_9
	rdf:type        gs1:OrganizationID_Type ;
	rdfs:comment    "Identification used for internal mapping purposes."@en ;
	rdfs:label      "Organization For Internal Use 9"@en ;
	skos:prefLabel  "ORG_FOR_INTERNAL_USE_9" .

gs1:OrganizationID_Type-PHYTOSANITARY_REGISTRATION_NUMBER
	rdf:type        gs1:OrganizationID_Type ;
	rdfs:comment    "Within the European Union, the phytosanitary registration number identifies an organisation responsible for introducing, or moving plants, plant products and other objects, for which a phytosanitary certificate or a plant passport is required to comply with EU regulation. A phytosanitary registration number is not the same as a phytosanitary certificate number, which identifies the certificate issued to the organisation exporting items subject to phytosanitary processes."@en ;
	rdfs:label      "Phytosanitary registration number "@en ;
	skos:prefLabel  "PHYTOSANITARY_REGISTRATION_NUMBER" .

gs1:OrganizationID_Type-TIN
	rdf:type        gs1:OrganizationID_Type ;
	rdfs:comment    "The taxpayer identification number (TIN) is an identifying number used for tax purposes in the United States and in other countries under the Common Reporting Standard. The unique identifier is assigned to the Account Holder by the tax administration in the Account Holder's jurisdiction of tax residence. It is a unique combination of letters and/or numbers used to identify an individual or entity for the purposes of administering the tax laws of that jurisdiction.  In some countries where the TIN is not used a national identification number, national identity number, or national insurance number is used by the governments of countries as a means of tracking their citizens, permanent residents, and temporary residents for the purposes of work, taxation, government benefits, health care, and other governmentally related functions."@en ;
	rdfs:label      "Taxpayer Identification Number"@en ;
	skos:prefLabel  "TIN" .

gs1:OrganizationID_Type-UK_CRN
	rdf:type        gs1:OrganizationID_Type ;
	rdfs:comment    "A company registration number is a unique combination of numbers and, in some cases, letters. The company registration number (also known as the company number, registration number or simply abbreviated to CRN) is used to identify a company and verify that it is an entity registered with Companies House (the executive agency of the British Government reponsible for providing registered company information to the public)."@en ;
	rdfs:label      "U.K. Company Registration Number "@en ;
	skos:prefLabel  "UK_CRN" .

gs1:OrganizationID_Type-US_498_ID
	rdf:type        gs1:OrganizationID_Type ;
	rdfs:comment    "A Service Provider Identification Number (SPIN) is a unique nine-digit number assigned to service providers by USAC when an FCC Form 498 is filed. This number is also known as the service provider's 498 ID."@en ;
	rdfs:label      "Service Provider and Billed Entity Identification Number (FCC Form 498 ID)"@en ;
	skos:prefLabel  "US_498_ID" .

gs1:OrganizationID_Type-US_499_FILER_ID
	rdf:type        gs1:OrganizationID_Type ;
	rdfs:comment    "The FCC Form 499 Filer Database is an identification system for all interstate telecommunications carriers, all interconnected VoIP providers, and certain other providers of interstate telecommunications.  The Universal Service Fund helps communities across the country afford telecommunications and advanced services."@en ;
	rdfs:label      "499 Filer ID"@en ;
	skos:prefLabel  "US_499_FILER_ID" .

gs1:OrganizationID_Type-US_BEA_ID
	rdf:type        gs1:OrganizationID_Type ;
	rdfs:comment    "The BEA foreign direct investment identification number is assigned to a new U.S. affiliate after their initial report has been accepted by the BEA. Filed by mail or facsimile, initial reports are due within 30 days of the end of the quarter in which the U.S. entity became foreign owned."@en ;
	rdfs:label      "BEA Foreign Direct Investment Identification Number"@en ;
	skos:prefLabel  "US_BEA_ID" .

gs1:OrganizationID_Type-US_CAGE
	rdf:type        gs1:OrganizationID_Type ;
	rdfs:comment    "The Defense Logistics Agency (DLA) Commercial and Government Entity. A CAGE code is a five character alpha-numeric identifier assigned to entities located IN the United States and its territories"@en ;
	rdfs:label      "Commercial and Government Entity"@en ;
	skos:prefLabel  "US_CAGE" .

gs1:OrganizationID_Type-US_CID
	rdf:type        gs1:OrganizationID_Type ;
	rdfs:comment    "A company identification number, or CID, is given to a company when it is formed and the articles of organization or incorporation are approved by the U.S. Secretary of State. The CID is an important step when establishing a new company as it acts as a way to track important company information."@en ;
	rdfs:label      "Company Identifier (CID)"@en ;
	skos:prefLabel  "US_CID" .

gs1:OrganizationID_Type-US_CRD
	rdf:type        gs1:OrganizationID_Type ;
	rdfs:comment    "Every stockbroker (registered representative) licensed to sell securities in the U.S. must have a CRD number, which is administered by the Financial Industry Regulatory Authority (FINRA)."@en ;
	rdfs:label      "Central Registration Depository (CRD) Numbers"@en ;
	skos:prefLabel  "US_CRD" .

gs1:OrganizationID_Type-US_DEA
	rdf:type        gs1:OrganizationID_Type ;
	rdfs:comment    "A DEA number (DEA Registration Number) is an identifier assigned to a health care provider (such as a physician, physician assistant, nurse practitioner, optometrist, podiatrist, dentist, or veterinarian) by the United States Drug Enforcement Administration allowing them to write prescriptions for controlled substances."@en ;
	rdfs:label      "Drug Enforcement Administration (DEA) Number"@en ;
	skos:prefLabel  "US_DEA" .

gs1:OrganizationID_Type-US_DODAAC
	rdf:type        gs1:OrganizationID_Type ;
	rdfs:comment    "Is a six position code that uniquely identifies a Department of Defense unit, activity, or organization that has the authority to requisition, contract for, receive, have custody of, issue, or ship DoD assets, or fund/pay bills for materials and/or services."@en ;
	rdfs:label      "Department of Defense Activity Address Code"@en ;
	skos:prefLabel  "US_DODAAC" .

gs1:OrganizationID_Type-US_EIN
	rdf:type        gs1:OrganizationID_Type ;
	rdfs:comment    "The U.S. Employer Identification Number, also known as the Federal Employer Identification Number or the Federal Tax Identification Number, is a unique nine-digit number assigned by the Internal Revenue Service to business entities operating in the United States for the purposes of identification."@en ;
	rdfs:label      "Employer Identification Number (EIN)"@en ;
	skos:prefLabel  "US_EIN" .

gs1:OrganizationID_Type-US_EPA_ID
	rdf:type        gs1:OrganizationID_Type ;
	rdfs:comment    "This number, issued either by the U. S. Environmental Protection Agency (U.S. EPA ID Number), or by DTSC (California ID Number), identifies each handler of hazardous waste on hazardous waste manifests and other paperwork."@en ;
	rdfs:label      "EPA Identification Number"@en ;
	skos:prefLabel  "US_EPA_ID" .

gs1:OrganizationID_Type-US_FCC_FRN
	rdf:type        gs1:OrganizationID_Type ;
	rdfs:comment    "An FRN, or FCC registration number, is a 10-digit number that is assigned to a business or individual registering with the FCC.  The FCC will use the FRN to determine if all of a registrant's fees have been paid."@en ;
	rdfs:label      "FCC Registration Number (FRN)"@en ;
	skos:prefLabel  "US_FCC_FRN" .

gs1:OrganizationID_Type-US_FDIC
	rdf:type        gs1:OrganizationID_Type ;
	rdfs:comment    "The FDIC Certificate ID is a unique number assigned to each depository institution by the Federal Deposit Insurance Corporation (FDIC)."@en ;
	rdfs:label      "Federal Deposit Insurance Corporation (FDIC) Certificate Number"@en ;
	skos:prefLabel  "US_FDIC" .

gs1:OrganizationID_Type-US_FHFA_ID
	rdf:type        gs1:OrganizationID_Type ;
	rdfs:comment    "FHFA ID number is the number assigned to a member by FHFA and used by FHFA and the Banks to identify a particular member."@en ;
	rdfs:label      "FHFA ID Number"@en ;
	skos:prefLabel  "US_FHFA_ID" .

gs1:OrganizationID_Type-US_FMC_ID
	rdf:type        gs1:OrganizationID_Type ;
	rdfs:comment    "The Federal Maritime Commission (FMC) is a USA federal agency. The FMC is responsible for regulating USA ocean transportation to and from the USA. To buy or sell sea freight services to or from the USA, a company must be licensed or registered with the FMC."@en ;
	rdfs:label      "FMC License Number "@en ;
	skos:prefLabel  "US_FMC_ID" .

gs1:OrganizationID_Type-US_GIIN
	rdf:type        gs1:OrganizationID_Type ;
	rdfs:comment    "GIIN is an abbreviation of Global Intermediary Identification Number. The FATCA Registration System approves foreign financial institutions (FFI), financial institution (FI) branches, direct reporting non-financial foreign entities (NFFE), sponsoring entities, sponsored entities, and sponsored subsidiary branches."@en ;
	rdfs:label      "Global Intermediary Identification Number (GIIN)"@en ;
	skos:prefLabel  "US_GIIN" .

gs1:OrganizationID_Type-US_LAB_ID
	rdf:type        gs1:OrganizationID_Type ;
	rdfs:comment    "Code to identify CPSC-Accepted Testing Laboratories. Section 14(a)(3)(E) of the Consumer Product Safety (CPSC) Act, as amended, requires the Commission to maintain on its website an up-to-date list of entities that have been accredited to assess conformity with children's product safety rules."@en ;
	rdfs:label      "U.S. Lab ID"@en ;
	skos:prefLabel  "US_LAB_ID" .

gs1:OrganizationID_Type-US_LIC
	rdf:type        gs1:OrganizationID_Type ;
	rdfs:comment    "The assigned LIC identifies the registered company, not an individual product or device; it can be used across multiple product lines. "@en ;
	rdfs:label      "Labeler Identification code (LIC) "@en ;
	skos:prefLabel  "US_LIC" .

gs1:OrganizationID_Type-US_MFG_ID
	rdf:type        gs1:OrganizationID_Type ;
	rdfs:comment    "The United States Customs use the Manufacturer's Identification Number (MID) in the electronic data processing and monitoring of manufacturers. MID is an identifying reference number given to manufacturers that import products into the United States."@en ;
	rdfs:label      "Manufacturer ID "@en ;
	skos:prefLabel  "US_MFG_ID" .

gs1:OrganizationID_Type-US_MIC
	rdf:type        gs1:OrganizationID_Type ;
	rdfs:comment    "Domestic boat manufacturers are required by U.S. federal law to obtain a unique Manufacturer's Identification Code (MIC). The same applies to domestic importers of foreign built vessels. This code must be incorporated as the first three characters of all hull identification numbers assigned to boats of their production."@en ;
	rdfs:label      "Manufacturer's Identification Code (MIC)"@en ;
	skos:prefLabel  "US_MIC" .

gs1:OrganizationID_Type-US_NPI
	rdf:type        gs1:OrganizationID_Type ;
	rdfs:comment    "The National Provider Identifier (NPI) is a Health Insurance Portability and Accountability Act (HIPAA) Administrative Simplification Standard. The NPI is a unique identification number for covered health care providers. The NPI is a 10-position, intelligence-free numeric identifier (10-digit number)."@en ;
	rdfs:label      "National Provider Identifier (NPI)"@en ;
	skos:prefLabel  "US_NPI" .

gs1:OrganizationID_Type-US_RN
	rdf:type        gs1:OrganizationID_Type ;
	rdfs:comment    "RN stands for Registered Identification Number. It is a number issued by the FTC to U.S. businesses that manufacture, import, distribute, or sell products covered by the Textile, Wool, and Fur Acts. Businesses can use this number on product labels instead of the company name."@en ;
	rdfs:label      "Registered Identification Number (RN)"@en ;
	skos:prefLabel  "US_RN" .

gs1:OrganizationID_Type-US_RSSD_ID
	rdf:type        gs1:OrganizationID_Type ;
	rdfs:comment    "The RSSD ID is a unique identifier assigned to financial institutions by the U.S. Federal Reserve. "@en ;
	rdfs:label      "Replication Server System Database ID (RSSD ID)"@en ;
	skos:prefLabel  "US_RSSD_ID" .

gs1:OrganizationID_Type-US_SCAC
	rdf:type        gs1:OrganizationID_Type ;
	rdfs:comment    "The Standard Carrier Alpha Code (SCAC) is a unique two-to-four-letter code used to identify transportation companies. SCAC codes can be obtained from the National Motor Freight Traffic Association (NMFTA), located in Alexandria, VA."@en ;
	rdfs:label      "Standard Carrier Alpha Code (SCAC)"@en ;
	skos:prefLabel  "US_SCAC" .

gs1:OrganizationID_Type-US_UEI
	rdf:type        gs1:OrganizationID_Type ;
	rdfs:comment    "Uniquely identify entities registered in the U.S. government  System for Award Management (SAM)"@en ;
	rdfs:label      "Unique Entity Identifier (UEI)"@en ;
	skos:prefLabel  "US_UEI" .

gs1:OrganizationRoleType-ACCEPTING_PARTY
	rdf:type        gs1:OrganizationRoleType ;
	rdfs:comment    "Organization accepting goods, products, services etc."@en ;
	rdfs:label      "Accepting Organization"@en ;
	skos:prefLabel  "ACCEPTING_PARTY" .

gs1:OrganizationRoleType-BILL_OF_LADING_RECIPIENT
	rdf:type        gs1:OrganizationRoleType ;
	rdfs:comment    "Organization to receive Bill of Lading."@en ;
	rdfs:label      "Bill of Lading Recipient"@en ;
	skos:prefLabel  "BILL_OF_LADING_RECIPIENT" .

gs1:OrganizationRoleType-BILL_TO
	rdf:type        gs1:OrganizationRoleType ;
	rdfs:comment    "Organization which receives goods and invoice."@en ;
	rdfs:label      "Bill To"@en ;
	skos:prefLabel  "BILL_TO" .

gs1:OrganizationRoleType-BRAND_OWNER
	rdf:type        gs1:OrganizationRoleType ;
	rdfs:comment    "The organisation that owns the specifications of the Organization regardless of where and by whom it is manufactured is normally responsible for the allocation of the Global Trade Item Number (GTIN)."@en ;
	rdfs:label      "Brand Owner"@en ;
	skos:prefLabel  "BRAND_OWNER" .

gs1:OrganizationRoleType-BREEDER
	rdf:type        gs1:OrganizationRoleType ;
	rdfs:comment    "The organization which breeds the animal."@en ;
	rdfs:label      "Breeder"@en ;
	skos:prefLabel  "BREEDER" .

gs1:OrganizationRoleType-BROKER_AGENT
	rdf:type        gs1:OrganizationRoleType ;
	rdfs:comment    "A person who buys or sells for another entity without having title to the property."@en ;
	rdfs:label      "Broker Agent"@en ;
	skos:prefLabel  "BROKER_AGENT" .

gs1:OrganizationRoleType-BUYER
	rdf:type        gs1:OrganizationRoleType ;
	rdfs:comment    "Organization to which merchandise are sold."@en ;
	rdfs:label      "Buyer"@en ;
	skos:prefLabel  "BUYER" .

gs1:OrganizationRoleType-BUYERS_AGENT_REPRESENTATIVE
	rdf:type        gs1:OrganizationRoleType ;
	rdfs:comment    "Third party who arranged the purchase of merchandise on behalf of the actual buyer."@en ;
	rdfs:label      "Buyers Agent Representative"@en ;
	skos:prefLabel  "BUYERS_AGENT_REPRESENTATIVE" .

gs1:OrganizationRoleType-CARRIER
	rdf:type        gs1:OrganizationRoleType ;
	rdfs:comment    "A company, which physically transports goods from one place to another."@en ;
	rdfs:label      "Carrier"@en ;
	skos:prefLabel  "CARRIER" .

gs1:OrganizationRoleType-CENTRAL_PAYMENT_SERVICE
	rdf:type        gs1:OrganizationRoleType ;
	rdfs:comment    "Master of the conveyance. An organization providing central (or consolidated payment) services."@en ;
	rdfs:label      "Central Payment Service"@en ;
	skos:prefLabel  "CENTRAL_PAYMENT_SERVICE" .

gs1:OrganizationRoleType-CHECKING_PARTY
	rdf:type        gs1:OrganizationRoleType ;
	rdfs:comment    "Organization or contact designated on behalf of carrier or his agent to establish the actual figures for quantities, weight, volume and/or (cube) measurements of goods or containers which are to appear in the transport contract and on which charges will be based"@en ;
	rdfs:label      "Checking Organization"@en ;
	skos:prefLabel  "CHECKING_PARTY" .

gs1:OrganizationRoleType-CHEQUE_ORDER
	rdf:type        gs1:OrganizationRoleType ;
	rdfs:comment    "Organization to which the cheque will be ordered, when different from the beneficiary."@en ;
	rdfs:label      "Cheque Order"@en ;
	skos:prefLabel  "CHEQUE_ORDER" .

gs1:OrganizationRoleType-CONSIGNEE
	rdf:type        gs1:OrganizationRoleType ;
	rdfs:comment    "Organization to which goods are consigned."@en ;
	rdfs:label      "Consignee."@en ;
	skos:prefLabel  "CONSIGNEE" .

gs1:OrganizationRoleType-CONSOLIDATOR
	rdf:type        gs1:OrganizationRoleType ;
	rdfs:comment    "Organization consolidating various consignments, payments etc."@en ;
	rdfs:label      "Consolidator"@en ;
	skos:prefLabel  "CONSOLIDATOR" .

gs1:OrganizationRoleType-CONSUMER
	rdf:type        gs1:OrganizationRoleType ;
	rdfs:comment    "The end user of a product or a service."@en ;
	rdfs:label      "Consumer"@en ;
	skos:prefLabel  "CONSUMER" .

gs1:OrganizationRoleType-CORPORATE_IDENTITY
	rdf:type        gs1:OrganizationRoleType ;
	rdfs:comment    "Identity of the organization to whom all other parties of the same commercial organization are linked."@en ;
	rdfs:label      "Corporate Identity"@en ;
	skos:prefLabel  "CORPORATE_IDENTITY" .

gs1:OrganizationRoleType-CUSTOMS
	rdf:type        gs1:OrganizationRoleType ;
	rdfs:comment    "Identification of customs authority relevant to the transaction or shipment."@en ;
	rdfs:label      "Customs"@en ;
	skos:prefLabel  "CUSTOMS" .

gs1:OrganizationRoleType-CUSTOMS_BROKER
	rdf:type        gs1:OrganizationRoleType ;
	rdfs:comment    "Organization responsible for the preparation of documents and/or electronic submissions, the calculation on behalf of the client of taxes, duties and excises, and facilitating communication between the importer/exporter and governmental authorities."@en ;
	rdfs:label      "Customs Broker"@en ;
	skos:prefLabel  "CUSTOMS_BROKER" .

gs1:OrganizationRoleType-CUTTER
	rdf:type        gs1:OrganizationRoleType ;
	rdfs:comment    "One engaged in carving meat (In EANCOM as Meat Cutter)."@en ;
	rdfs:label      "Cutter"@en ;
	skos:prefLabel  "CUTTER" .

gs1:OrganizationRoleType-DECLARANTS_AGENT_REPRESENTATIVE
	rdf:type        gs1:OrganizationRoleType ;
	rdfs:comment    "Any natural or legal person who makes a declaration to an official body on behalf of another natural or legal person, where legally permitted (CCC)."@en ;
	rdfs:label      "Declarants Agent Representative"@en ;
	skos:prefLabel  "DECLARANTS_AGENT_REPRESENTATIVE" .

gs1:OrganizationRoleType-DELIVERY_PARTY
	rdf:type        gs1:OrganizationRoleType ;
	rdfs:comment    "Organization to which goods are delivered."@en ;
	rdfs:label      "Delivery Organization"@en ;
	skos:prefLabel  "DELIVERY_PARTY" .

gs1:OrganizationRoleType-DESIGNER
	rdf:type        gs1:OrganizationRoleType ;
	rdfs:comment    "A Organization who designs."@en ;
	rdfs:label      "Designer"@en ;
	skos:prefLabel  "DESIGNER" .

gs1:OrganizationRoleType-DESPATCH_PARTY
	rdf:type        gs1:OrganizationRoleType ;
	rdfs:comment    "Organization where goods are collected or taken over by the carrier."@en ;
	rdfs:label      "Despatch Organization"@en ;
	skos:prefLabel  "DESPATCH_PARTY" .

gs1:OrganizationRoleType-DISTRIBUTOR
	rdf:type        gs1:OrganizationRoleType ;
	rdfs:comment    "Organization distributing goods, financial payments or documents."@en ;
	rdfs:label      "Distributor"@en ;
	skos:prefLabel  "DISTRIBUTOR" .

gs1:OrganizationRoleType-DOCK_DOOR
	rdf:type        gs1:OrganizationRoleType ;
	rdfs:comment    "A door or collection of doors where trucks or rail cars are loaded (shipping) or unloaded (receiving). Used to load or unload products for logistics."@en ;
	rdfs:label      "Dock Door"@en ;
	skos:prefLabel  "DOCK_DOOR" .

gs1:OrganizationRoleType-EMPTY_EQUIPMENT_DESPATCH_PARTY
	rdf:type        gs1:OrganizationRoleType ;
	rdfs:comment    "Organization from whose premises empty equipment will be or has been despatched."@en ;
	rdfs:label      "Empty Equipment Despatch Organization"@en ;
	skos:prefLabel  "EMPTY_EQUIPMENT_DESPATCH_PARTY" .

gs1:OrganizationRoleType-EMPTY_EQUIPMENT_RETURN_PARTY
	rdf:type        gs1:OrganizationRoleType ;
	rdfs:comment    "Organization from whose premises empty equipment will be or has been returned."@en ;
	rdfs:label      "Empty Equipment Return Organization"@en ;
	skos:prefLabel  "EMPTY_EQUIPMENT_RETURN_PARTY" .

gs1:OrganizationRoleType-EQUIPMENT_OWNER
	rdf:type        gs1:OrganizationRoleType ;
	rdfs:comment    "Owner of equipment (container, etc.)."@en ;
	rdfs:label      "Equipment Owner"@en ;
	skos:prefLabel  "EQUIPMENT_OWNER" .

gs1:OrganizationRoleType-EXPORTER
	rdf:type        gs1:OrganizationRoleType ;
	rdfs:comment    "Organization who makes - or on whose behalf a Customs clearing agent or other authorized person makes - an export declaration. This may include a manufacturer, seller or other person. Within a Customs union, consignor may have the same meaning as exporter"@en ;
	rdfs:label      "Exporter"@en ;
	skos:prefLabel  "EXPORTER" .

gs1:OrganizationRoleType-FACTOR
	rdf:type        gs1:OrganizationRoleType ;
	rdfs:comment    "An organization that purchases financial receiving instruments e.g. invoices"@en ;
	rdfs:label      "Factor"@en ;
	skos:prefLabel  "FACTOR" .

gs1:OrganizationRoleType-FATTENER
	rdf:type        gs1:OrganizationRoleType ;
	rdfs:comment    "The Organization which fattens the animal."@en ;
	rdfs:label      "Fattener"@en ;
	skos:prefLabel  "FATTENER" .

gs1:OrganizationRoleType-FREIGHT_FORWARDER
	rdf:type        gs1:OrganizationRoleType ;
	rdfs:comment    "A person or firm that arranges for a pick up or deliver goods by a carrier on instructions of a shipper or consignee from or to a point by various necessary conveyances and common carriers."@en ;
	rdfs:label      "Freight Forwarder"@en ;
	skos:prefLabel  "FREIGHT_FORWARDER" .

gs1:OrganizationRoleType-GOODS_OWNER
	rdf:type        gs1:OrganizationRoleType ;
	rdfs:comment    "The organization which owns the goods."@en ;
	rdfs:label      "Goods Owner"@en ;
	skos:prefLabel  "GOODS_OWNER" .

gs1:OrganizationRoleType-GROWER
	rdf:type        gs1:OrganizationRoleType ;
	rdfs:comment    "An organization which is responsible for the growth or production of the unit specifically refers to vegetation. This organization may or may not be a producer or packer."@en ;
	rdfs:label      "Grower"@en ;
	skos:prefLabel  "GROWER" .

gs1:OrganizationRoleType-HEAD_OFFICE
	rdf:type        gs1:OrganizationRoleType ;
	rdfs:comment    "The executive or main office of an enterprise."@en ;
	rdfs:label      "Head Office"@en ;
	skos:prefLabel  "HEAD_OFFICE" .

gs1:OrganizationRoleType-IMPORTER
	rdf:type        gs1:OrganizationRoleType ;
	rdfs:comment    "Organization who makes - or on whose behalf a Customs clearing agent or other authorized person makes - an import declaration. This may include a person who has possession of the goods or to whom the goods are consigned."@en ;
	rdfs:label      "Importer"@en ;
	skos:prefLabel  "IMPORTER" .

gs1:OrganizationRoleType-INFORMATION_PROVIDER
	rdf:type        gs1:OrganizationRoleType ;
	rdfs:comment    "The Organization providing the information contained in the document."@en ;
	rdfs:label      "Information Provider"@en ;
	skos:prefLabel  "INFORMATION_PROVIDER" .

gs1:OrganizationRoleType-INSURER
	rdf:type        gs1:OrganizationRoleType ;
	rdfs:comment    "A person or company offering insurance policies for premiums."@en ;
	rdfs:label      "Insurer"@en ;
	skos:prefLabel  "INSURER" .

gs1:OrganizationRoleType-INTERMEDIARY_BANK_1
	rdf:type        gs1:OrganizationRoleType ;
	rdfs:comment    "A financial institution between the ordered bank and the beneficiary's bank."@en ;
	rdfs:label      "Intermediary Bank 1"@en ;
	skos:prefLabel  "INTERMEDIARY_BANK_1" .

gs1:OrganizationRoleType-INTERMEDIARY_BANK_2
	rdf:type        gs1:OrganizationRoleType ;
	rdfs:comment    "A financial institution between the ordered bank and the beneficiary's bank."@en ;
	rdfs:label      "Intermediary Bank 2"@en ;
	skos:prefLabel  "INTERMEDIARY_BANK_2" .

gs1:OrganizationRoleType-INVENTORY_CONTROLLER
	rdf:type        gs1:OrganizationRoleType ;
	rdfs:comment    "To specifically identify the organisation in charge of inventory control."@en ;
	rdfs:label      "Inventory Controller"@en ;
	skos:prefLabel  "INVENTORY_CONTROLLER" .

gs1:OrganizationRoleType-INVENTORY_REPORTING_PARTY
	rdf:type        gs1:OrganizationRoleType ;
	rdfs:comment    "Organization reporting inventory information."@en ;
	rdfs:label      "Inventory Reporting Organization"@en ;
	skos:prefLabel  "INVENTORY_REPORTING_PARTY" .

gs1:OrganizationRoleType-INVOICEE
	rdf:type        gs1:OrganizationRoleType ;
	rdfs:comment    "Organization issuing an invoice."@en ;
	rdfs:label      "Invoicee"@en ;
	skos:prefLabel  "INVOICEE" .

gs1:OrganizationRoleType-ISSUER_OF_INVOICE
	rdf:type        gs1:OrganizationRoleType ;
	rdfs:comment    "Organization which issues an invoice."@en ;
	rdfs:label      "Issuer of Invoice"@en ;
	skos:prefLabel  "ISSUER_OF_INVOICE" .

gs1:OrganizationRoleType-LOGISTICS_SERVICE_PROVIDER
	rdf:type        gs1:OrganizationRoleType ;
	rdfs:comment    "An umbrella term for an entity, which provides a combination of many different logistics services for another entity."@en ;
	rdfs:label      "Logistics Service Provider"@en ;
	skos:prefLabel  "LOGISTICS_SERVICE_PROVIDER" .

gs1:OrganizationRoleType-MANUFACTURER_OF_GOODS
	rdf:type        gs1:OrganizationRoleType ;
	rdfs:comment    "Organization who manufactures the goods."@en ;
	rdfs:label      "Manufacturer of Goods"@en ;
	skos:prefLabel  "MANUFACTURER_OF_GOODS" .

gs1:OrganizationRoleType-MANUFACTURING_PLANT
	rdf:type        gs1:OrganizationRoleType ;
	rdfs:comment    "A physical location consisting of one or more buildings with facilities for manufacturing."@en ;
	rdfs:label      "Manufacturing Plant"@en ;
	skos:prefLabel  "MANUFACTURING_PLANT" .

gs1:OrganizationRoleType-MARK_FOR
	rdf:type        gs1:OrganizationRoleType ;
	rdfs:comment    "The ultimate destination of a unit load or transport package of goods where the Ship-To is a different location."@en ;
	rdfs:label      "Mark For"@en ;
	skos:prefLabel  "MARK_FOR" .

gs1:OrganizationRoleType-MESSAGE_FROM
	rdf:type        gs1:OrganizationRoleType ;
	rdfs:comment    "Organization where the message comes from."@en ;
	rdfs:label      "Message From."@en ;
	skos:prefLabel  "MESSAGE_FROM" .

gs1:OrganizationRoleType-MESSAGE_RECIPIENT
	rdf:type        gs1:OrganizationRoleType ;
	rdfs:comment    "Organization receiving the message."@en ;
	rdfs:label      "Message Recipient"@en ;
	skos:prefLabel  "MESSAGE_RECIPIENT" .

gs1:OrganizationRoleType-MINCER
	rdf:type        gs1:OrganizationRoleType ;
	rdfs:comment    "One engaged in the cutting or chopping of meat into very small pieces"@en ;
	rdfs:label      "Mincer"@en ;
	skos:prefLabel  "MINCER" .

gs1:OrganizationRoleType-OPERATING_DIVISION
	rdf:type        gs1:OrganizationRoleType ;
	rdfs:comment    "An entity that is part of another entity. For example, a Regional Marketing Office. Operating Divisions may have multiple days and times of operation."@en ;
	rdfs:label      "Operating Division"@en ;
	skos:prefLabel  "OPERATING_DIVISION" .

gs1:OrganizationRoleType-OPERATOR
	rdf:type        gs1:OrganizationRoleType ;
	rdfs:comment    "A person or persons who own or operate a business establishment, which services consumers directly. For example a restaurant owner as part of a chain or an independent operation."@en ;
	rdfs:label      "Operator"@en ;
	skos:prefLabel  "OPERATOR" .

gs1:OrganizationRoleType-ORDERING_PARTY
	rdf:type        gs1:OrganizationRoleType ;
	rdfs:comment    "To be used only if ordering organization and buyer are not identical."@en ;
	rdfs:label      "Ordering Organization"@en ;
	skos:prefLabel  "ORDERING_PARTY" .

gs1:OrganizationRoleType-OWNER_OF_EQUIPMENT
	rdf:type        gs1:OrganizationRoleType ;
	rdfs:comment    "Organization who owns equipment."@en ;
	rdfs:label      "Owner of equipment"@en ;
	skos:prefLabel  "OWNER_OF_EQUIPMENT" .

gs1:OrganizationRoleType-OWNER_OF_MEANS_OF_TRANSPORT
	rdf:type        gs1:OrganizationRoleType ;
	rdfs:comment    "Organization owning the means of transport. Not a synonym of carrier"@en ;
	rdfs:label      "Owner of Means of Transport"@en ;
	skos:prefLabel  "OWNER_OF_MEANS_OF_TRANSPORT" .

gs1:OrganizationRoleType-PARTY_DECLARING_THE_VALUE_ADDED_TAX
	rdf:type        gs1:OrganizationRoleType ;
	rdfs:comment    "A code to identify the organization who is responsible for declaring the Value Added Tax (VAT) on the sale of goods or services."@en ;
	rdfs:label      "Organization Declaring the Value Added Tax"@en ;
	skos:prefLabel  "PARTY_DECLARING_THE_VALUE_ADDED_TAX" .

gs1:OrganizationRoleType-PARTY_FOR_WHOM_ITEM_IS_ULTIMATELY_INTENDED
	rdf:type        gs1:OrganizationRoleType ;
	rdfs:label      "Organization For Whom Item is Ultimately Intended"@en ;
	skos:prefLabel  "PARTY_FOR_WHOM_ITEM_IS_ULTIMATELY_INTENDED" .

gs1:OrganizationRoleType-PARTY_RECEIVING_PRIVATE_DATA
	rdf:type        gs1:OrganizationRoleType ;
	rdfs:comment    "The organization who is allowed access to master data information by the data owner when the data is viewed as private."@en ;
	rdfs:label      "Organization Receiving Private Data"@en ;
	skos:prefLabel  "PARTY_RECEIVING_PRIVATE_DATA" .

gs1:OrganizationRoleType-PARTY_RECOVERING_THE_VALUE_ADDED_TAX
	rdf:type        gs1:OrganizationRoleType ;
	rdfs:comment    "A code to identify the organization who is eligible to recover the Value Added Tax (VAT) on the sale of goods or services."@en ;
	rdfs:label      "Organization Recovering the Value Added Tax"@en ;
	skos:prefLabel  "PARTY_RECOVERING_THE_VALUE_ADDED_TAX" .

gs1:OrganizationRoleType-PARTY_TO_RECEIVE_ALL_DOCUMENTS
	rdf:type        gs1:OrganizationRoleType ;
	rdfs:comment    "An organization which is named to be the recipient of all documents."@en ;
	rdfs:label      "Organization to Receive All Documents"@en ;
	skos:prefLabel  "PARTY_TO_RECEIVE_ALL_DOCUMENTS" .

gs1:OrganizationRoleType-PARTY_TO_RECEIVE_COMMERCIAL_INVOICE
	rdf:type        gs1:OrganizationRoleType ;
	rdfs:comment    "Organization to whom payment for a commercial invoice or bill should be remitted."@en ;
	rdfs:label      "Organization to Receive Commercial Invoice"@en ;
	skos:prefLabel  "PARTY_TO_RECEIVE_COMMERCIAL_INVOICE" .

gs1:OrganizationRoleType-PARTY_TO_RECEIVE_ELECTRONIC_MEMO_OF_INVOICE
	rdf:type        gs1:OrganizationRoleType ;
	rdfs:comment    "Organization being informed about invoice issue (via EDI)."@en ;
	rdfs:label      "Organization to Receive Electronic Memo of Invoice"@en ;
	skos:prefLabel  "PARTY_TO_RECEIVE_ELECTRONIC_MEMO_OF_INVOICE" .

gs1:OrganizationRoleType-PARTY_TO_RECEIVE_FREIGHT_BILL
	rdf:type        gs1:OrganizationRoleType ;
	rdfs:comment    "Organization to whom the freight bill should be sent."@en ;
	rdfs:label      "Organization to Receive Freight Bill"@en ;
	skos:prefLabel  "PARTY_TO_RECEIVE_FREIGHT_BILL" .

gs1:OrganizationRoleType-PARTY_TO_RECEIVE_REFUND
	rdf:type        gs1:OrganizationRoleType ;
	rdfs:comment    "Organization to whom a refund is given."@en ;
	rdfs:label      "Organization to Receive Refund"@en ;
	skos:prefLabel  "PARTY_TO_RECEIVE_REFUND" .

gs1:OrganizationRoleType-PAYEE
	rdf:type        gs1:OrganizationRoleType ;
	rdfs:comment    "Organization, which receives payment."@en ;
	rdfs:label      "Payee"@en ;
	skos:prefLabel  "PAYEE" .

gs1:OrganizationRoleType-PAYER
	rdf:type        gs1:OrganizationRoleType ;
	rdfs:comment    "Organization which initiates payment."@en ;
	rdfs:label      "Payer"@en ;
	skos:prefLabel  "PAYER" .

gs1:OrganizationRoleType-POINT_OF_SALE
	rdf:type        gs1:OrganizationRoleType ;
	rdfs:comment    "Refers to the retail type checkout where bar code symbols are normally scanned."@en ;
	rdfs:label      "Point Of Sale"@en ;
	skos:prefLabel  "POINT_OF_SALE" .

gs1:OrganizationRoleType-PRICE_LOCATION_PARTY
	rdf:type        gs1:OrganizationRoleType ;
	rdfs:comment    "An organization to which a price for a product is applicable. Within the context of GDSN Price Synchronization, it is also known as the 'Price Location' which is a GLN."@en ;
	rdfs:label      "Price Location Organization"@en ;
	skos:prefLabel  "PRICE_LOCATION_PARTY" .

gs1:OrganizationRoleType-PROXY
	rdf:type        gs1:OrganizationRoleType ;
	rdfs:comment    "A company that is selected by the Brand Owner to maintain their baseline attributes and Administrative Records in the GDSN."@en ;
	rdfs:label      "Proxy"@en ;
	skos:prefLabel  "PROXY" .

gs1:OrganizationRoleType-PUBLIC_WAREHOUSE
	rdf:type        gs1:OrganizationRoleType ;
	rdfs:comment    "A building, or a part of one, where storage space is offered to other companies for compensation (fee), for the storage of their goods, merchandise, etc."@en ;
	rdfs:label      "Public Warehouse"@en ;
	skos:prefLabel  "PUBLIC_WAREHOUSE" .

gs1:OrganizationRoleType-PURCHASE_ORDER_RECEIVER
	rdf:type        gs1:OrganizationRoleType ;
	rdfs:comment    "The organization that receives the purchase order for the goods or services."@en ;
	rdfs:label      "Purchase Order Receiver"@en ;
	skos:prefLabel  "PURCHASE_ORDER_RECEIVER" .

gs1:OrganizationRoleType-REGISTERED_AGENT
	rdf:type        gs1:OrganizationRoleType ;
	rdfs:comment    "The organization having legal responsibility for the product in the target market for example a company to which market authorization has been issued."@en ;
	rdfs:label      "Registered Agent"@en ;
	skos:prefLabel  "REGISTERED_AGENT" .

gs1:OrganizationRoleType-REMIT_TO
	rdf:type        gs1:OrganizationRoleType ;
	rdfs:comment    "Organization to whom funds are directed for payment of a commercial invoice."@en ;
	rdfs:label      "Remit To"@en ;
	skos:prefLabel  "REMIT_TO" .

gs1:OrganizationRoleType-RETURNABLE_ASSET_SERVICE_CENTRE
	rdf:type        gs1:OrganizationRoleType ;
	rdfs:comment    "The location where a returnable asset is serviced."@en ;
	rdfs:label      "Returnable Asset Service Centre"@en ;
	skos:prefLabel  "RETURNABLE_ASSET_SERVICE_CENTRE" .

gs1:OrganizationRoleType-SELLER
	rdf:type        gs1:OrganizationRoleType ;
	rdfs:comment    "Organization which sells products or services to a buyer."@en ;
	rdfs:label      "Seller"@en ;
	skos:prefLabel  "SELLER" .

gs1:OrganizationRoleType-SERVICE_PROVIDER
	rdf:type        gs1:OrganizationRoleType ;
	rdfs:comment    "An organization providing services for another organization (e.g. re-packing supplier's products)."@en ;
	rdfs:label      "Service Provider"@en ;
	skos:prefLabel  "SERVICE_PROVIDER" .

gs1:OrganizationRoleType-SHIP_FROM
	rdf:type        gs1:OrganizationRoleType ;
	rdfs:comment    "Organization from where goods will be or have been shipped."@en ;
	rdfs:label      "Ship From"@en ;
	skos:prefLabel  "SHIP_FROM" .

gs1:OrganizationRoleType-SHIP_TO
	rdf:type        gs1:OrganizationRoleType ;
	rdfs:comment    "Organization which receives goods and invoices."@en ;
	rdfs:label      "Ship To"@en ;
	skos:prefLabel  "SHIP_TO" .

gs1:OrganizationRoleType-SLAUGHTERER
	rdf:type        gs1:OrganizationRoleType ;
	rdfs:comment    "The Organization who has undertaken or will undertake a slaughter."@en ;
	rdfs:label      "Slaughterer"@en ;
	skos:prefLabel  "SLAUGHTERER" .

gs1:OrganizationRoleType-STORE
	rdf:type        gs1:OrganizationRoleType ;
	rdfs:comment    "A physical entity that sells products to a consumer."@en ;
	rdfs:label      "Store"@en ;
	skos:prefLabel  "STORE" .

gs1:OrganizationRoleType-SUBSTITUTE_SUPPLIER
	rdf:type        gs1:OrganizationRoleType ;
	rdfs:comment    "Organization which may be in a position to supply products or services should the main usual supplier be unable to do so."@en ;
	rdfs:label      "Substitute Supplier"@en ;
	skos:prefLabel  "SUBSTITUTE_SUPPLIER" .

gs1:OrganizationRoleType-SUPPLIER
	rdf:type        gs1:OrganizationRoleType ;
	rdfs:comment    "An organization that provides goods or services."@en ;
	rdfs:label      "Supplier"@en ;
	skos:prefLabel  "SUPPLIER" .

gs1:OrganizationRoleType-TRANSPORTATION_CARRIER
	rdf:type        gs1:OrganizationRoleType ;
	rdfs:comment    "Organization undertaking or arranging transport of goods between named points."@en ;
	rdfs:label      "Transportation Carrier"@en ;
	skos:prefLabel  "TRANSPORTATION_CARRIER" .

gs1:OrganizationRoleType-VISITING_ADDRESS
	rdf:type        gs1:OrganizationRoleType ;
	rdfs:comment    "An enterprise's physical location where guests are received during set working hours"@en ;
	rdfs:label      "Visiting Address"@en ;
	skos:prefLabel  "VISITING_ADDRESS" .

gs1:OrganizationRoleType-WAREHOUSE_AND_OR_DEPOT
	rdf:type        gs1:OrganizationRoleType ;
	rdfs:comment    "Industrial department of a company equipped with appropriate equipment and fittings in which goods are stored in appropriate conditions."@en ;
	rdfs:label      "Warehouse and or Depot"@en ;
	skos:prefLabel  "WAREHOUSE_AND_OR_DEPOT" .

gs1:OrganizationRoleType-WAREHOUSE_KEEPER
	rdf:type        gs1:OrganizationRoleType ;
	rdfs:comment    "Organization taking responsibility for goods entered into a warehouse."@en ;
	rdfs:label      "Warehouse Keeper"@en ;
	skos:prefLabel  "WAREHOUSE_KEEPER" .

gs1:OrganizationRoleType-WHOLESALER
	rdf:type        gs1:OrganizationRoleType ;
	rdfs:comment    "Seller of articles, often in large quantities, to be retailed by others."@en ;
	rdfs:label      "WholeSaler"@en ;
	skos:prefLabel  "WHOLESALER" .

gs1:PackagingFeatureCode-BASE
	rdf:type        gs1:PackagingFeatureCode ;
	rdfs:comment    "A general term applied to the support or pedestal of an object."@en ;
	rdfs:label      "Base"@en ;
	skos:prefLabel  "BASE" .

gs1:PackagingFeatureCode-BEAM
	rdf:type        gs1:PackagingFeatureCode ;
	rdfs:comment    "Long sturdy piece of squared timber or metal used in house-building etc."@en ;
	rdfs:label      "Beam"@en ;
	skos:prefLabel  "BEAM" .

gs1:PackagingFeatureCode-BUNG_SEAL
	rdf:type        gs1:PackagingFeatureCode ;
	rdfs:comment    "A bung is an apparatus used to seal a container, such as a bottle, barrel or tubes. A bung is partially inserted inside the container to act as a seal. The most common every-day example of a bung is the stopper of a wine bottle."@en ;
	rdfs:label      "Bung Seal"@en ;
	skos:prefLabel  "BUNG_SEAL" .

gs1:PackagingFeatureCode-CAP
	rdf:type        gs1:PackagingFeatureCode ;
	rdfs:comment    "A cap that seals a bottle or other form of packaging."@en ;
	rdfs:label      "Cap"@en ;
	skos:prefLabel  "CAP" .

gs1:PackagingFeatureCode-CARRIER
	rdf:type        gs1:PackagingFeatureCode ;
	rdfs:comment    "A device of various types attached to or hung from trolleys to support the load."@en ;
	rdfs:label      "Carrier"@en ;
	skos:prefLabel  "CARRIER" .

gs1:PackagingFeatureCode-CONSUMPTION_UTENSIL
	rdf:type        gs1:PackagingFeatureCode ;
	rdfs:comment    "An item which allows the user to extract and/or consume the content of a container."@en ;
	rdfs:label      "Consumption Utensil"@en ;
	skos:prefLabel  "CONSUMPTION_UTENSIL" .

gs1:PackagingFeatureCode-CORE
	rdf:type        gs1:PackagingFeatureCode ;
	rdfs:comment    "A tubular shape around which flexible material such as plastic film or paper are wound for purposes of transport and handling."@en ;
	rdfs:label      "Core"@en ;
	skos:prefLabel  "CORE" .

gs1:PackagingFeatureCode-CREEL
	rdf:type        gs1:PackagingFeatureCode ;
	rdfs:comment    "A creel is a device for holding the required number of roving spools or other supply packages of reinforcement fibers for Fiber Reinforced Plastics manufacturing. This device holds the rovings in the desired position for unwinding in continuous processes like Pultrusion and Filament Winding."@en ;
	rdfs:label      "Creel"@en ;
	skos:prefLabel  "CREEL" .

gs1:PackagingFeatureCode-EDGE_PROTECTION
	rdf:type        gs1:PackagingFeatureCode ;
	rdfs:comment    "A right-angle piece placed over the outermost perimeter edges of a container to distribute pressure and prevent collapse or cutting from banding, strapping, or handling."@en ;
	rdfs:label      "Edge Protection"@en ;
	skos:prefLabel  "EDGE_PROTECTION" .

gs1:PackagingFeatureCode-HANDLE
	rdf:type        gs1:PackagingFeatureCode ;
	rdfs:comment    "A grip attached to an object for using or moving the object, usually with the hands."@en ;
	rdfs:label      "Handle"@en ;
	skos:prefLabel  "HANDLE" .

gs1:PackagingFeatureCode-INNER_CONTAINER
	rdf:type        gs1:PackagingFeatureCode ;
	rdfs:comment    "Inner Container"@en ;
	rdfs:label      "Inner Container"@en ;
	skos:prefLabel  "INNER_CONTAINER" .

gs1:PackagingFeatureCode-INTERNAL_DIVIDER
	rdf:type        gs1:PackagingFeatureCode ;
	rdfs:comment    "An internal divider is an object, either flat or custom-shaped, used to separate the content of a container or to prevent the content from mixing."@en ;
	rdfs:label      "Internal Divider"@en ;
	skos:prefLabel  "INTERNAL_DIVIDER" .

gs1:PackagingFeatureCode-LABEL
	rdf:type        gs1:PackagingFeatureCode ;
	rdfs:comment    "A label is a piece of paper, polymer, cloth, metal, or other material affixed to a container or article (or printed directly upon it), which usually carries information about the article to.which it has been attached."@en ;
	rdfs:label      "Label"@en ;
	skos:prefLabel  "LABEL" .

gs1:PackagingFeatureCode-LID
	rdf:type        gs1:PackagingFeatureCode ;
	rdfs:comment    "In packaging, the top or bottom of a container, usually the part that closes the opening; may also be known as cap, over, or top"@en ;
	rdfs:label      "Lid"@en ;
	skos:prefLabel  "LID" .

gs1:PackagingFeatureCode-LINER
	rdf:type        gs1:PackagingFeatureCode ;
	rdfs:comment    "An internal chamber within a container which separates the content of the container from the walls. Inner liners provide additional isolation and protection to the content of a container. Sometimes coatings of certain materials may be applied as an alternative to inner liners."@en ;
	rdfs:label      "Liner"@en ;
	skos:prefLabel  "LINER" .

gs1:PackagingFeatureCode-LUG
	rdf:type        gs1:PackagingFeatureCode ;
	rdfs:comment    "A small indentation or raised portion on the surface of a bottle, provided as an indexing means for operations such as multi-pass decoration or labeling."@en ;
	rdfs:label      "Lug"@en ;
	skos:prefLabel  "LUG" .

gs1:PackagingFeatureCode-NESTING_EDGE
	rdf:type        gs1:PackagingFeatureCode ;
	rdfs:comment    "Edges which allow items of the same size to be partially stacked within one another in any direction thus reducing the space required in order to stack them."@en ;
	rdfs:label      "Nesting Edge"@en ;
	skos:prefLabel  "NESTING_EDGE" .

gs1:PackagingFeatureCode-PEG
	rdf:type        gs1:PackagingFeatureCode ;
	rdfs:comment    "A fastener which allows a product to be hanged."@en ;
	rdfs:label      "Peg"@en ;
	skos:prefLabel  "PEG" .

gs1:PackagingFeatureCode-PULL_OFF_TAB
	rdf:type        gs1:PackagingFeatureCode ;
	rdfs:comment    "A flexible cover which can be easily removed in order to open a container."@en ;
	rdfs:label      "Pull Off Tab"@en ;
	skos:prefLabel  "PULL_OFF_TAB" .

gs1:PackagingFeatureCode-RING_HOLDER
	rdf:type        gs1:PackagingFeatureCode ;
	rdfs:comment    "A hollow circular band of material wound around itself."@en ;
	rdfs:label      "Ring Holder"@en ;
	skos:prefLabel  "RING_HOLDER" .

gs1:PackagingFeatureCode-RIVET
	rdf:type        gs1:PackagingFeatureCode ;
	rdfs:comment    "A permanent fastener which consists of a cylindrical shaft with a head on one end and tail which is deformed to fixate the rivet in place."@en ;
	rdfs:label      "Rivet"@en ;
	skos:prefLabel  "RIVET" .

gs1:PackagingFeatureCode-SLEEVE
	rdf:type        gs1:PackagingFeatureCode ;
	rdfs:comment    "A tubular form, open at both ends, that is slipped over an item or package."@en ;
	rdfs:label      "Sleeve"@en ;
	skos:prefLabel  "SLEEVE" .

gs1:PackagingFeatureCode-SPOUT
	rdf:type        gs1:PackagingFeatureCode ;
	rdfs:comment    "A spout is a protruding edge which allows the lifting and pouring of liquids contained within a container."@en ;
	rdfs:label      "Spout"@en ;
	skos:prefLabel  "SPOUT" .

gs1:PackagingFeatureCode-TAG
	rdf:type        gs1:PackagingFeatureCode ;
	rdfs:comment    "A hanging card made of any material which is used to identify or provide additional information of a product."@en ;
	rdfs:label      "Tag"@en ;
	skos:prefLabel  "TAG" .

gs1:PackagingFeatureCode-WICKER_OUTER_CONTAINER
	rdf:type        gs1:PackagingFeatureCode ;
	rdfs:comment    "An outer container made of wicker which is fitted to the bottle usually a little less than half way up from the bottom of the bottle and is used to hold, hang or support the bottle."@en ;
	rdfs:label      "Wicker Outer Container"@en ;
	skos:prefLabel  "WICKER_OUTER_CONTAINER" .

gs1:PackagingFeatureCode-WRAP
	rdf:type        gs1:PackagingFeatureCode ;
	rdfs:comment    "A layer of any material which completely enclose a product. A wrap can have many purposes, from providing additional protection to an item to serving as a gift-wrap."@en ;
	rdfs:label      "Wrap"@en ;
	skos:prefLabel  "WRAP" .

gs1:PackagingFunctionCode-ANTISEPTIC
	rdf:type        gs1:PackagingFunctionCode ;
	rdfs:comment    "The process by which a sterile (aseptic) product (typically food or pharmaceutical) is packaged in a sterile container in a way which maintains sterility."@en ;
	rdfs:label      "Antiseptic"@en ;
	skos:prefLabel  "ANTISEPTIC" .

gs1:PackagingFunctionCode-ANTI_TAMPERING
	rdf:type        gs1:PackagingFunctionCode ;
	rdfs:comment    "A methodology used to hinder, or deter unauthorized access to a device."@en ;
	rdfs:label      "Anti-tampering"@en ;
	skos:prefLabel  "ANTI_TAMPERING" .

gs1:PackagingFunctionCode-COATED
	rdf:type        gs1:PackagingFunctionCode ;
	rdfs:comment    "Covered with a material (paraffin, wax) that protects the product or packaging."@en ;
	rdfs:label      "Coated"@en ;
	skos:prefLabel  "COATED" .

gs1:PackagingFunctionCode-COMPRESSED
	rdf:type        gs1:PackagingFunctionCode ;
	rdfs:comment    "Content has been pressed together to the maximum possible way."@en ;
	rdfs:label      "Compressed"@en ;
	skos:prefLabel  "COMPRESSED" .

gs1:PackagingFunctionCode-DISPENSER
	rdf:type        gs1:PackagingFunctionCode ;
	rdfs:comment    "A device or mechanism to supply or extract contents."@en ;
	rdfs:label      "Dispenser"@en ;
	skos:prefLabel  "DISPENSER" .

gs1:PackagingFunctionCode-GIFT_WRAPPED
	rdf:type        gs1:PackagingFunctionCode ;
	rdfs:comment    "Packaging is wrapped in a decorative way for the purposes of the consumer giving it as a gift."@en ;
	rdfs:label      "Gift Wrapped"@en ;
	skos:prefLabel  "GIFT_WRAPPED" .

gs1:PackagingFunctionCode-ISOTHERMIC
	rdf:type        gs1:PackagingFunctionCode ;
	rdfs:comment    "Thermal carry container designed for the carriage of temperature controlled goods such as vaccines, pharmaceuticals, and medicines."@en ;
	rdfs:label      "Isothermic"@en ;
	skos:prefLabel  "ISOTHERMIC" .

gs1:PackagingFunctionCode-MODIFIED_ATMOSPHERE
	rdf:type        gs1:PackagingFunctionCode ;
	rdfs:comment    "The practice of modifying the composition of the internal atmosphere of a package, (commonly food packages, and drugs) in order to improve the shelf life."@en ;
	rdfs:label      "Modified Atmosphere"@en ;
	skos:prefLabel  "MODIFIED_ATMOSPHERE" .

gs1:PackagingFunctionCode-OXYGEN_INFUSED
	rdf:type        gs1:PackagingFunctionCode ;
	rdfs:comment    "A barrier packaging material for an infusion solution, i.e., oxygen."@en ;
	rdfs:label      "Oxygen Infused"@en ;
	skos:prefLabel  "OXYGEN_INFUSED" .

gs1:PackagingFunctionCode-PEEL_OFF
	rdf:type        gs1:PackagingFunctionCode ;
	rdfs:comment    "A section of the packaging can be detached with ease in order to have access to the content or product, e.g. peel-off Lids used for packing Milk, Coffee and Cacao Powder."@en ;
	rdfs:label      "Peel Off"@en ;
	skos:prefLabel  "PEEL_OFF" .

gs1:PackagingFunctionCode-PINPACK
	rdf:type        gs1:PackagingFunctionCode ;
	rdfs:comment    "The package is equipped to be hung up on a hook."@en ;
	rdfs:label      "Pinpack"@en ;
	skos:prefLabel  "PINPACK" .

gs1:PackagingFunctionCode-PROTECTED
	rdf:type        gs1:PackagingFunctionCode ;
	rdfs:comment    "Functionality to keep from being damaged, attacked, stolen, or injured; guard."@en ;
	rdfs:label      "Protected"@en ;
	skos:prefLabel  "PROTECTED" .

gs1:PackagingFunctionCode-REINFORCED
	rdf:type        gs1:PackagingFunctionCode ;
	rdfs:comment    "A component is added to a container for a particular application to lend additional support under severe applications."@en ;
	rdfs:label      "Reinforced"@en ;
	skos:prefLabel  "REINFORCED" .

gs1:PackagingFunctionCode-SIFT_PROOF
	rdf:type        gs1:PackagingFunctionCode ;
	rdfs:comment    "Packaging is designed to prevent leaking of the content specially when it is on powdered or liquid state."@en ;
	rdfs:label      "Sift Proof"@en ;
	skos:prefLabel  "SIFT_PROOF" .

gs1:PackagingFunctionCode-TAMPER_EVIDENT
	rdf:type        gs1:PackagingFunctionCode ;
	rdfs:comment    "The packaging is designed to show when there has been some interference with the original sealing or configuration of the packaging."@en ;
	rdfs:label      "Tamper Evident"@en ;
	skos:prefLabel  "TAMPER_EVIDENT" .

gs1:PackagingFunctionCode-WATER_RESISTANT
	rdf:type        gs1:PackagingFunctionCode ;
	rdfs:comment    "Coated with materials that make the packaging impervious to the effects of water."@en ;
	rdfs:label      "Water Resistant"@en ;
	skos:prefLabel  "WATER_RESISTANT" .

gs1:PackagingMarkedDietAllergenCode-APPROVED_BY_ASTHMA_AND_ALLERGY_ASSOC
	rdf:type        gs1:PackagingMarkedDietAllergenCode ;
	rdfs:comment    "Definitions made by the asthma and allergist association."@en ;
	rdfs:label      "Asthma and Allergist Association"@en ;
	skos:prefLabel  "APPROVED_BY_ASTHMA_AND_ALLERGY_ASSOC" .

gs1:PackagingMarkedDietAllergenCode-APPROVED_FOR_TUBE_FEEDING
	rdf:type        gs1:PackagingMarkedDietAllergenCode ;
	rdfs:comment    "The item is physically marked that it is approved for tube feeding by the appropriate authority of the target market."@en ;
	rdfs:label      "Approved for Tube Feeding"@en ;
	skos:prefLabel  "APPROVED_FOR_TUBE_FEEDING" .

gs1:PackagingMarkedDietAllergenCode-BIOLOGICAL
	rdf:type        gs1:PackagingMarkedDietAllergenCode ;
	rdfs:comment    "Indicates the product has been marked as a biological item which indicates a food product that was produced with the use of feed or fertilizer of plant or animal origin, without employment of chemically formulated fertilizers, growth stimulants, antibiotics or pesticides."@en ;
	rdfs:label      "Biological"@en ;
	skos:prefLabel  "BIOLOGICAL" .

gs1:PackagingMarkedDietAllergenCode-CALORIES_PER_PORTION
	rdf:type        gs1:PackagingMarkedDietAllergenCode ;
	rdfs:comment    "Indicates the product has a marking with the calories per portion contained in the product."@en ;
	rdfs:label      "Calories Per Portion"@en ;
	skos:prefLabel  "CALORIES_PER_PORTION" .

gs1:PackagingMarkedDietAllergenCode-CONTAINS_LATEX
	rdf:type        gs1:PackagingMarkedDietAllergenCode ;
	rdfs:comment    "The item is physically marked as containing Latex (rubber)."@en ;
	rdfs:label      "Contains Latex"@en ;
	skos:prefLabel  "CONTAINS_LATEX" .

gs1:PackagingMarkedDietAllergenCode-CONTAINS_PVC
	rdf:type        gs1:PackagingMarkedDietAllergenCode ;
	rdfs:comment    "The item is physically marked as containing PVC (Polyvinyl chloride). Phthalate content is unspecified."@en ;
	rdfs:label      "Contains PVC"@en ;
	skos:prefLabel  "CONTAINS_PVC" .

gs1:PackagingMarkedDietAllergenCode-CONTAINS_PVC_WITHOUT_PHTHALATES
	rdf:type        gs1:PackagingMarkedDietAllergenCode ;
	rdfs:comment    "The item is physically marked as containing PVC (Polyvinyl chloride) without phthalates."@en ;
	rdfs:label      "Contains PVC Without Phthalates"@en ;
	skos:prefLabel  "CONTAINS_PVC_WITHOUT_PHTHALATES" .

gs1:PackagingMarkedDietAllergenCode-CONTAINS_PVC_WITH_PHTHALATES
	rdf:type        gs1:PackagingMarkedDietAllergenCode ;
	rdfs:comment    "The item is physically marked as containing PVC (Polyvinyl chloride) with phthalates."@en ;
	rdfs:label      "Contains PVC With Phthalates"@en ;
	skos:prefLabel  "CONTAINS_PVC_WITH_PHTHALATES" .

gs1:PackagingMarkedDietAllergenCode-DIET_PRODUCT_450_800_KCAL_PER_DAY
	rdf:type        gs1:PackagingMarkedDietAllergenCode ;
	rdfs:comment    "The item is physically marked that it is approved for a 450-800 kilocalorie/day diet by the appropriate authority of the target market."@en ;
	rdfs:label      "450-800 Kilocalorie Per Day Diet"@en ;
	skos:prefLabel  "DIET_PRODUCT_450_800_KCAL_PER_DAY" .

gs1:PackagingMarkedDietAllergenCode-DIET_PRODUCT_800_1200_KCAL_PER_DAY
	rdf:type        gs1:PackagingMarkedDietAllergenCode ;
	rdfs:comment    "The item is physically marked that it is approved for a 800-1200 kilocalorie/day diet by the appropriate authority of the target market."@en ;
	rdfs:label      "800-1200 Kilocalorie Per Day Diet"@en ;
	skos:prefLabel  "DIET_PRODUCT_800_1200_KCAL_PER_DAY" .

gs1:PackagingMarkedDietAllergenCode-GEZONDE_KEUZE_KLAVERTJE
	rdf:type        gs1:PackagingMarkedDietAllergenCode ;
	rdfs:comment    "Health symbol used in the Netherlands Target Market which indicates that the item is a cholesterol-reducing product."@en ;
	rdfs:label      "Gezonde Keuze Klavertje"@en ;
	skos:prefLabel  "GEZONDE_KEUZE_KLAVERTJE" .

gs1:PackagingMarkedDietAllergenCode-HALAL
	rdf:type        gs1:PackagingMarkedDietAllergenCode ;
	rdfs:comment    "Indicates the product has been marked as Halal which denotes selling or serving food ritually fit according to Islamic dietary laws."@en ;
	rdfs:label      "Halal"@en ;
	skos:prefLabel  "HALAL" .

gs1:PackagingMarkedDietAllergenCode-IK_KIES_BEWUST
	rdf:type        gs1:PackagingMarkedDietAllergenCode ;
	rdfs:comment    "Conscious choice symbol used in the Netherlands Target Market which may be used for products low in saturated fat, trans fatty acids, sugar and salt."@en ;
	rdfs:label      "Ik Kies Bewust"@en ;
	skos:prefLabel  "IK_KIES_BEWUST" .

gs1:PackagingMarkedDietAllergenCode-KOSHER
	rdf:type        gs1:PackagingMarkedDietAllergenCode ;
	rdfs:comment    "Indicates the product has been marked as Kosher which denotes selling or serving food ritually fit according to Jewish dietary laws."@en ;
	rdfs:label      "Kosher"@en ;
	skos:prefLabel  "KOSHER" .

gs1:PackagingMarkedDietAllergenCode-LACTASE_ENZYME
	rdf:type        gs1:PackagingMarkedDietAllergenCode ;
	rdfs:comment    "The item is physically marked that it is approved as lactase enzyme by the appropriate authority of the target market."@en ;
	rdfs:label      "Lactase Enzyme"@en ;
	skos:prefLabel  "LACTASE_ENZYME" .

gs1:PackagingMarkedDietAllergenCode-LOW_ON_PHENYLALANINE
	rdf:type        gs1:PackagingMarkedDietAllergenCode ;
	rdfs:comment    "The item is physically marked as containing a low level of phenylalanine as approved by the appropriate authority of the target market."@en ;
	rdfs:label      "Low in Phenylalanine"@en ;
	skos:prefLabel  "LOW_ON_PHENYLALANINE" .

gs1:PackagingMarkedDietAllergenCode-LOW_ON_SUGAR
	rdf:type        gs1:PackagingMarkedDietAllergenCode ;
	rdfs:comment    "The item is physically marked as containing a low level of sugar as approved by the appropriate authority of the target market."@en ;
	rdfs:label      "Low Sugar"@en ;
	skos:prefLabel  "LOW_ON_SUGAR" .

gs1:PackagingMarkedDietAllergenCode-MOTHERS_MILK_SUBSTITUTE
	rdf:type        gs1:PackagingMarkedDietAllergenCode ;
	rdfs:comment    "The item is physically marked that it is approved as substitute mother's milk the appropriate authority of the target market."@en ;
	rdfs:label      "Mother's Milk Substitute"@en ;
	skos:prefLabel  "MOTHERS_MILK_SUBSTITUTE" .

gs1:PackagingMarkedDietAllergenCode-NUTRITION_SUPPLEMENT
	rdf:type        gs1:PackagingMarkedDietAllergenCode ;
	rdfs:comment    "The item is physically marked that it is approved as nutrition supplement by the appropriate authority of the target market."@en ;
	rdfs:label      "Nutrition Supplement"@en ;
	skos:prefLabel  "NUTRITION_SUPPLEMENT" .

gs1:PackagingMarkedDietAllergenCode-NYCKELHAL_MARK
	rdf:type        gs1:PackagingMarkedDietAllergenCode ;
	rdfs:comment    "Lean product."@en ;
	rdfs:label      "Nyckelhal Mark"@en ;
	skos:prefLabel  "NYCKELHAL_MARK" .

gs1:PackagingMarkedDietAllergenCode-VEGETARIAN
	rdf:type        gs1:PackagingMarkedDietAllergenCode ;
	rdfs:comment    "Indicates the product has been marked as vegetarian which denotes a product that contains no meat, fish or other animal products."@en ;
	rdfs:label      "Vegetarian"@en ;
	skos:prefLabel  "VEGETARIAN" .

gs1:PackagingMarkedFreeFromCode-FREE_FROM_ARTIFICIAL_COLOURING
	rdf:type        gs1:PackagingMarkedFreeFromCode ;
	rdfs:comment    "The item is physically marked as having no artificial colouring."@en ;
	rdfs:label      "Free From Artificial Colouring"@en ;
	skos:prefLabel  "FREE_FROM_ARTIFICIAL_COLOURING" .

gs1:PackagingMarkedFreeFromCode-FREE_FROM_ARTIFICIAL_FLAVOURING
	rdf:type        gs1:PackagingMarkedFreeFromCode ;
	rdfs:comment    "The item is physically marked as having no artificial flavouring."@en ;
	rdfs:label      "Free From Artificial Flavouring"@en ;
	skos:prefLabel  "FREE_FROM_ARTIFICIAL_FLAVOURING" .

gs1:PackagingMarkedFreeFromCode-FREE_FROM_ARTIFICIAL_PRESERVATIVES
	rdf:type        gs1:PackagingMarkedFreeFromCode ;
	rdfs:comment    "The item is physically marked as having no artificial preservatives."@en ;
	rdfs:label      "Free From Artificial Preservatives"@en ;
	skos:prefLabel  "FREE_FROM_ARTIFICIAL_PRESERVATIVES" .

gs1:PackagingMarkedFreeFromCode-FREE_FROM_CHOLESTEROL
	rdf:type        gs1:PackagingMarkedFreeFromCode ;
	rdfs:comment    "The item is physically marked as having no Cholesterol."@en ;
	rdfs:label      "Free From Cholesterol"@en ;
	skos:prefLabel  "FREE_FROM_CHOLESTEROL" .

gs1:PackagingMarkedFreeFromCode-FREE_FROM_CLONED_FOOD
	rdf:type        gs1:PackagingMarkedFreeFromCode ;
	rdfs:comment    "The item is physically marked as being free from cloned food."@en ;
	rdfs:label      "Free From Cloned Food"@en ;
	skos:prefLabel  "FREE_FROM_CLONED_FOOD" .

gs1:PackagingMarkedFreeFromCode-FREE_FROM_DAIRY
	rdf:type        gs1:PackagingMarkedFreeFromCode ;
	rdfs:comment    "The item is physically marked as being free from dairy and dairy products, as approved by the appropriate authority of the target market."@en ;
	rdfs:label      "Free From Dairy and Dairy Products"@en ;
	skos:prefLabel  "FREE_FROM_DAIRY" .

gs1:PackagingMarkedFreeFromCode-FREE_FROM_EGG
	rdf:type        gs1:PackagingMarkedFreeFromCode ;
	rdfs:comment    "The item is physically marked as free from egg."@en ;
	rdfs:label      "Free From Egg"@en ;
	skos:prefLabel  "FREE_FROM_EGG" .

gs1:PackagingMarkedFreeFromCode-FREE_FROM_FISH
	rdf:type        gs1:PackagingMarkedFreeFromCode ;
	rdfs:comment    "The item is physically marked as being free from fish."@en ;
	rdfs:label      "Free From Fish"@en ;
	skos:prefLabel  "FREE_FROM_FISH" .

gs1:PackagingMarkedFreeFromCode-FREE_FROM_GLUTEN
	rdf:type        gs1:PackagingMarkedFreeFromCode ;
	rdfs:comment    "The item is physically marked as free from gluten. This level of containment is frequently determined through regulation."@en ;
	rdfs:label      "Free From Gluten"@en ;
	skos:prefLabel  "FREE_FROM_GLUTEN" .

gs1:PackagingMarkedFreeFromCode-FREE_FROM_LACTOSE
	rdf:type        gs1:PackagingMarkedFreeFromCode ;
	rdfs:comment    "The item is physically marked as being free of lactose."@en ;
	rdfs:label      "Free Of Lactose"@en ;
	skos:prefLabel  "FREE_FROM_LACTOSE" .

gs1:PackagingMarkedFreeFromCode-FREE_FROM_LATEX
	rdf:type        gs1:PackagingMarkedFreeFromCode ;
	rdfs:comment    "The item is physically marked being free from Latex (rubber)."@en ;
	rdfs:label      "Free From Latex"@en ;
	skos:prefLabel  "FREE_FROM_LATEX" .

gs1:PackagingMarkedFreeFromCode-FREE_FROM_LEGUME_PROTEIN
	rdf:type        gs1:PackagingMarkedFreeFromCode ;
	rdfs:comment    "The item is physically marked as being free from legume protein."@en ;
	rdfs:label      "Free From Legume Protein"@en ;
	skos:prefLabel  "FREE_FROM_LEGUME_PROTEIN" .

gs1:PackagingMarkedFreeFromCode-FREE_FROM_MILK
	rdf:type        gs1:PackagingMarkedFreeFromCode ;
	rdfs:comment    "The item is physically marked as being free from milk and any of its derivatives."@en ;
	rdfs:label      "Free From Milk"@en ;
	skos:prefLabel  "FREE_FROM_MILK" .

gs1:PackagingMarkedFreeFromCode-FREE_FROM_MILK_PROTEIN
	rdf:type        gs1:PackagingMarkedFreeFromCode ;
	rdfs:comment    "The item is physically marked as being free from milk protein."@en ;
	rdfs:label      "Free From Milk Protein"@en ;
	skos:prefLabel  "FREE_FROM_MILK_PROTEIN" .

gs1:PackagingMarkedFreeFromCode-FREE_FROM_NATURAL_GLUTEN
	rdf:type        gs1:PackagingMarkedFreeFromCode ;
	rdfs:comment    "The item is physically marked as being naturally free from gluten and not extracted as part of the manufacturing process."@en ;
	rdfs:label      "Naturally Free From Gluten"@en ;
	skos:prefLabel  "FREE_FROM_NATURAL_GLUTEN" .

gs1:PackagingMarkedFreeFromCode-FREE_FROM_PEANUTS
	rdf:type        gs1:PackagingMarkedFreeFromCode ;
	rdfs:comment    "The item is physically marked as being free from peanuts."@en ;
	rdfs:label      "Free From Peanuts"@en ;
	skos:prefLabel  "FREE_FROM_PEANUTS" .

gs1:PackagingMarkedFreeFromCode-FREE_FROM_PROTEIN
	rdf:type        gs1:PackagingMarkedFreeFromCode ;
	rdfs:comment    "The item is physically marked as being free from protein."@en ;
	rdfs:label      "Free from Protein"@en ;
	skos:prefLabel  "FREE_FROM_PROTEIN" .

gs1:PackagingMarkedFreeFromCode-FREE_FROM_PVC
	rdf:type        gs1:PackagingMarkedFreeFromCode ;
	rdfs:comment    "The item is physically marked as being free from PVC (Polyvinyl chloride)."@en ;
	rdfs:label      "Free from PVC"@en ;
	skos:prefLabel  "FREE_FROM_PVC" .

gs1:PackagingMarkedFreeFromCode-FREE_FROM_SOYA
	rdf:type        gs1:PackagingMarkedFreeFromCode ;
	rdfs:comment    "The item is physically marked as being free from soya."@en ;
	rdfs:label      "Free From Soya"@en ;
	skos:prefLabel  "FREE_FROM_SOYA" .

gs1:PackagingMarkedFreeFromCode-FREE_FROM_SUGAR
	rdf:type        gs1:PackagingMarkedFreeFromCode ;
	rdfs:comment    "The item is physically marked as being free from sugar."@en ;
	rdfs:label      "Free From Sugar"@en ;
	skos:prefLabel  "FREE_FROM_SUGAR" .

gs1:PackagingMarkedFreeFromCode-FREE_FROM_TRANSFAT
	rdf:type        gs1:PackagingMarkedFreeFromCode ;
	rdfs:comment    "The item is physically marked being free from Trans Fatty Acids (Trans Fat)"@en ;
	rdfs:label      "Free from Trans Fatty Acids"@en ;
	skos:prefLabel  "FREE_FROM_TRANSFAT" .

gs1:PackagingMarkedFreeFromCode-REDUCED_LACTOSE
	rdf:type        gs1:PackagingMarkedFreeFromCode ;
	rdfs:comment    "The item is physically marked as having a reduced amount of lactose"@en ;
	rdfs:label      "Reduced Amount of Lactose"@en ;
	skos:prefLabel  "REDUCED_LACTOSE" .

gs1:PackagingMarkedFreeFromCode-REDUCED_PROTEIN
	rdf:type        gs1:PackagingMarkedFreeFromCode ;
	rdfs:comment    "The item is physically marked as containing a low level of protein."@en ;
	rdfs:label      "Low Level of Protein"@en ;
	skos:prefLabel  "REDUCED_PROTEIN" .

gs1:PackagingMarkedFreeFromCode-REDUCED_TRANSFAT
	rdf:type        gs1:PackagingMarkedFreeFromCode ;
	rdfs:comment    "The item is physically marked as having a reduced amount of transfats (unsaturated)."@en ;
	rdfs:label      "Reduced Amount of Transfats"@en ;
	skos:prefLabel  "REDUCED_TRANSFAT" .

gs1:PackagingMarkedFreeFromCode-VERY_LOW_GLUTEN
	rdf:type        gs1:PackagingMarkedFreeFromCode ;
	rdfs:comment    "The item is physically marked as a very low amount of gluten. Very low is frequently determined through regulation for example, per EU Regulation (EC) No 41/2009 [of 20 January 2009], this is defined as containing between 20 and 100 mg/kg)."@en ;
	rdfs:label      "Very Low Amount of Gluten"@en ;
	skos:prefLabel  "VERY_LOW_GLUTEN" .

gs1:PackagingMarkedFreeFromCode-WITHOUT_ADDED_SALT
	rdf:type        gs1:PackagingMarkedFreeFromCode ;
	rdfs:comment    "The item is physically marked that no salt has been added when manufacturing the product but it still can contain salt that is naturally part of the ingredients, as approved by the appropriate authority of the target market."@en ;
	rdfs:label      "Without Added Salt"@en ;
	skos:prefLabel  "WITHOUT_ADDED_SALT" .

gs1:PackagingMarkedFreeFromCode-WITHOUT_ADDED_SUGAR
	rdf:type        gs1:PackagingMarkedFreeFromCode ;
	rdfs:comment    "The item is physically marked that no sugar has been added when manufacturing the product but it still can contain sugars that are naturally part of the ingredients, as approved by the appropriate authority of the target market."@en ;
	rdfs:label      "Without Added Sugar"@en ;
	skos:prefLabel  "WITHOUT_ADDED_SUGAR" .

gs1:PackagingMarkedFreeFromCode-WITHOUT_ADDED_SWEETENER
	rdf:type        gs1:PackagingMarkedFreeFromCode ;
	rdfs:comment    "The item is physically marked that no sweetener has been added when manufacturing the product."@en ;
	rdfs:label      "Without Added Sweetener"@en ;
	skos:prefLabel  "WITHOUT_ADDED_SWEETENER" .

gs1:PackagingMarkedLabelAccreditationCode-AMA_ORGANIC_SEAL
	rdf:type        gs1:PackagingMarkedLabelAccreditationCode ;
	rdfs:comment    "Austria Ministry of Agriculture Organic Label, AMA Marketing licenses the AMA organic logo. Red, white and black indicates the majority of ingredients are of Austrian origin."@en ;
	rdfs:label      "Austria Ministry of Agriculture Organic Label"@en ;
	skos:prefLabel  "AMA_ORGANIC_SEAL" .

gs1:PackagingMarkedLabelAccreditationCode-AUS_KAUP_ESTONIA
	rdf:type        gs1:PackagingMarkedLabelAccreditationCode ;
	rdfs:comment    "Used to specify Estonia Meat in their product."@en ;
	rdfs:label      "Aus Kaup Estonia"@en ;
	skos:prefLabel  "AUS_KAUP_ESTONIA" .

gs1:PackagingMarkedLabelAccreditationCode-BDIH_LOGO
	rdf:type        gs1:PackagingMarkedLabelAccreditationCode ;
	rdfs:label      "BDIH Germany guidelines for Certified Natural Cosmetics"@en ;
	skos:prefLabel  "BDIH_LOGO" .

gs1:PackagingMarkedLabelAccreditationCode-BETER_LEVEN_1_STER
	rdf:type        gs1:PackagingMarkedLabelAccreditationCode ;
	rdfs:comment    "The one-star Beter Leven (better life) mark indicates that the product comes from a company that cares that animals are kept according to the minimal requirements for sanitation and well-being for the cattle industry."@en ;
	rdfs:label      "Beter Leven One Star Mark"@en ;
	skos:prefLabel  "BETER_LEVEN_1_STER" .

gs1:PackagingMarkedLabelAccreditationCode-BETER_LEVEN_2_STER
	rdf:type        gs1:PackagingMarkedLabelAccreditationCode ;
	rdfs:comment    "The two-star Beter Leven (better life) mark indicates that the product comes from a company that provides for a higher well-being of animals than that established by the minimal requirements for sanitation and well-being for the cattle industry, yet the conditions are inferior to those of Biological-class products."@en ;
	rdfs:label      "Beter Leven Two Star Mark"@en ;
	skos:prefLabel  "BETER_LEVEN_2_STER" .

gs1:PackagingMarkedLabelAccreditationCode-BETER_LEVEN_3_STER
	rdf:type        gs1:PackagingMarkedLabelAccreditationCode ;
	rdfs:comment    "The three-star Beter Leven (better life) mark is awarded to products that come from companies that excel in keeping animals according to top guidelines for Biological-class products. In some cases this mark is accompanied by an EKO indication."@en ;
	rdfs:label      "Beter Leven Three Star Mark"@en ;
	skos:prefLabel  "BETER_LEVEN_3_STER" .

gs1:PackagingMarkedLabelAccreditationCode-BIO_AUSTRIA_LABEL
	rdf:type        gs1:PackagingMarkedLabelAccreditationCode ;
	rdfs:label      "Bio Austria"@en ;
	skos:prefLabel  "BIO_AUSTRIA_LABEL" .

gs1:PackagingMarkedLabelAccreditationCode-BIO_LABEL_GERMAN
	rdf:type        gs1:PackagingMarkedLabelAccreditationCode ;
	rdfs:label      "German national organic certification label (Bio-Siegel)"@en ;
	skos:prefLabel  "BIO_LABEL_GERMAN" .

gs1:PackagingMarkedLabelAccreditationCode-BIO_SUISSE_BUD_SEAL
	rdf:type        gs1:PackagingMarkedLabelAccreditationCode ;
	rdfs:label      "Represents interests of Swiss organic farmers"@en ;
	skos:prefLabel  "BIO_SUISSE_BUD_SEAL" .

gs1:PackagingMarkedLabelAccreditationCode-BLUE_ANGEL
	rdf:type        gs1:PackagingMarkedLabelAccreditationCode ;
	rdfs:comment    "The Blue Angel is awarded to companies as kind of a reward for their commitment to environmental protection. They use it to professionally promote their eco-friendly products in the market. The Blue Angel is an ecological beacon showing the consumer the way to the ecologically superior product and promotes environmentally conscious consumption."@en ;
	rdfs:label      "Blue Angel"@en ;
	skos:prefLabel  "BLUE_ANGEL" .

gs1:PackagingMarkedLabelAccreditationCode-BORD_BIA_APPROVED
	rdf:type        gs1:PackagingMarkedLabelAccreditationCode ;
	rdfs:comment    "The Bord Bia Approved logo is awarded to a company which has been audited by Bord Bia to verify that processes, from farm to fork, comply with the highest Quality Assurance Standards. These standards include animal welfare, traceability, environment, safety, feed, water, testing, inspection, hygiene and good manufacturing practice. Bord Bia Approved is awarded to a company where all the ingredients including meat content satisfy the Bord Bia requirements."@en ;
	rdfs:label      "Bord Bia Approved Logo"@en ;
	skos:prefLabel  "BORD_BIA_APPROVED" .

gs1:PackagingMarkedLabelAccreditationCode-BORD_BIA_APPROVED_MEAT
	rdf:type        gs1:PackagingMarkedLabelAccreditationCode ;
	rdfs:comment    "Bord Bia Approved - Meat Content Only applies to companies where only the meat content satisfies certain conditions detailed in the Bord Bia requirements document."@en ;
	rdfs:label      "Bord Bia Approved - Meat Content Only"@en ;
	skos:prefLabel  "BORD_BIA_APPROVED_MEAT" .

gs1:PackagingMarkedLabelAccreditationCode-BRA_MILJOVAL_LABEL_SWEDISH
	rdf:type        gs1:PackagingMarkedLabelAccreditationCode ;
	rdfs:comment    "Bra Miljoval Bra is the ecolabel of SSNC. It is referred to as Good Environmental Choice in English. SSNC started ecolabelling."@en ;
	rdfs:label      "Bra Miljoval"@en ;
	skos:prefLabel  "BRA_MILJOVAL_LABEL_SWEDISH" .

gs1:PackagingMarkedLabelAccreditationCode-CROSSED_GRAIN_SYMBOL
	rdf:type        gs1:PackagingMarkedLabelAccreditationCode ;
	rdfs:comment    "Crossed grain logo is a trademark owned and administered by Coeliac. It is a worldwide symbol for safe gluten-free foods. Each country has their own Coeliac"@en ;
	rdfs:label      "Crossed grain logo"@en ;
	skos:prefLabel  "CROSSED_GRAIN_SYMBOL" .

gs1:PackagingMarkedLabelAccreditationCode-DEMETER_LABEL
	rdf:type        gs1:PackagingMarkedLabelAccreditationCode ;
	rdfs:comment    "Demeter International trademark for products of certified biodynamic production."@en ;
	rdfs:label      "Demeter International Trademark"@en ;
	skos:prefLabel  "DEMETER_LABEL" .

gs1:PackagingMarkedLabelAccreditationCode-ECOCERT_CERTIFICATE
	rdf:type        gs1:PackagingMarkedLabelAccreditationCode ;
	rdfs:comment    "ECOCERT is a certification body for sustainable development."@en ;
	rdfs:label      "ECOCERT Certification"@en ;
	skos:prefLabel  "ECOCERT_CERTIFICATE" .

gs1:PackagingMarkedLabelAccreditationCode-ECO_LABEL_LADYBUG
	rdf:type        gs1:PackagingMarkedLabelAccreditationCode ;
	rdfs:comment    "This is a Finnish label used by the Organic union, which represents the entire Finnish organic industry, consumers and producers in a common interest group. They work as a neutral voice in various working groups and consultations, and prepare position papers and presentations. The Federation also organizes training events and professional seminars. The Organic Federation also publishes the magazine Organic."@en ;
	rdfs:label      "Eco Label Ladybug"@en ;
	skos:prefLabel  "ECO_LABEL_LADYBUG" .

gs1:PackagingMarkedLabelAccreditationCode-EC_NATIONAL_HEALTH_MARK
	rdf:type        gs1:PackagingMarkedLabelAccreditationCode ;
	rdfs:comment    "The package is physically marked with EC National Health Mark. The EC National Health Mark is the health mark for specific hygiene regulations for food of animal origin. The regulation (EC) Nr. 853/2004 of 29. April 2004 of the European Parliament on hygiene rules for food of animal origin demands that companies handling products of animal origin are authorised according to this regulation. The official body responsible for this authorisation assigns a health mark to the food producing company"@en ;
	rdfs:label      "EC National Health Mark"@en ;
	skos:prefLabel  "EC_NATIONAL_HEALTH_MARK" .

gs1:PackagingMarkedLabelAccreditationCode-EESTI_OKOMARK
	rdf:type        gs1:PackagingMarkedLabelAccreditationCode ;
	rdfs:comment    "Estonian Eco Label: Ministry of Agriculture Okomark (Label of Organic Food)."@en ;
	rdfs:label      "EESTI OKOMARK (Label of Organic Food)"@en ;
	skos:prefLabel  "EESTI_OKOMARK" .

gs1:PackagingMarkedLabelAccreditationCode-EESTI_PARIM_TOIDUAINE
	rdf:type        gs1:PackagingMarkedLabelAccreditationCode ;
	rdfs:comment    "Best Food Association of Estonia Food Industry http://www.toiduliit.ee/. An organisation that supports and promote Estonian food industry and economy, and contribute to a balanced and appropriate ethics to members of a favourable business environment for development."@en ;
	rdfs:label      "Best Food Association of Estonia Food Industry"@en ;
	skos:prefLabel  "EESTI_PARIM_TOIDUAINE" .

gs1:PackagingMarkedLabelAccreditationCode-EKO
	rdf:type        gs1:PackagingMarkedLabelAccreditationCode ;
	rdfs:comment    "This symbol stands for organic production certified by Skal that meets the requirements of the EU-regulation for organic production. Skal is the inspection body for the organic production in the Netherlands."@en ;
	rdfs:label      "Skal EKO Label"@en ;
	skos:prefLabel  "EKO" .

gs1:PackagingMarkedLabelAccreditationCode-EU_ECO_LABEL
	rdf:type        gs1:PackagingMarkedLabelAccreditationCode ;
	rdfs:comment    "The item is physically marked with the European Union Eco label a European environmental initiative supported by the European Commission."@en ;
	rdfs:label      "European Union Eco Label"@en ;
	skos:prefLabel  "EU_ECO_LABEL" .

gs1:PackagingMarkedLabelAccreditationCode-EU_ORGANIC_FARMING
	rdf:type        gs1:PackagingMarkedLabelAccreditationCode ;
	rdfs:comment    "New EU organic logo the EU introduced a new organic logo to ensure consumer protection and common standards."@en ;
	rdfs:label      "EU Organic Farming Logo"@en ;
	skos:prefLabel  "EU_ORGANIC_FARMING" .

gs1:PackagingMarkedLabelAccreditationCode-FAIR_TRADE_MARK
	rdf:type        gs1:PackagingMarkedLabelAccreditationCode ;
	rdfs:comment    "The Fair Trade Mark certifies that products meet the social, economic and environmental International Fair trade Standards. The Fair Trade Mark is usually supported by a local Fair Trade Labelling Organization and certifies products not companies. It does not cover the companies or organizations selling the product"@en ;
	rdfs:label      "The Fair Trade Mark"@en ;
	skos:prefLabel  "FAIR_TRADE_MARK" .

gs1:PackagingMarkedLabelAccreditationCode-FALKEN
	rdf:type        gs1:PackagingMarkedLabelAccreditationCode ;
	rdfs:label      "Falken"@en ;
	skos:prefLabel  "FALKEN" .

gs1:PackagingMarkedLabelAccreditationCode-FINNISH_HEART_SYMBOL
	rdf:type        gs1:PackagingMarkedLabelAccreditationCode ;
	rdfs:comment    "The heart symbol to inform the consumer at one glance that the product marked with this symbol is a preferred choice in its product group with regard to fat and sodium. Finnish Heart Association."@en ;
	rdfs:label      "Finnish Heart Symbol"@en ;
	skos:prefLabel  "FINNISH_HEART_SYMBOL" .

gs1:PackagingMarkedLabelAccreditationCode-FOREST_STEWARDSHIP_COUNCIL_LABEL
	rdf:type        gs1:PackagingMarkedLabelAccreditationCode ;
	rdfs:comment    "The item is physically marked with the Forest Stewardship Council label."@en ;
	rdfs:label      "Forest Stewardship Council Label"@en ;
	skos:prefLabel  "FOREST_STEWARDSHIP_COUNCIL_LABEL" .

gs1:PackagingMarkedLabelAccreditationCode-GMO_MARKED
	rdf:type        gs1:PackagingMarkedLabelAccreditationCode ;
	rdfs:comment    "The item is physically marked as of genetically modified origin."@en ;
	rdfs:label      "GMO Marked"@en ;
	skos:prefLabel  "GMO_MARKED" .

gs1:PackagingMarkedLabelAccreditationCode-GOODS_FROM_FINLAND_BLUE_SWAN
	rdf:type        gs1:PackagingMarkedLabelAccreditationCode ;
	rdfs:label      "Finfood Suomen Ruokatieto Ry"@en ;
	skos:prefLabel  "GOODS_FROM_FINLAND_BLUE_SWAN" .

gs1:PackagingMarkedLabelAccreditationCode-GREEN_DOT
	rdf:type        gs1:PackagingMarkedLabelAccreditationCode ;
	rdfs:label      "Green Dot"@en ;
	skos:prefLabel  "GREEN_DOT" .

gs1:PackagingMarkedLabelAccreditationCode-GREEN_RESTAURANT_ASSOCIATION_ENDORSED
	rdf:type        gs1:PackagingMarkedLabelAccreditationCode ;
	rdfs:comment    "The item is physically marked with the Green Restaurant Association Endorsed symbol."@en ;
	rdfs:label      "Green Restaurant Association Endorsed symbol"@en ;
	skos:prefLabel  "GREEN_RESTAURANT_ASSOCIATION_ENDORSED" .

gs1:PackagingMarkedLabelAccreditationCode-GREEN_SEAL_CERTIFIED
	rdf:type        gs1:PackagingMarkedLabelAccreditationCode ;
	rdfs:comment    "The item is physically marked with the Green Seal Certified symbol."@en ;
	rdfs:label      "Green Seal Certified Symbol"@en ;
	skos:prefLabel  "GREEN_SEAL_CERTIFIED" .

gs1:PackagingMarkedLabelAccreditationCode-GUARANTEED_IRISH
	rdf:type        gs1:PackagingMarkedLabelAccreditationCode ;
	rdfs:comment    "Ireland: The Guaranteed Irish symbol makes shopping for Irish products and services a lot easier. Shoppers know that when they buy a product or service featuring the guaranteed Irish logo they are supporting Irish companies and safeguarding Irish jobs."@en ;
	rdfs:label      "Guaranteed Irish Symbol"@en ;
	skos:prefLabel  "GUARANTEED_IRISH" .

gs1:PackagingMarkedLabelAccreditationCode-KRAV_MARK
	rdf:type        gs1:PackagingMarkedLabelAccreditationCode ;
	rdfs:label      "KRAV Mark"@en ;
	skos:prefLabel  "KRAV_MARK" .

gs1:PackagingMarkedLabelAccreditationCode-LABEL_OF_THE_ALLERGY_AND_ASTHMA_FEDERATION
	rdf:type        gs1:PackagingMarkedLabelAccreditationCode ;
	rdfs:comment    "Allergy and Asthma Federation is a non-profit public health organisation. Our aim is to improve quality of life of the allergy and asthma patients."@en ;
	rdfs:label      "Allergy and Asthma Federation"@en ;
	skos:prefLabel  "LABEL_OF_THE_ALLERGY_AND_ASTHMA_FEDERATION" .

gs1:PackagingMarkedLabelAccreditationCode-LEAPING_BUNNY
	rdf:type        gs1:PackagingMarkedLabelAccreditationCode ;
	rdfs:comment    "The Coalition for Consumer Information on Cosmetics (CCIC) Leaping Bunny Program administers a cruelty-free standard and the internationally recognized Leaping Bunny Logo for companies producing cosmetic, personal care, and household products. The Leaping Bunny Program provides the best assurance that no new animal testing is used in any phase of product development by the company, its laboratories, or suppliers."@en ;
	rdfs:label      "Leaping Bunny Program"@en ;
	skos:prefLabel  "LEAPING_BUNNY" .

gs1:PackagingMarkedLabelAccreditationCode-LOODUSSOBRALIK_TOODE_ESTONIA
	rdf:type        gs1:PackagingMarkedLabelAccreditationCode ;
	rdfs:comment    "Eco-friendly product The sign eco-friendly product is designed to make environmentally friendly products on store shelves more as significant. When it comes to food shall be used for agriculture, natural farming methods. No use of mineral fertilizers, insect control and plant poisons."@en ;
	rdfs:label      "Loodussobralik Toode Estonia"@en ;
	skos:prefLabel  "LOODUSSOBRALIK_TOODE_ESTONIA" .

gs1:PackagingMarkedLabelAccreditationCode-LOVE_IRISH_FOOD
	rdf:type        gs1:PackagingMarkedLabelAccreditationCode ;
	rdfs:comment    "Love Irish Food - a promotional label printed on the product packaging to indicate to the consumer that the food is manufactured in Ireland using Irish ingredients."@en ;
	rdfs:label      "Love Irish Food"@en ;
	skos:prefLabel  "LOVE_IRISH_FOOD" .

gs1:PackagingMarkedLabelAccreditationCode-MADE_IN_FINLAND_FLAG_WITH_KEY
	rdf:type        gs1:PackagingMarkedLabelAccreditationCode ;
	rdfs:comment    "Made in Finland Products that are made in Finland Avainlippu (Key Flag) Suomalaisen Tyon"@en ;
	rdfs:label      "Made in Finland"@en ;
	skos:prefLabel  "MADE_IN_FINLAND_FLAG_WITH_KEY" .

gs1:PackagingMarkedLabelAccreditationCode-MARINE_STEWARDSHIP_COUNCIL_LABEL
	rdf:type        gs1:PackagingMarkedLabelAccreditationCode ;
	rdfs:label      "Marine Stewardship Council label"@en ;
	skos:prefLabel  "MARINE_STEWARDSHIP_COUNCIL_LABEL" .

gs1:PackagingMarkedLabelAccreditationCode-MAX_HAVELAAR
	rdf:type        gs1:PackagingMarkedLabelAccreditationCode ;
	rdfs:comment    "Fair trade symbol used in the Netherlands Target Market awarded to manufacturers which contribute to improving the living and working conditions of small farmers and agricultural workers in disadvantaged regions."@en ;
	rdfs:label      "Max Havelaar"@en ;
	skos:prefLabel  "MAX_HAVELAAR" .

gs1:PackagingMarkedLabelAccreditationCode-NATRUE_LABEL
	rdf:type        gs1:PackagingMarkedLabelAccreditationCode ;
	rdfs:comment    "The NATRUE Label guarantees that the products that carry it are made only with natural and organic ingredients, through soft manufacturing processes and environmentally friendly practices. The NATRUE Label is awarded by NATRUE, a non-profit organisation committed to promote and protect high standards of quality and environmental integrity."@en ;
	rdfs:label      "NATRUE Label"@en ;
	skos:prefLabel  "NATRUE_LABEL" .

gs1:PackagingMarkedLabelAccreditationCode-NYCKELHALET
	rdf:type        gs1:PackagingMarkedLabelAccreditationCode ;
	rdfs:comment    "The green key hole is to be put on the healthy foods in Sweden, Denmark, and Norway within certain product groups in order to make it easier for the customers to make a healthy choice. http://www.norden.org/"@en ;
	rdfs:label      "Green Key Hole"@en ;
	skos:prefLabel  "NYCKELHALET" .

gs1:PackagingMarkedLabelAccreditationCode-OEKO_TEX_LABEL
	rdf:type        gs1:PackagingMarkedLabelAccreditationCode ;
	rdfs:comment    "Confidence in textiles. This has been the motto of the independent test institutes of the International Oeko-Tex Association since 1992, with their tests for harmful substances according to Oeko-Tex Standard 100 for textile products of all types which pose no risk whatsoever to health."@en ;
	rdfs:label      "Confidence in Textiles Oeko-Tex"@en ;
	skos:prefLabel  "OEKO_TEX_LABEL" .

gs1:PackagingMarkedLabelAccreditationCode-OFFICIAL_ECO_LABEL_SUN
	rdf:type        gs1:PackagingMarkedLabelAccreditationCode ;
	rdfs:comment    "Luomo Sun Sign Denotes controlled organic production. The official label of the Finnish inspection authorities; owned by the Ministry of Agriculture and Forestry."@en ;
	rdfs:label      "Luomo Sun Sign"@en ;
	skos:prefLabel  "OFFICIAL_ECO_LABEL_SUN" .

gs1:PackagingMarkedLabelAccreditationCode-PEFC
	rdf:type        gs1:PackagingMarkedLabelAccreditationCode ;
	rdfs:comment    "Programme for Endorsement of Forest Certification (PEFCC_ is an international non-profit, non-governmental organisation dedicated to promoting Sustainable Forest Management (SFM) through independent third-party certification"@en ;
	rdfs:label      "Programme for Endorsement of Forest Certification"@en ;
	skos:prefLabel  "PEFC" .

gs1:PackagingMarkedLabelAccreditationCode-PROTECTED_DESIGNATION_OF_ORIGIN
	rdf:type        gs1:PackagingMarkedLabelAccreditationCode ;
	rdfs:comment    "The Protected designation of origin is the name of an area, a specific place or, in exceptional cases, the name of a country, used as a designation for an agricultural product or a foodstuff, the entire product must be traditionally and ENTIRELY manufactured (prepared, processed AND produced) within the specific region and thus acquire unique properties. Protected Geographical Status (PGS) is a legal framework defined in European Union law to protect the names of regional foods."@en ;
	rdfs:label      "Protected Designation of Origin"@en ;
	skos:prefLabel  "PROTECTED_DESIGNATION_OF_ORIGIN" .

gs1:PackagingMarkedLabelAccreditationCode-PROTECTED_GEOGRAPHICAL_INDICATION
	rdf:type        gs1:PackagingMarkedLabelAccreditationCode ;
	rdfs:comment    "The Protected geographical indication is the name of an area, a specific place or, in exceptional cases, the name of a country, used as a description of an agricultural product or a foodstuff, the entire product must be traditionally and at least PARTIALLY manufactured (prepared, processed OR produced) within the specific region and thus acquire unique properties. Protected Geographical Status (PGS) is a legal framework[1] defined in European Union law to protect the names of regional foods."@en ;
	rdfs:label      "Protected Geographical Indication"@en ;
	skos:prefLabel  "PROTECTED_GEOGRAPHICAL_INDICATION" .

gs1:PackagingMarkedLabelAccreditationCode-PROTECTED_HARVEST_CERTIFIED
	rdf:type        gs1:PackagingMarkedLabelAccreditationCode ;
	rdfs:comment    "The item is physically marked with the Protected Harvest Certified symbol."@en ;
	rdfs:label      "Protected Harvest Certified Symbol"@en ;
	skos:prefLabel  "PROTECTED_HARVEST_CERTIFIED" .

gs1:PackagingMarkedLabelAccreditationCode-QUALITY_MARK_IRELAND
	rdf:type        gs1:PackagingMarkedLabelAccreditationCode ;
	rdfs:comment    "Control IMO Organic farming is an alternative, environmentally friendly method of food production. It forbids the use of chemicals and requires production methods that respect animal welfare and do not damage the environment. The term organic can only be used on food labels in Ireland if the food product meets strict Irish and EU organic standards and is licensed by an approved certification body."@en ;
	rdfs:label      "Quality Mark Ireland"@en ;
	skos:prefLabel  "QUALITY_MARK_IRELAND" .

gs1:PackagingMarkedLabelAccreditationCode-RAINFOREST_ALLIANCE
	rdf:type        gs1:PackagingMarkedLabelAccreditationCode ;
	rdfs:comment    "The item is physically marked with the Rainforest Alliance Certified symbol."@en ;
	rdfs:label      "Rainforest Alliance Certified Symbol"@en ;
	skos:prefLabel  "RAINFOREST_ALLIANCE" .

gs1:PackagingMarkedLabelAccreditationCode-SCHARRELVLEES
	rdf:type        gs1:PackagingMarkedLabelAccreditationCode ;
	rdfs:comment    "A symbol used in the Netherlands Target Market intended for meat based products which guarantees that the animals has been growth without the use of antibiotics."@en ;
	rdfs:label      "Scharrelvlees"@en ;
	skos:prefLabel  "SCHARRELVLEES" .

gs1:PackagingMarkedLabelAccreditationCode-SOIL_ASSOCIATION_ORGANIC_SYMBOL
	rdf:type        gs1:PackagingMarkedLabelAccreditationCode ;
	rdfs:comment    "The Soil Association Organic Symbol is a symbol used in the UK to show that products meet a strict set of organic standards that protect health, sustainability and the environment."@en ;
	rdfs:label      "Soil Association Organic Symbol"@en ;
	skos:prefLabel  "SOIL_ASSOCIATION_ORGANIC_SYMBOL" .

gs1:PackagingMarkedLabelAccreditationCode-SUSTAINABLE_PALM_OIL_RSPO
	rdf:type        gs1:PackagingMarkedLabelAccreditationCode ;
	rdfs:comment    "In response to the urgent and pressing global call for sustainably produced palm oil, the Roundtable on Sustainable Palm Oil (RSPO) was formed in 2004 with the objective of promoting the growth and use of sustainable oil palm products through credible global standards and engagement of stakeholders."@en ;
	rdfs:label      "Sustainably Produced Palm Oil"@en ;
	skos:prefLabel  "SUSTAINABLE_PALM_OIL_RSPO" .

gs1:PackagingMarkedLabelAccreditationCode-SVANEN
	rdf:type        gs1:PackagingMarkedLabelAccreditationCode ;
	rdfs:comment    "The Swan is the Nordic environmental label. It was established by the Nordic Council of Ministers in 1989 and Denmark joined in 1997. The Swan is used in all Nordic countries, i.e. Denmark, Norway, Sweden, Finland and Iceland."@en ;
	rdfs:label      "Svanen"@en ;
	skos:prefLabel  "SVANEN" .

gs1:PackagingMarkedLabelAccreditationCode-SWEDISH_SEAL_OF_QUALITY
	rdf:type        gs1:PackagingMarkedLabelAccreditationCode ;
	rdfs:comment    "The item is physically marked with the Swedish Seal of Quality label which intends to guarantee the responsibility for the environment of the product."@en ;
	rdfs:label      "Swedish Seal of Quality Label"@en ;
	skos:prefLabel  "SWEDISH_SEAL_OF_QUALITY" .

gs1:PackagingMarkedLabelAccreditationCode-TRADITIONAL_SPECIALTY_GUARANTEED
	rdf:type        gs1:PackagingMarkedLabelAccreditationCode ;
	rdfs:comment    "The Traditional specialty guaranteed is a trademark for an agricultural product or a foodstuff, which has a certain feature or a set of features, setting it clearly apart from other similar products or foodstuffs belonging to the same category. The product or foodstuff must be manufactured using traditional ingredients or must be characteristic for its traditional composition, production process, or processing reflecting a traditional type of manufacturing or processing."@en ;
	rdfs:label      "Traditional Specialty Guaranteed"@en ;
	skos:prefLabel  "TRADITIONAL_SPECIALTY_GUARANTEED" .

gs1:PackagingMarkedLabelAccreditationCode-TUNNUSTATUD_EESTI_MAITSE
	rdf:type        gs1:PackagingMarkedLabelAccreditationCode ;
	rdfs:comment    "Approved Estonian Taste - Quality/Tradition/Origin/Traceability for Estonian products. All raw materials must be 100% Estonian. Estonian Chamber of Agriculture and Commerce."@en ;
	rdfs:label      "Approved Estonian Taste"@en ;
	skos:prefLabel  "TUNNUSTATUD_EESTI_MAITSE" .

gs1:PackagingMarkedLabelAccreditationCode-TUNNUSTATUD_MAITSE
	rdf:type        gs1:PackagingMarkedLabelAccreditationCode ;
	rdfs:comment    "Approved Taste label (designed as a barn swallow) denoting Estonian origin and high quality was introduced. This label has been given to products for Food quality and safety. Estonian Chamber of Agriculture and Commerce (ECAC)."@en ;
	rdfs:label      "Tunnustatud Maitse"@en ;
	skos:prefLabel  "TUNNUSTATUD_MAITSE" .

gs1:PackagingMarkedLabelAccreditationCode-UNIQUELY_FINNISH
	rdf:type        gs1:PackagingMarkedLabelAccreditationCode ;
	rdfs:comment    "Uniquely Finnish http://www.maakuntienparhaat.fi/en/ The Uniquely Finnish label is a national quality label for small entrepreneurs. ProAgria Association of Rural Advisory Centres grants the label to qualified foodstuff, handicraft and rural tourism companies based on applications."@en ;
	rdfs:label      "Uniquely Finnish"@en ;
	skos:prefLabel  "UNIQUELY_FINNISH" .

gs1:PackagingMarkedLabelAccreditationCode-USDA
	rdf:type        gs1:PackagingMarkedLabelAccreditationCode ;
	rdfs:label      "US Department of Agriculture"@en ;
	skos:prefLabel  "USDA" .

gs1:PackagingMarkedLabelAccreditationCode-UTZ_CERTIFIED
	rdf:type        gs1:PackagingMarkedLabelAccreditationCode ;
	rdfs:comment    "A certification which is intended to assure the social and environmental quality in coffee production. Coffee based products may be marked with this certification."@en ;
	rdfs:label      "UTZ Certified"@en ;
	skos:prefLabel  "UTZ_CERTIFIED" .

gs1:PackagingMarkedLabelAccreditationCode-VAELG_FULDKORN_FORST
	rdf:type        gs1:PackagingMarkedLabelAccreditationCode ;
	rdfs:comment    "Grain based foods (bread, breakfast products, baking articles etc.) which have got a high content of whole grain will be puffed with a nutritional puff from the beginning of 2009: Please choose whole grain first."@en ;
	rdfs:label      "Vaelg Fuldkorn forst"@en ;
	skos:prefLabel  "VAELG_FULDKORN_FORST" .

gs1:PackagingMarkedLabelAccreditationCode-WWF_PANDA_LABEL
	rdf:type        gs1:PackagingMarkedLabelAccreditationCode ;
	rdfs:comment    "Products that support the World Wildlife Federation."@en ;
	rdfs:label      "World Wildlife Federation Panda"@en ;
	skos:prefLabel  "WWF_PANDA_LABEL" .

gs1:PackagingMaterialTypeCode-BAMBOO
	rdf:type        gs1:PackagingMaterialTypeCode ;
	rdfs:comment    "Any of various woody or arborescent grasses (as of the genera Bambusa, Arundinaria, and Dendrocalamus of the subfamily Bambusoideae) of tropical and temperate regions having hollow stems, thick rhizomes, and shoots. The packaging may be in the form of paper, wood or leaves."@en ;
	rdfs:label      "Bamboo"@en ;
	skos:prefLabel  "BAMBOO" .

gs1:PackagingMaterialTypeCode-CELLULOSE_HYDRATE
	rdf:type        gs1:PackagingMaterialTypeCode ;
	rdfs:comment    "A class of materials manufactured by the conversion of natural cellulose to a soluble cellulosic derivative and subsequent regeneration, typically forming a film (e.g., cellophane). "@en ;
	rdfs:label      "Cellulose hydrate"@en ;
	skos:prefLabel  "CELLULOSE_HYDRATE" .

gs1:PackagingMaterialTypeCode-CERAMIC
	rdf:type        gs1:PackagingMaterialTypeCode ;
	rdfs:comment    "A non-specific material made from clay and hardened by firing at a high temperatures. Examples can include Terra-cotta, Earthenware, Stoneware, Porcelain, and High-Tech Ceramics."@en ;
	rdfs:label      "Ceramic"@en ;
	skos:prefLabel  "CERAMIC" .

gs1:PackagingMaterialTypeCode-CLOTH_OR_FABRIC
	rdf:type        gs1:PackagingMaterialTypeCode ;
	rdfs:comment    "A non specific material made by weaving, felting, knitting, or crocheting natural and/or synthetic fibers."@en ;
	rdfs:label      "Cloth or Fabric"@en ;
	skos:prefLabel  "CLOTH_OR_FABRIC" .

gs1:PackagingMaterialTypeCode-COMPOSITE
	rdf:type        gs1:PackagingMaterialTypeCode ;
	rdfs:comment    "A material that is made from multiple materials."@en ;
	rdfs:label      "Composite"@en ;
	skos:prefLabel  "COMPOSITE" .

gs1:PackagingMaterialTypeCode-CORK_NATURAL
	rdf:type        gs1:PackagingMaterialTypeCode ;
	rdfs:comment    "Cork is an impermeable buoyant material, the phellem layer of bark tissue that is harvested for commercial use primarily from Quercus suber (the cork oak)."@en ;
	rdfs:label      "Natural cork"@en ;
	skos:prefLabel  "CORK_NATURAL" .

gs1:PackagingMaterialTypeCode-CORRUGATED_BOARD_DOUBLE_WALL
	rdf:type        gs1:PackagingMaterialTypeCode ;
	rdfs:comment    "A structure formed by two layers of corrugated cardboard (flutes), with a linerboard facing between them."@en ;
	rdfs:label      "Double Wall Corrugated Board"@en ;
	skos:prefLabel  "CORRUGATED_BOARD_DOUBLE_WALL" .

gs1:PackagingMaterialTypeCode-CORRUGATED_BOARD_OTHER
	rdf:type        gs1:PackagingMaterialTypeCode ;
	rdfs:comment    "The value needed is not listed or is not defined within this list's individual code value and definitions of corrugated boards. Please send a work request into GS1 or your solution provider requesting the code you are searching for."@en ;
	rdfs:label      "Corrugated Board Other"@en ;
	skos:prefLabel  "CORRUGATED_BOARD_OTHER" .

gs1:PackagingMaterialTypeCode-CORRUGATED_BOARD_SINGLE_WALL
	rdf:type        gs1:PackagingMaterialTypeCode ;
	rdfs:comment    "A structure formed by three layers of paper that are glued using starch into one single, sturdy sheet; also termed double faced."@en ;
	rdfs:label      "Single Wall Corrugated Board"@en ;
	skos:prefLabel  "CORRUGATED_BOARD_SINGLE_WALL" .

gs1:PackagingMaterialTypeCode-CORRUGATED_BOARD_TRIPLE_WALL
	rdf:type        gs1:PackagingMaterialTypeCode ;
	rdfs:comment    "A structure formed by an inner and outer liner with three fluted sheets in between, each separated by a layer of paper."@en ;
	rdfs:label      "Triple Wall Corrugated Board"@en ;
	skos:prefLabel  "CORRUGATED_BOARD_TRIPLE_WALL" .

gs1:PackagingMaterialTypeCode-FIBRE_BURLAP
	rdf:type        gs1:PackagingMaterialTypeCode ;
	rdfs:comment    "The American name for cloth woven from jute plant skins and other vegetable fibres. In other parts of the world it is known as Hessian, Hessian cloth, or gunny from the Indian gain."@en ;
	rdfs:label      "Fibre Burlap"@en ;
	skos:prefLabel  "FIBRE_BURLAP" .

gs1:PackagingMaterialTypeCode-FIBRE_COTTON
	rdf:type        gs1:PackagingMaterialTypeCode ;
	rdfs:comment    "A natural cellulosic seed-hair fiber, obtained from the seed pod of the cotton plant. First known in India about 3000 B.C."@en ;
	rdfs:label      "Cotton"@en ;
	skos:prefLabel  "FIBRE_COTTON" .

gs1:PackagingMaterialTypeCode-FIBRE_FLAX
	rdf:type        gs1:PackagingMaterialTypeCode ;
	rdfs:comment    "The plant from the stem of which bast fiber is extracted by retting to produce linen. An erroneous term for linen fiber, particularly in blends."@en ;
	rdfs:label      "Flax"@en ;
	skos:prefLabel  "FIBRE_FLAX" .

gs1:PackagingMaterialTypeCode-FIBRE_HEMP
	rdf:type        gs1:PackagingMaterialTypeCode ;
	rdfs:comment    "Hemp is a commonly used term for varieties of the Cannabis plant. Hemp can yield fibre which can be used in ropes, cloths, weaves, as a reinforcement of polymer composites as well as pulps for paper making."@en ;
	rdfs:label      "Hemp"@en ;
	skos:prefLabel  "FIBRE_HEMP" .

gs1:PackagingMaterialTypeCode-FIBRE_JUTE
	rdf:type        gs1:PackagingMaterialTypeCode ;
	rdfs:comment    "A bast fiber obtained from the round pod jute or the long pod jute of the family Tiliaceae. Jute ribbon is purely made from the jute plant. Grown extensively in Pakistan and India, mainly in the Bengal district of Pakistan."@en ;
	rdfs:label      "Jute"@en ;
	skos:prefLabel  "FIBRE_JUTE" .

gs1:PackagingMaterialTypeCode-FIBRE_OTHER
	rdf:type        gs1:PackagingMaterialTypeCode ;
	rdfs:comment    "A non specific material made of a unit of matter, either natural or manufactured, that forms the basic element of fabrics and other textile structures."@en ;
	rdfs:label      "Fibre Other"@en ;
	skos:prefLabel  "FIBRE_OTHER" .

gs1:PackagingMaterialTypeCode-FOAM
	rdf:type        gs1:PackagingMaterialTypeCode ;
	rdfs:comment    "A non specific material in a lightweight cellular form resulting from introduction of gas bubbles during manufacture, used to reduce shock and vibration or abrasion. "@en ;
	rdfs:label      "Solidified Foam"@en ;
	skos:prefLabel  "FOAM" .

gs1:PackagingMaterialTypeCode-GLASS
	rdf:type        gs1:PackagingMaterialTypeCode ;
	rdfs:comment    "A substance mainly consisting of sand, lime and soda, fused at high temperatures and cooled quickly so that it solidifies to a vitreous or noncrystalline condition. This term applies to transparent clear glass or as a generic term if distinction with coloured glass is not desired. Example: sodocalcite."@en ;
	rdfs:label      "Glass"@en ;
	skos:prefLabel  "GLASS" .

gs1:PackagingMaterialTypeCode-GLASS_BOROSILICATE
	rdf:type        gs1:PackagingMaterialTypeCode ;
	rdfs:comment    "Glass composed of silicon, boron, sodium and aluminum oxides (+ other alkaline oxides). It is a technical glass, not recyclable."@en ;
	rdfs:label      "Borosilicate glass"@en ;
	skos:prefLabel  "GLASS_BOROSILICATE" .

gs1:PackagingMaterialTypeCode-GLASS_COLOURED
	rdf:type        gs1:PackagingMaterialTypeCode ;
	rdfs:comment    "Glass containing external colouring or glass that has been coloured by the addition of colouring agents/particles in its creation"@en ;
	rdfs:label      "Coloured Glass"@en ;
	skos:prefLabel  "GLASS_COLOURED" .

gs1:PackagingMaterialTypeCode-GLASS_CRYSTAL
	rdf:type        gs1:PackagingMaterialTypeCode ;
	rdfs:comment    "Glass rich in lead oxide. It is a technical glass, not recyclable, typically used in decorative objects and also in certain cosmetic packaging."@en ;
	rdfs:label      "Crystal glass"@en ;
	skos:prefLabel  "GLASS_CRYSTAL" .

gs1:PackagingMaterialTypeCode-LAMINATED_CARTON
	rdf:type        gs1:PackagingMaterialTypeCode ;
	rdfs:comment    "A material made up of laminates of paperboard, foil and polyethylene which combined form a sheet suitable for asceptic processing."@en ;
	rdfs:label      "Laminated Carton"@en ;
	skos:prefLabel  "LAMINATED_CARTON" .

gs1:PackagingMaterialTypeCode-METAL_ALUMINUM
	rdf:type        gs1:PackagingMaterialTypeCode ;
	rdfs:comment    "A non specific material made from aluminum or aluminum alloy."@en ;
	rdfs:label      "Aluminum"@en ;
	skos:prefLabel  "METAL_ALUMINUM" .

gs1:PackagingMaterialTypeCode-METAL_BRASS
	rdf:type        gs1:PackagingMaterialTypeCode ;
	rdfs:comment    "Brass is an alloy of copper and zinc."@en ;
	rdfs:label      "Brass"@en ;
	skos:prefLabel  "METAL_BRASS" .

gs1:PackagingMaterialTypeCode-METAL_COMPOSITE
	rdf:type        gs1:PackagingMaterialTypeCode ;
	rdfs:comment    "Refers to an object that is composed of two separate metals joined together. Instead of being a mixture of two or more metals, like alloys, metal composites consist of layers of different metals."@en ;
	rdfs:label      "Metal Composite"@en ;
	skos:prefLabel  "METAL_COMPOSITE" .

gs1:PackagingMaterialTypeCode-METAL_IRON
	rdf:type        gs1:PackagingMaterialTypeCode ;
	rdfs:comment    "A heavy metallic element (Fe) capable of being fashioned into a variety of forms.  "@en ;
	rdfs:label      "Iron"@en ;
	skos:prefLabel  "METAL_IRON" .

gs1:PackagingMaterialTypeCode-METAL_LEAD
	rdf:type        gs1:PackagingMaterialTypeCode ;
	rdfs:comment    "A bluish-white soft malleable ductile plastic but inelastic heavy metallic element (Pb)"@en ;
	rdfs:label      "Lead"@en ;
	skos:prefLabel  "METAL_LEAD" .

gs1:PackagingMaterialTypeCode-METAL_OTHER
	rdf:type        gs1:PackagingMaterialTypeCode ;
	rdfs:comment    "A non specific material made from metal or metal alloy material."@en ;
	rdfs:label      "Metal other"@en ;
	skos:prefLabel  "METAL_OTHER" .

gs1:PackagingMaterialTypeCode-METAL_STAINLESS_STEEL
	rdf:type        gs1:PackagingMaterialTypeCode ;
	rdfs:comment    "An alloy of steel with chromium and sometimes another element (as nickel or molybdenum) that is practically immune to rusting and ordinary corrosion "@en ;
	rdfs:label      "Stainless Steel"@en ;
	skos:prefLabel  "METAL_STAINLESS_STEEL" .

gs1:PackagingMaterialTypeCode-METAL_STEEL
	rdf:type        gs1:PackagingMaterialTypeCode ;
	rdfs:comment    "Commercial iron that contains carbon in any amount up to about 1.7 percent as an essential alloying constituent, is malleable when under suitable conditions, and is distinguished from cast iron by its malleability and lower carbon content."@en ;
	rdfs:label      "Steel"@en ;
	skos:prefLabel  "METAL_STEEL" .

gs1:PackagingMaterialTypeCode-METAL_TIN
	rdf:type        gs1:PackagingMaterialTypeCode ;
	rdfs:comment    "Tin is a chemical element that is obtained chiefly from the mineral cassiterite, where it occurs as an oxide, SnO2. This silvery, malleable poor metal is not easily oxidized in air, and is used to coat other metals to prevent corrosion. It is used in many alloys, most notably bronze"@en ;
	rdfs:label      "Tin"@en ;
	skos:prefLabel  "METAL_TIN" .

gs1:PackagingMaterialTypeCode-METAL_ZAMAC
	rdf:type        gs1:PackagingMaterialTypeCode ;
	rdfs:comment    "Zamac is a family of alloys with a base metal of zinc and alloying elements of aluminium, magnesium, and copper."@en ;
	rdfs:label      "Metal zamac"@en ;
	skos:prefLabel  "METAL_ZAMAC" .

gs1:PackagingMaterialTypeCode-MINERAL_CALCIUM_CARBONATE
	rdf:type        gs1:PackagingMaterialTypeCode ;
	rdfs:comment    "Ground calcium carbonate and precipitated calcium carbonate products serve as functional fillers in plastic and rubber applications. Calcium carbonate is widely used as in polyvinyl chloride (PVC), polyolefin, polypropylene (PP), polyethylene (PE) and unsaturated polyester resins applications. "@en ;
	rdfs:label      "Calcium Carbonate"@en ;
	skos:prefLabel  "MINERAL_CALCIUM_CARBONATE" .

gs1:PackagingMaterialTypeCode-MINERAL_OTHER
	rdf:type        gs1:PackagingMaterialTypeCode ;
	rdfs:comment    "Any other mineral-based material not available in this list.  Should be used as a temporary measure while a proper code is established"@en ;
	rdfs:label      "Mineral Other"@en ;
	skos:prefLabel  "MINERAL_OTHER" .

gs1:PackagingMaterialTypeCode-MINERAL_TALC
	rdf:type        gs1:PackagingMaterialTypeCode ;
	rdfs:comment    "Talc is used to stiffen thermoplastics, mainly polypropylene but also polyethylene and polyamide (Nylon)."@en ;
	rdfs:label      "Talc"@en ;
	skos:prefLabel  "MINERAL_TALC" .

gs1:PackagingMaterialTypeCode-NATURAL_RUBBER
	rdf:type        gs1:PackagingMaterialTypeCode ;
	rdfs:comment    "A strong elastic material made by drying the sap from various tropical trees, especially the American rubber tree."@en ;
	rdfs:label      "Natural rubber"@en ;
	skos:prefLabel  "NATURAL_RUBBER" .

gs1:PackagingMaterialTypeCode-OTHER
	rdf:type        gs1:PackagingMaterialTypeCode ;
	rdfs:comment    "The value needed is not listed or is not defined within this list's individual code values and definitions. Please send a work request into GS1 or your solution provider requesting the code you are searching for."@en ;
	rdfs:label      "Other"@en ;
	skos:prefLabel  "OTHER" .

gs1:PackagingMaterialTypeCode-PAPER_CORRUGATED
	rdf:type        gs1:PackagingMaterialTypeCode ;
	rdfs:comment    "Heavy paper with ridges and grooves, used in packing fragile articles."@en ;
	rdfs:label      "Corrugated Paper"@en ;
	skos:prefLabel  "PAPER_CORRUGATED" .

gs1:PackagingMaterialTypeCode-PAPER_KRAFT
	rdf:type        gs1:PackagingMaterialTypeCode ;
	rdfs:comment    "Kraft paper is the paper grade with the highest strength. It is used for the production of e.g. paper bags, emery paper or shopping bags."@en ;
	rdfs:label      "Kraft paper"@en ;
	skos:prefLabel  "PAPER_KRAFT" .

gs1:PackagingMaterialTypeCode-PAPER_KRAFT_WET_STRENGTH
	rdf:type        gs1:PackagingMaterialTypeCode ;
	rdfs:comment    "The wet-strength kraft paper has a certain tear strength when wet due to special additives. It is used for the production of e.g. paper bags, emery paper or shopping bags. "@en ;
	rdfs:label      "Kraft paper (wet strength)"@en ;
	skos:prefLabel  "PAPER_KRAFT_WET_STRENGTH" .

gs1:PackagingMaterialTypeCode-PAPER_MOLDED_PULP
	rdf:type        gs1:PackagingMaterialTypeCode ;
	rdfs:comment    "Used for producing pulp-based or fibrous products by pressing; example products: egg packages, trays and boxes for fruits and vegetables."@en ;
	rdfs:label      "Molded Pulp"@en ;
	skos:prefLabel  "PAPER_MOLDED_PULP" .

gs1:PackagingMaterialTypeCode-PAPER_OTHER
	rdf:type        gs1:PackagingMaterialTypeCode ;
	rdfs:comment    "Any other paper-based material not available in this list.  Should be used as a temporary measure while a proper code is established."@en ;
	rdfs:label      "Paper Other"@en ;
	skos:prefLabel  "PAPER_OTHER" .

gs1:PackagingMaterialTypeCode-PAPER_PAPER
	rdf:type        gs1:PackagingMaterialTypeCode ;
	rdfs:comment    "A non-specific sheet material produced by the matting of fibres from wood, rags, or other fibrous materials.  Generally, paper is of a lesser thickness or weight than paperboard."@en ;
	rdfs:label      "Paper"@en ;
	skos:prefLabel  "PAPER_PAPER" .

gs1:PackagingMaterialTypeCode-PAPER_PAPERBOARD
	rdf:type        gs1:PackagingMaterialTypeCode ;
	rdfs:comment    "A non specific material, generally made from cotton or wood, that describe a variety or of board materials used in the production of boxes, folding cartons, and solid fibre and corrugated shipping containers; also termed cardboard"@en ;
	rdfs:label      "Paperboard"@en ;
	skos:prefLabel  "PAPER_PAPERBOARD" .

gs1:PackagingMaterialTypeCode-PAPER_RAYON
	rdf:type        gs1:PackagingMaterialTypeCode ;
	rdfs:comment    "Generic term for a manmade fiber derived from regenerated cellulose."@en ;
	rdfs:label      "Rayon Paper "@en ;
	skos:prefLabel  "PAPER_RAYON" .

gs1:PackagingMaterialTypeCode-PLANT_LEAVES
	rdf:type        gs1:PackagingMaterialTypeCode ;
	rdfs:comment    "Plant leaves, such as banana leaves, including wet or dry leaves. In some cases, leaves are pre-softened by steaming."@en ;
	rdfs:label      "Plant Leaves"@en ;
	skos:prefLabel  "PLANT_LEAVES" .

gs1:PackagingMaterialTypeCode-PLASTIC_BIOPLASTIC
	rdf:type        gs1:PackagingMaterialTypeCode ;
	rdfs:comment    "Plastic materials made from biomass, but may have exactly the same properties as ordinary plastic. Sometimes these plastics are biodegradable."@en ;
	rdfs:label      "Bioplastic"@en ;
	skos:prefLabel  "PLASTIC_BIOPLASTIC" .

gs1:PackagingMaterialTypeCode-PLASTIC_OTHER
	rdf:type        gs1:PackagingMaterialTypeCode ;
	rdfs:comment    "A non-specific material made of any of numerous organic synthetic or processed materials that are mostly thermoplastic or thermosetting polymers of high molecular weight and that can be made into objects, films, or filaments."@en ;
	rdfs:label      "Plastic Other"@en ;
	skos:prefLabel  "PLASTIC_OTHER" .

gs1:PackagingMaterialTypeCode-PLASTIC_THERMOPLASTICS
	rdf:type        gs1:PackagingMaterialTypeCode ;
	rdfs:comment    "A non-specific substance that becomes soft and pliable when heated, without a change in its intrinsic properties. Polystyrene and polyethylene are thermoplastics."@en ;
	rdfs:label      "Thermoplastics"@en ;
	skos:prefLabel  "PLASTIC_THERMOPLASTICS" .

gs1:PackagingMaterialTypeCode-POLYMER_APET
	rdf:type        gs1:PackagingMaterialTypeCode ;
	rdfs:comment    "Polyethylene Terephthalate, amorphous (APET) has a very high transparency, is flame retardant and suitable for direct food contact. It is used for packaging of all kinds."@en ;
	rdfs:label      "Polyethylene Terephthalate, amorphous (APET)"@en ;
	skos:prefLabel  "POLYMER_APET" .

gs1:PackagingMaterialTypeCode-POLYMER_BOPP
	rdf:type        gs1:PackagingMaterialTypeCode ;
	rdfs:comment    "Biaxially oriented PP (BOPP) films are characterized by their tear, impact and puncture resistance. The film is mainly used in food packaging, e.g. as candy wrap or wrapping for chocolate bars."@en ;
	rdfs:label      "Polypropylene, longitudinally and laterally stretched (BOPP)"@en ;
	skos:prefLabel  "POLYMER_BOPP" .

gs1:PackagingMaterialTypeCode-POLYMER_CELLULOSE_ACETATE
	rdf:type        gs1:PackagingMaterialTypeCode ;
	rdfs:comment    "Cellulose acetate is one of the most important esters of cellulose. Depending on the way it has been processed cellulose acetate can be used for a wide variety of applications, e.g. films, membranes or fibers."@en ;
	rdfs:label      "Cellulose Acetate"@en ;
	skos:prefLabel  "POLYMER_CELLULOSE_ACETATE" .

gs1:PackagingMaterialTypeCode-POLYMER_CPET
	rdf:type        gs1:PackagingMaterialTypeCode ;
	rdfs:comment    "Crystallized polyethylene terephthalate (CPET) is a variation of standard PET which has been crystallized for heat resistance, rigidity, and toughness"@en ;
	rdfs:label      "Crystallized polyethylene terephthalate (CPET)"@en ;
	skos:prefLabel  "POLYMER_CPET" .

gs1:PackagingMaterialTypeCode-POLYMER_EPE
	rdf:type        gs1:PackagingMaterialTypeCode ;
	rdfs:comment    "EPE is foamed polyethylene, which is a type of environmentally friendly material, that is, pearl cotton like. EPE is made of low-density polyethylene grease through a physical foaming process to produce a non-crosslinked closed cell structure. EPE can be recycled and allows a certain amount of EPE recycled material to be matched in the manufacturing process. Also known as EPE Foam."@en ;
	rdfs:label      "Expanded Polyethylene"@en ;
	skos:prefLabel  "POLYMER_EPE" .

gs1:PackagingMaterialTypeCode-POLYMER_EPOXY
	rdf:type        gs1:PackagingMaterialTypeCode ;
	rdfs:comment    "Epoxy resins are thermoset polymers which are frequently used as coatings for metal packaging such as soft-drink cans."@en ;
	rdfs:label      "Epoxy"@en ;
	skos:prefLabel  "POLYMER_EPOXY" .

gs1:PackagingMaterialTypeCode-POLYMER_EPS
	rdf:type        gs1:PackagingMaterialTypeCode ;
	rdfs:comment    "Expanded polystyrene is a rigid, tough, closed cell and lightweight thermoplastic foam material. It is manufactured by expanding spherical beads in a mold, using heat and pressure to fuse the beads together. While each individual bead is a closed cell environment, there are significant open spaces between each bead."@en ;
	rdfs:label      "Expanded polystyrene (EPS)"@en ;
	skos:prefLabel  "POLYMER_EPS" .

gs1:PackagingMaterialTypeCode-POLYMER_EVA
	rdf:type        gs1:PackagingMaterialTypeCode ;
	rdfs:comment    "Ethylene vinyl acetate, a copolymer of 60 to 90% ethylene and 40 to 10% vinyl acetate.  Packaging applications include soft films, coatings, hot melt adhesives, wine cork substitutes, and closure seals for plastic and metal container caps."@en ;
	rdfs:label      "Ethylene vinyl acetate, (EVA)"@en ;
	skos:prefLabel  "POLYMER_EVA" .

gs1:PackagingMaterialTypeCode-POLYMER_EVOH
	rdf:type        gs1:PackagingMaterialTypeCode ;
	rdfs:comment    "Ethylene vinyl alcohol, a copolymer of ethylene and vinyl alcohol. A plastic resin commonly used in food applications to provide barrier to oxygen and other gases. "@en ;
	rdfs:label      "Ethylene vinyl alcohol, (EVOH)"@en ;
	skos:prefLabel  "POLYMER_EVOH" .

gs1:PackagingMaterialTypeCode-POLYMER_HDPE
	rdf:type        gs1:PackagingMaterialTypeCode ;
	rdfs:comment    "High-Density PolyEthylene (HDPE) is a polyethylene thermoplastic made from petroleum.  A strong, relatively opaque form of polyethylene having a dense structure with few side branches off the main carbon backbone. Can be applied to bottles, flasks and caps."@en ;
	rdfs:label      "High Density Polyethylene (HDPE) "@en ;
	skos:prefLabel  "POLYMER_HDPE" .

gs1:PackagingMaterialTypeCode-POLYMER_IONOMER
	rdf:type        gs1:PackagingMaterialTypeCode ;
	rdfs:comment    "Ionically is a cross-linked polyethylene (ionomer), can be used in combination with PE for its barrier properties."@en ;
	rdfs:label      "Polymer ionomer"@en ;
	skos:prefLabel  "POLYMER_IONOMER" .

gs1:PackagingMaterialTypeCode-POLYMER_LDPE
	rdf:type        gs1:PackagingMaterialTypeCode ;
	rdfs:comment    "Low-density polyethylene (LDPE) is a polyethylene thermoplastic made from petroleum.  A strong form of polyethylene having a less dense structure with more side branches off the main carbon backbone (on about 2% of the carbon atoms) than HDPE; therefore its tensile strength is lower, and its resilience is higherMade in translucent or opaque variations, it is quite flexible, and tough to the degree of being almost unbreakable.  It is widely used for manufacturing various containers, dispensing bottles, wash bottles, tubing, plastic bags for computer components, and various moulded laboratory equipment. Its most common use is in plastic bags."@en ;
	rdfs:label      "Low-density polyethylene (LDPE)"@en ;
	skos:prefLabel  "POLYMER_LDPE" .

gs1:PackagingMaterialTypeCode-POLYMER_LLDPE
	rdf:type        gs1:PackagingMaterialTypeCode ;
	rdfs:comment    "Linear low density polyethylene is a linear polyethylene with a significant number of short branches on the polymer backbone. It is commonly made by copolymerization of ethylene with longer-chain olefins. It is different from LDPE due to the absence of long chain branches which gives it higher tensile strength, impact and puncture resistance than LDPE. Common uses of LLDPE are plastic bags, wraps, stretch wraps, pouches, covers and lids."@en ;
	rdfs:label      "Linear Low Density Polyethylene"@en ;
	skos:prefLabel  "POLYMER_LLDPE" .

gs1:PackagingMaterialTypeCode-POLYMER_MDPE
	rdf:type        gs1:PackagingMaterialTypeCode ;
	rdfs:comment    "Medium-density polyethylene is a type of polyethylene defined by a density range of 0.926-0.940 g/cm3. MDPE is typically used in shrink films, sacks, packaging film and carrier bags."@en ;
	rdfs:label      "Medium-density Polyethylene"@en ;
	skos:prefLabel  "POLYMER_MDPE" .

gs1:PackagingMaterialTypeCode-POLYMER_MIX
	rdf:type        gs1:PackagingMaterialTypeCode ;
	rdfs:comment    "A polymer blend or mixture of least two polymers that are blended to create a new material with different physical properties. These tend to be a proprietary mix of polymers and cannot be separated. The individual materials may not be known by the seller."@en ;
	rdfs:label      "Polymer mix"@en ;
	skos:prefLabel  "POLYMER_MIX" .

gs1:PackagingMaterialTypeCode-POLYMER_NYLON
	rdf:type        gs1:PackagingMaterialTypeCode ;
	rdfs:comment    "Packaging applications include oven-baking bags (nylon 6 and nylon 66) and barrier layers (MXD6 and nylon 6) for PET and HDPE bottles. Very occasionally, bottles can be made of nylon."@en ;
	rdfs:label      "Nylon"@en ;
	skos:prefLabel  "POLYMER_NYLON" .

gs1:PackagingMaterialTypeCode-POLYMER_OPP
	rdf:type        gs1:PackagingMaterialTypeCode ;
	rdfs:comment    "Oriented polypropylene (OPP) is made of a soft polypropylene material which is stretched in a transverse or longitudinal direction (monoaxial) and becomes therefore brittle. Also known as: biaxially oriented polypropylene (BOPP), CAS Registry Number: 9003-07-0"@en ;
	rdfs:label      "Oriented polypropylene (OPP)"@en ;
	skos:prefLabel  "POLYMER_OPP" .

gs1:PackagingMaterialTypeCode-POLYMER_OTHER
	rdf:type        gs1:PackagingMaterialTypeCode ;
	rdfs:comment    "A non-specific chemical compound or mixture of compounds formed by polymerization and consisting essentially of repeating structural units "@en ;
	rdfs:label      "Polymers Other"@en ;
	skos:prefLabel  "POLYMER_OTHER" .

gs1:PackagingMaterialTypeCode-POLYMER_PA
	rdf:type        gs1:PackagingMaterialTypeCode ;
	rdfs:comment    "A polymer with repeating units linked by amide bonds. Polyamides (PA) occur both naturally and artificially, examples of naturally occurring polyamides are proteins, such as wool and silk. Artificially made polyamides can be  nylons, aramids, and sodium poly(aspartate)."@en ;
	rdfs:label      "Polyamide (PA)"@en ;
	skos:prefLabel  "POLYMER_PA" .

gs1:PackagingMaterialTypeCode-POLYMER_PAN
	rdf:type        gs1:PackagingMaterialTypeCode ;
	rdfs:comment    "Polyacrylonitril is a organic polymer which is frequently used in fibres for textiles. As fibres the material is frequently referred to as Acrylic. "@en ;
	rdfs:label      "Polyacrylonitril (PAN)"@en ;
	skos:prefLabel  "POLYMER_PAN" .

gs1:PackagingMaterialTypeCode-POLYMER_PC
	rdf:type        gs1:PackagingMaterialTypeCode ;
	rdfs:comment    "Polycarbonate, a transparent thermoplastic which is used in a wide variety of applications including CDs and DVDs, eyeglasses, cell phone covers, laptops as well as packaging applications such as bottles."@en ;
	rdfs:label      "Polycarbonate (PC)"@en ;
	skos:prefLabel  "POLYMER_PC" .

gs1:PackagingMaterialTypeCode-POLYMER_PCL
	rdf:type        gs1:PackagingMaterialTypeCode ;
	rdfs:comment    "Polycaprolactone is a biodegradable polyester which is also used in in the manufacturing of polyurethanes. It is also used in blends with thermoplastic starch to improve properties and can also be used as a plasticizer to PVC."@en ;
	rdfs:label      "Polycaprolactone (PCL)"@en ;
	skos:prefLabel  "POLYMER_PCL" .

gs1:PackagingMaterialTypeCode-POLYMER_PE
	rdf:type        gs1:PackagingMaterialTypeCode ;
	rdfs:comment    "A thermoplastic composed of the polymers of ethylene. "@en ;
	rdfs:label      "Polyethylene (PE)"@en ;
	skos:prefLabel  "POLYMER_PE" .

gs1:PackagingMaterialTypeCode-POLYMER_PEN
	rdf:type        gs1:PackagingMaterialTypeCode ;
	rdfs:comment    "Polyethylene naphthalate is a polymer with good barrier properties (unlike Polyethylene terephthalate). It is well-suited for production of the amber-colored bottles meant for packing beverages like beer."@en ;
	rdfs:label      "Polyethylene Naphthalate (PEN)"@en ;
	skos:prefLabel  "POLYMER_PEN" .

gs1:PackagingMaterialTypeCode-POLYMER_PET
	rdf:type        gs1:PackagingMaterialTypeCode ;
	rdfs:comment    "Polyethylene terephthalate is a thermoplastic polymer resin of the polyester family and is used in synthetic fibers. Can be applied to bottles, flasks and caps."@en ;
	rdfs:label      "Polyethylene Terephthalate (PET)"@en ;
	skos:prefLabel  "POLYMER_PET" .

gs1:PackagingMaterialTypeCode-POLYMER_PETG
	rdf:type        gs1:PackagingMaterialTypeCode ;
	rdfs:comment    "Polyethylene Terephthalate Glycol (PETG) is a PET modified with glycol, which is characterized by its aqueous properties (viscosity). Applications are found in injection molding."@en ;
	rdfs:label      "Polyethylene Terephthalate Glycol (PETG)"@en ;
	skos:prefLabel  "POLYMER_PETG" .

gs1:PackagingMaterialTypeCode-POLYMER_PHA
	rdf:type        gs1:PackagingMaterialTypeCode ;
	rdfs:comment    "Polyhydroxyalkanoates are linear polyesters produced in nature by bacterial fermentation of sugar or lipids."@en ;
	rdfs:label      "Polyhydroxyalkanoates (PHA)"@en ;
	skos:prefLabel  "POLYMER_PHA" .

gs1:PackagingMaterialTypeCode-POLYMER_PLA
	rdf:type        gs1:PackagingMaterialTypeCode ;
	rdfs:comment    "Polylactic acid or Polylactide is a biodegradable, thermoplastic, aliphatic polyester derived from lactic acid."@en ;
	rdfs:label      "Polylactic Acid or Polylactide (PLA)"@en ;
	skos:prefLabel  "POLYMER_PLA" .

gs1:PackagingMaterialTypeCode-POLYMER_PMMA
	rdf:type        gs1:PackagingMaterialTypeCode ;
	rdfs:comment    "Polymethyl Methacrylate (PMMA) is often used as a lightweight and shatterproof alternative to glass, due to its transparency, brilliance and scratch resistance, PMMA is therefore often referred to as acrylic glass."@en ;
	rdfs:label      "Polymethyl Methacrylate (PMMA)"@en ;
	skos:prefLabel  "POLYMER_PMMA" .

gs1:PackagingMaterialTypeCode-POLYMER_POM
	rdf:type        gs1:PackagingMaterialTypeCode ;
	rdfs:comment    "Polyoxymethylene (POM) is a thermoplastic with good mechanical properties and high dimensional stability. Fields of application are the automotive industry and electrical engineering, in packaging it is used for e.g. spray cans, gas lighter tanks, gas ampoules. Also known as acetal, polyacetal, and polyformaldehyde."@en ;
	rdfs:label      "Polyoxymethylene (POM)"@en ;
	skos:prefLabel  "POLYMER_POM" .

gs1:PackagingMaterialTypeCode-POLYMER_PP
	rdf:type        gs1:PackagingMaterialTypeCode ;
	rdfs:comment    "A non-specific material made of various thermoplastic plastics or fibers that are polymers of propylene. "@en ;
	rdfs:label      "Polypropylene (PP)"@en ;
	skos:prefLabel  "POLYMER_PP" .

gs1:PackagingMaterialTypeCode-POLYMER_PS
	rdf:type        gs1:PackagingMaterialTypeCode ;
	rdfs:comment    "A polymer prepared by the polymerization of styrene as the sole monomer"@en ;
	rdfs:label      "Polystyrene (PS)"@en ;
	skos:prefLabel  "POLYMER_PS" .

gs1:PackagingMaterialTypeCode-POLYMER_PU
	rdf:type        gs1:PackagingMaterialTypeCode ;
	rdfs:comment    "Polyurethanes are primarily thermoset resins which are used in the manufacture of flexible and rigid foams, microcellular foam seals and gaskets, as well as high performance adhesives, surface coatings and sealants. Polyurethane can also be used to make synthetic fibers."@en ;
	rdfs:label      "Polyurethanes (PU)"@en ;
	skos:prefLabel  "POLYMER_PU" .

gs1:PackagingMaterialTypeCode-POLYMER_PVA
	rdf:type        gs1:PackagingMaterialTypeCode ;
	rdfs:comment    "Polyvinyl alcohol (PVA or PVOH) is a biodegradable and highly water soluble polymer with high gas and grease barrier. Common uses for PVA are paper adhesives, paper coatings, as a self-standing water soluble films as well as blends to improve processability of thermoplastic starch. "@en ;
	rdfs:label      "Polyvinyl Alcohol (PVA)"@en ;
	skos:prefLabel  "POLYMER_PVA" .

gs1:PackagingMaterialTypeCode-POLYMER_PVC
	rdf:type        gs1:PackagingMaterialTypeCode ;
	rdfs:comment    "A polymer of vinyl chloride used especially for electrical insulation, films, and pipes"@en ;
	rdfs:label      "Polyvinyl Chloride (PVC)"@en ;
	skos:prefLabel  "POLYMER_PVC" .

gs1:PackagingMaterialTypeCode-POLYMER_PVDC
	rdf:type        gs1:PackagingMaterialTypeCode ;
	rdfs:comment    "Polyvinylidene chloride is primarily used as a barrier coating to provide barrier against fat, vapour and gases."@en ;
	rdfs:label      "Polyvinylidene Chloride (PVDC)"@en ;
	skos:prefLabel  "POLYMER_PVDC" .

gs1:PackagingMaterialTypeCode-POLYMER_SAN
	rdf:type        gs1:PackagingMaterialTypeCode ;
	rdfs:comment    "Styrene acrylonitrile (SAN) is a copolymer transparent and rigid plastic. Examples of applications are kitchenware and cosmetic packaging."@en ;
	rdfs:label      "Styrene acrylonitrile (SAN)"@en ;
	skos:prefLabel  "POLYMER_SAN" .

gs1:PackagingMaterialTypeCode-POLYMER_SILICONE
	rdf:type        gs1:PackagingMaterialTypeCode ;
	rdfs:comment    "Polymer is generally composed of organic chains linked together by the silicon-oxygen bond. Used in particular for valves. Also know as polysiloxane."@en ;
	rdfs:label      "Polymer silicone"@en ;
	skos:prefLabel  "POLYMER_SILICONE" .

gs1:PackagingMaterialTypeCode-POLYMER_TPS
	rdf:type        gs1:PackagingMaterialTypeCode ;
	rdfs:comment    "Thermoplastic starch is obtained through destructurization of natural starch through exposure to shear and heat. TPS is most frequently used in blends with biodegradable synthetic polymers such as PCL and PVA."@en ;
	rdfs:label      "Thermoplastic Starch (TPS)"@en ;
	skos:prefLabel  "POLYMER_TPS" .

gs1:PackagingMaterialTypeCode-POLYMER_XPS
	rdf:type        gs1:PackagingMaterialTypeCode ;
	rdfs:comment    "Extruded polystyrene is a rigid, tough, closed cell and lightweight thermoplastic foam material. It is manufactured using a process of extrusion that produces a homogeneous 'closed cell' matrix with each cell fully enclosed by polystyrene walls."@en ;
	rdfs:label      "Extruded polystyrene (XPS)"@en ;
	skos:prefLabel  "POLYMER_XPS" .

gs1:PackagingMaterialTypeCode-RUBBER
	rdf:type        gs1:PackagingMaterialTypeCode ;
	rdfs:comment    "A strong elastic synthetic substance made either by improving the qualities of natural rubber or by an industrial process using petroleum and coal products"@en ;
	rdfs:label      "Rubber"@en ;
	skos:prefLabel  "RUBBER" .

gs1:PackagingMaterialTypeCode-VINYL
	rdf:type        gs1:PackagingMaterialTypeCode ;
	rdfs:comment    "A non-specific polymer of a vinyl compound or a product (as a resin or a textile fiber) made from such a polymer "@en ;
	rdfs:label      "Vinyl"@en ;
	skos:prefLabel  "VINYL" .

gs1:PackagingMaterialTypeCode-WOOD_HARDBOARD
	rdf:type        gs1:PackagingMaterialTypeCode ;
	rdfs:comment    "Hardboard (not to be confused with hardwood), also called High-Density Fiberboard (HDF), is a type of fiberboard, which is similar to particle board and medium-density fiberboard, but is denser, much stronger and harder because it is made out of exploded wood fibers which have been highly compressed. Consequently, the density of hardboard is 31 lbs or more per cubic foot (500 kg/m_)[2] and is usually about 50-65 lbs per cubic foot (800-1040 kg/m_). It differs from particle board in that the bonding of the wood fibers requires no additional materials, although resin is often added. Unlike particle board, it will not split or crack."@en ;
	rdfs:label      "Hardboard"@en ;
	skos:prefLabel  "WOOD_HARDBOARD" .

gs1:PackagingMaterialTypeCode-WOOD_HARDWOOD
	rdf:type        gs1:PackagingMaterialTypeCode ;
	rdfs:comment    "A general term referring to any variety of broad-leaved, deciduous trees, and the wood from those trees. The term has nothing to do with the actual hardness of the wood; some hardwoods are softer than certain softwood (evergreen) species."@en ;
	rdfs:label      "Hardwood"@en ;
	skos:prefLabel  "WOOD_HARDWOOD" .

gs1:PackagingMaterialTypeCode-WOOD_MEDIUM_DENSITY_FIBREBOARD
	rdf:type        gs1:PackagingMaterialTypeCode ;
	rdfs:comment    "Medium-Density Fibreboard (MDF) is an engineered wood product made by breaking down hardwood or softwood residuals into wood fibres, combining them with wax and a resin binder, and forming panels by applying high temperature and pressure. MDF is generally denser than plywood. It is made up of separated fibres, but can be used as a building material similar in application to plywood. It is stronger and much more dense than particle board."@en ;
	rdfs:label      "Medium density fibreboard"@en ;
	skos:prefLabel  "WOOD_MEDIUM_DENSITY_FIBREBOARD" .

gs1:PackagingMaterialTypeCode-WOOD_ORIENTED_STRANDBOARD
	rdf:type        gs1:PackagingMaterialTypeCode ;
	rdfs:comment    "Oriented Strand Board (OSB), also known as sterling board, sterling OSB, aspenite, and smartply, is an engineered wood particle board formed by adding adhesives and then compressing layers of wood strands (flakes) in specific orientations. OSB may have a rough and variegated surface with the individual strips of around 2.5 - 15 cm (1 - 6 inch), lying unevenly across each other and comes in a variety of types."@en ;
	rdfs:label      "Oriented strand board (OSB)"@en ;
	skos:prefLabel  "WOOD_ORIENTED_STRANDBOARD" .

gs1:PackagingMaterialTypeCode-WOOD_OTHER
	rdf:type        gs1:PackagingMaterialTypeCode ;
	rdfs:comment    "A non specific material made from the hard fibrous lignified substance under the bark of trees."@en ;
	rdfs:label      "Wood other"@en ;
	skos:prefLabel  "WOOD_OTHER" .

gs1:PackagingMaterialTypeCode-WOOD_PARTICLE_BOARD
	rdf:type        gs1:PackagingMaterialTypeCode ;
	rdfs:comment    "Particle Board, also known as particleboard, chipboard, and Low-Density Fiberboard (LDF), is an engineered wood product manufactured from wood chips, sawmill shavings, or sawdust, and a synthetic resin or other suitable binder, which is pressed and extruded. Particle board is a composite material."@en ;
	rdfs:label      "Particle board"@en ;
	skos:prefLabel  "WOOD_PARTICLE_BOARD" .

gs1:PackagingMaterialTypeCode-WOOD_PLYWOOD
	rdf:type        gs1:PackagingMaterialTypeCode ;
	rdfs:comment    "Plywood, a manufactured wood panel similar to LDF, MDF, and HDF, is made from layering thin sheets of wood. Plywood layers (called veneers or plies) are glued together, with adjacent plies having their wood grain rotated relative to adjacent layers up to 90 degrees.  All plywoods bind resin and wood fibre sheets (cellulose cells are long, strong and thin) to form a composite material. "@en ;
	rdfs:label      "Plywood"@en ;
	skos:prefLabel  "WOOD_PLYWOOD" .

gs1:PackagingMaterialTypeCode-WOOD_SOFTWOOD
	rdf:type        gs1:PackagingMaterialTypeCode ;
	rdfs:comment    "General term used to describe lumber produced from needle and/or cone bearing trees (Conifers)."@en ;
	rdfs:label      "Softwood"@en ;
	skos:prefLabel  "WOOD_SOFTWOOD" .

gs1:PackagingRecyclingProcessTypeCode-COMPOSTABLE
	rdf:type        gs1:PackagingRecyclingProcessTypeCode ;
	rdfs:comment    "Packaging that can biodegrade generating a relatively homogeneous and stable humus-like substance."@en ;
	rdfs:label      "Compostable"@en ;
	skos:prefLabel  "COMPOSTABLE" .

gs1:PackagingRecyclingProcessTypeCode-ENERGY_RECOVERABLE
	rdf:type        gs1:PackagingRecyclingProcessTypeCode ;
	rdfs:comment    "Packaging which allows for a net calorific gain in energy recovery operations."@en ;
	rdfs:label      "Energy Recoverable"@en ;
	skos:prefLabel  "ENERGY_RECOVERABLE" .

gs1:PackagingRecyclingProcessTypeCode-RECYCLABLE
	rdf:type        gs1:PackagingRecyclingProcessTypeCode ;
	rdfs:comment    "Packaging material and format which can be diverted from the waste stream through available processes and programmes and can be collected, processed and returned to use in the form of raw materials or products."@en ;
	rdfs:label      "Recyclable"@en ;
	skos:prefLabel  "RECYCLABLE" .

gs1:PackagingRecyclingProcessTypeCode-REUSABLE
	rdf:type        gs1:PackagingRecyclingProcessTypeCode ;
	rdfs:comment    "Packaging that has been conceived and designed to accomplished within its life cycle a certain number of trips, rotations or uses for the same purpose for which it was conceived."@en ;
	rdfs:label      "Reusable"@en ;
	skos:prefLabel  "REUSABLE" .

gs1:PackagingRecyclingSchemeCode-ALKO
	rdf:type        gs1:PackagingRecyclingSchemeCode ;
	rdfs:comment    "Alko inc. is an independent, entirely State-owned company. Alko is administered and supervised by the Ministry of Social Affairs and Health. They have own recycling system for alcohol products bottles called Alko. This is a recycling system used in Finland"@en ;
	rdfs:label      "Alko Inc"@en ;
	skos:prefLabel  "ALKO" .

gs1:PackagingRecyclingSchemeCode-A_PULLO
	rdf:type        gs1:PackagingRecyclingSchemeCode ;
	rdfs:comment    "PALPA stands for Suomen Palautuspakkaus Oy. PALPA administers the recycling of beverage containers and promotes recycling in Finland. A-pullo is one of the recycling systems. PALPA is the administrator. This is a recycling system used in Finland."@en ;
	rdfs:label      "A Pullo"@en ;
	skos:prefLabel  "A_PULLO" .

gs1:PackagingRecyclingSchemeCode-EKO_PULLO
	rdf:type        gs1:PackagingRecyclingSchemeCode ;
	rdfs:comment    "PALPA Standas for Suomen Palautuspakkaus Oy. PALPA administers the recycling of beverage containers and promotes recycling in Finland. EKO-pullo is one of the recycling systems PALPA is administer. This is a recycling system used in Finland."@en ;
	rdfs:label      "EKO Pullo"@en ;
	skos:prefLabel  "EKO_PULLO" .

gs1:PackagingRecyclingSchemeCode-PALPA
	rdf:type        gs1:PackagingRecyclingSchemeCode ;
	rdfs:comment    "PALPA stands for Suomen Palautuspakkaus Oy. PALPA administers the recycling of beverage containers and promotes recycling in Finland. PALPA is on of the recycling systems PALPA is administer. This is a recycling system used in Finland."@en ;
	rdfs:label      "PALPA"@en ;
	skos:prefLabel  "PALPA" .

gs1:PackagingShapeCode-BAR
	rdf:type        gs1:PackagingShapeCode ;
	rdfs:comment    "A relatively long, evenly shaped piece of some solid substance"@en ;
	rdfs:label      "Bar"@en ;
	skos:prefLabel  "BAR" .

gs1:PackagingShapeCode-COIL
	rdf:type        gs1:PackagingShapeCode ;
	rdfs:comment    "A spiral structure made by winding a material into a series of loops. A coil may or may not have a spindle around which the loops are formed."@en ;
	rdfs:label      "Coil"@en ;
	skos:prefLabel  "COIL" .

gs1:PackagingShapeCode-CONE
	rdf:type        gs1:PackagingShapeCode ;
	rdfs:comment    "A cone is a three-dimensional geometric shape that tapers smoothly from a flat, round base to a point."@en ;
	rdfs:label      "Cone"@en ;
	skos:prefLabel  "CONE" .

gs1:PackagingShapeCode-CYLINDRICAL
	rdf:type        gs1:PackagingShapeCode ;
	rdfs:comment    "A long shape that has a circular base and an equally-sized circular top."@en ;
	rdfs:label      "Cylindrical"@en ;
	skos:prefLabel  "CYLINDRICAL" .

gs1:PackagingShapeCode-POLYGON
	rdf:type        gs1:PackagingShapeCode ;
	rdfs:comment    "A plane figure that is bounded by a closed path or circuit composed of a finite sequence of equally-sized straight line segments. A polygon may have a varying number of segments or faces resulting in different configurations, for example a 5-faced polygon: pentagon, 6-faced: hexagon, 8-faced: octagon, 12-faced: dodecahedron, etc."@en ;
	rdfs:label      "Polygon"@en ;
	skos:prefLabel  "POLYGON" .

gs1:PackagingShapeCode-RECTANGULAR
	rdf:type        gs1:PackagingShapeCode ;
	rdfs:comment    "A closed planar quadrilateral with four right angles."@en ;
	rdfs:label      "Rectangular"@en ;
	skos:prefLabel  "RECTANGULAR" .

gs1:PackagingShapeCode-SPHERICAL
	rdf:type        gs1:PackagingShapeCode ;
	rdfs:comment    "A perfectly round geometrical object in three-dimensional space, such as the shape of a round ball. Like a circle in two dimensions, a perfect sphere is completely symmetrical around its centre, with all points on the surface lying the same distance from the centre point."@en ;
	rdfs:label      "Spherical"@en ;
	skos:prefLabel  "SPHERICAL" .

gs1:PackagingShapeCode-TABLET
	rdf:type        gs1:PackagingShapeCode ;
	rdfs:comment    "The result of different materials being compressed into a solid block usually of small dimensions."@en ;
	rdfs:label      "Tablet"@en ;
	skos:prefLabel  "TABLET" .

gs1:PackagingShapeCode-UNSPECIFIED
	rdf:type        gs1:PackagingShapeCode ;
	rdfs:comment    "Shape is not currently specified in the list. To be used as a temporary means until a specific missing value is added to the list."@en ;
	rdfs:label      "Unspecified"@en ;
	skos:prefLabel  "UNSPECIFIED" .

gs1:PaymentMethod-BANKERS_DRAFT
	rdf:type        gs1:PaymentMethod ;
	rdfs:comment    "Issue of a banker's draft in payment of the funds."@en ;
	rdfs:label      "Bankers Draft"@en ;
	skos:prefLabel  "BANKERS_DRAFT" .

gs1:PaymentMethod-BANK_CHEQUE
	rdf:type        gs1:PaymentMethod ;
	rdfs:comment    "Payment by a pre-printed form, which has been completed by a financial institution, on which instructions are given to an account holder (a bank or building society) to pay a stated sum to a named recipient."@en ;
	rdfs:label      "Bank Cheque"@en ;
	skos:prefLabel  "BANK_CHEQUE" .

gs1:PaymentMethod-BANK_GIRO
	rdf:type        gs1:PaymentMethod ;
	rdfs:comment    "The payment was originally made by bankgiro."@en ;
	rdfs:label      "Bank Giro"@en ;
	skos:prefLabel  "BANK_GIRO" .

gs1:PaymentMethod-BOOKENTRY_CREDIT
	rdf:type        gs1:PaymentMethod ;
	rdfs:comment    "House Credit."@en ;
	rdfs:label      "Book Entry Credit"@en ;
	skos:prefLabel  "BOOKENTRY_CREDIT" .

gs1:PaymentMethod-BOOKENTRY_DEBIT
	rdf:type        gs1:PaymentMethod ;
	rdfs:comment    "House Debit."@en ;
	rdfs:label      "Book Entry Debit"@en ;
	skos:prefLabel  "BOOKENTRY_DEBIT" .

gs1:PaymentMethod-BOP
	rdf:type        gs1:PaymentMethod ;
	rdfs:coment     "Payment by balance of payments"@en ;
	rdfs:label      "BOP"@en ;
	skos:prefLabel  "BOP" .

gs1:PaymentMethod-CASH
	rdf:type        gs1:PaymentMethod ;
	rdfs:comment    "Payment by currency (including bills and coins) in circulation, including checking account deposits."@en ;
	rdfs:label      "Cash"@en ;
	skos:prefLabel  "CASH" .

gs1:PaymentMethod-CERTIFIED_CHEQUE
	rdf:type        gs1:PaymentMethod ;
	rdfs:comment    "Payment by a pre-printed form stamped with the paying bank's certification on which instructions are given to an account holder (a bank or building society) to pay a stated sum to a named recipient ."@en ;
	rdfs:label      "Certified Cheque"@en ;
	skos:prefLabel  "CERTIFIED_CHEQUE" .

gs1:PaymentMethod-CHEQUE
	rdf:type        gs1:PaymentMethod ;
	rdfs:comment    "Payment by a pre-printed form on which instructions are given to an account holder (a bank or building society) to pay a stated sum to a named recipient."@en ;
	rdfs:label      "Cheque"@en ;
	skos:prefLabel  "CHEQUE" .

gs1:PaymentMethod-CREDIT_CARD
	rdf:type        gs1:PaymentMethod ;
	rdfs:comment    "Payment by means of a card issued by a bank or other financial institution."@en ;
	rdfs:label      "Credit Card"@en ;
	skos:prefLabel  "CREDIT_CARD" .

gs1:PaymentMethod-CREDIT_CARD_AMEX
	rdf:type        gs1:PaymentMethod ;
	rdfs:comment    "Payment by American Express credit card"@en ;
	rdfs:label      "American Express Credit Card"@en ;
	skos:prefLabel  "CREDIT_CARD_AMEX" .

gs1:PaymentMethod-CREDIT_CARD_DINERS_CLUB
	rdf:type        gs1:PaymentMethod ;
	rdfs:comment    "Payment by Diners Club credit card"@en ;
	rdfs:label      "Diners Club Credit Card"@en ;
	skos:prefLabel  "CREDIT_CARD_DINERS_CLUB" .

gs1:PaymentMethod-CREDIT_CARD_DISCOVER
	rdf:type        gs1:PaymentMethod ;
	rdfs:comment    "Payment by Discover credit card"@en ;
	rdfs:label      "Discover Credit Card"@en ;
	skos:prefLabel  "CREDIT_CARD_DISCOVER" .

gs1:PaymentMethod-CREDIT_CARD_MASTERCARD
	rdf:type        gs1:PaymentMethod ;
	rdfs:comment    "Payment by Mastercard credit card"@en ;
	rdfs:label      "Mastercard Credit Card"@en ;
	skos:prefLabel  "CREDIT_CARD_MASTERCARD" .

gs1:PaymentMethod-CREDIT_CARD_VISA
	rdf:type        gs1:PaymentMethod ;
	rdfs:comment    "Payment by Visa credit card"@en ;
	rdfs:label      "Visa Credit Card"@en ;
	skos:prefLabel  "CREDIT_CARD_VISA" .

gs1:PaymentMethod-DEBIT_CARD
	rdf:type        gs1:PaymentMethod ;
	rdfs:comment    "The amount is to be, or has been, directly debited to the customer's bank account through a bank card."@en ;
	rdfs:label      "Debit Card"@en ;
	skos:prefLabel  "DEBIT_CARD" .

gs1:PaymentMethod-DEBIT_CARD_MAESTRO
	rdf:type        gs1:PaymentMethod ;
	rdfs:comment    "Payment by Maestro debit card"@en ;
	rdfs:label      "Maestro Debit Card"@en ;
	skos:prefLabel  "DEBIT_CARD_MAESTRO" .

gs1:PaymentMethod-DEBIT_CARD_MASTERCARD
	rdf:type        gs1:PaymentMethod ;
	rdfs:comment    "Payment by Mastercard debit card"@en ;
	rdfs:label      "Mastercard Debit Card"@en ;
	skos:prefLabel  "DEBIT_CARD_MASTERCARD" .

gs1:PaymentMethod-DEBIT_CARD_VISA
	rdf:type        gs1:PaymentMethod ;
	rdfs:comment    "Payment by Visa debit card"@en ;
	rdfs:label      "Visa Debit Card"@en ;
	skos:prefLabel  "DEBIT_CARD_VISA" .

gs1:PaymentMethod-DEBIT_CARD_VISA_ELECTRON
	rdf:type        gs1:PaymentMethod ;
	rdfs:comment    "Payment by Visa Electron debit card"@en ;
	rdfs:label      "Visa Electron Debit Card"@en ;
	skos:prefLabel  "DEBIT_CARD_VISA_ELECTRON" .

gs1:PaymentMethod-ELECTRONIC_CREDIT_ACH
	rdf:type        gs1:PaymentMethod ;
	rdfs:comment    "A credit transaction made through the automated clearing house system"@en ;
	rdfs:label      "Electronic Credit ACH"@en ;
	skos:prefLabel  "ELECTRONIC_CREDIT_ACH" .

gs1:PaymentMethod-ELECTRONIC_DEBIT_ACH
	rdf:type        gs1:PaymentMethod ;
	rdfs:comment    "A debit transaction made through the automated clearing house system."@en ;
	rdfs:label      "Electronic Debit ACH"@en ;
	skos:prefLabel  "ELECTRONIC_DEBIT_ACH" .

gs1:PaymentMethod-FED_WIRE_NON_REPETITIVE
	rdf:type        gs1:PaymentMethod ;
	rdfs:comment    "Fedwire is a real time gross settlement funds transfer system operated by the Federal Reserve Banks that enables financial institutions to electronically transfer funds between its participants."@en ;
	rdfs:label      "Fedwire Non-repetitive"@en ;
	skos:prefLabel  "FED_WIRE_NON_REPETITIVE" .

gs1:PaymentMethod-FED_WIRE_REPETITIVE
	rdf:type        gs1:PaymentMethod ;
	rdfs:comment    "Repetitive Fedwire is a real time gross settlement funds transfer system operated by the Federal Reserve Banks that enables financial institutions to electronically transfer funds between its participants. Repetitive wire transfers are sent by the same party to the same recipient through the same financial institution with the same wiring instructions"@en ;
	rdfs:label      "Fedwire Repetitive"@en ;
	skos:prefLabel  "FED_WIRE_REPETITIVE" .

gs1:PaymentMethod-INTERNATIONAL_WIRE
	rdf:type        gs1:PaymentMethod ;
	rdfs:comment    "Payment by international wire transfer"@en ;
	rdfs:label      "International Wire"@en ;
	skos:prefLabel  "INTERNATIONAL_WIRE" .

gs1:PaymentMethod-LETTER_OF_CREDIT
	rdf:type        gs1:PaymentMethod ;
	rdfs:comment    "The financial operation is a letter of credit."@en ;
	rdfs:label      "Letter of Credit"@en ;
	skos:prefLabel  "LETTER_OF_CREDIT" .

gs1:PaymentMethod-ONLINE_PAYMENT
	rdf:type        gs1:PaymentMethod ;
	rdfs:comment    "Payment by online payment mechanisms"@en ;
	rdfs:label      "Online Payment"@en ;
	skos:prefLabel  "ONLINE_PAYMENT" .

gs1:PaymentMethod-ONLINE_PAYMENT_APPLE_PAY
	rdf:type        gs1:PaymentMethod ;
	rdfs:comment    "Online payment via Apple Pay"@en ;
	rdfs:label      "Apple Pay"@en ;
	skos:prefLabel  "ONLINE_PAYMENT_APPLE_PAY" .

gs1:PaymentMethod-ONLINE_PAYMENT_GOOGLE_WALLET
	rdf:type        gs1:PaymentMethod ;
	rdfs:comment    "Online payment via Google Wallet"@en ;
	rdfs:label      "Google Wallet"@en ;
	skos:prefLabel  "ONLINE_PAYMENT_GOOGLE_WALLET" .

gs1:PaymentMethod-ONLINE_PAYMENT_PAYPAL
	rdf:type        gs1:PaymentMethod ;
	rdfs:comment    "Online payment via PayPal"@en ;
	rdfs:label      "PayPal"@en ;
	skos:prefLabel  "ONLINE_PAYMENT_PAYPAL" .

gs1:PaymentMethod-POSTGIRO
	rdf:type        gs1:PaymentMethod ;
	rdfs:comment    "The financial operation has been done by postgiro."@en ;
	rdfs:label      "Postgiro"@en ;
	skos:prefLabel  "POSTGIRO" .

gs1:PaymentMethod-WIRE_TRANSFER_CREDIT
	rdf:type        gs1:PaymentMethod ;
	rdfs:comment    "Payment by wire transfer credit"@en ;
	rdfs:label      "Wire Transfer Credit"@en ;
	skos:prefLabel  "WIRE_TRANSFER_CREDIT" .

gs1:PaymentMethod-WIRE_TRANSFER_DEBIT
	rdf:type        gs1:PaymentMethod ;
	rdfs:comment    "Payment by wire transfer debit"@en ;
	rdfs:label      "Wire Transfer Debit"@en ;
	skos:prefLabel  "WIRE_TRANSFER_DEBIT" .

gs1:Power
	rdf:type     gs1:MeasurementType ;
	rdfs:comment    "The rate of doing work or rate of production, transfer or consumption of energy; the amount of energy transferred or converted per unit time.  SI Units: watt"@en ;
	rdfs:label      "Power"@en ;
	skos:prefLabel  "Power" .

gs1:PreparationTypeCode-AS_DRAINED
	rdf:type        gs1:PreparationTypeCode ;
	rdfs:comment    "The state of the product after it has been separated from any liquid within the package. For example, a can of apricots in syrup would have a different nutritional composition if the apricots are consumed with the syrup rather than if the syrup is drained before consuming the apricots (because of the high sugar and energy content of the syrup)."@en ;
	rdfs:label      "As Drained"@en ;
	skos:prefLabel  "AS_DRAINED" .

gs1:PreparationTypeCode-BAKE
	rdf:type        gs1:PreparationTypeCode ;
	rdfs:comment    "Cooking food in an oven by dry heat applied evenly throughout the oven"@en ;
	rdfs:label      "Bake"@en ;
	skos:prefLabel  "BAKE" .

gs1:PreparationTypeCode-BARBECUE
	rdf:type        gs1:PreparationTypeCode ;
	rdfs:comment    "Method of cooking meat with the heat and hot gasses of a fire"@en ;
	rdfs:label      "Barbecue"@en ;
	skos:prefLabel  "BARBECUE" .

gs1:PreparationTypeCode-BLANCH
	rdf:type        gs1:PreparationTypeCode ;
	rdfs:comment    "Food preparation wherein the food substance is rapidly plunged into boiling water and then removed after a brief, timed interval and then plunged into iced water or placed under cold running water"@en ;
	rdfs:label      "Blanch"@en ;
	skos:prefLabel  "BLANCH" .

gs1:PreparationTypeCode-BLIND_BAKE
	rdf:type        gs1:PreparationTypeCode ;
	rdfs:comment    "Baking a pie crust or other pastry without the filling"@en ;
	rdfs:label      "Blind Bake"@en ;
	skos:prefLabel  "BLIND_BAKE" .

gs1:PreparationTypeCode-BOIL
	rdf:type        gs1:PreparationTypeCode ;
	rdfs:comment    "Cooking food in boiling water, or other water-based liquid such as stock or milk"@en ;
	rdfs:label      "Boil"@en ;
	skos:prefLabel  "BOIL" .

gs1:PreparationTypeCode-BRAISE
	rdf:type        gs1:PreparationTypeCode ;
	rdfs:comment    "Cooking with moist heat, typically in a covered pot with a small amount of liquid"@en ;
	rdfs:label      "Braise"@en ;
	skos:prefLabel  "BRAISE" .

gs1:PreparationTypeCode-BROIL
	rdf:type        gs1:PreparationTypeCode ;
	rdfs:comment    "Cooking food with high heat with the heat applied directly to the food, most commonly from above. Heat transfer to the food is primarily via radiant heat"@en ;
	rdfs:label      "Broil"@en ;
	skos:prefLabel  "BROIL" .

gs1:PreparationTypeCode-DEEP_FRY
	rdf:type        gs1:PreparationTypeCode ;
	rdfs:comment    "Cooking method whereby food is submerged in hot oil or fat."@en ;
	rdfs:label      "Deep Fry"@en ;
	skos:prefLabel  "DEEP_FRY" .

gs1:PreparationTypeCode-DOUBLE_STEAM
	rdf:type        gs1:PreparationTypeCode ;
	rdfs:comment    "Cooking technique to prepare delicate food such as bird nests, shark fins etc. The food is covered with water and put in a covered ceramic jar"@en ;
	rdfs:label      "Double Steam"@en ;
	skos:prefLabel  "DOUBLE_STEAM" .

gs1:PreparationTypeCode-FREEZE
	rdf:type        gs1:PreparationTypeCode ;
	rdfs:comment    "Convert the product from room temperature to a frozen state.Simple"@en ;
	rdfs:label      "Freeze"@en ;
	skos:prefLabel  "FREEZE" .

gs1:PreparationTypeCode-FRY
	rdf:type        gs1:PreparationTypeCode ;
	rdfs:comment    "Cooking of food in fat."@en ;
	rdfs:label      "Fry"@en ;
	skos:prefLabel  "FRY" .

gs1:PreparationTypeCode-GRIDDLE_FRY
	rdf:type        gs1:PreparationTypeCode ;
	rdfs:comment    "Form of cooking where the food is fried with its own fat."@en ;
	rdfs:label      "Griddle Fry"@en ;
	skos:prefLabel  "GRIDDLE_FRY" .

gs1:PreparationTypeCode-GRILL
	rdf:type        gs1:PreparationTypeCode ;
	rdfs:comment    "Form of cooking that involves direct heat. The definition varies widely by region and culture"@en ;
	rdfs:label      "Grill"@en ;
	skos:prefLabel  "GRILL" .

gs1:PreparationTypeCode-HEAT_AND_SERVE
	rdf:type        gs1:PreparationTypeCode ;
	rdfs:comment    "Prepare the item by simply heating or warming to a desired temperature or visual state prior to serving"@en ;
	rdfs:label      "Heat and Serve"@en ;
	skos:prefLabel  "HEAT_AND_SERVE" .

gs1:PreparationTypeCode-MICROWAVE
	rdf:type        gs1:PreparationTypeCode ;
	rdfs:comment    "Cooking food by employing microwave radiation"@en ;
	rdfs:label      "Microwave"@en ;
	skos:prefLabel  "MICROWAVE" .

gs1:PreparationTypeCode-PAN_FRY
	rdf:type        gs1:PreparationTypeCode ;
	rdfs:comment    "Form of frying characterised by the use of less cooking oil than deep frying"@en ;
	rdfs:label      "Pan Fry"@en ;
	skos:prefLabel  "PAN_FRY" .

gs1:PreparationTypeCode-POACH
	rdf:type        gs1:PreparationTypeCode ;
	rdfs:comment    "Cooking food by gently simmering food in liquid, generally water, stock or wine"@en ;
	rdfs:label      "Poach"@en ;
	skos:prefLabel  "POACH" .

gs1:PreparationTypeCode-PREPARED
	rdf:type        gs1:PreparationTypeCode ;
	rdfs:comment    "The state of the product after preparation (e.g. after adding milk or water)."@en ;
	rdfs:label      "Prepared"@en ;
	skos:prefLabel  "PREPARED" .

gs1:PreparationTypeCode-PRESSURE_COOK
	rdf:type        gs1:PreparationTypeCode ;
	rdfs:comment    "Method of cooking in a sealed vessel that does not permit air or liquids to escape below a preset pressure"@en ;
	rdfs:label      "Pressure Cook"@en ;
	skos:prefLabel  "PRESSURE_COOK" .

gs1:PreparationTypeCode-PRESSURE_FRY
	rdf:type        gs1:PreparationTypeCode ;
	rdfs:comment    "Meat and cooking oil are brought to high temperatures while pressure is held high enough that the water within is prevented from boiling off"@en ;
	rdfs:label      "Pressure Fry"@en ;
	skos:prefLabel  "PRESSURE_FRY" .

gs1:PreparationTypeCode-READY_TO_DRINK
	rdf:type        gs1:PreparationTypeCode ;
	rdfs:comment    "No Preparation. The product is ready for use after being taken out of the packaging (if packaging exists) without the need of any further action prior to consumption or use"@en ;
	rdfs:label      "Ready To Drink"@en ;
	skos:prefLabel  "READY_TO_DRINK" .

gs1:PreparationTypeCode-READY_TO_EAT
	rdf:type        gs1:PreparationTypeCode ;
	rdfs:comment    "Besides unpacking no additional preparation required."@en ;
	rdfs:label      "Ready To Eat"@en ;
	skos:prefLabel  "READY_TO_EAT" .

gs1:PreparationTypeCode-RECONSTITUTE
	rdf:type        gs1:PreparationTypeCode ;
	rdfs:comment    "Restore a dry or concentrated food to its original strength or consistency by adding water."@en ;
	rdfs:label      "Reconstitute"@en ;
	skos:prefLabel  "RECONSTITUTE" .

gs1:PreparationTypeCode-REFRIGERATE
	rdf:type        gs1:PreparationTypeCode ;
	rdfs:comment    "Convert the product from room temperature to a chilled state."@en ;
	rdfs:label      "Refrigerate"@en ;
	skos:prefLabel  "REFRIGERATE" .

gs1:PreparationTypeCode-ROAST
	rdf:type        gs1:PreparationTypeCode ;
	rdfs:comment    "Cooking method that uses dry heat, whether an open flame, oven, or other heat source."@en ;
	rdfs:label      "Roast."@en ;
	skos:prefLabel  "ROAST" .

gs1:PreparationTypeCode-ROTISSERIE
	rdf:type        gs1:PreparationTypeCode ;
	rdfs:comment    "Style of roasting where meat is skewered on a spit and revolves over a flame"@en ;
	rdfs:label      "Rotisserie"@en ;
	skos:prefLabel  "ROTISSERIE" .

gs1:PreparationTypeCode-SAUTE
	rdf:type        gs1:PreparationTypeCode ;
	rdfs:comment    "Cooking food using a small amount of fat in a shallow pan over relatively high heat"@en ;
	rdfs:label      "Saute"@en ;
	skos:prefLabel  "SAUTE" .

gs1:PreparationTypeCode-SEAR
	rdf:type        gs1:PreparationTypeCode ;
	rdfs:comment    "Technique used in grilling, roasting, braising, sauteing, etc. That cooks the surface of the food (usually meat, poultry or fish) at high temperature so that a caramelised crust forms"@en ;
	rdfs:label      "Sear"@en ;
	skos:prefLabel  "SEAR" .

gs1:PreparationTypeCode-SIMMER
	rdf:type        gs1:PreparationTypeCode ;
	rdfs:comment    "Cook food by heating it in water kept just below the boiling point (same as coddling)"@en ;
	rdfs:label      "Simmer"@en ;
	skos:prefLabel  "SIMMER" .

gs1:PreparationTypeCode-SMOKE
	rdf:type        gs1:PreparationTypeCode ;
	rdfs:comment    "Process of curing, cooking, or seasoning food by exposing it for long periods of time to the smoke from a wood fire"@en ;
	rdfs:label      "Smoke"@en ;
	skos:prefLabel  "SMOKE" .

gs1:PreparationTypeCode-STEAM
	rdf:type        gs1:PreparationTypeCode ;
	rdfs:comment    "Cooking by first boiling the water so it will evaporate into steam, then the steam will carry heat to the food, thus achieving heating the food"@en ;
	rdfs:label      "Steam"@en ;
	skos:prefLabel  "STEAM" .

gs1:PreparationTypeCode-STEW
	rdf:type        gs1:PreparationTypeCode ;
	rdfs:comment    "Preparing meat cut into smaller pieces or cubes by simmering it in liquid, usually together with vegetables"@en ;
	rdfs:label      "Stew"@en ;
	skos:prefLabel  "STEW" .

gs1:PreparationTypeCode-STIR_FRY
	rdf:type        gs1:PreparationTypeCode ;
	rdfs:comment    "Chinese cooking technique used because of its fast cooking speed"@en ;
	rdfs:label      "Stir Fry"@en ;
	skos:prefLabel  "STIR_FRY" .

gs1:PreparationTypeCode-THAW
	rdf:type        gs1:PreparationTypeCode ;
	rdfs:comment    "Convert the product from a frozen state to a chilled or room temperature state."@en ;
	rdfs:label      "Thaw"@en ;
	skos:prefLabel  "THAW" .

gs1:PreparationTypeCode-UNPREPARED
	rdf:type        gs1:PreparationTypeCode ;
	rdfs:comment    "The initial state of the product."@en ;
	rdfs:label      "Unprepared"@en ;
	skos:prefLabel  "UNPREPARED" .

gs1:PreparationTypeCode-UNSPECIFIED
	rdf:type        gs1:PreparationTypeCode ;
	rdfs:comment    "Unknown, not applicable"@en ;
	rdfs:label      "Unknown"@en ;
	skos:prefLabel  "UNSPECIFIED" .

gs1:PreservationTechniqueCode-ACIDIFICATION
	rdf:type        gs1:PreservationTechniqueCode ;
	rdfs:comment    "Dropping pH of food"@en ;
	rdfs:label      "Acidification"@en ;
	skos:prefLabel  "ACIDIFICATION" .

gs1:PreservationTechniqueCode-ALCOHOL_CURING
	rdf:type        gs1:PreservationTechniqueCode ;
	rdfs:comment    "Treatment of food by adding alcohol in order to preserve the product"@en ;
	rdfs:label      "Alcohol Curing"@en ;
	skos:prefLabel  "ALCOHOL_CURING" .

gs1:PreservationTechniqueCode-ATTESTED_MILK
	rdf:type        gs1:PreservationTechniqueCode ;
	rdfs:comment    "Raw Milk (without heat treatment)"@en ;
	rdfs:label      "Attested Milk"@en ;
	skos:prefLabel  "ATTESTED_MILK" .

gs1:PreservationTechniqueCode-BOILING
	rdf:type        gs1:PreservationTechniqueCode ;
	rdfs:comment    "Cooking"@en ;
	rdfs:label      "Cooking"@en ;
	skos:prefLabel  "BOILING" .

gs1:PreservationTechniqueCode-BRINING
	rdf:type        gs1:PreservationTechniqueCode ;
	rdfs:comment    "Water saturating or strongly impregnating with salt"@en ;
	rdfs:label      "Brining"@en ;
	skos:prefLabel  "BRINING" .

gs1:PreservationTechniqueCode-CANNING
	rdf:type        gs1:PreservationTechniqueCode ;
	rdfs:comment    "Preserved in a sealed airtight container, usually made of tin-coated iron"@en ;
	rdfs:label      "Canning"@en ;
	skos:prefLabel  "CANNING" .

gs1:PreservationTechniqueCode-COLD_SMOKE_CURING
	rdf:type        gs1:PreservationTechniqueCode ;
	rdfs:comment    "To smoke the food at between 70 degrees to 90 degrees F."@en ;
	rdfs:label      "Cold Smoke Curing"@en ;
	skos:prefLabel  "COLD_SMOKE_CURING" .

gs1:PreservationTechniqueCode-CONSERVE
	rdf:type        gs1:PreservationTechniqueCode ;
	rdfs:comment    "Keep from harm or damage"@en ;
	rdfs:label      "Conserve"@en ;
	skos:prefLabel  "CONSERVE" .

gs1:PreservationTechniqueCode-DEHYDRATION
	rdf:type        gs1:PreservationTechniqueCode ;
	rdfs:comment    "To remove water from food"@en ;
	rdfs:label      "Dehydration"@en ;
	skos:prefLabel  "DEHYDRATION" .

gs1:PreservationTechniqueCode-DRYING
	rdf:type        gs1:PreservationTechniqueCode ;
	rdfs:comment    "Making with moisture having evaporated, drained away"@en ;
	rdfs:label      "Drying"@en ;
	skos:prefLabel  "DRYING" .

gs1:PreservationTechniqueCode-FERMENTATION
	rdf:type        gs1:PreservationTechniqueCode ;
	rdfs:comment    "Any of a group of chemical reactions induced by living or nonliving ferments that split complex organic compounds into relatively simple substance"@en ;
	rdfs:label      "Fermentation"@en ;
	skos:prefLabel  "FERMENTATION" .

gs1:PreservationTechniqueCode-FREEZE_DRYING
	rdf:type        gs1:PreservationTechniqueCode ;
	rdfs:comment    "Preserving food by freezing and then drying in a vacuum"@en ;
	rdfs:label      "Freeze Drying"@en ;
	skos:prefLabel  "FREEZE_DRYING" .

gs1:PreservationTechniqueCode-FREEZING
	rdf:type        gs1:PreservationTechniqueCode ;
	rdfs:comment    "Turning into ice or another solid by cold"@en ;
	rdfs:label      "Freezing"@en ;
	skos:prefLabel  "FREEZING" .

gs1:PreservationTechniqueCode-HIGH_TEMPERATURE_TREATED_MILK
	rdf:type        gs1:PreservationTechniqueCode ;
	rdfs:comment    "Legally also pasteurisation, MHD for longer (about 2 to 3 weeks), ESL-milk"@en ;
	rdfs:label      "High Temperature Treated Milk"@en ;
	skos:prefLabel  "HIGH_TEMPERATURE_TREATED_MILK" .

gs1:PreservationTechniqueCode-HOT_SMOKE_CURING
	rdf:type        gs1:PreservationTechniqueCode ;
	rdfs:comment    "Hot-smoking partially or totally cooks the food by treating it at temperatures ranging from 100 degrees to 190 degrees F."@en ;
	rdfs:label      "Hot Smoke Curing"@en ;
	skos:prefLabel  "HOT_SMOKE_CURING" .

gs1:PreservationTechniqueCode-IONISATION
	rdf:type        gs1:PreservationTechniqueCode ;
	rdfs:comment    "To convert into an ion or ions"@en ;
	rdfs:label      "Ionisation"@en ;
	skos:prefLabel  "IONISATION" .

gs1:PreservationTechniqueCode-IRRADIATION
	rdf:type        gs1:PreservationTechniqueCode ;
	rdfs:comment    "Food irradiation is the process of exposing food to ionising radiation in order to disinfest, sterilise, or preserve food."@en ;
	rdfs:label      "Irradiation"@en ;
	skos:prefLabel  "IRRADIATION" .

gs1:PreservationTechniqueCode-PASTEURISATION
	rdf:type        gs1:PreservationTechniqueCode ;
	rdfs:comment    "Partially sterilisation by heating"@en ;
	rdfs:label      "Pasteurisation"@en ;
	skos:prefLabel  "PASTEURISATION" .

gs1:PreservationTechniqueCode-QUICK_FREEZING
	rdf:type        gs1:PreservationTechniqueCode ;
	rdfs:comment    "Freezing (food) rapidly so as to preserve its qualities"@en ;
	rdfs:label      "Quick Freezing"@en ;
	skos:prefLabel  "QUICK_FREEZING" .

gs1:PreservationTechniqueCode-SALT_CURING
	rdf:type        gs1:PreservationTechniqueCode ;
	rdfs:comment    "Preserving by using a salt brine"@en ;
	rdfs:label      "Salt Curing"@en ;
	skos:prefLabel  "SALT_CURING" .

gs1:PreservationTechniqueCode-SOUS_VIDE
	rdf:type        gs1:PreservationTechniqueCode ;
	rdfs:comment    "Low temperature long time cooking under vacuum"@en ;
	rdfs:label      "Sous Vide"@en ;
	skos:prefLabel  "SOUS_VIDE" .

gs1:PreservationTechniqueCode-STERILISATION
	rdf:type        gs1:PreservationTechniqueCode ;
	rdfs:comment    "A process that effectively kills or eliminates transmissibleagents (such as fungi, bacteria, viruses, spore forms, etc.)."@en ;
	rdfs:label      "Sterilisation"@en ;
	skos:prefLabel  "STERILISATION" .

gs1:PreservationTechniqueCode-SUGAR_CURING
	rdf:type        gs1:PreservationTechniqueCode ;
	rdfs:comment    "Treatment of food by adding sugar in order to preserve the product"@en ;
	rdfs:label      "Sugar Curing"@en ;
	skos:prefLabel  "SUGAR_CURING" .

gs1:PreservationTechniqueCode-ULTRA_HIGH_TEMPERATURE
	rdf:type        gs1:PreservationTechniqueCode ;
	rdfs:comment    "Ultra heat treated (especially for milk)"@en ;
	rdfs:label      "Ultra High Temperature"@en ;
	skos:prefLabel  "ULTRA_HIGH_TEMPERATURE" .

gs1:PreservationTechniqueCode-UNDER_MODIFIED_ATMOSPHERE
	rdf:type        gs1:PreservationTechniqueCode ;
	rdfs:comment    "Packed with a gas with protective proprieties"@en ;
	rdfs:label      "Under Modified Atmosphere"@en ;
	skos:prefLabel  "UNDER_MODIFIED_ATMOSPHERE" .

gs1:PreservationTechniqueCode-VACUUM_PACKED
	rdf:type        gs1:PreservationTechniqueCode ;
	rdfs:comment    "Sealed after the partial removal of air"@en ;
	rdfs:label      "Vacuum Packed"@en ;
	skos:prefLabel  "VACUUM_PACKED" .

gs1:Pressure
	rdf:type  gs1:MeasurementType ;
	rdfs:comment    "The perpendicular force per unit area acting on a material and tending to change its dimensions.  SI Units: pascal, newton per square metre"@en ;
	rdfs:label      "Pressure"@en ;
	skos:prefLabel  "Pressure" .

gs1:ProductYieldTypeCode-AFTER_COOKING
	rdf:type        gs1:ProductYieldTypeCode ;
	rdfs:comment    "Weight or volume of food product after it has been prepared."@en ;
	rdfs:label      "After Cooking"@en ;
	skos:prefLabel  "AFTER_COOKING" .

gs1:ProductYieldTypeCode-AFTER_DILUTION
	rdf:type        gs1:ProductYieldTypeCode ;
	rdfs:comment    "Volume of food product after a fluid has been added."@en ;
	rdfs:label      "After Dilution"@en ;
	skos:prefLabel  "AFTER_DILUTION" .

gs1:ProductYieldTypeCode-DRAINED_WEIGHT
	rdf:type        gs1:ProductYieldTypeCode ;
	rdfs:comment    "Weight of food product after the fluid in which the food product was preserved has been removed."@en ;
	rdfs:label      "Drained Weight"@en ;
	skos:prefLabel  "DRAINED_WEIGHT" .

gs1:ProductYieldTypeCode-UNSPECIFIED
	rdf:type        gs1:ProductYieldTypeCode ;
	rdfs:comment    "Product yield type is unknown or irrelevant"@en ;
	rdfs:label      "Unspecified"@en ;
	skos:prefLabel  "UNSPECIFIED" .

gs1:RadiantFlux
	rdf:type  gs1:MeasurementType ;
	rdfs:comment    "The total power emitted, received or passing in the form of electromagnetic radiation; a measure of electromagnetic energy per unit time.  SI Units: watt"@en ;
	rdfs:label      "Radiant flux"@en ;
	skos:prefLabel  "RadiantFlux" .

gs1:RadiantIntensity
	rdf:type  gs1:MeasurementType ;
	rdfs:comment    "The radiant flux per unit solid angle emitted by a point source.  SI Units: watt / steradian"@en ;
	rdfs:label      "Radiant intensity"@en ;
	skos:prefLabel  "RadiantIntensity" .

gs1:Radioactivity
	rdf:type  gs1:MeasurementType ;
	rdfs:comment    "The rate of spontaneous disintegration or decay of certain natural heavy elements, accompanied by alpha-rays, beta-rays or gamma-rays.  SI Units: becquerel"@en ;
	rdfs:label      "Radioactivity"@en ;
	skos:altLabel   "Activity" ;
	skos:prefLabel  "Radioactivity" .

gs1:ReferencedFileTypeCode-360_DEGREE_IMAGE
	rdf:type        gs1:ReferencedFileTypeCode ;
	rdfs:comment    "Allows x-axis interactive rotation of product via website."@en ;
	rdfs:label      "360 Degree Image"@en ;
	skos:prefLabel  "360_DEGREE_IMAGE" .

gs1:ReferencedFileTypeCode-AMBIENCE_MOOD_IMAGE
	rdf:type        gs1:ReferencedFileTypeCode ;
	rdfs:comment    "Trade Item image representing the image the manufacturer is supplying to the consumer to invoke a connection to the item by setting a 'mood' or feeling for the item and its use."@en ;
	rdfs:label      "Ambience/mood image"@en ;
	skos:prefLabel  "AMBIENCE_MOOD_IMAGE" .

gs1:ReferencedFileTypeCode-APPLICATION_IMAGE
	rdf:type        gs1:ReferencedFileTypeCode ;
	rdfs:comment    "Trade Item image representing the image the manufacturer is supplying to the consumer to depict how the product itself is used."@en ;
	rdfs:label      "Application image"@en ;
	skos:prefLabel  "APPLICATION_IMAGE" .

gs1:ReferencedFileTypeCode-ASSEMBLY_INSTRUCTIONS
	rdf:type        gs1:ReferencedFileTypeCode ;
	rdfs:comment    "Link to a file the explains how to assemble (put together) the trade item."@en ;
	rdfs:label      "Assembly Instructions"@en ;
	skos:prefLabel  "ASSEMBLY_INSTRUCTIONS" .

gs1:ReferencedFileTypeCode-AUDIO
	rdf:type        gs1:ReferencedFileTypeCode ;
	rdfs:comment    "Link to a file containing an audio clip which is relevant to the product. Examples are commercials, or instructional/ how to use audio files."@en ;
	rdfs:label      "Audio"@en ;
	skos:prefLabel  "AUDIO" .

gs1:ReferencedFileTypeCode-AWARD_CERTIFICATE
	rdf:type        gs1:ReferencedFileTypeCode ;
	rdfs:comment    "The award certificate is a written document created by the Award Committee that describes the terms and conditions of the Award. Example: http://www.cronierwines.com/awards-in-2016/"@en ;
	rdfs:label      "Award certificate"@en ;
	skos:prefLabel  "AWARD_CERTIFICATE" .

gs1:ReferencedFileTypeCode-BARCODE
	rdf:type        gs1:ReferencedFileTypeCode ;
	rdfs:comment    "Link to a file containing a visual representation of the barcode which is on the product or its packaging."@en ;
	rdfs:label      "Barcode"@en ;
	skos:prefLabel  "BARCODE" .

gs1:ReferencedFileTypeCode-CERTIFICATION
	rdf:type        gs1:ReferencedFileTypeCode ;
	rdfs:comment    "Document which contains a special certification by a third party (e.g. International Food Standard [IFS], QS-Approval Mark for meat product, sausage, fruit, vegetables and potatoes or bio audits)."@en ;
	rdfs:label      "Certification"@en ;
	skos:prefLabel  "CERTIFICATION" .

gs1:ReferencedFileTypeCode-CHEMICAL_ASSESSMENT_SUMMARY
	rdf:type        gs1:ReferencedFileTypeCode ;
	rdfs:comment    "Link to a file containing the chemical ingredient information sent to the supplier from a third party as a result of the assessment."@en ;
	rdfs:label      "Chemical Assessment Summary"@en ;
	skos:prefLabel  "CHEMICAL_ASSESSMENT_SUMMARY" .

gs1:ReferencedFileTypeCode-CHEMICAL_SAFETY_REPORT
	rdf:type        gs1:ReferencedFileTypeCode ;
	rdfs:comment    "Link to the file containing a report detailing the risks arising from the manufacture and/or use of a substance and to ensure that they are adequately controlled."@en ;
	rdfs:label      "Chemical Safety Report"@en ;
	skos:prefLabel  "CHEMICAL_SAFETY_REPORT" .

gs1:ReferencedFileTypeCode-CHILD_NUTRITION_LABEL
	rdf:type        gs1:ReferencedFileTypeCode ;
	rdfs:comment    "Link to a file containing the Child Nutrition Label as formatted according to regulations and rules of an appropriate regulatory body for the target market."@en ;
	rdfs:label      "Child Nutrition Label"@en ;
	skos:prefLabel  "CHILD_NUTRITION_LABEL" .

gs1:ReferencedFileTypeCode-CLEANING_DISINFECTION_STERILISATION_INSTRUCTIONS
	rdf:type        gs1:ReferencedFileTypeCode ;
	rdfs:comment    "The cleaning, disinfection and/or sterilisation instructions that apply to the product. These may be in accordance with EN-ISO 17664."@en ;
	rdfs:label      "Cleaning, disinfection and sterilisation instructions"@en ;
	skos:prefLabel  "CLEANING_DISINFECTION_STERILISATION_INSTRUCTIONS" .

gs1:ReferencedFileTypeCode-CLINICIAN_MEDICINE_INFORMATION
	rdf:type        gs1:ReferencedFileTypeCode ;
	rdfs:comment    "A clinician focused product information document that is written by the pharmaceutical company responsible for the medicine. This document is intended to assist doctors, pharmacists and other health professionals in prescribing and dispensing medicines. In addition, this information can be used by health professionals in their consultations with patients, so that the patient can be better informed about their medicines. "@en ;
	rdfs:label      "Clinician medicine information"@en ;
	skos:prefLabel  "CLINICIAN_MEDICINE_INFORMATION" .

gs1:ReferencedFileTypeCode-CONSUMER_HANDLING_AND_STORAGE
	rdf:type        gs1:ReferencedFileTypeCode ;
	rdfs:comment    "Link to a website, file, or image containing the manufacturer's recommendations for how the consumer or end user should store and handle the product."@en ;
	rdfs:label      "Consumer Handling and Storage"@en ;
	skos:prefLabel  "CONSUMER_HANDLING_AND_STORAGE" .

gs1:ReferencedFileTypeCode-CONTENT_TEXTURE_IMAGE
	rdf:type        gs1:ReferencedFileTypeCode ;
	rdfs:comment    "Trade Item image representing the image the manufacturer is supplying to the consumer to depict the content or texture of an item. The image should be designed in such a way that the texture can be experienced by the consumer similar to stationary retail, e.g. creme, lipstick."@en ;
	rdfs:label      "Content/texture image"@en ;
	skos:prefLabel  "CONTENT_TEXTURE_IMAGE" .

gs1:ReferencedFileTypeCode-CROSSSECTION_VIEW
	rdf:type        gs1:ReferencedFileTypeCode ;
	rdfs:comment    " A picture of a trade item with a cut away vertical plane removed (e.g. Cross-section of a Tire revealing steel belts and tire tread detail)."@en ;
	rdfs:label      "Crosssection View"@en ;
	skos:prefLabel  "CROSSSECTION_VIEW" .

gs1:ReferencedFileTypeCode-DECLARATION_OF_CONFORMITY
	rdf:type        gs1:ReferencedFileTypeCode ;
	rdfs:comment    "A Declaration of Conformity is a document in which the manufacturer states that the product satisfies the essential requirements of the applicable legislation(s), e.g. for toys, medical devices or electrical equipment. By drawing up and signing the EU Declaration of Conformity, the manufacturer assumes responsibility for the compliance of the product. For more information please see https://eur-lex.europa.eu/legal-content/EN/TXT/PDF/?uri=CELEX:32019R1020&from=DE"@en ;
	rdfs:label      "Declaration of Conformity"@en ;
	skos:prefLabel  "DECLARATION_OF_CONFORMITY" .

gs1:ReferencedFileTypeCode-DIET_CERTIFICATE
	rdf:type        gs1:ReferencedFileTypeCode ;
	rdfs:comment    "Link to a website or file containing a diet certificate granted to the product"@en ;
	rdfs:label      "Diet Certificate"@en ;
	skos:prefLabel  "DIET_CERTIFICATE" .

gs1:ReferencedFileTypeCode-DISPOSAL_INSTRUCTIONS
	rdf:type        gs1:ReferencedFileTypeCode ;
	rdfs:comment    "Link to a website, file or instruction movie how to dispose a product properly or how to clean up a broken product in case the product contains materials like mercury."@en ;
	rdfs:label      "Instructions for disposal"@en ;
	skos:prefLabel  "DISPOSAL_INSTRUCTIONS" .

gs1:ReferencedFileTypeCode-DOCUMENT
	rdf:type        gs1:ReferencedFileTypeCode ;
	rdfs:comment    "Link to a document or text file containing product information. Examples of this type could be an instruction manual, assembly guide, or warranty document."@en ;
	rdfs:label      "Document"@en ;
	skos:prefLabel  "DOCUMENT" .

gs1:ReferencedFileTypeCode-DOP_SHEET
	rdf:type        gs1:ReferencedFileTypeCode ;
	rdfs:comment    "Link to a file containing the product's Declaration of Performance Sheet (DOP). This file can be either an image or a document."@en ;
	rdfs:label      "Dop Sheet"@en ;
	skos:prefLabel  "DOP_SHEET" .

gs1:ReferencedFileTypeCode-DRUG_FACT_LABEL
	rdf:type        gs1:ReferencedFileTypeCode ;
	rdfs:comment    "The file link is to a drug fact panel of the trade item. A drug fact label usually contains such items as active ingredients, uses, warnings, purpose, directions, etc."@en ;
	rdfs:label      "Drug Fact Label"@en ;
	skos:prefLabel  "DRUG_FACT_LABEL" .

gs1:ReferencedFileTypeCode-ECOLOGICAL_FACT_SHEET
	rdf:type        gs1:ReferencedFileTypeCode ;
	rdfs:comment    "Link to a file containing the details of a product with its environmental impact and performance. E.g. Beelong.ch Eco-Score Fact Sheet."@en ;
	rdfs:label      "Ecological fact sheet"@en ;
	skos:prefLabel  "ECOLOGICAL_FACT_SHEET" .

gs1:ReferencedFileTypeCode-ENERGY_LABEL
	rdf:type        gs1:ReferencedFileTypeCode ;
	rdfs:comment    "Link to the energy label for a trade item.  On 19 May 2010, the EU adopted the Directive 2010/30/EU on energy labels. Energy labels help consumers choosing products which save energy and thus money. They also provide incentives for the industry to develop and invest in energy efficient product design. They are found on a selection of white goods and other products and are designed to help customers see how energy efficient a model is before they buy."@en ;
	rdfs:label      "Energy Label"@en ;
	skos:prefLabel  "ENERGY_LABEL" .

gs1:ReferencedFileTypeCode-FOOD_CONTACT_CONFORMITY_CERTIFICATE
	rdf:type        gs1:ReferencedFileTypeCode ;
	rdfs:comment    "The certificate of conformity for suitability for food contact is a document issued by the manufacturer or the person placing the product on the European market. It certifies that the product sold complies with the EC Regulation 1935/2004. Thus, it is proven to be safe to get in contact with food."@en ;
	rdfs:label      "Food contact conformity certificate"@en ;
	skos:prefLabel  "FOOD_CONTACT_CONFORMITY_CERTIFICATE" .

gs1:ReferencedFileTypeCode-GROUP_CHARACTERISTIC_SHEET
	rdf:type        gs1:ReferencedFileTypeCode ;
	rdfs:label      "Group Characteristic Sheet"@en ;
	skos:prefLabel  "GROUP_CHARACTERISTIC_SHEET" .

gs1:ReferencedFileTypeCode-HAZARDOUS_SUBSTANCES_DATA
	rdf:type        gs1:ReferencedFileTypeCode ;
	rdfs:comment    "Link to a file where to locate the 'out of network data' additional data concerning the control of substances can be found."@en ;
	rdfs:label      "Hazardous Substances Data"@en ;
	skos:prefLabel  "HAZARDOUS_SUBSTANCES_DATA" .

gs1:ReferencedFileTypeCode-IFU
	rdf:type        gs1:ReferencedFileTypeCode ;
	rdfs:comment    "Link to a file containing the (electronic) Instructions For Use (IFU or eIFU)."@en ;
	rdfs:label      "IFU/eIFU (Instructions for use)"@en ;
	skos:prefLabel  "IFU" .

gs1:ReferencedFileTypeCode-IFU_INCLUDING_CLEANING_DISINFECTION_STERILISATION_INSTRUCTIONS
	rdf:type        gs1:ReferencedFileTypeCode ;
	rdfs:comment    "Indicates that the instructions for cleaning/disinfecting/sterilisation are included in the IFU (Instructions For Use). "@en ;
	rdfs:label      "Instructions for use including cleaning disinfection sterilisation instructions"@en ;
	skos:prefLabel  "IFU_INCLUDING_CLEANING_DISINFECTION_STERILISATION_INSTRUCTIONS" .

gs1:ReferencedFileTypeCode-INGREDIENTS_LABEL
	rdf:type        gs1:ReferencedFileTypeCode ;
	rdfs:comment    "The Ingredients label image is a list of ingredients printed on the packaging. It may be separated by language in multiple areas on the product."@en ;
	rdfs:label      "Ingredients label"@en ;
	skos:prefLabel  "INGREDIENTS_LABEL" .

gs1:ReferencedFileTypeCode-INTERNAL_VIEW
	rdf:type        gs1:ReferencedFileTypeCode ;
	rdfs:comment    "The picture of the inside of a trade item mainly used for non food products (e.g., The inside of a refrigerator or the inside of a suitcase. "@en ;
	rdfs:label      "Internal View"@en ;
	skos:prefLabel  "INTERNAL_VIEW" .

gs1:ReferencedFileTypeCode-LIGHTING_FACT_LABEL
	rdf:type        gs1:ReferencedFileTypeCode ;
	rdfs:comment    "Link to a file containing a visual representation of the product label containing information related to the light characteristics of the product. The lighting facts label makes it easy to compare bulb characteristics such as brightness, colour, life, and estimated operating cost for the year."@en ;
	rdfs:label      "Lighting fact label"@en ;
	skos:prefLabel  "LIGHTING_FACT_LABEL" .

gs1:ReferencedFileTypeCode-LOGO
	rdf:type        gs1:ReferencedFileTypeCode ;
	rdfs:comment    "Link to a file containing the Manufacturer or Brand Logo(s) associated with the product."@en ;
	rdfs:label      "Logo"@en ;
	skos:prefLabel  "LOGO" .

gs1:ReferencedFileTypeCode-MARKETING_INFORMATION
	rdf:type        gs1:ReferencedFileTypeCode ;
	rdfs:comment    "Link to a file with product information associated with selling a product or service."@en ;
	rdfs:label      "Marketing Information"@en ;
	skos:prefLabel  "MARKETING_INFORMATION" .

gs1:ReferencedFileTypeCode-MATERIAL_SAMPLES
	rdf:type        gs1:ReferencedFileTypeCode ;
	rdfs:comment    "URL to website, images that the potential material, swatches, finishes the trade item might be available in."@en ;
	rdfs:label      "Material Samples"@en ;
	skos:prefLabel  "MATERIAL_SAMPLES" .

gs1:ReferencedFileTypeCode-MOBILE_DEVICE_IMAGE
	rdf:type        gs1:ReferencedFileTypeCode ;
	rdfs:comment    "Trade Item image that represents the image the manufacturer supplies to the consumer for mobile device applications. This would be a pack shot or image of the trade item that may be optimised for digital mobile display or added elements to help consumer recoginise the product. This should not be used as the Mobile Ready Hero Image. Some regulations require an actual image of the product and do not allow Mobile Ready Hero Images."@en ;
	rdfs:label      "Mobile Device Image"@en ;
	skos:prefLabel  "MOBILE_DEVICE_IMAGE" .

gs1:ReferencedFileTypeCode-MOBILE_READY_HERO_IMAGE
	rdf:type        gs1:ReferencedFileTypeCode ;
	rdfs:comment    "A Mobile Ready Hero Image (MRHI) is a representation of a real world product that may differ from a standard pack shot, but that maintains the majority of the physical pack's key elements of design, shape and colour, and is therefore recognisable on a digital shelf. In addition the image should contain elements of The 4 Ws: Who is the brand,What it is,Which variety it isandhow much. The Mobile Ready Hero Image (MRHI) is specified in the GS1 Mobile Ready Hero Image Guideline https://www.gs1.org/standards/Mobile-Ready-Hero-Image"@en ;
	rdfs:label      "Mobile Ready Hero Image"@en ;
	skos:prefLabel  "MOBILE_READY_HERO_IMAGE" .

gs1:ReferencedFileTypeCode-MONTAGE_IMAGE
	rdf:type        gs1:ReferencedFileTypeCode ;
	rdfs:comment    "A Montage is the physical over layering of distinct images to create a final digital image. This process allows for a composite to be created with the future possibility of reconstruction without having to return to studio for correction, should an element be added or removed."@en ;
	rdfs:label      "Montage image"@en ;
	skos:prefLabel  "MONTAGE_IMAGE" .

gs1:ReferencedFileTypeCode-NUTRITION_FACT_LABEL
	rdf:type        gs1:ReferencedFileTypeCode ;
	rdfs:comment    "Link to a file containing a visual representation of the product label containing the nutritional information."@en ;
	rdfs:label      "Nutrition Fact Label"@en ;
	skos:prefLabel  "NUTRITION_FACT_LABEL" .

gs1:ReferencedFileTypeCode-NUTRITION_FACT_LABEL_WITH_INGREDIENTS
	rdf:type        gs1:ReferencedFileTypeCode ;
	rdfs:comment    "Link to a file containing a visual representation of the product label containing the nutritional information with the inclusion of the ingredient statement."@en ;
	rdfs:label      "Nutrition Fact Label with Ingredients"@en ;
	skos:prefLabel  "NUTRITION_FACT_LABEL_WITH_INGREDIENTS" .

gs1:ReferencedFileTypeCode-OPTIMISED_HERO_IMAGE
	rdf:type        gs1:ReferencedFileTypeCode ;
	rdfs:comment    "An Optimised Hero Image type is to support retail, consumers, distributors and foodservice operators in completing their online sites. These images will assist consumers to identify specific information about the products they are purchasing. The image is a representation of a real world product, built specifically for use on larger screens that may differ from a standard pack shot, but that maintains the majority of the physical pack's key elements of design, shape and colour, and is therefore recognisable on a digital shelf."@en ;
	rdfs:label      "Optimised hero image"@en ;
	skos:prefLabel  "OPTIMISED_HERO_IMAGE" .

gs1:ReferencedFileTypeCode-ORGANIC_CERTIFICATE
	rdf:type        gs1:ReferencedFileTypeCode ;
	rdfs:comment    "Link to a website or file containing an organic certificate granted to the product."@en ;
	rdfs:label      "Organic Certificate"@en ;
	skos:prefLabel  "ORGANIC_CERTIFICATE" .

gs1:ReferencedFileTypeCode-OTHER_EXTERNAL_INFORMATION
	rdf:type        gs1:ReferencedFileTypeCode ;
	rdfs:comment    "Link to a file containing product information of an unspecified type."@en ;
	rdfs:label      "Other External Information"@en ;
	skos:prefLabel  "OTHER_EXTERNAL_INFORMATION" .

gs1:ReferencedFileTypeCode-OUT_OF_PACKAGE_IMAGE
	rdf:type        gs1:ReferencedFileTypeCode ;
	rdfs:comment    "Link to an image of an item out of its packaging and, if necessary, assembled ready for use by the end user. This type of file is subject the current version of the GDSN Product Image Specification Standard."@en ;
	rdfs:label      "Out of Package Image"@en ;
	skos:prefLabel  "OUT_OF_PACKAGE_IMAGE" .

gs1:ReferencedFileTypeCode-PACKAGING_ARTWORK
	rdf:type        gs1:ReferencedFileTypeCode ;
	rdfs:comment    "Design files for packaging artwork for example Adobe source files."@en ;
	rdfs:label      "Packaging Artwork"@en ;
	skos:prefLabel  "PACKAGING_ARTWORK" .

gs1:ReferencedFileTypeCode-PATIENT_INFORMATION_LEAFLET
	rdf:type        gs1:ReferencedFileTypeCode ;
	rdfs:comment    "A leaflet or brochure containing important information to patients/consumers about the product to facilitate discussion and assist with the decision-making process. Example: A leaflet on a medical device like a hip joint. Or a consumer/patient-focused leaflet that contains information on the safe and effective use of a medicines. Often known in some markets as Consumer Medicines Information sheet (CMI), Product Information Leaflet (PiL/ePIL)."@en ;
	rdfs:label      "Patient information leaflet"@en ;
	skos:prefLabel  "PATIENT_INFORMATION_LEAFLET" .

gs1:ReferencedFileTypeCode-PETFOOD_FEEDING_INSTRUCTIONS
	rdf:type        gs1:ReferencedFileTypeCode ;
	rdfs:comment    "Link to a file containing a visual representation of the product label containing the feeding instructions for the petfood product."@en ;
	rdfs:label      "Petfood Feeding Instructions"@en ;
	skos:prefLabel  "PETFOOD_FEEDING_INSTRUCTIONS" .

gs1:ReferencedFileTypeCode-PLANOGRAM
	rdf:type        gs1:ReferencedFileTypeCode ;
	rdfs:comment    "Link to a file illustrating how and where retail products should be displayed."@en ;
	rdfs:label      "Planogram"@en ;
	skos:prefLabel  "PLANOGRAM" .

gs1:ReferencedFileTypeCode-PREPARATION_INSTRUCTIONS
	rdf:type        gs1:ReferencedFileTypeCode ;
	rdfs:comment    "Link to a file containing a visual representation of the product label containing the preparation instructions."@en ;
	rdfs:label      "Preparation Instructions"@en ;
	skos:prefLabel  "PREPARATION_INSTRUCTIONS" .

gs1:ReferencedFileTypeCode-PRODUCT_FORMULATION_STATEMENT
	rdf:type        gs1:ReferencedFileTypeCode ;
	rdfs:comment    "Link to a file containing the Product Formulation Statement, in lieu of a Child Nutrition Label, as formatted according to regulations and rules of an appropriate regulatory body for the target market."@en ;
	rdfs:label      "Product Formulation Statement"@en ;
	skos:prefLabel  "PRODUCT_FORMULATION_STATEMENT" .

gs1:ReferencedFileTypeCode-PRODUCT_IMAGE
	rdf:type        gs1:ReferencedFileTypeCode ;
	rdfs:comment    "Link to a file containing a visual representation of the product."@en ;
	rdfs:label      "Product Image"@en ;
	skos:prefLabel  "PRODUCT_IMAGE" .

gs1:ReferencedFileTypeCode-PRODUCT_IMAGE_FORMED
	rdf:type        gs1:ReferencedFileTypeCode ;
	rdfs:comment    "An image of a product that has the supporting shape/form (for example a model, mannequin, hanger) removed to give the product a 3-D look."@en ;
	rdfs:label      "Product image formed"@en ;
	skos:prefLabel  "PRODUCT_IMAGE_FORMED" .

gs1:ReferencedFileTypeCode-PRODUCT_LABEL_IMAGE
	rdf:type        gs1:ReferencedFileTypeCode ;
	rdfs:comment    "Link to a file containing a visual representation of the product label."@en ;
	rdfs:label      "Product Label Image"@en ;
	skos:prefLabel  "PRODUCT_LABEL_IMAGE" .

gs1:ReferencedFileTypeCode-PRODUCT_WEBSITE
	rdf:type        gs1:ReferencedFileTypeCode ;
	rdfs:comment    "Link to a website containing product specific information. Examples of this could be a link to a website dedicated to the product or a link to the area within the manufacturer or brand owner website that contains the product information"@en ;
	rdfs:label      "Product Website"@en ;
	skos:prefLabel  "PRODUCT_WEBSITE" .

gs1:ReferencedFileTypeCode-QR_CODE
	rdf:type        gs1:ReferencedFileTypeCode ;
	rdfs:comment    "Link to a QR code URL/URI."@en ;
	rdfs:label      "Link to QR Code"@en ;
	skos:prefLabel  "QR_CODE" .

gs1:ReferencedFileTypeCode-QUALITY_CONTROL_PLAN
	rdf:type        gs1:ReferencedFileTypeCode ;
	rdfs:comment    "Document which detailed information about the quantity of laboratory/analytical tests and the evaluated parameters."@en ;
	rdfs:label      "Quality Control Plan"@en ;
	skos:prefLabel  "QUALITY_CONTROL_PLAN" .

gs1:ReferencedFileTypeCode-RECIPE_WEBSITE
	rdf:type        gs1:ReferencedFileTypeCode ;
	rdfs:comment    "Link to a website containing recipes associated with the product"@en ;
	rdfs:label      "Recipe Website"@en ;
	skos:prefLabel  "RECIPE_WEBSITE" .

gs1:ReferencedFileTypeCode-RECYCLABILITY_ASSESSMENT_CERTIFICATE
	rdf:type        gs1:ReferencedFileTypeCode ;
	rdfs:comment    "Link to a file containing the certificate for recyclability granted to the packaging of the item."@en ;
	rdfs:label      "Recyclability assessment certificate"@en ;
	skos:prefLabel  "RECYCLABILITY_ASSESSMENT_CERTIFICATE" .

gs1:ReferencedFileTypeCode-REGULATORY_INSPECTION_AUDIT
	rdf:type        gs1:ReferencedFileTypeCode ;
	rdfs:comment    "Inspection report of the inspections. For example foodstuffs, pharmaceuticals and other types of products that are regulated."@en ;
	rdfs:label      "Regulatory Inspection Audit"@en ;
	skos:prefLabel  "REGULATORY_INSPECTION_AUDIT" .

gs1:ReferencedFileTypeCode-RISK_ANALYSIS_DOCUMENT
	rdf:type        gs1:ReferencedFileTypeCode ;
	rdfs:comment    "Document which describes how the supplier assured the quality control of the end products or during the production process. The process can be a supplier internal control system, a simple kind of risk analysis or systematic preventive approach according Hazard Analysis and Critical Control Points (HACCP)."@en ;
	rdfs:label      "Risk Analysis Document"@en ;
	skos:prefLabel  "RISK_ANALYSIS_DOCUMENT" .

gs1:ReferencedFileTypeCode-SAFETY_DATA_SHEET
	rdf:type        gs1:ReferencedFileTypeCode ;
	rdfs:comment    "Link to a file containing the product's Safety Data Sheet (SDS). This file can be either an image or a document"@en ;
	rdfs:label      "Safety Data Sheet"@en ;
	skos:prefLabel  "SAFETY_DATA_SHEET" .

gs1:ReferencedFileTypeCode-SAFETY_SUMMARY_SHEET
	rdf:type        gs1:ReferencedFileTypeCode ;
	rdfs:comment    "A link to a summary sheet document that is available to workers to understand how to deal with chemicals in an emergency situation."@en ;
	rdfs:label      "Safety Summary Sheet"@en ;
	skos:prefLabel  "SAFETY_SUMMARY_SHEET" .

gs1:ReferencedFileTypeCode-SAMPLE_SHIPPING_ORDER
	rdf:type        gs1:ReferencedFileTypeCode ;
	rdfs:comment    "Document is a sample shipping order. A sample shipping order isn't needed for every item (GTIN), but a shipping order can differ from GTIN to GTIN. E.g. in case an item is an organic product the sample shipping order needs to contain the organic product origin number according article 31 of the implementing regulations EG Nr. 889/2008. For non-organic items this information isn't needed.    "@en ;
	rdfs:label      "Sample Shipping Order"@en ;
	skos:prefLabel  "SAMPLE_SHIPPING_ORDER" .

gs1:ReferencedFileTypeCode-SIDEKICK_IMAGE
	rdf:type        gs1:ReferencedFileTypeCode ;
	rdfs:comment    "Retail, consumers, distributors and foodservice operators complete their online transactions using their smart devices. These images may be used to inform a customer of benefits or nutritional claims of a product. This is a supplementary image or graphic, generally used to support the Hero image."@en ;
	rdfs:label      "Sidekick image"@en ;
	skos:prefLabel  "SIDEKICK_IMAGE" .

gs1:ReferencedFileTypeCode-SOCIAL_MEDIA_IMAGE
	rdf:type        gs1:ReferencedFileTypeCode ;
	rdfs:comment    "Trade Item image representing the image the manufacturer is supplying to the consumer to depict the social media associated to the item. This image is being shared on the social media outlet."@en ;
	rdfs:label      "Social media image"@en ;
	skos:prefLabel  "SOCIAL_MEDIA_IMAGE" .

gs1:ReferencedFileTypeCode-SUMMARY_OF_PRODUCT_CHARACTERISTICS
	rdf:type        gs1:ReferencedFileTypeCode ;
	rdfs:comment    "Specific document required before any medicinal product or biocidal product is authorized for marketing.  Example European Commission"@en ;
	rdfs:label      "Summary of Product Characteristics"@en ;
	skos:prefLabel  "SUMMARY_OF_PRODUCT_CHARACTERISTICS" .

gs1:ReferencedFileTypeCode-SUPPLEMENT_FACT_LABEL
	rdf:type        gs1:ReferencedFileTypeCode ;
	rdfs:comment    "Link to a file containing a visual representation of the product label containing information related to the supplement or nutrient product. The supplement facts label provides about what active/nutritional ingredients are used in the formula along with dosage recommendations for dietary supplements."@en ;
	rdfs:label      "Supplement facts label"@en ;
	skos:prefLabel  "SUPPLEMENT_FACT_LABEL" .

gs1:ReferencedFileTypeCode-TECHNICAL_DATA_SHEET
	rdf:type        gs1:ReferencedFileTypeCode ;
	rdfs:comment    "The product specification sheet, created by the manufacturer, summarises the technical characteristics and other properties of the product, relating to technological and commercial purposes. Example: https://dl.gedal.fr/docsgedal/FP/3255290252425.pdf"@en ;
	rdfs:label      "Technical data sheet"@en ;
	skos:prefLabel  "TECHNICAL_DATA_SHEET" .

gs1:ReferencedFileTypeCode-TECHNICAL_DRAWING
	rdf:type        gs1:ReferencedFileTypeCode ;
	rdfs:comment    "A precise and detailed technical drawing of an object, as employed in industries such as engineering, construction, architecture etc. https://en.wikipedia.org/wiki/Engineering_drawing https://en.wikipedia.org/wiki/Technical_drawing"@en ;
	rdfs:label      "Technical Drawing"@en ;
	skos:prefLabel  "TECHNICAL_DRAWING" .

gs1:ReferencedFileTypeCode-TESTING_METHODOLOGY_RESULTS
	rdf:type        gs1:ReferencedFileTypeCode ;
	rdfs:comment    "Document which contains microbiological and physico-chemical findings of the product which are observed during product testing."@en ;
	rdfs:label      "Testing Methodology Results"@en ;
	skos:prefLabel  "TESTING_METHODOLOGY_RESULTS" .

gs1:ReferencedFileTypeCode-TRADE_ITEM_DESCRIPTION
	rdf:type        gs1:ReferencedFileTypeCode ;
	rdfs:comment    "Identifies the reference to an external description of a Trade Item. The link (e.g. URL) to the external description. will be in the appropriate attribute"@en ;
	rdfs:label      "Trade Item Description"@en ;
	skos:prefLabel  "TRADE_ITEM_DESCRIPTION" .

gs1:ReferencedFileTypeCode-TRADE_ITEM_IMAGE_WITH_DIMENSIONS
	rdf:type        gs1:ReferencedFileTypeCode ;
	rdfs:comment    "Link to a website, file, or image containing the product's image with its dimensions. This especially important for built-in products as ovens and fridges. Ex : http://www.docstoc.com/docs/125126778/GSS-GEW-Food-Savers-Food-Storage-Containers."@en ;
	rdfs:label      "Trade Item Image With Dimensions"@en ;
	skos:prefLabel  "TRADE_ITEM_IMAGE_WITH_DIMENSIONS" .

gs1:ReferencedFileTypeCode-VIDEO
	rdf:type        gs1:ReferencedFileTypeCode ;
	rdfs:comment    "Link to a file containing a video clip which is relevant to the product. Examples are commercials, trailers, or instructional/ how to use video files."@en ;
	rdfs:label      "Video"@en ;
	skos:prefLabel  "VIDEO" .

gs1:ReferencedFileTypeCode-VISUAL_VERIFICATION_IMAGE
	rdf:type        gs1:ReferencedFileTypeCode ;
	rdfs:comment    "Link to a file containing a visual representation of the product for the purpose of visual verification. Usage may be to examine the trade item master data against the product image. Note these images might not necessarily comply with image standards and may be restricted for a visual verification usage.  "@en ;
	rdfs:label      "Visual verification image"@en ;
	skos:prefLabel  "VISUAL_VERIFICATION_IMAGE" .

gs1:ReferencedFileTypeCode-WARRANTY_INFORMATION
	rdf:type        gs1:ReferencedFileTypeCode ;
	rdfs:comment    "Link to a file with information associated with any guarantee given by a company stating that a product is reliable and free from known defects and that the seller will, without charge, repair or replace defective parts within a given time limit and under certain conditions."@en ;
	rdfs:label      "Warranty Information"@en ;
	skos:prefLabel  "WARRANTY_INFORMATION" .

gs1:ReferencedFileTypeCode-WEBSITE
	rdf:type        gs1:ReferencedFileTypeCode ;
	rdfs:comment    "Link to a website containing product or manufacturer information."@en ;
	rdfs:label      "Website"@en ;
	skos:prefLabel  "WEBSITE" .

gs1:ReferencedFileTypeCode-ZOOM_VIEW
	rdf:type        gs1:ReferencedFileTypeCode ;
	rdfs:comment    "A picture of a portion of a trade item (e.g., the wheels of a suitcase or the ingredients list of a food trade item). "@en ;
	rdfs:label      "Zoom View"@en ;
	skos:prefLabel  "ZOOM_VIEW" .

gs1:RelativeHumidity
	rdf:type  gs1:MeasurementType ;
	rdfs:comment    "The ratio of the partial pressure of water vapour in an an air-water mixture to the saturated vapour pressure of water at a prescribed temperature.  Typically expressed as a percentage."@en ;
	rdfs:label      "Relative humidity"@en ;
	skos:prefLabel  "RelativeHumidity" .

gs1:Resistance
	rdf:type  gs1:MeasurementType ;
	rdfs:comment    "The ratio of the potential difference across an electrical component to the current passing through it. It is a measure of the opposition to the flow of electric charge. The real part of the impedance, characterised by the dissipation of energy as opposed to its storage.  SI Units: ohm"@en ;
	rdfs:label      "Resistance"@en ;
	skos:prefLabel  "Resistance" .

gs1:Resistivity
	rdf:type  gs1:MeasurementType ;
	rdfs:comment    "A measure of how strongly a material resists the flow of electric current. The electric field required to achieve unit current density flowing through the material.  SI Units: ohm metre"@en ;
	rdfs:label      "Resistivity"@en ;
	skos:prefLabel  "Resistivity" .

gs1:SeasonParameterCode-ALL_YEAR
	rdf:type        gs1:SeasonParameterCode ;
	rdfs:comment    "All Year"@en ;
	rdfs:label      "All Year"@en ;
	skos:prefLabel  "ALL_YEAR" .

gs1:SeasonParameterCode-AUTUMN
	rdf:type        gs1:SeasonParameterCode ;
	rdfs:comment    "For products that are seasonal in nature and apply to the Autumn selling season only"@en ;
	rdfs:label      "Autumn"@en ;
	skos:prefLabel  "AUTUMN" .

gs1:SeasonParameterCode-AUTUMN_WINTER
	rdf:type        gs1:SeasonParameterCode ;
	rdfs:comment    "For products that are seasonal in nature and apply to both the Autumn and Winter selling seasons"@en ;
	rdfs:label      "Autumn and Winter"@en ;
	skos:prefLabel  "AUTUMN_WINTER" .

gs1:SeasonParameterCode-SPRING
	rdf:type        gs1:SeasonParameterCode ;
	rdfs:comment    "For products that are seasonal in nature and apply to the Spring selling season only"@en ;
	rdfs:label      "Spring"@en ;
	skos:prefLabel  "SPRING" .

gs1:SeasonParameterCode-SPRING_SUMMER
	rdf:type        gs1:SeasonParameterCode ;
	rdfs:comment    "For products that are seasonal in nature and apply to both the Spring and Summer selling seasons"@en ;
	rdfs:label      "Spring and Summer"@en ;
	skos:prefLabel  "SPRING_SUMMER" .

gs1:SeasonParameterCode-SUMMER
	rdf:type        gs1:SeasonParameterCode ;
	rdfs:comment    "For products that are seasonal in nature and apply to the Summer selling season only"@en ;
	rdfs:label      "Summer"@en ;
	skos:prefLabel  "SUMMER" .

gs1:SeasonParameterCode-WINTER
	rdf:type        gs1:SeasonParameterCode ;
	rdfs:comment    "For products that are seasonal in nature and apply to the Winter selling season only"@en ;
	rdfs:label      "Winter"@en ;
	skos:prefLabel  "WINTER" .

gs1:SecurityMarking-HOLOGRAM
	rdf:type        gs1:SecurityMarking ;
	rdfs:comment    "A holographic image formed using light diffraction and interference of light waves, capable of representing a three-dimensional object or multiple images, depending on the angle of observation."@en ;
	rdfs:label      "hologram"@en ;
	skos:prefLabel  "HOLOGRAM" .

gs1:SecurityMarking-MICROPRINTING
	rdf:type        gs1:SecurityMarking ;
	rdfs:comment    "A hidden pattern that is too small to read easily without means of optical magnification such as a microscope"@en ;
	rdfs:label      "microprinting"@en ;
	skos:prefLabel  "MICROPRINTING" .

gs1:SecurityMarking-UVINK
	rdf:type        gs1:SecurityMarking ;
	rdfs:comment    "A hidden pattern or marking that is invisible when observed under normal visible light but which fluoresces when observed using ultra-violet light"@en ;
	rdfs:label      "ultra-violet fluorescent ink"@en ;
	skos:prefLabel  "UVINK" .

gs1:SecurityMarking-WATERMARK
	rdf:type        gs1:SecurityMarking ;
	rdfs:comment    "A conventional watermark in which a pattern within a translucent sheet becomes visible when observed via transmitted light (typically due to reduced opacity of the pattern), whereas the pattern remains hidden when observed via light reflected off the surface"@en ;
	rdfs:label      "watermark"@en ;
	skos:prefLabel  "WATERMARK" .

gs1:SharpnessOfCheeseCode-EXTRA_EXTRA_SHARP
	rdf:type        gs1:SharpnessOfCheeseCode ;
	rdfs:label      "Extra Extra Sharp"@en ;
	skos:prefLabel  "EXTRA_EXTRA_SHARP" .

gs1:SharpnessOfCheeseCode-EXTRA_SHARP
	rdf:type        gs1:SharpnessOfCheeseCode ;
	rdfs:label      "Extra Sharp"@en ;
	skos:prefLabel  "EXTRA_SHARP" .

gs1:SharpnessOfCheeseCode-MILD
	rdf:type        gs1:SharpnessOfCheeseCode ;
	rdfs:label      "Mild"@en ;
	skos:prefLabel  "MILD" .

gs1:SharpnessOfCheeseCode-REGULAR
	rdf:type        gs1:SharpnessOfCheeseCode ;
	rdfs:label      "Regular"@en ;
	skos:prefLabel  "REGULAR" .

gs1:SharpnessOfCheeseCode-SHARP
	rdf:type        gs1:SharpnessOfCheeseCode ;
	rdfs:label      "Sharp"@en ;
	skos:prefLabel  "SHARP" .

gs1:SharpnessOfCheeseCode-UNCLASSIFIED
	rdf:type        gs1:SharpnessOfCheeseCode ;
	rdfs:label      "Unclassified"@en ;
	skos:prefLabel  "UNCLASSIFIED" .

gs1:SizeGroupCode-BOYS
	rdf:type        gs1:SizeGroupCode ;
	rdfs:label      "Boys"@en ;
	skos:prefLabel  "BOYS" .

gs1:SizeGroupCode-GIRLS
	rdf:type        gs1:SizeGroupCode ;
	rdfs:label      "Girls"@en ;
	skos:prefLabel  "GIRLS" .

gs1:SizeGroupCode-INFANTS
	rdf:type        gs1:SizeGroupCode ;
	rdfs:label      "Infants"@en ;
	skos:prefLabel  "INFANTS" .

gs1:SizeGroupCode-JUNIORS
	rdf:type        gs1:SizeGroupCode ;
	rdfs:label      "Juniors"@en ;
	skos:prefLabel  "JUNIORS" .

gs1:SizeGroupCode-MATERNITY
	rdf:type        gs1:SizeGroupCode ;
	rdfs:label      "Maternity"@en ;
	skos:prefLabel  "MATERNITY" .

gs1:SizeGroupCode-MENS
	rdf:type        gs1:SizeGroupCode ;
	rdfs:label      "Mens"@en ;
	skos:prefLabel  "MENS" .

gs1:SizeGroupCode-MENS_TALL
	rdf:type        gs1:SizeGroupCode ;
	rdfs:label      "Mens Tall"@en ;
	skos:prefLabel  "MENS_TALL" .

gs1:SizeGroupCode-MISSES
	rdf:type        gs1:SizeGroupCode ;
	rdfs:label      "Misses"@en ;
	skos:prefLabel  "MISSES" .

gs1:SizeGroupCode-PETITE
	rdf:type        gs1:SizeGroupCode ;
	rdfs:label      "Petite"@en ;
	skos:prefLabel  "PETITE" .

gs1:SizeGroupCode-WOMENS
	rdf:type        gs1:SizeGroupCode ;
	rdfs:label      "Womens"@en ;
	skos:prefLabel  "WOMENS" .

gs1:SizeGroupCode-WOMENS_TALL
	rdf:type        gs1:SizeGroupCode ;
	rdfs:label      "Womens Tall"@en ;
	skos:prefLabel  "WOMENS_TALL" .

gs1:SizeSystemCode-AUSTRALIA
	rdf:type        gs1:SizeSystemCode ;
	rdfs:label      "Australia"@en ;
	skos:prefLabel  "AUSTRALIA" .

gs1:SizeSystemCode-CONTINENTAL
	rdf:type        gs1:SizeSystemCode ;
	rdfs:label      "Continental"@en ;
	skos:prefLabel  "CONTINENTAL" .

gs1:SizeSystemCode-EUROPE
	rdf:type        gs1:SizeSystemCode ;
	rdfs:label      "Europe"@en ;
	skos:prefLabel  "EUROPE" .

gs1:SizeSystemCode-JAPAN
	rdf:type        gs1:SizeSystemCode ;
	rdfs:label      "Japan"@en ;
	skos:prefLabel  "JAPAN" .

gs1:SizeSystemCode-MEXICO
	rdf:type        gs1:SizeSystemCode ;
	rdfs:label      "Mexico"@en ;
	skos:prefLabel  "MEXICO" .

gs1:SizeSystemCode-UK
	rdf:type        gs1:SizeSystemCode ;
	rdfs:label      "UK"@en ;
	skos:prefLabel  "UK" .

gs1:SizeSystemCode-US
	rdf:type        gs1:SizeSystemCode ;
	rdfs:label      "US"@en ;
	skos:prefLabel  "US" .

gs1:SizeTypeCode-BACK
	rdf:type        gs1:SizeTypeCode ;
	rdfs:label      "Back"@en ;
	skos:prefLabel  "BACK" .

gs1:SizeTypeCode-CHEST_BUST
	rdf:type        gs1:SizeTypeCode ;
	rdfs:comment    "The measurement around the widest part of the chest/bust."@en ;
	rdfs:label      "Chest or Bust"@en ;
	skos:prefLabel  "CHEST_BUST" .

gs1:SizeTypeCode-COLLAR
	rdf:type        gs1:SizeTypeCode ;
	rdfs:label      "Collar"@en ;
	skos:prefLabel  "COLLAR" .

gs1:SizeTypeCode-CUP
	rdf:type  gs1:SizeTypeCode ;
	rdfs:label      "Cup"@en ;
	skos:prefLabel  "CUP" .

gs1:SizeTypeCode-HIPS
	rdf:type        gs1:SizeTypeCode ;
	rdfs:comment    "The measurement around the fullest part of the hips."@en ;
	rdfs:label      "Hips"@en ;
	skos:prefLabel  "HIPS" .

gs1:SizeTypeCode-INSEAM
	rdf:type        gs1:SizeTypeCode ;
	rdfs:label      "Inseam"@en ;
	skos:prefLabel  "INSEAM" .

gs1:SizeTypeCode-LENGTH
	rdf:type        gs1:SizeTypeCode ;
	rdfs:label      "Length"@en ;
	skos:prefLabel  "LENGTH" .

gs1:SizeTypeCode-ONE_DIMENSION
	rdf:type        gs1:SizeTypeCode ;
	rdfs:label      "One Dimension"@en ;
	skos:prefLabel  "ONE_DIMENSION" .

gs1:SizeTypeCode-OUTSIDE_LEG
	rdf:type        gs1:SizeTypeCode ;
	rdfs:comment    "The measurement of the outside leg seam. This is the distance from the waist to the bottom of the trousers."@en ;
	rdfs:label      "Outside Leg"@en ;
	skos:prefLabel  "OUTSIDE_LEG" .

gs1:SizeTypeCode-SLEEVE
	rdf:type        gs1:SizeTypeCode ;
	rdfs:label      "Sleeve"@en ;
	skos:prefLabel  "SLEEVE" .

gs1:SizeTypeCode-WAIST
	rdf:type        gs1:SizeTypeCode ;
	rdfs:label      "Waist"@en ;
	skos:prefLabel  "WAIST" .

gs1:SizeTypeCode-WIDTH
	rdf:type        gs1:SizeTypeCode ;
	rdfs:label      "Width"@en ;
	skos:prefLabel  "WIDTH" .

gs1:SolidAngle
	rdf:type  gs1:MeasurementType ;
	rdfs:comment    "A three-dimensional equivalent to planar angle, indicating a measure of the field of view subtended by an object when viewed from a specified point, the apex.  The solid angle is the surface area subtended at radius r from the apex divided by the square of that radius r.    SI Units: steradian etc."@en ;
	rdfs:label      "Solid angle"@en ;
	skos:prefLabel  "SolidAngle" .

gs1:SourceAnimalCode-ALLIGATOR
	rdf:type        gs1:SourceAnimalCode ;
	rdfs:comment    "A crocodilian in the genus Alligator of the family Alligatoridae."@en ;
	rdfs:label      "Alligator"@en ;
	skos:prefLabel  "ALLIGATOR" .

gs1:SourceAnimalCode-ASS
	rdf:type        gs1:SourceAnimalCode ;
	rdfs:comment    "A domesticated member of the horse family."@en ;
	rdfs:label      "Ass"@en ;
	skos:prefLabel  "ASS" .

gs1:SourceAnimalCode-BEAR
	rdf:type        gs1:SourceAnimalCode ;
	rdfs:comment    "Mammals of the family Ursidae."@en ;
	rdfs:label      "Bear"@en ;
	skos:prefLabel  "BEAR" .

gs1:SourceAnimalCode-BEEF_COW
	rdf:type        gs1:SourceAnimalCode ;
	rdfs:comment    "Cattle raised principally for meat production, other uses include leather and products used in shampoo and cosmetics."@en ;
	rdfs:label      "Beef Cow"@en ;
	skos:prefLabel  "BEEF_COW" .

gs1:SourceAnimalCode-BOAR
	rdf:type        gs1:SourceAnimalCode ;
	rdfs:comment    "A wild relative of the domestic pig."@en ;
	rdfs:label      "Boar"@en ;
	skos:prefLabel  "BOAR" .

gs1:SourceAnimalCode-BUFFALO
	rdf:type        gs1:SourceAnimalCode ;
	rdfs:comment    "A large bovine animal, frequently used as livestock."@en ;
	rdfs:label      "Buffalo"@en ;
	skos:prefLabel  "BUFFALO" .

gs1:SourceAnimalCode-CALF
	rdf:type        gs1:SourceAnimalCode ;
	rdfs:comment    "A general term for a juvenile member of any species of domestic cattle which is intentionally raised to be processed at a young age."@en ;
	rdfs:label      "Calf"@en ;
	skos:prefLabel  "CALF" .

gs1:SourceAnimalCode-CAMEL
	rdf:type        gs1:SourceAnimalCode ;
	rdfs:comment    "Even-toed ungulates within the genus Camelus."@en ;
	rdfs:label      "Camel"@en ;
	skos:prefLabel  "CAMEL" .

gs1:SourceAnimalCode-CHICKEN
	rdf:type        gs1:SourceAnimalCode ;
	rdfs:comment    "A domesticated fowl."@en ;
	rdfs:label      "Chicken"@en ;
	skos:prefLabel  "CHICKEN" .

gs1:SourceAnimalCode-COCKEREL
	rdf:type        gs1:SourceAnimalCode ;
	rdfs:comment    "A male chicken."@en ;
	rdfs:label      "Cockerel"@en ;
	skos:prefLabel  "COCKEREL" .

gs1:SourceAnimalCode-COW
	rdf:type        gs1:SourceAnimalCode ;
	rdfs:comment    "A domesticated member of the subfamily Bovinae."@en ;
	rdfs:label      "Cow"@en ;
	skos:prefLabel  "COW" .

gs1:SourceAnimalCode-CROCODILE
	rdf:type        gs1:SourceAnimalCode ;
	rdfs:comment    "Any species belonging to the family Crocodylidae."@en ;
	rdfs:label      "Crocodile"@en ;
	skos:prefLabel  "CROCODILE" .

gs1:SourceAnimalCode-DEER
	rdf:type        gs1:SourceAnimalCode ;
	rdfs:comment    "Ruminant mammals forming the family Cervidae."@en ;
	rdfs:label      "Deer"@en ;
	skos:prefLabel  "DEER" .

gs1:SourceAnimalCode-DOG
	rdf:type        gs1:SourceAnimalCode ;
	rdfs:comment    "A domesticated form of the Wolf, a member of the Canidae family of the order Carnivora."@en ;
	rdfs:label      "Dog"@en ;
	skos:prefLabel  "DOG" .

gs1:SourceAnimalCode-DUCK
	rdf:type        gs1:SourceAnimalCode ;
	rdfs:comment    "Aquatic birds, mostly smaller than the swans and geese, and may be found in both fresh water and sea water."@en ;
	rdfs:label      "Duck"@en ;
	skos:prefLabel  "DUCK" .

gs1:SourceAnimalCode-DUCKLING
	rdf:type        gs1:SourceAnimalCode ;
	rdfs:comment    "A young duck."@en ;
	rdfs:label      "Duckling"@en ;
	skos:prefLabel  "DUCKLING" .

gs1:SourceAnimalCode-FISH
	rdf:type        gs1:SourceAnimalCode ;
	rdfs:comment    "Fresh or sea water fish."@en ;
	rdfs:label      "Fish"@en ;
	skos:prefLabel  "FISH" .

gs1:SourceAnimalCode-FOWL
	rdf:type        gs1:SourceAnimalCode ;
	rdfs:comment    "Non-domesticated birds in general but usually refers to birds belonging to one of two biological orders, namely the gamefowl or landfowl and the waterfowl."@en ;
	rdfs:label      "Fowl"@en ;
	skos:prefLabel  "FOWL" .

gs1:SourceAnimalCode-FROG
	rdf:type        gs1:SourceAnimalCode ;
	rdfs:comment    "Amphibians in the order Anura."@en ;
	rdfs:label      "Frog"@en ;
	skos:prefLabel  "FROG" .

gs1:SourceAnimalCode-GOAT
	rdf:type        gs1:SourceAnimalCode ;
	rdfs:comment    "A member of the Bovidae family and is closely related to the sheep."@en ;
	rdfs:label      "Goat"@en ;
	skos:prefLabel  "GOAT" .

gs1:SourceAnimalCode-GOOSE
	rdf:type        gs1:SourceAnimalCode ;
	rdfs:comment    "A bird belonging to the family Anatidae"@en ;
	rdfs:label      "Goose"@en ;
	skos:prefLabel  "GOOSE" .

gs1:SourceAnimalCode-GROUSE
	rdf:type        gs1:SourceAnimalCode ;
	rdfs:comment    "A group of birds from the order Galliformes."@en ;
	rdfs:label      "Grouse"@en ;
	skos:prefLabel  "GROUSE" .

gs1:SourceAnimalCode-GUINEAFOWL
	rdf:type        gs1:SourceAnimalCode ;
	rdfs:comment    "A family of birds in the Galliformes order"@en ;
	rdfs:label      "Guinea Fowl"@en ;
	skos:prefLabel  "GUINEAFOWL" .

gs1:SourceAnimalCode-HARE
	rdf:type        gs1:SourceAnimalCode ;
	rdfs:comment    "Leporidaes belonging to the genus Lepus."@en ;
	rdfs:label      "Hare"@en ;
	skos:prefLabel  "HARE" .

gs1:SourceAnimalCode-HORSE
	rdf:type        gs1:SourceAnimalCode ;
	rdfs:comment    "a hoofed (ungulate) mammal, a subspecies of one of seven extant species of the family Equidae."@en ;
	rdfs:label      "Horse"@en ;
	skos:prefLabel  "HORSE" .

gs1:SourceAnimalCode-INVERTEBRATE
	rdf:type        gs1:SourceAnimalCode ;
	rdfs:comment    "Fresh or sea water invertebrate."@en ;
	rdfs:label      "Invertebrate"@en ;
	skos:prefLabel  "INVERTEBRATE" .

gs1:SourceAnimalCode-LAMB
	rdf:type        gs1:SourceAnimalCode ;
	rdfs:comment    "A young domestic sheep."@en ;
	rdfs:label      "Lamb"@en ;
	skos:prefLabel  "LAMB" .

gs1:SourceAnimalCode-LAND_SNAIL
	rdf:type        gs1:SourceAnimalCode ;
	rdfs:comment    "A member of the molluscan class Gastropoda that have coiled shells in the adult stage and live on land."@en ;
	rdfs:label      "Land Snail"@en ;
	skos:prefLabel  "LAND_SNAIL" .

gs1:SourceAnimalCode-MILK_COW
	rdf:type        gs1:SourceAnimalCode ;
	rdfs:comment    "Also referred to Milk Cattle, this cow is bred to produce large quantities of Milk, from which dairy products are made."@en ;
	rdfs:label      "Milk Cow"@en ;
	skos:prefLabel  "MILK_COW" .

gs1:SourceAnimalCode-MOOSE
	rdf:type        gs1:SourceAnimalCode ;
	rdfs:comment    "The largest extant species in the deer family."@en ;
	rdfs:label      "Moose"@en ;
	skos:prefLabel  "MOOSE" .

gs1:SourceAnimalCode-OSTRICH
	rdf:type        gs1:SourceAnimalCode ;
	rdfs:comment    "Large flightless bird native to Africa."@en ;
	rdfs:label      "Ostrich"@en ;
	skos:prefLabel  "OSTRICH" .

gs1:SourceAnimalCode-OTHER
	rdf:type        gs1:SourceAnimalCode ;
	rdfs:comment    "Other animal not specified on this list."@en ;
	rdfs:label      "Other"@en ;
	skos:prefLabel  "OTHER" .

gs1:SourceAnimalCode-PARTRIDGE
	rdf:type        gs1:SourceAnimalCode ;
	rdfs:comment    "Medium-sized birds, intermediate between the larger pheasants and the smaller quails."@en ;
	rdfs:label      "Partridge"@en ;
	skos:prefLabel  "PARTRIDGE" .

gs1:SourceAnimalCode-PHEASANT
	rdf:type        gs1:SourceAnimalCode ;
	rdfs:comment    "A bird in the subfamily of Phasianidae in the order Galliformes."@en ;
	rdfs:label      "Pheasant"@en ;
	skos:prefLabel  "PHEASANT" .

gs1:SourceAnimalCode-PIGEON
	rdf:type        gs1:SourceAnimalCode ;
	rdfs:comment    "A bird in the family Columbidae."@en ;
	rdfs:label      "Pigeon"@en ;
	skos:prefLabel  "PIGEON" .

gs1:SourceAnimalCode-PORK
	rdf:type        gs1:SourceAnimalCode ;
	rdfs:comment    "Meat from the domestic pig"@en ;
	rdfs:label      "Pork"@en ;
	skos:prefLabel  "PORK" .

gs1:SourceAnimalCode-POUSSIN
	rdf:type        gs1:SourceAnimalCode ;
	rdfs:comment    "A young chicken, less than 28 days old at slaughter"@en ;
	rdfs:label      "Poussin"@en ;
	skos:prefLabel  "POUSSIN" .

gs1:SourceAnimalCode-QUAIL
	rdf:type        gs1:SourceAnimalCode ;
	rdfs:comment    "Several genus of mid-sized birds in the pheasant family."@en ;
	rdfs:label      "Quail"@en ;
	skos:prefLabel  "QUAIL" .

gs1:SourceAnimalCode-RABBIT
	rdf:type        gs1:SourceAnimalCode ;
	rdfs:comment    "Small mammals in the family Leporidae of the order Lagomorpha"@en ;
	rdfs:label      "Rabbit"@en ;
	skos:prefLabel  "RABBIT" .

gs1:SourceAnimalCode-RAT
	rdf:type        gs1:SourceAnimalCode ;
	rdfs:comment    "Rats are various medium-sized, long-tailed rodents of the superfamily Muroidea."@en ;
	rdfs:label      "Rat"@en ;
	skos:prefLabel  "RAT" .

gs1:SourceAnimalCode-REINDEER
	rdf:type        gs1:SourceAnimalCode ;
	rdfs:comment    "An Arctic and Subarctic-dwelling deer, widespread and numerous across the Arctic and Subarctic."@en ;
	rdfs:label      "Reindeer"@en ;
	skos:prefLabel  "REINDEER" .

gs1:SourceAnimalCode-ROE_DEER
	rdf:type        gs1:SourceAnimalCode ;
	rdfs:comment    "A deer species of Europe, Asia Minor, and Caspian coastal regions."@en ;
	rdfs:label      "Roe Deer"@en ;
	skos:prefLabel  "ROE_DEER" .

gs1:SourceAnimalCode-SHEEP
	rdf:type        gs1:SourceAnimalCode ;
	rdfs:comment    "Small ruminants, usually with a crimped hair called wool and often with horns forming a lateral spiral."@en ;
	rdfs:label      "Sheep"@en ;
	skos:prefLabel  "SHEEP" .

gs1:SourceAnimalCode-SHELLFISH
	rdf:type        gs1:SourceAnimalCode ;
	rdfs:comment    "A fresh or sea water animal, such as a mollusk or crustacean, that has a shell or shell-like exoskeleton."@en ;
	rdfs:label      "Shellfish"@en ;
	skos:prefLabel  "SHELLFISH" .

gs1:SourceAnimalCode-SNAKE
	rdf:type        gs1:SourceAnimalCode ;
	rdfs:comment    "Elongate legless carnivorous reptiles of the suborder Serpentes."@en ;
	rdfs:label      "Snake"@en ;
	skos:prefLabel  "SNAKE" .

gs1:SourceAnimalCode-SNIPE
	rdf:type        gs1:SourceAnimalCode ;
	rdfs:comment    "Any of nearly 20 wading bird species in three genera in the family Scolopacidae."@en ;
	rdfs:label      "Snipe"@en ;
	skos:prefLabel  "SNIPE" .

gs1:SourceAnimalCode-SPARROW
	rdf:type        gs1:SourceAnimalCode ;
	rdfs:comment    "Small passerine birds in the family Passeridae."@en ;
	rdfs:label      "Sparrow"@en ;
	skos:prefLabel  "SPARROW" .

gs1:SourceAnimalCode-THRUSH
	rdf:type        gs1:SourceAnimalCode ;
	rdfs:comment    "Plump, soft-plumaged, small to medium-sized passerine birds."@en ;
	rdfs:label      "Thrush"@en ;
	skos:prefLabel  "THRUSH" .

gs1:SourceAnimalCode-TURKEY
	rdf:type        gs1:SourceAnimalCode ;
	rdfs:comment    "A large bird in the genus Meleagris."@en ;
	rdfs:label      "Turkey"@en ;
	skos:prefLabel  "TURKEY" .

gs1:SourceAnimalCode-TURTLE
	rdf:type        gs1:SourceAnimalCode ;
	rdfs:comment    "Reptiles characterised by a special bony or cartilaginous shell developed from their ribs that acts as a shield."@en ;
	rdfs:label      "Turtle"@en ;
	skos:prefLabel  "TURTLE" .

gs1:SourceAnimalCode-WOODCOCK
	rdf:type        gs1:SourceAnimalCode ;
	rdfs:comment    "The woodcocks are a group of seven or eight very similar living species of wading birds in the genus Scolopax."@en ;
	rdfs:label      "Woodcock"@en ;
	skos:prefLabel  "WOODCOCK" .

gs1:SourceAnimalCode-YAK
	rdf:type        gs1:SourceAnimalCode ;
	rdfs:comment    "A long-haired bovine found throughout the Himalayan region of south Central Asia, the Tibetan Plateau and as far north as Mongolia."@en ;
	rdfs:label      "Yak"@en ;
	skos:prefLabel  "YAK" .

gs1:SpecificVolume
	rdf:type  gs1:MeasurementType ;
	rdfs:comment    "The volume of a substance per unit mass. The reciprocal of density.  SI Units: cubic metres per kilogram"@en ;
	rdfs:label      "Specific volume"@en ;
	skos:prefLabel  "SpecificVolume" .

gs1:Speed
	rdf:type     gs1:MeasurementType ;
	rdfs:comment    "The ratio of the linear distance travelled by a body to the time taken. Speed is a scalar quantity. Velocity is a vector with magnitude and direction.  SI Units: metre per second"@en ;
	rdfs:label      "Speed or Velocity"@en ;
	skos:prefLabel  "Speed" .

gs1:SportingActivityTypeCode-AMERICAN_FOOTBALL
	rdf:type        gs1:SportingActivityTypeCode ;
	rdfs:label      "American Football"@en ;
	skos:prefLabel  "AMERICAN_FOOTBALL" .

gs1:SportingActivityTypeCode-ARCHERY
	rdf:type        gs1:SportingActivityTypeCode ;
	rdfs:label      "Archery"@en ;
	skos:prefLabel  "ARCHERY" .

gs1:SportingActivityTypeCode-BADMINTON
	rdf:type        gs1:SportingActivityTypeCode ;
	rdfs:label      "Badminton"@en ;
	skos:prefLabel  "BADMINTON" .

gs1:SportingActivityTypeCode-BASEBALL
	rdf:type        gs1:SportingActivityTypeCode ;
	rdfs:label      "Baseball"@en ;
	skos:prefLabel  "BASEBALL" .

gs1:SportingActivityTypeCode-BASKETBALL
	rdf:type        gs1:SportingActivityTypeCode ;
	rdfs:label      "Basketball"@en ;
	skos:prefLabel  "BASKETBALL" .

gs1:SportingActivityTypeCode-BOXING
	rdf:type        gs1:SportingActivityTypeCode ;
	rdfs:label      "Boxing"@en ;
	skos:prefLabel  "BOXING" .

gs1:SportingActivityTypeCode-CLIMBING
	rdf:type        gs1:SportingActivityTypeCode ;
	rdfs:label      "Climbing"@en ;
	skos:prefLabel  "CLIMBING" .

gs1:SportingActivityTypeCode-CRICKET
	rdf:type        gs1:SportingActivityTypeCode ;
	rdfs:label      "Cricket"@en ;
	skos:prefLabel  "CRICKET" .

gs1:SportingActivityTypeCode-CYCLING
	rdf:type        gs1:SportingActivityTypeCode ;
	rdfs:label      "Cycling"@en ;
	skos:prefLabel  "CYCLING" .

gs1:SportingActivityTypeCode-DIVING
	rdf:type        gs1:SportingActivityTypeCode ;
	rdfs:label      "Diving"@en ;
	skos:prefLabel  "DIVING" .

gs1:SportingActivityTypeCode-EQUESTRIAN
	rdf:type        gs1:SportingActivityTypeCode ;
	rdfs:label      "Equestrian"@en ;
	skos:prefLabel  "EQUESTRIAN" .

gs1:SportingActivityTypeCode-FENCING
	rdf:type        gs1:SportingActivityTypeCode ;
	rdfs:label      "Fencing"@en ;
	skos:prefLabel  "FENCING" .

gs1:SportingActivityTypeCode-FISHING
	rdf:type        gs1:SportingActivityTypeCode ;
	rdfs:label      "Fishing"@en ;
	skos:prefLabel  "FISHING" .

gs1:SportingActivityTypeCode-FOOTBALL
	rdf:type        gs1:SportingActivityTypeCode ;
	rdfs:label      "Football"@en ;
	skos:prefLabel  "FOOTBALL" .

gs1:SportingActivityTypeCode-GOLF
	rdf:type        gs1:SportingActivityTypeCode ;
	rdfs:label      "Golf"@en ;
	skos:prefLabel  "GOLF" .

gs1:SportingActivityTypeCode-GYMNASTICS
	rdf:type        gs1:SportingActivityTypeCode ;
	rdfs:label      "Gymnastics"@en ;
	skos:prefLabel  "GYMNASTICS" .

gs1:SportingActivityTypeCode-HOCKEY
	rdf:type        gs1:SportingActivityTypeCode ;
	rdfs:label      "Hockey"@en ;
	skos:prefLabel  "HOCKEY" .

gs1:SportingActivityTypeCode-ICE_HOCKEY
	rdf:type        gs1:SportingActivityTypeCode ;
	rdfs:label      "Ice Hockey"@en ;
	skos:prefLabel  "ICE_HOCKEY" .

gs1:SportingActivityTypeCode-ICE_SKATING
	rdf:type        gs1:SportingActivityTypeCode ;
	rdfs:label      "Ice Skating"@en ;
	skos:prefLabel  "ICE_SKATING" .

gs1:SportingActivityTypeCode-MOTOR_CYCLING
	rdf:type        gs1:SportingActivityTypeCode ;
	rdfs:label      "Motor Cycling"@en ;
	skos:prefLabel  "MOTOR_CYCLING" .

gs1:SportingActivityTypeCode-RUGBY
	rdf:type        gs1:SportingActivityTypeCode ;
	rdfs:label      "Rugby"@en ;
	skos:prefLabel  "RUGBY" .

gs1:SportingActivityTypeCode-RUNNING
	rdf:type        gs1:SportingActivityTypeCode ;
	rdfs:label      "Running"@en ;
	skos:prefLabel  "RUNNING" .

gs1:SportingActivityTypeCode-SKIING
	rdf:type        gs1:SportingActivityTypeCode ;
	rdfs:label      "Skiing"@en ;
	skos:prefLabel  "SKIING" .

gs1:SportingActivityTypeCode-SQUASH
	rdf:type        gs1:SportingActivityTypeCode ;
	rdfs:label      "Squash"@en ;
	skos:prefLabel  "SQUASH" .

gs1:SportingActivityTypeCode-SURFING
	rdf:type        gs1:SportingActivityTypeCode ;
	rdfs:label      "Surfing"@en ;
	skos:prefLabel  "SURFING" .

gs1:SportingActivityTypeCode-SWIMMING
	rdf:type        gs1:SportingActivityTypeCode ;
	rdfs:label      "Swimming"@en ;
	skos:prefLabel  "SWIMMING" .

gs1:SportingActivityTypeCode-TENNIS
	rdf:type        gs1:SportingActivityTypeCode ;
	rdfs:label      "Tennis"@en ;
	skos:prefLabel  "TENNIS" .

gs1:SportingActivityTypeCode-UNCLASSIFIED
	rdf:type        gs1:SportingActivityTypeCode ;
	rdfs:label      "Unclassified"@en ;
	skos:prefLabel  "UNCLASSIFIED" .

gs1:SportingActivityTypeCode-UNIDENTIFIED
	rdf:type        gs1:SportingActivityTypeCode ;
	rdfs:label      "Unidentified"@en ;
	skos:prefLabel  "UNIDENTIFIED" .

gs1:StatusType-ACTIVE
	rdf:type        gs1:StatusType ;
	rdfs:comment    "Designation stating that an organisation/party or location is operating. Note that this is independent of whether or not the GLN is active."@en ;
	rdfs:label      "Active"@en ;
	skos:prefLabel  "ACTIVE" .

gs1:StatusType-INACTIVE
	rdf:type        gs1:StatusType ;
	rdfs:comment    "Designation stating that an organisation/party or location is not operating. Note that this is independent of whether or not the GLN is inactive."@en ;
	rdfs:label      "Inactive"@en ;
	skos:prefLabel  "INACTIVE" .

gs1:SurfaceDensity
	rdf:type  gs1:MeasurementType ;
	rdfs:comment    "The mass per unit area distributed over a surface.  SI Units: kilogram per square metre"@en ;
	rdfs:label      "Surface density"@en ;
	skos:prefLabel  "SurfaceDensity" .

gs1:SurfaceTension
	rdf:type  gs1:MeasurementType ;
	rdfs:comment    "The attractive force exerted upon the surface molecules of a liquid by the molecules beneath that tends to draw the surface molecules into the bulk of the liquid and makes the liquid assume the shape having the minimum surface area.  SI Units: newton per metre"@en ;
	rdfs:label      "Surface tension"@en ;
	skos:prefLabel  "SurfaceTension" .

gs1:TargetConsumerGenderCode-FEMALE
	rdf:type        gs1:TargetConsumerGenderCode ;
	rdfs:label      "Female"@en ;
	skos:prefLabel  "FEMALE" .

gs1:TargetConsumerGenderCode-MALE
	rdf:type        gs1:TargetConsumerGenderCode ;
	rdfs:label      "Male"@en ;
	skos:prefLabel  "MALE" .

gs1:TargetConsumerGenderCode-UNISEX
	rdf:type        gs1:TargetConsumerGenderCode ;
	rdfs:label      "Unisex"@en ;
	skos:prefLabel  "UNISEX" .

gs1:Temperature
	rdf:type  gs1:MeasurementType ;
	rdfs:comment    "A measure of whether two systems are relatively hot or cold with respect to one another; two systems brought into contact will eventually reach thermal equilibrium and reach the same temperature as thermal energy (heat) flows from the system with higher temperature to the system with lower temperature.  SI Units: kelvin"@en ;
	rdfs:label      "Temperature"@en ;
	skos:prefLabel  "Temperature" .

gs1:Time
	rdf:type      gs1:MeasurementType ;
	rdfs:comment    "A dimension that enables distinction between two otherwise identical events that occur at the same point in space. The interval between such events is the basis of time measurement.  SI Units: second"@en ;
	rdfs:label      "Time"@en ;
	skos:prefLabel  "Time" .

gs1:Torque
	rdf:type    gs1:MeasurementType ;
	rdfs:comment    "The product of a force and its perpendicular distance from a point about which it causes rotation or torsion.  SI Units: newton metre"@en ;
	rdfs:label      "Torque"@en ;
	skos:prefLabel  "Torque" .

gs1:TradeChannelCode-INSTORE_ONLY
	rdf:type        gs1:TradeChannelCode ;
	rdfs:comment    "Offer avalilable only in stores."@en ;
	rdfs:label      "Instore Only"@en ;
	skos:prefLabel  "INSTORE_ONLY" .

gs1:TradeChannelCode-OMNICHANNEL
	rdf:type        gs1:TradeChannelCode ;
	rdfs:comment    "Offer avalilable both in stores and online."@en ;
	rdfs:label      "Omni-channel"@en ;
	skos:prefLabel  "OMNICHANNEL" .

gs1:TradeChannelCode-ONLINE_ONLY
	rdf:type        gs1:TradeChannelCode ;
	rdfs:comment    "Offer avalilable online only."@en ;
	rdfs:label      "Online Only"@en ;
	skos:prefLabel  "ONLINE_ONLY" .

gs1:UpperTypeCode-CLOSED_TOE_CLOSED_BACK_OPEN_INSTEP
	rdf:type        gs1:UpperTypeCode ;
	rdfs:label      "Closed Toe Closed Back Open Instep"@en ;
	skos:prefLabel  "CLOSED_TOE_CLOSED_BACK_OPEN_INSTEP" .

gs1:UpperTypeCode-CLOSED_TOE_OPEN_BACK
	rdf:type        gs1:UpperTypeCode ;
	rdfs:label      "Closed Toe Open Back"@en ;
	skos:prefLabel  "CLOSED_TOE_OPEN_BACK" .

gs1:UpperTypeCode-CLOSED_TOE_STRAP_BACK
	rdf:type        gs1:UpperTypeCode ;
	rdfs:label      "Closed Toe Strap Back"@en ;
	skos:prefLabel  "CLOSED_TOE_STRAP_BACK" .

gs1:UpperTypeCode-FULLY_CLOSED
	rdf:type        gs1:UpperTypeCode ;
	rdfs:label      "Fully Closed"@en ;
	skos:prefLabel  "FULLY_CLOSED" .

gs1:UpperTypeCode-OPEN_TOE_FULLY_CLOSED_BACK
	rdf:type        gs1:UpperTypeCode ;
	rdfs:label      "Open Toe Fully Closed Back"@en ;
	skos:prefLabel  "OPEN_TOE_FULLY_CLOSED_BACK" .

gs1:UpperTypeCode-OPEN_TOE_OPEN_BACK
	rdf:type        gs1:UpperTypeCode ;
	rdfs:label      "Open Toe Open Back"@en ;
	skos:prefLabel  "OPEN_TOE_OPEN_BACK" .

gs1:UpperTypeCode-OPEN_TOE_STRAP_BACK
	rdf:type        gs1:UpperTypeCode ;
	rdfs:label      "Open Toe Strap Back"@en ;
	skos:prefLabel  "OPEN_TOE_STRAP_BACK" .

gs1:UpperTypeCode-UNCLASSIFIED
	rdf:type        gs1:UpperTypeCode ;
	rdfs:label      "Unclassified"@en ;
	skos:prefLabel  "UNCLASSIFIED" .

gs1:Voltage
	rdf:type   gs1:MeasurementType ;
	rdfs:comment    "The value of an electromotive force or electrostatic potential difference, expressed in volts.  SI Units: volt"@en ;
	rdfs:label      "Voltage"@en ;
	skos:prefLabel  "Voltage" .

gs1:Volume
	rdf:type    gs1:MeasurementType ;
	rdfs:comment    "The amount of three-dimensional space occupied by a body, measured in cubic length units.  SI Units: cubic metre"@en ;
	rdfs:label      "Volume"@en ;
	skos:prefLabel  "Volume" .

gs1:VolumeFlowRate
	rdf:type  gs1:MeasurementType ;
	rdfs:comment    "The volume of fluid that passes per unit of time.  SI Units: cubic metre per second"@en ;
	rdfs:label      "Volume flow rate"@en ;
	skos:prefLabel  "VolumeFlowRate" .

gs1:VolumeFraction
	rdf:type  gs1:MeasurementType ;
	rdfs:comment    "The dimensionless ratio of a volume of one substance to the volume of solid, liquid or gas in which it is contained.  Typical units: parts per million, parts per billion, etc."@en ;
	rdfs:label      "Volume fraction"@en ;
	skos:prefLabel  "VolumeFraction" .

gs1:VolumetricFlux
	rdf:type  gs1:MeasurementType ;
	rdfs:comment    "The volume of fluid that passes per unit of time per unit area perpendicular to the flow direction.  SI Units: cubic metre per second per square metre"@en ;
	rdfs:label      "Volumetric flux"@en ;
	skos:prefLabel  "VolumetricFlux" .

gs1:Wavenumber
	rdf:type  gs1:MeasurementType ;
	rdfs:comment    "The number of waves per unit length.  SI Units: reciprocal metre"@en ;
	rdfs:label      "Wavenumber"@en ;
	skos:prefLabel  "Wavenumber" .


gs1:AI
	rdf:type          rdfs:Datatype ;
	rdfs:comment      "A Data Type that corresponds to GS1 Application Identifiers defined in the GS1 General Specifications"@en ;
	rdfs:isDefinedBy  gs1: ;
	rdfs:label        "GS1 Application Identifier"@en ;
	sw:term_status    "stable" .


